# baseURI: http://data.gov.au/def/agift2014
# imports: http://purl.org/dc/elements/1.1/
# imports: http://www.w3.org/2004/02/skos/core

@prefix agift: <http://data.gov.au/def/agift/> .
@prefix dc: <http://purl.org/dc/elements/1.1/> .
@prefix dcterms: <http://purl.org/dc/terms/> .
@prefix owl: <http://www.w3.org/2002/07/owl#> .
@prefix rdf: <http://www.w3.org/1999/02/22-rdf-syntax-ns#> .
@prefix rdf123: <http://rdf123.umbc.edu/ns/> .
@prefix rdfs: <http://www.w3.org/2000/01/rdf-schema#> .
@prefix skos: <http://www.w3.org/2004/02/skos/core#> .
@prefix spin: <http://spinrdf.org/spin#> .
@prefix vann: <http://purl.org/vocab/vann/> .
@prefix xsd: <http://www.w3.org/2001/XMLSchema#> .

agift:
  rdf:type skos:Collection ;
  rdfs:label "Australian Governments' Interactive Functions Thesaurus (AGIFT)"@en ;
  rdfs:seeAlso agift:scheme2014 ;
  skos:member agift:accommodation-services ;
  skos:member agift:administrative-decision-appeal ;
  skos:member agift:administrative-decision-review ;
  skos:member agift:administrative-law ;
  skos:member agift:adoption-services ;
  skos:member agift:adult-education-programs ;
  skos:member agift:adult-migrant-education ;
  skos:member agift:advertising-campaigns ;
  skos:member agift:advertising-standards ;
  skos:member agift:aged-care-services ;
  skos:member agift:agreement-bargaining-processes ;
  skos:member agift:agreement-dispute-mediation ;
  skos:member agift:agricultural-industry ;
  skos:member agift:agricultural-sciences ;
  skos:member agift:air-force ;
  skos:member agift:air-transport ;
  skos:member agift:air-transport-safety ;
  skos:member agift:aircraft-standards ;
  skos:member agift:airport-services ;
  skos:member agift:ambulance-services ;
  skos:member agift:animal-and-veterinary-sciences ;
  skos:member agift:apparatus-licensing ;
  skos:member agift:applied-sciences ;
  skos:member agift:appointment-management ;
  skos:member agift:apprenticeship-programs ;
  skos:member agift:aquaculture-industry ;
  skos:member agift:architectural-services ;
  skos:member agift:army ;
  skos:member agift:army-reserve-training ;
  skos:member agift:artefact-export-regulation ;
  skos:member agift:arts-development ;
  skos:member agift:arts-education ;
  skos:member agift:arts-funding ;
  skos:member agift:arts-incentive-schemes ;
  skos:member agift:arts-promotion ;
  skos:member agift:asset-assessment ;
  skos:member agift:association-registration ;
  skos:member agift:associations-and-corporate-law ;
  skos:member agift:astronomical-sciences ;
  skos:member agift:athlete-scholarship-programs ;
  skos:member agift:atmospheric-sciences ;
  skos:member agift:atomic-and-molecular-sciences ;
  skos:member agift:australian-defence-forces ;
  skos:member agift:australian-theatre-of-war ;
  skos:member agift:authentication ;
  skos:member agift:award-conditions ;
  skos:member agift:badges-and-insignia ;
  skos:member agift:bankruptcy-proceedings ;
  skos:member agift:benefits ;
  skos:member agift:biochemistry ;
  skos:member agift:biodiversity-preservation ;
  skos:member agift:biological-sciences ;
  skos:member agift:biotechnology-development ;
  skos:member agift:blood-and-organ-donation-management ;
  skos:member agift:border-protection ;
  skos:member agift:botany ;
  skos:member agift:broadcasting ;
  skos:member agift:broadcasting-standards ;
  skos:member agift:building-acoustics ;
  skos:member agift:building-approval-services ;
  skos:member agift:building-preservation ;
  skos:member agift:building-regulations-and-standards ;
  skos:member agift:built-environment ;
  skos:member agift:burial-ground-management ;
  skos:member agift:business-association ;
  skos:member agift:business-process-auditing ;
  skos:member agift:business-registration-and-licensing ;
  skos:member agift:business-sponsorship ;
  skos:member agift:business-support-and-regulation ;
  skos:member agift:cadets ;
  skos:member agift:call-centre-administration ;
  skos:member agift:capital-equipment-programs ;
  skos:member agift:caravan-and-camping-services ;
  skos:member agift:cargo-control ;
  skos:member agift:carriage-service-providers ;
  skos:member agift:carrier-licensing ;
  skos:member agift:censorship-standards ;
  skos:member agift:ceremonial-events-and-representation ;
  skos:member agift:certified-employment-conditions ;
  skos:member agift:charting-sea-lanes ;
  skos:member agift:chemical-and-pesticide-regulation ;
  skos:member agift:child-and-youth-support ;
  skos:member agift:child-care-services ;
  skos:member agift:citizenship ;
  skos:member agift:civic-celebrations ;
  skos:member agift:civic-infrastructure ;
  skos:member agift:civic-management ;
  skos:member agift:civil-community-assistance ;
  skos:member agift:civil-law ;
  skos:member agift:civil-registration ;
  skos:member agift:climate-information-services ;
  skos:member agift:clinical-health-services ;
  skos:member agift:collection-access ;
  skos:member agift:collection-accessioning ;
  skos:member agift:collection-acquisition ;
  skos:member agift:collection-management ;
  skos:member agift:collection-promotion ;
  skos:member agift:collection-storage ;
  skos:member agift:commissions-of-inquiry ;
  skos:member agift:commonwealth-state-funding ;
  skos:member agift:communications ;
  skos:member agift:communications-infrastructure ;
  skos:member agift:community-based-corrections ;
  skos:member agift:community-education ;
  skos:member agift:community-engagement ;
  skos:member agift:community-health-services ;
  skos:member agift:community-housing ;
  skos:member agift:community-policing ;
  skos:member agift:community-recreational-programs ;
  skos:member agift:community-services ;
  skos:member agift:community-support ;
  skos:member agift:conservation-programs ;
  skos:member agift:constitutional-conventions ;
  skos:member agift:constitutional-matters ;
  skos:member agift:constitutional-referenda ;
  skos:member agift:consular-services ;
  skos:member agift:consumer-protection ;
  skos:member agift:contract-management ;
  skos:member agift:conveyancing ;
  skos:member agift:copyright-registration ;
  skos:member agift:copyright-regulation ;
  skos:member agift:coronial-law ;
  skos:member agift:corrective-services ;
  skos:member agift:corruption-prevention ;
  skos:member agift:counselling-services ;
  skos:member agift:counterfeiting-control ;
  skos:member agift:courier-services ;
  skos:member agift:court-reporting ;
  skos:member agift:criminal-law ;
  skos:member agift:criminology ;
  skos:member agift:cross-border-cooperation ;
  skos:member agift:crown-land-administration ;
  skos:member agift:cultural-affairs ;
  skos:member agift:cultural-artefact-repatriation ;
  skos:member agift:cultural-awards-and-scholarships ;
  skos:member agift:cultural-centre-management ;
  skos:member agift:cultural-festivals ;
  skos:member agift:cultural-gifts-programs ;
  skos:member agift:currency ;
  skos:member agift:curriculum-development ;
  skos:member agift:cybersafety ;
  skos:member agift:data-management ;
  skos:member agift:declaration-of-interests ;
  skos:member agift:defence ;
  skos:member agift:defence-attaches ;
  skos:member agift:defence-career-development ;
  skos:member agift:defence-college-training ;
  skos:member agift:defence-community-programs ;
  skos:member agift:defence-cooperation-programs ;
  skos:member agift:defence-efficiency-review ;
  skos:member agift:defence-estate-management ;
  skos:member agift:defence-force-careers ;
  skos:member agift:defence-force-commands ;
  skos:member agift:defence-housing ;
  skos:member agift:defence-industry ;
  skos:member agift:defence-liaison ;
  skos:member agift:defence-personnel-exchanges ;
  skos:member agift:defence-reform-program ;
  skos:member agift:defence-science-and-technology ;
  skos:member agift:defence-strategic-development ;
  skos:member agift:defence-strategic-policy ;
  skos:member agift:defence-strategic-support ;
  skos:member agift:dental-health-services ;
  skos:member agift:deportation ;
  skos:member agift:descriptive-standards ;
  skos:member agift:design-rights-management ;
  skos:member agift:detention-centre-management ;
  skos:member agift:detention-programs ;
  skos:member agift:development-assistance-programs ;
  skos:member agift:diplomatic-missions ;
  skos:member agift:disarmament-and-arms-control ;
  skos:member agift:disaster-recovery ;
  skos:member agift:disaster-relief ;
  skos:member agift:disaster-support ;
  skos:member agift:discipline-programs ;
  skos:member agift:dispute-mediation-programs ;
  skos:member agift:doping-detection-research ;
  skos:member agift:draft-bill-amendment-process ;
  skos:member agift:driving-licences-administration ;
  skos:member agift:drugs-and-poisons-regulation ;
  skos:member agift:early-childhood-education ;
  skos:member agift:earth-sciences ;
  skos:member agift:economic-research ;
  skos:member agift:education-and-training ;
  skos:member agift:election-campaigning ;
  skos:member agift:electoral-boundary-assessment ;
  skos:member agift:electoral-matters ;
  skos:member agift:electronic-commerce ;
  skos:member agift:electronic-postal-services ;
  skos:member agift:electronic-publishing ;
  skos:member agift:emergency-accommodation ;
  skos:member agift:emergency-funding ;
  skos:member agift:emergency-management ;
  skos:member agift:emergency-services ;
  skos:member agift:employment ;
  skos:member agift:employment-advocacy-services ;
  skos:member agift:employment-services-marketing ;
  skos:member agift:endangered-species-protection ;
  skos:member agift:energy-resources ;
  skos:member agift:energy-supply ;
  skos:member agift:engineering-and-technology-sciences ;
  skos:member agift:engineering-services ;
  skos:member agift:entomology ;
  skos:member agift:environment ;
  skos:member agift:environmental-impact-assessment ;
  skos:member agift:epidemiology ;
  skos:member agift:equipment-licensing ;
  skos:member agift:ethical-compliance ;
  skos:member agift:exchange-rates ;
  skos:member agift:exhibition-programs ;
  skos:member agift:export-promotion ;
  skos:member agift:export-regulation ;
  skos:member agift:external-security ;
  skos:member agift:fair-trading-compliance ;
  skos:member agift:family-law-proceedings ;
  skos:member agift:family-reunion-programs ;
  skos:member agift:feral-pest-control ;
  skos:member agift:finance-management ;
  skos:member agift:financial-administration ;
  skos:member agift:financial-assistance ;
  skos:member agift:financial-budgeting ;
  skos:member agift:financial-institutions-regulation ;
  skos:member agift:financial-investment ;
  skos:member agift:financial-system-management ;
  skos:member agift:financial-system-monitoring ;
  skos:member agift:finding-aids-development ;
  skos:member agift:firefighting-services ;
  skos:member agift:fiscal-policy ;
  skos:member agift:fisheries-industry ;
  skos:member agift:food-hygiene-regulation ;
  skos:member agift:food-quality-assurance ;
  skos:member agift:foreign-investment-control ;
  skos:member agift:forensic-analysis ;
  skos:member agift:forestry-industry ;
  skos:member agift:fossil-fuel-management ;
  skos:member agift:freedom-of-information ;
  skos:member agift:freight-movement-regulation ;
  skos:member agift:fundraising-and-donation-schemes ;
  skos:member agift:gambling-support-services ;
  skos:member agift:games-administration ;
  skos:member agift:games-promotion ;
  skos:member agift:gaming-industry-regulation ;
  skos:member agift:garden-management ;
  skos:member agift:general-insurance ;
  skos:member agift:genetic-engineering ;
  skos:member agift:governance ;
  skos:member agift:government-auditing ;
  skos:member agift:government-media ;
  skos:member agift:government-procurement-regulation ;
  skos:member agift:hansard-services ;
  skos:member agift:harbour-management ;
  skos:member agift:head-of-government-protocol ;
  skos:member agift:health-care ;
  skos:member agift:health-disaster-preparedness ;
  skos:member agift:health-hazard-prevention ;
  skos:member agift:health-insurance-schemes ;
  skos:member agift:health-promotion ;
  skos:member agift:health-protocol-administration ;
  skos:member agift:historic-relic-protection ;
  skos:member agift:honours-and-awards-programs ;
  skos:member agift:horticultural-industry ;
  skos:member agift:hospital-administration ;
  skos:member agift:hospital-services ;
  skos:member agift:hospital-teaching-programs ;
  skos:member agift:housing-industry-policy ;
  skos:member agift:human-resources-development ;
  skos:member agift:human-rights-obligations ;
  skos:member agift:hydrology ;
  skos:member agift:immigration ;
  skos:member agift:import-regulation ;
  skos:member agift:income-assessment ;
  skos:member agift:income-support-schemes ;
  skos:member agift:independent-living-services ;
  skos:member agift:indigenous-advocacy ;
  skos:member agift:indigenous-affairs ;
  skos:member agift:indigenous-cultural-heritage ;
  skos:member agift:indigenous-enterprise-development ;
  skos:member agift:indigenous-health-services ;
  skos:member agift:indigenous-heritage-conservation ;
  skos:member agift:indigenous-land-management ;
  skos:member agift:indigenous-reconciliation ;
  skos:member agift:indigenous-welfare-programs ;
  skos:member agift:industrial-awards-and-conditions ;
  skos:member agift:industry-assistance-schemes ;
  skos:member agift:industry-collaboration ;
  skos:member agift:industry-development ;
  skos:member agift:inflation ;
  skos:member agift:information-dissemination ;
  skos:member agift:information-management-standards ;
  skos:member agift:information-security ;
  skos:member agift:information-technology-standards ;
  skos:member agift:infrastructure-planning ;
  skos:member agift:insurance-regulation ;
  skos:member agift:integrated-services-planning ;
  skos:member agift:integrity-compliance ;
  skos:member agift:intellectual-property-management ;
  skos:member agift:intelligence ;
  skos:member agift:intelligence-liaison ;
  skos:member agift:intelligence-support ;
  skos:member agift:interest-rates ;
  skos:member agift:intergovernment-policy-dissemination ;
  skos:member agift:intergovernmental-relations ;
  skos:member agift:international-affairs ;
  skos:member agift:international-monetary-regulation ;
  skos:member agift:international-relations ;
  skos:member agift:international-trade-agreements ;
  skos:member agift:international-treaties ;
  skos:member agift:internet ;
  skos:member agift:interpreter-services ;
  skos:member agift:interstate-trade-agreements ;
  skos:member agift:investment-scheme-regulation ;
  skos:member agift:job-placement-programs ;
  skos:member agift:job-vacancy-data-management ;
  skos:member agift:justice-administration ;
  skos:member agift:juvenile-justice ;
  skos:member agift:labour-market-programs ;
  skos:member agift:land-councils ;
  skos:member agift:land-rehabilitation-programs ;
  skos:member agift:land-use-planning ;
  skos:member agift:land-use-zoning ;
  skos:member agift:land-valuation ;
  skos:member agift:landcare-programs ;
  skos:member agift:law-enforcement ;
  skos:member agift:legal-aid-services ;
  skos:member agift:legislation-review ;
  skos:member agift:legislative-drafting ;
  skos:member agift:life-insurance ;
  skos:member agift:light-station-maintenance ;
  skos:member agift:local-laws-and-ordinances ;
  skos:member agift:logistics ;
  skos:member agift:marina-management ;
  skos:member agift:marine-and-rural-regulation ;
  skos:member agift:marine-and-rural-support ;
  skos:member agift:marine-life-protection-programs ;
  skos:member agift:maritime-services ;
  skos:member agift:mathematical-sciences ;
  skos:member agift:media-ownership-regulation ;
  skos:member agift:medical-aids-regulation ;
  skos:member agift:medical-and-health-sciences ;
  skos:member agift:medical-quarantine-services ;
  skos:member agift:medical-radiation-services ;
  skos:member agift:medical-research ;
  skos:member agift:medical-research-funding ;
  skos:member agift:memorial-maintenance ;
  skos:member agift:mental-health-services ;
  skos:member agift:merger-regulation ;
  skos:member agift:migrant-accommodation-services ;
  skos:member agift:migrant-services ;
  skos:member agift:migrant-settlement-programs ;
  skos:member agift:military-advisors ;
  skos:member agift:military-bands ;
  skos:member agift:military-education-and-training ;
  skos:member agift:military-employment-services ;
  skos:member agift:military-exercises ;
  skos:member agift:military-law ;
  skos:member agift:military-operations ;
  skos:member agift:mineral-exploration ;
  skos:member agift:mineral-resources ;
  skos:member agift:mining-regulations ;
  skos:member agift:mobile-telephone-services ;
  skos:member agift:monetary-policy ;
  skos:member agift:multicultural-festivals ;
  skos:member agift:multicultural-heritage-promotion ;
  skos:member agift:multicultural-services ;
  skos:member agift:national-park-management ;
  skos:member agift:national-referral-laboratory-services ;
  skos:member agift:national-security ;
  skos:member agift:native-title-claims ;
  skos:member agift:native-title-mediation-programs ;
  skos:member agift:native-title-settlement-negotiations ;
  skos:member agift:natural-disasters ;
  skos:member agift:natural-heritage-protection ;
  skos:member agift:natural-resources ;
  skos:member agift:naturalisation-assessment ;
  skos:member agift:nature-reserve-management ;
  skos:member agift:navigation ;
  skos:member agift:navigation-systems-development ;
  skos:member agift:navy ;
  skos:member agift:notifiable-disease-management ;
  skos:member agift:nuclear-safeguards ;
  skos:member agift:nuclear-sciences ;
  skos:member agift:occupational-health-and-safety ;
  skos:member agift:oceanography ;
  skos:member agift:oceans-governance ;
  skos:member agift:official-establishment-management ;
  skos:member agift:official-hospitality ;
  skos:member agift:official-protocol ;
  skos:member agift:official-visits ;
  skos:member agift:online-transaction-standards ;
  skos:member agift:open-government ;
  skos:member agift:overseas-aid-programs ;
  skos:member agift:overseas-promotion ;
  skos:member agift:overseas-skills-recognition ;
  skos:member agift:overseas-student-scholarship-programs ;
  skos:member agift:park-and-reserve-services ;
  skos:member agift:parliamentary-chamber-support ;
  skos:member agift:parliamentary-committee-and-member-support ;
  skos:member agift:parliamentary-papers ;
  skos:member agift:passenger-services ;
  skos:member agift:passport-services ;
  skos:member agift:pastoral-industry ;
  skos:member agift:patent-rights-management ;
  skos:member agift:patient-care ;
  skos:member agift:payments-management ;
  skos:member agift:peacekeeping-forces ;
  skos:member agift:permanent-entry-arrangements ;
  skos:member agift:personnel-safety-standards ;
  skos:member agift:pharmaceutical-and-drug-support ;
  skos:member agift:physical-sciences ;
  skos:member agift:physiology ;
  skos:member agift:pilot-licensing ;
  skos:member agift:pilotage-management ;
  skos:member agift:place-names ;
  skos:member agift:planning-approvals ;
  skos:member agift:plant-breeders-rights-management ;
  skos:member agift:police-administration ;
  skos:member agift:pollutant-prevention-programs ;
  skos:member agift:pollution-emission-control ;
  skos:member agift:population-based-research ;
  skos:member agift:port-regulation ;
  skos:member agift:postal-services ;
  skos:member agift:practitioner-discipline ;
  skos:member agift:practitioner-registration ;
  skos:member agift:preparation-of-legislative-regulations ;
  skos:member agift:presentation-arrangements ;
  skos:member agift:preservation-services ;
  skos:member agift:prices-surveillance ;
  skos:member agift:primary-health-care ;
  skos:member agift:primary-industries ;
  skos:member agift:privacy- ;
  skos:member agift:probate-applications ;
  skos:member agift:product-safety ;
  skos:member agift:productivity ;
  skos:member agift:professional-accreditation ;
  skos:member agift:prohibited-export-control ;
  skos:member agift:prohibited-import-control ;
  skos:member agift:prosecution-services ;
  skos:member agift:protective-services ;
  skos:member agift:public-administration ;
  skos:member agift:public-borrowing ;
  skos:member agift:public-debt ;
  skos:member agift:public-expenditure ;
  skos:member agift:public-fitness-promotion ;
  skos:member agift:public-health-services ;
  skos:member agift:public-housing ;
  skos:member agift:public-housing-construction ;
  skos:member agift:public-housing-design ;
  skos:member agift:public-housing-entitlements ;
  skos:member agift:public-housing-maintenance ;
  skos:member agift:public-land-management ;
  skos:member agift:public-service ;
  skos:member agift:public-transport ;
  skos:member agift:publicity-programs ;
  skos:member agift:publishing ;
  skos:member agift:publishing-standards ;
  skos:member agift:quarantine ;
  skos:member agift:radiation-protection ;
  skos:member agift:radio-broadcasting ;
  skos:member agift:radio-communication ;
  skos:member agift:rail-harmonisation-standards ;
  skos:member agift:rail-land-acquisition-regulation ;
  skos:member agift:rail-transport ;
  skos:member agift:rail-transport-safety ;
  skos:member agift:railway-maintenance ;
  skos:member agift:recordkeeping-standards ;
  skos:member agift:recreational-park-management ;
  skos:member agift:recruitment-programs ;
  skos:member agift:reference-services ;
  skos:member agift:refuge-support ;
  skos:member agift:refugee-services ;
  skos:member agift:regional-development ;
  skos:member agift:remuneration-review ;
  skos:member agift:renewable-energy-development ;
  skos:member agift:rescue-coordination ;
  skos:member agift:reserves ;
  skos:member agift:residential-services ;
  skos:member agift:resource-management ;
  skos:member agift:retail-postal-services ;
  skos:member agift:retirement-income ;
  skos:member agift:retirement-saving ;
  skos:member agift:revenue-raising ;
  skos:member agift:road-safety-awareness ;
  skos:member agift:road-surface-maintenance ;
  skos:member agift:road-traffic-regulation ;
  skos:member agift:road-transport ;
  skos:member agift:road-transport-safety ;
  skos:member agift:rolling-stock-regulation ;
  skos:member agift:rural-community-development ;
  skos:member agift:rural-field-day-promotion ;
  skos:member agift:rural-partnership-programs ;
  skos:member agift:satellite-communication ;
  skos:member agift:school-education ;
  skos:member agift:school-transport-regulation ;
  skos:member agift:science ;
  skos:member agift:sea-passengers ;
  skos:member agift:search-and-rescue ;
  skos:member agift:search-technology-development ;
  skos:member agift:seaworthiness ;
  skos:member agift:security ;
  skos:member agift:seismology ;
  skos:member agift:ship-commissioning ;
  skos:member agift:ship-inspection ;
  skos:member agift:ship-personnel ;
  skos:member agift:ship-safety ;
  skos:member agift:silvicultural-industry ;
  skos:member agift:small-business-advocacy ;
  skos:member agift:small-business-development ;
  skos:member agift:small-business-services ;
  skos:member agift:social-club-support ;
  skos:member agift:social-justice-and-equity ;
  skos:member agift:social-media ;
  skos:member agift:social-research ;
  skos:member agift:soil-preservation-programs ;
  skos:member agift:spatial-information-research ;
  skos:member agift:special-needs-programs ;
  skos:member agift:special-needs-services ;
  skos:member agift:special-operations ;
  skos:member agift:spectrum-management ;
  skos:member agift:sport-and-fitness-development ;
  skos:member agift:sport-and-recreation ;
  skos:member agift:sporting-facilities-management ;
  skos:member agift:sporting-grants-administration ;
  skos:member agift:sports-drugs-monitoring ;
  skos:member agift:statistical-analysis ;
  skos:member agift:statistical-collection ;
  skos:member agift:statistical-design ;
  skos:member agift:statistical-services ;
  skos:member agift:statistical-standards ;
  skos:member agift:statistics-dissemination ;
  skos:member agift:stock-market-regulation ;
  skos:member agift:strategic-decisions ;
  skos:member agift:strategic-planning ;
  skos:member agift:superannuation-regulation ;
  skos:member agift:tabling-of-official-documents ;
  skos:member agift:tariff-regulation ;
  skos:member agift:taxation ;
  skos:member agift:taxation-compliance ;
  skos:member agift:telecommunications ;
  skos:member agift:telephone-services ;
  skos:member agift:television-broadcasting ;
  skos:member agift:temporary-entry-arrangements ;
  skos:member agift:termination-processes ;
  skos:member agift:territories-administration ;
  skos:member agift:tertiary-education ;
  skos:member agift:tourism ;
  skos:member agift:tourism-industry-development ;
  skos:member agift:tourist-event-promotion ;
  skos:member agift:town-planning ;
  skos:member agift:trade ;
  skos:member agift:trade-development-programs ;
  skos:member agift:trade-expositions ;
  skos:member agift:trade-measurement-compliance ;
  skos:member agift:trade-practices-compliance ;
  skos:member agift:trademark-registration ;
  skos:member agift:trainee-programs ;
  skos:member agift:transport ;
  skos:member agift:transport-access-schemes ;
  skos:member agift:transport-accessibility ;
  skos:member agift:transport-infrastructure-development ;
  skos:member agift:transport-network-maintenance ;
  skos:member agift:travel-authorisation ;
  skos:member agift:travel-missions ;
  skos:member agift:treaty-administration ;
  skos:member agift:vehicle-registration ;
  skos:member agift:vehicle-standards ;
  skos:member agift:veterans-entitlements ;
  skos:member agift:veterans-health-services ;
  skos:member agift:viticultural-industry ;
  skos:member agift:vocational-education ;
  skos:member agift:volunteer-support-programs ;
  skos:member agift:warfare ;
  skos:member agift:waste-management ;
  skos:member agift:water-conservation-plans ;
  skos:member agift:water-quality-monitoring ;
  skos:member agift:water-resources ;
  skos:member agift:water-usage-management ;
  skos:member agift:waterway-management ;
  skos:member agift:website-development ;
  skos:member agift:weights-and-measures-standards ;
  skos:member agift:whistleblowing ;
  skos:member agift:wilderness-area-management ;
  skos:member agift:wildlife-sanctuary-management ;
  skos:member agift:workers-compensation-schemes ;
  skos:member agift:workplace-agreement-processes ;
  skos:member agift:workplace-discrimination-monitoring ;
  skos:member agift:workplace-equity-and-justice-programs ;
  skos:member agift:workplace-training ;
  skos:member agift:world-heritage-listings ;
  skos:prefLabel "Australian Governments' Interactive Functions Thesaurus (AGIFT)"@en ;
.
agift:accommodation-services
  rdf:type skos:Concept ;
  rdfs:label "Accommodation Services"@en ;
  skos:broader agift:community-services ;
  skos:hiddenLabel "Homelessness support" ;
  skos:hiddenLabel "Housing services" ;
  skos:hiddenLabel "Indigenous housing" ;
  skos:hiddenLabel "Public housing services" ;
  skos:narrower agift:defence-housing ;
  skos:narrower agift:emergency-accommodation ;
  skos:narrower agift:public-housing-entitlements ;
  skos:narrower agift:refuge-support ;
  skos:prefLabel "Accommodation Services"@en ;
  skos:related agift:public-housing ;
.
agift:administrative-decision-appeal
  rdf:type skos:Concept ;
  rdfs:label "Administrative decision appeal"@en ;
  skos:broader agift:administrative-law ;
  skos:definition """Developing processes to support applications to an independent authority to have a determination or judgement reviewed. Includes activities associated with receiving and managing appeals.

See also JUSTICE ADMINISTRATION - Administrative law - Administrative decision review: for the process of reconsidering a determination and handing down a new decision.""" ;
  skos:hiddenLabel "Administrative appeals" ;
  skos:hiddenLabel "Appeals" ;
  skos:prefLabel "Administrative decision appeal"@en ;
  skos:related agift:administrative-decision-review ;
.
agift:administrative-decision-review
  rdf:type skos:Concept ;
  rdfs:label "Administrative decision review"@en ;
  skos:broader agift:administrative-law ;
  skos:definition """Examining and reconsidering a determination or judgement made by a public authority. Responding to the advice of an independent body which may reverse or uphold an earlier decision.

See also JUSTICE ADMINISTRATION - Administrative law - Administrative decision appeal: for applications to have a determination reconsidered.""" ;
  skos:hiddenLabel "Independent review" ;
  skos:hiddenLabel "Ombudsman" ;
  skos:prefLabel "Administrative decision review"@en ;
  skos:related agift:administrative-decision-appeal ;
.
agift:administrative-law
  rdf:type skos:Concept ;
  rdfs:label "Administrative law"@en ;
  skos:broader agift:justice-administration ;
  skos:definition "Administering the body of law that relates to the executive functions of government. Establishing the relationship between the government and the citizens of its jurisdiction. Regulating the powers, duties and organisation of public administration authorities." ;
  skos:hiddenLabel "Executive government" ;
  skos:hiddenLabel "Public authorities" ;
  skos:hiddenLabel "Tribunals" ;
  skos:narrower agift:administrative-decision-appeal ;
  skos:narrower agift:administrative-decision-review ;
  skos:narrower agift:censorship-standards ;
  skos:narrower agift:copyright-regulation ;
  skos:narrower agift:freedom-of-information ;
  skos:narrower agift:recordkeeping-standards ;
  skos:prefLabel "Administrative law"@en ;
  skos:related agift:public-administration ;
.
agift:adoption-services
  rdf:type skos:Concept ;
  rdfs:label "Adoption services"@en ;
  skos:broader agift:community-support ;
  skos:definition """Assisting parents seeking to legally take responsibility for a child, or birth parents wishing to have their child adopted. Includes advice on the legal aspects of adoption and monitoring the adoption of overseas children.

See also COMMUNITY SERVICES - Community support - Childcare services: for emergency and foster care.

See also COMMUNITY SERVICES - Community support - Family reunion programs: for helping birth parents and adopted children make contact.""" ;
  skos:hiddenLabel "Child adoption services" ;
  skos:hiddenLabel "Overseas adoption services" ;
  skos:prefLabel "Adoption services"@en ;
  skos:related agift:child-care-services ;
.
agift:adult-education-programs
  rdf:type skos:Concept ;
  rdfs:label "Adult education programs"@en ;
  skos:broader agift:community-education ;
  skos:definition """Administering training designed to meet the needs of specific groups of adult learners. Includes life skills, literacy programs and bridging courses to assist adults moving into school, tertiary or vocational education.

See also COMMUNITY SERVICES - Community support - Child and youth support: for parental education programs.

See also HEALTH CARE - Community health services - Health promotion: for basic information to support good health.""" ;
  skos:hiddenLabel "Adult literacy" ;
  skos:hiddenLabel "Bridging courses" ;
  skos:hiddenLabel "Health education" ;
  skos:hiddenLabel "Learning English" ;
  skos:hiddenLabel "Sex education" ;
  skos:hiddenLabel "Third age learning" ;
  skos:prefLabel "Adult education programs"@en ;
  skos:related agift:child-and-youth-support ;
  skos:related agift:primary-health-care ;
.
agift:adult-migrant-education
  rdf:type skos:Concept ;
  rdfs:label "Adult migrant education"@en ;
  skos:broader agift:community-education ;
  skos:definition """Administering training designed to assist adults from various ethnic backgrounds to live and work in Australia. Includes English language programs, courses on Australian society and laws, learning to deal with government or health facilities.

See also EDUCATION AND TRAINING - School education - Special needs programs: for educational assistance to migrant children.

See also IMMIGRATION - Migrant services: for other programs to assist citizens from various ethnic backgrounds.""" ;
  skos:hiddenLabel "English-as-a-second-language courses" ;
  skos:hiddenLabel "Immigrant education" ;
  skos:hiddenLabel "Migrant education" ;
  skos:prefLabel "Adult migrant education"@en ;
  skos:related agift:interpreter-services ;
  skos:related agift:migrant-services ;
  skos:related agift:special-needs-programs ;
.
agift:advertising-campaigns
  rdf:type skos:Concept ;
  rdfs:label "Advertising campaigns"@en ;
  skos:broader agift:tourist-event-promotion ;
  skos:definition """Delivering television, printed and electronic marketing, public relations and information programs to promote Australia or a particular region as a travel and tourism destination. Includes advertising campaigns to promote tourist events and local products.

See also COMMUNICATIONS - Government media: for managing media releases and dealing with journalists.

See also COMMUNICATIONS - Publishing: for producing information resources in print.""" ;
  skos:hiddenLabel "Tourist advertising" ;
  skos:prefLabel "Advertising campaigns"@en ;
  skos:related agift:government-media ;
.
agift:advertising-standards
  rdf:type skos:Concept ;
  rdfs:label "Advertising standards"@en ;
  skos:broader agift:communications ;
  skos:definition """Regulating the content and presentation of marketing material disseminated via any medium. Developing guidelines to guard against misleading or offensive advertising. Providing advice on the implementation of standards and monitoring compliance.

See also BUSINESS SUPPORT AND REGULATION - Business sponsorship: for restricting the advertisement of certain products at events.

See also BUSINESS SUPPORT AND REGULATION - Consumer protection: for handling complaints about advertising.

See also COMMUNICATIONS - Broadcasting - Broadcasting standards: for regulating the content of other material disseminated via mass media.

See also GOVERNANCE - Electoral matters - Election campaigning: for regulating the media activities of election candidates and political parties.""" ;
  skos:hiddenLabel "Commercial standards" ;
  skos:hiddenLabel "Media advertising standards" ;
  skos:hiddenLabel "Radio advertising standards" ;
  skos:hiddenLabel "Television advertising standards" ;
  skos:prefLabel "Advertising standards"@en ;
  skos:related agift:broadcasting-standards ;
  skos:related agift:business-sponsorship ;
  skos:related agift:censorship-standards ;
.
agift:aged-care-services
  rdf:type skos:Concept ;
  rdfs:label "Aged care services"@en ;
  skos:broader agift:community-support ;
  skos:definition """Managing social support and services for elderly persons and their families. Providing advice on rights to financial or other assistance such as residential care or medical services. Includes funding and support for community-based or volunteer programs providing aged care services.

See also COMMUNITY SERVICES - Community support - Veterans' entitlements: for services to returned defence services personnel.

See also COMMUNITY SERVICES - Financial assistance: for monetary support to aged persons.

See also HEALTH CARE - Special needs services: for aged care health programs.

See also HEALTH CARE - Special needs services - Independent living services: for in-home care.

See also HEALTH CARE - Special needs services - Residential services: for live-in aged care facilities.""" ;
  skos:hiddenLabel "Aged care standards" ;
  skos:hiddenLabel "Aged persons services" ;
  skos:hiddenLabel "Geriatric services" ;
  skos:prefLabel "Aged care services"@en ;
  skos:related agift:special-needs-services ;
  skos:related agift:veterans-entitlements ;
.
agift:agreement-bargaining-processes
  rdf:type skos:Concept ;
  rdfs:label "Agreement bargaining processes"@en ;
  skos:broader agift:workplace-agreement-processes ;
  skos:definition "Negotiating agreements to regulate the conduct of employer and employees across an organisation, or between an employer and an individual employee. Includes consultation between parties, drafting of agreements and liaison with bargaining agents or advisors." ;
  skos:hiddenLabel "Certified agreement negotiation" ;
  skos:hiddenLabel "Enterprise bargaining processes" ;
  skos:prefLabel "Agreement bargaining processes"@en ;
.
agift:agreement-dispute-mediation
  rdf:type skos:Concept ;
  rdfs:label "Agreement dispute mediation"@en ;
  skos:broader agift:workplace-agreement-processes ;
  skos:definition """Hearing disagreements between parties to a workplace agreement. Promoting conciliation and offering independent arbitration. Providing access to advice or representation. Managing resolution processes.

See also EMPLOYMENT - Human resources development - Workplace equity and justice programs: for resolving disputes with respect to harassment or discrimination.

See also EMPLOYMENT - Industrial awards and conditions: for disputes between parties operating under an award.""" ;
  skos:hiddenLabel "Certified agreement disputes" ;
  skos:hiddenLabel "Workplace agreement disputes" ;
  skos:prefLabel "Agreement dispute mediation"@en ;
  skos:related agift:workplace-equity-and-justice-programs ;
.
agift:agricultural-industry
  rdf:type skos:Concept ;
  rdfs:label "Agricultural industry"@en ;
  skos:broader agift:marine-and-rural-regulation ;
  skos:definition """Regulating crop and livestock farming industries. Administering quotas and issuing licenses for controlled activities. Certifying products and production methods. Conducting assessments and inspections to ensure compliance with standards and policy. Applying penalties for breaches of regulations.

See also PRIMARY INDUSTRIES - Marine and rural support - Horticultural industry: for programs to support and develop crop farming industries.

See also PRIMARY INDUSTRIES - Marine and rural support - Pastoral industry: for programs to support and develop livestock industries.

See also PRIMARY INDUSTRIES - Marine and rural support - Viticultural industry: for programs to support and develop grape growing and wine making industries.

See also SCIENCE - Agricultural sciences: for research into farming practices.""" ;
  skos:hiddenLabel "Animal food supplements" ;
  skos:hiddenLabel "Crop farming regulation" ;
  skos:hiddenLabel "Farming industries regulation" ;
  skos:hiddenLabel "Livestock industries regulation" ;
  skos:hiddenLabel "Pastoral lease registration" ;
  skos:hiddenLabel "Sustainable agriculture" ;
  skos:prefLabel "Agricultural industry"@en ;
  skos:related agift:horticultural-industry ;
  skos:related agift:pastoral-industry ;
  skos:related agift:viticultural-industry ;
.
agift:agricultural-sciences
  rdf:type skos:Concept ;
  rdfs:label "Agricultural sciences"@en ;
  skos:broader agift:science ;
  skos:definition """Conducting research into forestry, food, fibre and other crops or plants grown for commercial purposes. Providing input into quality control for the processing of agricultural products. Includes scientific advice on soil, weed and pest management, and information on new plant species.

See also ENVIRONMENT - Conservation programs - Soil preservation programs: for activities to improve or restore the quality of agricultural land.

See also PRIMARY INDUSTRIES - Chemical and pesticide regulation: for the registration and use of agricultural chemicals.

See also PRIMARY INDUSTRIES - Marine and rural support - Horticultural industry: for programs to support the commercial production of fruit and vegetables.

See also SCIENCE - Animal and veterinary sciences: for research into livestock health and management.

See also SCIENCE - Biological sciences - Biotechnology development: for research into the development of new plant species.

See also SCIENCE - Biological sciences - Botany: for research into non-commercial plants.

See also SCIENCE - Biological sciences - Genetic engineering: for research into the development of new plant species.""" ;
  skos:hiddenLabel "Agricultural research" ;
  skos:hiddenLabel "Farm research" ;
  skos:hiddenLabel "Farm sciences" ;
  skos:prefLabel "Agricultural sciences"@en ;
  skos:related agift:soil-preservation-programs ;
.
agift:air-force
  rdf:type skos:Concept ;
  rdfs:label "Air Force"@en ;
  skos:broader agift:australian-defence-forces ;
  skos:definition """Raising, equipping and maintaining the air capacity of Australia's defence forces. Administering Air Force activities, implementing defence policy and coordinating joint defence force operations. Includes on-the-job and basic training of new Air Force recruits.

See also DEFENCE - Australian Defence Forces - Reserves: for activities involving Air Force Reserves.

See also TRANSPORT - Air transport: for regulating the airline industry.""" ;
  skos:hiddenLabel "Airforce" ;
  skos:hiddenLabel "RAAF" ;
  skos:hiddenLabel "Royal Australian Air Force" ;
  skos:prefLabel "Air Force"@en ;
  skos:related agift:air-transport ;
  skos:related agift:reserves ;
.
agift:air-transport
  rdf:type skos:Concept ;
  rdfs:label "Air transport"@en ;
  skos:broader agift:transport ;
  skos:definition """Regulating the airline industry and developing policy relating to all aspects of private or commercial aviation. Administering air transport standards, security and services and maintaining air transport infrastructure. Includes liaison with other governments and international bodies to negotiate air lanes and airspace jurisdiction.

See also DEFENCE - Australian Defence Forces - Air Force: for the air capability of Australia's defence forces.

See also TRANSPORT - Freight movement regulation: for managing the transportation of goods by air.""" ;
  skos:hiddenLabel "Aerospace" ;
  skos:hiddenLabel "Airlines" ;
  skos:hiddenLabel "Airspace" ;
  skos:hiddenLabel "Aviation" ;
  skos:hiddenLabel "Civil aviation" ;
  skos:narrower agift:air-transport-safety ;
  skos:narrower agift:aircraft-standards ;
  skos:narrower agift:airport-services ;
  skos:prefLabel "Air transport"@en ;
  skos:related agift:air-force ;
.
agift:air-transport-safety
  rdf:type skos:Concept ;
  rdfs:label "Air transport safety"@en ;
  skos:broader agift:air-transport ;
  skos:definition """Regulating private and commercial aviation activities to improve security and reduce the risk of accidents or emergencies. Investigating accidents and incidents. Monitoring compliance with in-flight safety standards and regulations for security screening procedures. Includes training and advice, consultation and inspection services and cooperation on aviation safety issues across jurisdictions.

See also TRANSPORT - Air transport - Aircraft standards: for regulating the safe design, maintenance and operation of aircraft.

See also TRANSPORT - Air transport - Airport services: for air navigation support.""" ;
  skos:hiddenLabel "Accident investigation" ;
  skos:hiddenLabel "Air safety" ;
  skos:hiddenLabel "Airport security" ;
  skos:hiddenLabel "Safety investigation" ;
  skos:prefLabel "Air transport safety"@en ;
  skos:related agift:aircraft-standards ;
  skos:related agift:airport-services ;
.
agift:aircraft-standards
  rdf:type skos:Concept ;
  rdfs:label "Aircraft standards"@en ;
  skos:broader agift:air-transport ;
  skos:definition """Regulating the design, construction, maintenance and operation of any machine supported for flight - such as airplanes, helicopters, gliders or hot air balloons. Registering aircraft to ensure they meet agreed specifications and are fit to fly. Monitoring conformance through inspections, testing and licensing. Includes certification of personnel such as flight crews, pilots, aviation engineers and others engaged in the maintenance of aircraft and equipment.

See also SCIENCE - Applied sciences - Engineering and technology sciences: for research into the design and construction of aircraft.

See also SCIENCE - Earth sciences - Atmospheric sciences: for research into aerodynamics.""" ;
  skos:hiddenLabel "Aeroplanes" ;
  skos:hiddenLabel "Airline pilots" ;
  skos:hiddenLabel "Airplanes" ;
  skos:hiddenLabel "Pilots" ;
  skos:prefLabel "Aircraft standards"@en ;
  skos:related agift:air-transport-safety ;
  skos:related agift:engineering-and-technology-sciences ;
.
agift:airport-services
  rdf:type skos:Concept ;
  rdfs:label "Airport services"@en ;
  skos:broader agift:air-transport ;
  skos:definition """Managing facilities for aircraft take-off, landing and storage. Regulating air traffic and providing air navigation support. Monitoring air lanes and registering flight paths for private or commercial aircraft. Includes maintenance of airports and air transport infrastructure.

See also TRANSPORT - Air transport - Air transport safety: for regulation of security and screening procedures.

See also TRANSPORT - Passenger services: for managing the transportation of people by air.

See also TRANSPORT - Transport infrastructure development: for designing and installing transport systems.""" ;
  skos:hiddenLabel "Aerodromes" ;
  skos:hiddenLabel "Air navigation" ;
  skos:hiddenLabel "Air traffic control" ;
  skos:hiddenLabel "Airfields" ;
  skos:hiddenLabel "Airports" ;
  skos:hiddenLabel "Airstrips" ;
  skos:hiddenLabel "Airways" ;
  skos:hiddenLabel "Flight paths" ;
  skos:hiddenLabel "Flight regulation" ;
  skos:hiddenLabel "Landing strips" ;
  skos:hiddenLabel "Runways" ;
  skos:prefLabel "Airport services"@en ;
  skos:related agift:air-transport-safety ;
.
agift:ambulance-services
  rdf:type skos:Concept ;
  rdfs:label "Ambulance services"@en ;
  skos:broader agift:emergency-services ;
  skos:definition """Providing specially equipped vehicles and trained personnel to attend and transport sick or injured persons. Includes managing ambulance stations and attendance at special events.

See also COMMUNITY SERVICES - Natural disasters: for emergencies caused by the elements such as floods, earthquakes, and cyclones.

See also DEFENCE - Emergency management: for cross-jurisdictional operations to deal with large-scale emergencies.

See also EDUCATION AND TRAINING - Community education: for first aid training.""" ;
  skos:hiddenLabel "Aero-medical services" ;
  skos:hiddenLabel "Emergency transport" ;
  skos:hiddenLabel "Medical transport" ;
  skos:prefLabel "Ambulance services"@en ;
  skos:related agift:natural-disasters ;
.
agift:animal-and-veterinary-sciences
  rdf:type skos:Concept ;
  rdfs:label "Animal and veterinary sciences"@en ;
  skos:broader agift:science ;
  skos:definition """Conducting research into the health care and management of wild and domestic animals. Providing scientific advice on nutrition, breeding, diagnosis and treatment of diseases. Includes livestock, pets and other domestic animals, fish, birds and native animals - in the wild or in captivity.

See also PRIMARY INDUSTRIES - Chemical and pesticide regulation: for the registration and use of chemicals such as those used on livestock.

See also SCIENCE - Biological sciences - Entomology: for research into insects.

See also SCIENCE - Biological sciences - Physiology: for research into specific biological functions of animals.""" ;
  skos:hiddenLabel "Animal sciences" ;
  skos:hiddenLabel "Vet sciences" ;
  skos:hiddenLabel "Veterinary research" ;
  skos:hiddenLabel "Veterinary science" ;
  skos:prefLabel "Animal and veterinary sciences"@en ;
  skos:related agift:chemical-and-pesticide-regulation ;
.
agift:apparatus-licensing
  rdf:type skos:Concept ;
  rdfs:label "Apparatus licensing"@en ;
  skos:broader agift:radio-communication ;
  skos:definition """Administering standards for radio communications equipment. Monitoring compliance with government regulations. Processing licence applications for radio communications or transmission equipment. Ensuring that any emissions from apparatus, identified by qualified health authorities as being potentially harmful, are properly controlled.

See also SCIENCE - Medical and health sciences: for research into any health effects resulting from electromagnetic energy emissions from radio communications equipment.""" ;
  skos:hiddenLabel "Radio communication licensing" ;
  skos:prefLabel "Apparatus licensing"@en ;
  skos:related agift:medical-and-health-sciences ;
.
agift:applied-sciences
  rdf:type skos:Concept ;
  rdfs:label "Applied sciences"@en ;
  skos:broader agift:science ;
  skos:definition """Conducting research into the active use of scientific knowledge and principles from a range of fields and disciplines. Providing advice and practical solutions to problems in various sectors, such as industry, security, communications and health care.

See also SCIENCE - Biological sciences - Biotechnology development: for the application of scientific knowledge in a particular field.

See also SCIENCE - Earth sciences - Mineral exploration: for the application of scientific knowledge in a particular field.

See also SCIENCE - Medical and health sciences: for the application of scientific knowledge in a particular field.

See also SCIENCE - Spatial information research: for the application of scientific knowledge in a particular field.""" ;
  skos:hiddenLabel "Industrial chemistry" ;
  skos:narrower agift:engineering-and-technology-sciences ;
  skos:narrower agift:weights-and-measures-standards ;
  skos:prefLabel "Applied sciences"@en ;
  skos:related agift:biotechnology-development ;
  skos:related agift:physical-sciences ;
.
agift:appointment-management
  rdf:type skos:Concept ;
  rdfs:label "Appointment management"@en ;
  skos:broader agift:governance ;
  skos:definition "Management of appointments authorised by the Governor-General and Prime-Minister to support portfolio responsibilities." ;
  skos:prefLabel "Appointment management"@en ;
.
agift:apprenticeship-programs
  rdf:type skos:Concept ;
  rdfs:label "Apprenticeship programs"@en ;
  skos:broader agift:vocational-education ;
  skos:definition """Administering programs of industry-based training for trade and technical vocations. Monitoring compliance with standards and guidelines. Managing accreditation processes. Implementing schemes to assist employers to take on apprentices.

See also EDUCATION AND TRAINING - Vocational education - Trainee programs: for industry-based training in other vocational areas.

See also EMPLOYMENT - Industrial awards and conditions: for the employment conditions of apprentices.""" ;
  skos:hiddenLabel "Trade apprenticeships" ;
  skos:prefLabel "Apprenticeship programs"@en ;
  skos:related agift:trainee-programs ;
.
agift:aquaculture-industry
  rdf:type skos:Concept ;
  rdfs:label "Aquaculture industry"@en ;
  skos:broader agift:marine-and-rural-support ;
  skos:definition """Administering programs to support marine and freshwater fish or crop farming. Assisting industry growth and development. Encouraging businesses to adopt innovative practices, processes and products. Providing advice on production methods and business management to improve competitiveness.

See also ENVIRONMENT - Oceans governance: for management of ocean-based resources.

See also PRIMARY INDUSTRIES - Marine and rural regulation - Fisheries industry: for monitoring and regulating fishing industries.

See also SCIENCE - Animal and veterinary science: for fish and shellfish research.""" ;
  skos:hiddenLabel "Fish farming industry" ;
  skos:prefLabel "Aquaculture industry"@en ;
  skos:related agift:oceans-governance ;
.
agift:architectural-services
  rdf:type skos:Concept ;
  rdfs:label "Architectural services"@en ;
  skos:broader agift:civic-management ;
  skos:definition """Providing professional advice and supervising the design and construction of public buildings. Approving plans and conducting inspections to ensure building is completed in accordance with approved plans. Includes heritage value assessments.

See also CIVIC INFRASTRUCTURE - Civic management - Building regulations and standards: for ensuring structures meet legal requirements.

See also CIVIC INFRASTRUCTURE - Civic management - Engineering services: for professional advice on the design and construction of public works.

See also ENVIRONMENT - Built environment - Building preservation: for programs to conserve buildings of heritage value.""" ;
  skos:hiddenLabel "Architect services" ;
  skos:hiddenLabel "Architecture" ;
  skos:hiddenLabel "Building design services" ;
  skos:hiddenLabel "Heritage value assessments" ;
  skos:prefLabel "Architectural services"@en ;
  skos:related agift:building-preservation ;
  skos:related agift:building-regulations-and-standards ;
  skos:related agift:engineering-services ;
  skos:related agift:public-housing-construction ;
  skos:related agift:public-housing-design ;
.
agift:army
  rdf:type skos:Concept ;
  rdfs:label "Army"@en ;
  skos:broader agift:australian-defence-forces ;
  skos:definition """Raising, equipping and maintaining the land capability of Australia's defence forces. Administering Army activities, implementing defence policy and coordinating joint defence forces operations. Includes on-the-job and basic training of new Army recruits.

See also DEFENCE - Australian Defence Forces - Reserves: for activities involving Army Reserves.

See also EDUCATION AND TRAINING - Military education and training - Army reserve training: for educational programs for Army Reservists.""" ;
  skos:hiddenLabel "Australian Army" ;
  skos:prefLabel "Army"@en ;
  skos:related agift:reserves ;
.
agift:army-reserve-training
  rdf:type skos:Concept ;
  rdfs:label "Army reserve training"@en ;
  skos:broader agift:military-education-and-training ;
  skos:definition """Administering educational programs for part-time voluntary defence units in the Army. Providing ongoing training through coursework and residential schools. Includes liaison with employers when sustained absence from work is required.

See also DEFENCE - Australian Defence Forces - Reserves: for management of part-time voluntary defence units in the Army, Navy or Air Force.""" ;
  skos:hiddenLabel "Army reserves" ;
  skos:hiddenLabel "Reserve training" ;
  skos:prefLabel "Army reserve training"@en ;
  skos:related agift:reserves ;
.
agift:artefact-export-regulation
  rdf:type skos:Concept ;
  rdfs:label "Artefact export regulation"@en ;
  skos:broader agift:collection-management ;
  skos:definition """Negotiating the international movement of cultural material. Liaising with government and private sector bodies for the temporary import or export of artefacts for exhibition purposes. Obtaining valuations to confirm the worth of items. Assisting the return of illegally imported cultural property. Seeking export prevention orders for protected artefacts.

See also INDIGENOUS AFFAIRS - Indigenous cultural heritage - Cultural artefact repatriation: for returning Indigenous cultural materials to their traditional owners.

See also TRADE - Export regulation - Prohibited export control: for policy governing the international movement of cultural material.

See also TRADE - Import regulation - Prohibited import control: for policy governing the international movement of cultural material.""" ;
  skos:hiddenLabel "Art export" ;
  skos:hiddenLabel "Cultural material export regulation" ;
  skos:prefLabel "Artefact export regulation"@en ;
  skos:related agift:cultural-artefact-repatriation ;
  skos:related agift:prohibited-export-control ;
  skos:related agift:prohibited-import-control ;
.
agift:arts-development
  rdf:type skos:Concept ;
  rdfs:label "Arts development"@en ;
  skos:broader agift:cultural-affairs ;
  skos:definition """Providing support for the production of skilled performance or craft. Administering programs to develop funding and promotional strategies for the arts, and to encourage participation from across the community. Assisting the growth of artistic companies such as orchestras and dance companies through business advice and planning. Includes support for work spaces and liaison with education and exhibition facilities.

See also EDUCATION AND TRAINING - Arts education: for programs to further artistic talent at individual or community level.

See also TRADE - Export regulation - Export promotion: for advertising Australian cultural industries in the global marketplace.

See also TRADE - Trade development programs: for cultural industry assistance programs.""" ;
  skos:hiddenLabel "Arts councils" ;
  skos:hiddenLabel "Ballet" ;
  skos:hiddenLabel "Creative arts development" ;
  skos:hiddenLabel "Dance" ;
  skos:hiddenLabel "Film industry development" ;
  skos:hiddenLabel "Fine arts development" ;
  skos:hiddenLabel "Indigenous arts development" ;
  skos:hiddenLabel "Literary arts development" ;
  skos:hiddenLabel "Musical arts development" ;
  skos:hiddenLabel "Opera" ;
  skos:hiddenLabel "Performing arts development" ;
  skos:hiddenLabel "Visual arts development" ;
  skos:narrower agift:arts-funding ;
  skos:narrower agift:arts-incentive-schemes ;
  skos:narrower agift:arts-promotion ;
  skos:prefLabel "Arts development"@en ;
  skos:related agift:arts-education ;
.
agift:arts-education
  rdf:type skos:Concept ;
  rdfs:label "Arts education"@en ;
  skos:broader agift:education-and-training ;
  skos:definition """Administering programs that offer training and facilities to support the production of skilled performance or craft. Managing specialised institutions or schemes to foster artistic talent at individual or community level. Includes the provision of scholarships and study grants.

See also CULTURAL AFFAIRS - Arts development: for supporting cultural industries.

See also INTERNATIONAL RELATIONS - Overseas aid programs - Overseas student scholarship programs: for access to higher education for students from developing countries or the Pacific region.""" ;
  skos:hiddenLabel "Arts councils" ;
  skos:prefLabel "Arts education"@en ;
  skos:related agift:arts-development ;
  skos:related agift:school-education ;
  skos:related agift:tertiary-education ;
.
agift:arts-funding
  rdf:type skos:Concept ;
  rdfs:label "Arts funding"@en ;
  skos:broader agift:arts-development ;
  skos:definition "Providing financial support for the production of skilled performance or craft. Assessing applications for funding. Allocating grants and subsidies to projects that meet selection criteria. Advising artists about funding programs and application procedures." ;
  skos:hiddenLabel "Art subsidy schemes" ;
  skos:hiddenLabel "Artistic grants" ;
  skos:prefLabel "Arts funding"@en ;
.
agift:arts-incentive-schemes
  rdf:type skos:Concept ;
  rdfs:label "Arts incentive schemes"@en ;
  skos:broader agift:arts-development ;
  skos:definition """Developing strategies to encourage investment in artistic activities or moveable cultural materials. Negotiating tax deductions for approved activities and setting guidelines for donor benefits. Certifying valuers to assess the worth of artistic works. Maintaining a register of cultural organisations qualified to offer incentives.

See also CULTURAL AFFAIRS - Cultural gifts programs: for managing the donation of artistic materials under arts incentive schemes.""" ;
  skos:hiddenLabel "Register of cultural organisations" ;
  skos:hiddenLabel "Taxation incentives for the arts" ;
  skos:prefLabel "Arts incentive schemes"@en ;
  skos:related agift:cultural-gifts-programs ;
.
agift:arts-promotion
  rdf:type skos:Concept ;
  rdfs:label "Arts promotion"@en ;
  skos:broader agift:arts-development ;
  skos:definition """Managing programs to encourage participation in artistic pursuits and support for performances or exhibitions. Developing strategies for marketing and information dissemination to raise community awareness of the arts.

See also CULTURAL AFFAIRS - Collection promotion: for strategies to raise the profiles of cultural institutions and their holdings.""" ;
  skos:hiddenLabel "Arts marketing" ;
  skos:prefLabel "Arts promotion"@en ;
  skos:related agift:collection-promotion ;
.
agift:asset-assessment
  rdf:type skos:Concept ;
  rdfs:label "Asset assessment"@en ;
  skos:broader agift:retirement-income ;
  skos:definition """Estimating the value of resources owned by a retired individual in order to identify applicable taxes or benefits. Determining whether an asset meets criteria for exemption or inclusion for assessment purposes.

See also COMMUNITY SERVICES - Financial assistance: for monetary support to individuals.""" ;
  skos:hiddenLabel "Retiree assets" ;
  skos:hiddenLabel "Retirement assets" ;
  skos:prefLabel "Asset assessment"@en ;
  skos:related agift:financial-assistance ;
.
agift:association-registration
  rdf:type skos:Concept ;
  rdfs:label "Association registration"@en ;
  skos:definition """Recording the details of incorporated associations. Assessing applications and issuing registration numbers. Maintaining records of registered details. Processing registration updates and renewals.

See also BUSINESS SUPPORT AND REGULATION - Business registration and licensing: for recording details of companies.

See also JUSTICE ADMINISTRATION - Associations and corporate law: for regulating the formation and governance of companies and associations.""" ;
  skos:hiddenLabel "Incorporation" ;
  skos:hiddenLabel "Organisation registration" ;
  skos:prefLabel "Association registration"@en ;
  skos:related agift:associations-and-corporate-law ;
  skos:related agift:business-registration-and-licensing ;
  skos:related agift:fundraising-and-donation-schemes ;
  skos:related agift:sport-and-fitness-development ;
.
agift:associations-and-corporate-law
  rdf:type skos:Concept ;
  rdfs:label "Associations and corporate law"@en ;
  skos:broader agift:justice-administration ;
  skos:definition """Administering the body of law that relates to companies or other organisations that have a distinct legal identity from that of their members. Regulating the formation, governance and dissolution of such organisations and establishing the limits of their powers or liability.

See also BUSINESS SUPPORT AND REGULATION - Association registration: for recording and issuing registrations.""" ;
  skos:hiddenLabel "Business law" ;
  skos:hiddenLabel "Corporate law" ;
  skos:hiddenLabel "Corporations law" ;
  skos:narrower agift:bankruptcy-proceedings ;
  skos:narrower agift:merger-regulation ;
  skos:prefLabel "Associations and corporate law"@en ;
  skos:related agift:association-registration ;
.
agift:astronomical-sciences
  rdf:type skos:Concept ;
  rdfs:label "Astronomical sciences"@en ;
  skos:broader agift:physical-sciences ;
  skos:definition """Conducting research into celestial bodies, such as planets, stars, solar systems and galaxies. Measuring motions, positions, distances, magnitudes and structures to understand the states of matter and physical processes in space. Includes radio astronomy and the management of telescopes, observatories and other specialist equipment.

See also COMMUNICATIONS - Satellite communication: for management of equipment in space.""" ;
  skos:hiddenLabel "Astronomy" ;
  skos:hiddenLabel "Cosmology" ;
  skos:hiddenLabel "Space research" ;
  skos:prefLabel "Astronomical sciences"@en ;
  skos:related agift:satellite-communication ;
.
agift:athlete-scholarship-programs
  rdf:type skos:Concept ;
  rdfs:label "Athlete scholarship programs"@en ;
  skos:broader agift:sport-and-fitness-development ;
  skos:definition """Administering schemes to encourage excellence in sport across local and national levels. Providing financial assistance to highly skilled athletes to attend advanced training programs. Enabling access to elite facilities, performance coaching, sports science services, career planning and education services. Sponsoring travel, accommodation and living expenses to support attendance at competitions.

See also SPORT AND RECREATION - Sport and fitness development - Sporting grants administration: for allocation of funding to athletes in target groups.""" ;
  skos:hiddenLabel "Athletics scholarships" ;
  skos:hiddenLabel "Sports scholarships" ;
  skos:prefLabel "Athlete scholarship programs"@en ;
  skos:related agift:sporting-grants-administration ;
.
agift:atmospheric-sciences
  rdf:type skos:Concept ;
  rdfs:label "Atmospheric sciences"@en ;
  skos:broader agift:earth-sciences ;
  skos:definition """Conducting research into weather, climate and air pollution. Providing scientific advice on severe weather and climatic variation, such as acid deposition and ozone depletion. Includes middle atmosphere climate and space weather analysis, studies of the thermosphere and observatory experiments.

See also COMMUNITY SERVICES - Natural disasters: for emergency response to severe weather conditions.

See also ENVIRONMENT - Climate information services: for providing climatic advice and weather forecasts.""" ;
  skos:hiddenLabel "Atmospheric research" ;
  skos:hiddenLabel "Climate change" ;
  skos:hiddenLabel "Climate research" ;
  skos:hiddenLabel "Global warming" ;
  skos:hiddenLabel "Greenhouse effect" ;
  skos:hiddenLabel "Ionospheric prediction" ;
  skos:hiddenLabel "Meteorology" ;
  skos:hiddenLabel "Weather research" ;
  skos:prefLabel "Atmospheric sciences"@en ;
  skos:related agift:natural-disasters ;
.
agift:atomic-and-molecular-sciences
  rdf:type skos:Concept ;
  rdfs:label "Atomic and molecular sciences"@en ;
  skos:broader agift:physical-sciences ;
  skos:definition """Conducting research into the structure and nature of the smallest particles of matter. Analysing the interaction of atoms with electromagnetic radiation, and changes to their chemical identity, weight or behaviour. Observing atomic reactions to identify or develop products or processes for use in medical, industrial or defence applications, or to support other fields of scientific research.

See also SCIENCE - Biological sciences - Biochemistry: for molecular biology.

See also SCIENCE - Physical sciences - Nuclear sciences: for research into subatomic particles.""" ;
  skos:hiddenLabel "Atomic research" ;
  skos:hiddenLabel "Molecular science" ;
  skos:prefLabel "Atomic and molecular sciences"@en ;
  skos:related agift:biochemistry ;
.
agift:australian-defence-forces
  rdf:type skos:Concept ;
  rdfs:label "Australian Defence Forces"@en ;
  skos:broader agift:defence ;
  skos:definition """Maintaining and administering the combined Australian Defence Forces to ensure Australia's ability to resist foreign aggression or attack. Includes policies and programs for the development of the defence forces as a whole, arrangements for force generation, mobilisation and support.

See also EDUCATION AND TRAINING - Military education and training: for training and development programs for defence personnel.

See also INTERNATIONAL RELATIONS - Defence liaison: for cooperating with other countries in defence matters.""" ;
  skos:hiddenLabel "ADF" ;
  skos:hiddenLabel "Armed forces" ;
  skos:hiddenLabel "Defence forces" ;
  skos:hiddenLabel "Military forces" ;
  skos:narrower agift:air-force ;
  skos:narrower agift:army ;
  skos:narrower agift:badges-and-insignia ;
  skos:narrower agift:cadets ;
  skos:narrower agift:defence-force-commands ;
  skos:narrower agift:military-bands ;
  skos:narrower agift:navy ;
  skos:narrower agift:reserves ;
  skos:prefLabel "Australian Defence Forces"@en ;
  skos:related agift:military-education-and-training ;
  skos:related agift:military-exercises ;
.
agift:australian-theatre-of-war
  rdf:type skos:Concept ;
  rdfs:label "Australian theatre of war"@en ;
  skos:broader agift:military-operations ;
  skos:definition """Coordinating activities across the entire air, sea and land areas where Australia is likely to be directly involved in warfare or military action. Planning and conducting campaigns for the defence of Australia and its interests.

See also DEFENCE - Military operations - Special operations: for unconventional warfare or the deployment of highly trained military personnel.

See also DEFENCE - Military operations - Warfare: for entering into armed combat with opposing defence forces.""" ;
  skos:hiddenLabel "Campaigns" ;
  skos:hiddenLabel "Theatre of war" ;
  skos:prefLabel "Australian theatre of war"@en ;
  skos:related agift:special-operations ;
  skos:related agift:warfare ;
.
agift:authentication
  rdf:type skos:Concept ;
  rdfs:label "Authentication"@en ;
  skos:broader agift:electronic-commerce ;
  skos:definition """Managing infrastructure to support the validation of electronic transactions to ensure commerce can be conducted free from abuse or fraud. Includes accreditation of certification authorities, management of public key certificates, related agreements and audits.

See also COMMUNICATIONS - Electronic commerce - Online transaction standards: for standards governing electronic commerce.

See also SECURITY - Information security: for data security standards.""" ;
  skos:hiddenLabel "Digital signatures" ;
  skos:hiddenLabel "Electronic signatures" ;
  skos:hiddenLabel "Encryption" ;
  skos:hiddenLabel "Online security" ;
  skos:hiddenLabel "PKI" ;
  skos:hiddenLabel "Public Key Technology" ;
  skos:prefLabel "Authentication"@en ;
  skos:related agift:information-security ;
  skos:related agift:online-transaction-standards ;
.
agift:award-conditions
  rdf:type skos:Concept ;
  rdfs:label "Award conditions"@en ;
  skos:broader agift:industrial-awards-and-conditions ;
  skos:definition """Implementing the provisions of industrial awards with regard to employment conditions and rates of pay. Providing advice on hours of work, working conditions, leave and other entitlements. Administering the payment of wages, allowances, overtime and penalties.

See also EMPLOYMENT - Human resources development - Occupational health and safety: for programs to prevent death, injury or disease in the workplace.


See also EMPLOYMENT - Workplace agreement processes - Certified employment conditions: for implementing the provisions of certified agreements.""" ;
  skos:hiddenLabel "Allowances" ;
  skos:hiddenLabel "Annual leave" ;
  skos:hiddenLabel "Award wages" ;
  skos:hiddenLabel "Bereavement leave" ;
  skos:hiddenLabel "Carer's leave" ;
  skos:hiddenLabel "Employment conditions" ;
  skos:hiddenLabel "Entitlements" ;
  skos:hiddenLabel "Junior wages" ;
  skos:hiddenLabel "Leave entitlements" ;
  skos:hiddenLabel "Long service leave" ;
  skos:hiddenLabel "Maternity leave" ;
  skos:hiddenLabel "Minimum wage" ;
  skos:hiddenLabel "Overtime rates" ;
  skos:hiddenLabel "Parental leave" ;
  skos:hiddenLabel "Penalty rates" ;
  skos:hiddenLabel "Personal leave" ;
  skos:hiddenLabel "Rates of pay and salary" ;
  skos:hiddenLabel "Salary regulation" ;
  skos:hiddenLabel "Shift penalties" ;
  skos:hiddenLabel "Sick leave" ;
  skos:hiddenLabel "Wages" ;
  skos:hiddenLabel "Work life balance" ;
  skos:hiddenLabel "Working conditions" ;
  skos:hiddenLabel "Youth wages and allowances" ;
  skos:prefLabel "Award conditions"@en ;
  skos:related agift:occupational-health-and-safety ;
.
agift:badges-and-insignia
  rdf:type skos:Concept ;
  rdfs:label "Badges and insignia"@en ;
  skos:broader agift:australian-defence-forces ;
  skos:definition """Managing military badges, insignia, crests, medals and awards. Registering designs and regulating their use. Includes ceremonies for conferring military awards.

See also GOVERNANCE - Honours and award programs: for civilian tributes and decorations.""" ;
  skos:hiddenLabel "Defence badges" ;
  skos:hiddenLabel "Medals" ;
  skos:hiddenLabel "Military awards" ;
  skos:hiddenLabel "Military badges" ;
  skos:hiddenLabel "Military insignia" ;
  skos:hiddenLabel "Military medals" ;
  skos:prefLabel "Badges and insignia"@en ;
  skos:related agift:honours-and-awards-programs ;
.
agift:bankruptcy-proceedings
  rdf:type skos:Concept ;
  rdfs:label "Bankruptcy proceedings"@en ;
  skos:broader agift:associations-and-corporate-law ;
  skos:definition "Administering insolvent parties' assets for the benefit of creditors. Includes providing bankruptcy notices, winding up of companies and the appointment of trustees." ;
  skos:hiddenLabel "Insolvency proceedings" ;
  skos:hiddenLabel "Receivership management" ;
  skos:prefLabel "Bankruptcy proceedings"@en ;
.
agift:benefits
  rdf:type skos:Concept ;
  rdfs:label "Benefits"@en ;
  skos:broader agift:financial-assistance ;
  skos:definition """Administering programs to provide financial assistance to individuals, based on criteria other than income. Providing advice on entitlements. Assessing eligibility and processing payments. Includes ongoing benefits, one-off payments following a specific event, rebates for costs already incurred or subsidies for upcoming expenses.

See also COMMUNITY SERVICES - Community support - Veteran's entitlements: for social support to returned service personnel.

See also COMMUNITY SERVICES - Financial assistance - Income support schemes: for financial assistance to those with low earnings.

See also FINANCE MANAGEMENT - Taxation - Taxation compliance: for payments made by individuals through withholding schemes.

See also INDIGENOUS AFFAIRS - Indigenous welfare programs: for social support to Aboriginal and Islander communities.""" ;
  skos:hiddenLabel "Allowances" ;
  skos:hiddenLabel "Baby bonus" ;
  skos:hiddenLabel "Entitlements" ;
  skos:hiddenLabel "Farmer's rebate" ;
  skos:hiddenLabel "Financial incentives" ;
  skos:hiddenLabel "First homeowner's grant" ;
  skos:hiddenLabel "Gap cover" ;
  skos:hiddenLabel "LPG subsidy scheme" ;
  skos:hiddenLabel "Maternity payment" ;
  skos:hiddenLabel "Pharmaceutical benefits" ;
  skos:hiddenLabel "Private health insurance rebate" ;
  skos:hiddenLabel "Rebates" ;
  skos:hiddenLabel "Seniors cards" ;
  skos:hiddenLabel "Subsidies" ;
  skos:prefLabel "Benefits"@en ;
  skos:related agift:veterans-entitlements ;
.
agift:biochemistry
  rdf:type skos:Concept ;
  rdfs:label "Biochemistry"@en ;
  skos:broader agift:biological-sciences ;
  skos:definition """Conducting research into the chemical processes and molecular makeup of plants, animals and micro-organisms. Investigating the biological functions of plants and animals at a cellular level. Includes DNA and serum analysis.

See also SCIENCE - Biological sciences - Genetic engineering: for analysis and manipulation of reproductive cells.""" ;
  skos:hiddenLabel "Cell biology" ;
  skos:hiddenLabel "Molecular biology" ;
  skos:prefLabel "Biochemistry"@en ;
  skos:related agift:atomic-and-molecular-sciences ;
  skos:related agift:genetic-engineering ;
.
agift:biodiversity-preservation
  rdf:type skos:Concept ;
  rdfs:label "Biodiversity preservation"@en ;
  skos:broader agift:biological-sciences ;
  skos:definition """Conducting research into the variety of plant and animal life in a region, and the actions necessary to conserve and sustain it. Identifying biota of environmental or economic significance. Includes studies of the origin, evolution and relationships between native plant and animal species, and programs to reintroduce locally extinct organisms in certain habitats.

See also ENVIRONMENT - Conservation programs: for activities to protect and sustain plant or animal life in a region.""" ;
  skos:hiddenLabel "Biodiversity management" ;
  skos:hiddenLabel "Biodiversity" ;
  skos:prefLabel "Biodiversity preservation"@en ;
  skos:related agift:conservation-programs ;
.
agift:biological-sciences
  rdf:type skos:Concept ;
  rdfs:label "Biological sciences"@en ;
  skos:broader agift:science ;
  skos:definition """Conducting research into the lives of plants, animals and micro-organisms. Investigating their origin, distribution, behaviour and physical makeup. Includes studies of evolution, ecosystem dynamics, identification and manipulation of biological processes.

See also SCIENCE - Medical and health sciences: for research into human health and disease.""" ;
  skos:hiddenLabel "Biology" ;
  skos:hiddenLabel "Life sciences" ;
  skos:narrower agift:biochemistry ;
  skos:narrower agift:biodiversity-preservation ;
  skos:narrower agift:biotechnology-development ;
  skos:narrower agift:botany ;
  skos:narrower agift:entomology ;
  skos:narrower agift:genetic-engineering ;
  skos:narrower agift:physiology ;
  skos:prefLabel "Biological sciences"@en ;
  skos:related agift:medical-and-health-sciences ;
.
agift:biotechnology-development
  rdf:type skos:Concept ;
  rdfs:label "Biotechnology development"@en ;
  skos:broader agift:biological-sciences ;
  skos:definition """Conducting research into the use of living things to make or alter organic material. Involves the use of micro-organisms or fungi, or strategies such as selective breeding to develop products for medical, agricultural and other commercial purposes. Includes health and environmental impact assessment of biotechnology products.

See also DEFENCE - Defence strategic support - Defence science and technology: for the application of specialist knowledge to military activities.

See also PRIMARY INDUSTRIES - Marine and rural regulation - Food quality assurance: for regulating the use of biotechnology in food production.

See also SCIENCE - Biological sciences - Genetic engineering: for artificial modification of cellular material.""" ;
  skos:hiddenLabel "Fermentation" ;
  skos:hiddenLabel "Genetically modified organisms" ;
  skos:hiddenLabel "Grafting" ;
  skos:hiddenLabel "Selective breeding" ;
  skos:prefLabel "Biotechnology development"@en ;
  skos:related agift:applied-sciences ;
  skos:related agift:defence-science-and-technology ;
.
agift:blood-and-organ-donation-management
  rdf:type skos:Concept ;
  rdfs:label "Blood and organ donation management"@en ;
  skos:broader agift:public-health-services ;
  skos:definition "Developing policies and programs to establish a nationally coordinated approach to blood, organ and tissue donation. Promoting measures to raise community awareness of blood, organ and tissue donation." ;
  skos:prefLabel "Blood and organ donation management"@en ;
.
agift:border-protection
  rdf:type skos:Concept ;
  rdfs:label "Border protection"@en ;
  skos:broader agift:national-security ;
  skos:definition """Coordinating operations to monitor Australian borders for unauthorised sea or air arrivals. Developing and implementing response procedures to prevent illegal entry. Includes liaison with law enforcement, immigration or defence services personnel to apprehend individuals who breach Australia’s borders.
See also IMMIGRATION - Detention programs: for the custody and treatment of illegal immigrants.
See also TRADE - Import regulation - Prohibited import control: for customs surveillance.""" ;
  skos:hiddenLabel "Coastal surveillance" ;
  skos:hiddenLabel "Coastwatch" ;
  skos:hiddenLabel "Maritime surveillance" ;
  skos:prefLabel "Border protection"@en ;
.
agift:botany
  rdf:type skos:Concept ;
  rdfs:label "Botany"@en ;
  skos:broader agift:biological-sciences ;
  skos:definition """Conducting research into the structure, classification and distribution of plants. Developing taxonomic and geographic representations of botanical collections. Investigating potential uses for plant products in medicine or industry. Providing plant identification and botanical information services.

See also PRIMARY INDUSTRIES - Marine and rural support - Silvicultural industry: for programs that support the commercial cultivation of forests.

See also SCIENCE - Biological sciences - Physiology: for research into specific biological functions of plants.""" ;
  skos:hiddenLabel "Botanical research" ;
  skos:prefLabel "Botany"@en ;
  skos:related agift:silvicultural-industry ;
.
agift:broadcasting
  rdf:type skos:Concept ;
  rdfs:label "Broadcasting"@en ;
  skos:broader agift:communications ;
  skos:definition "Developing policy to support and regulate industries that transmit content simultaneously to many recipients. Providing advice on the introduction of new technology and the effects of government communications policy on the broadcasting industry. Encouraging the use of mass marketing and content distribution strategies. Supporting the editorial and programming independence of national broadcasters. Includes liaison with arts and cultural sectors." ;
  skos:hiddenLabel "Cable television services" ;
  skos:hiddenLabel "Community broadcasting" ;
  skos:hiddenLabel "Digital television services" ;
  skos:hiddenLabel "Internet television services" ;
  skos:hiddenLabel "Mass media services" ;
  skos:hiddenLabel "Multicultural broadcasting" ;
  skos:hiddenLabel "National broadcasters" ;
  skos:hiddenLabel "Pay television services" ;
  skos:hiddenLabel "Satellite television services" ;
  skos:narrower agift:broadcasting-standards ;
  skos:narrower agift:radio-broadcasting ;
  skos:narrower agift:television-broadcasting ;
  skos:prefLabel "Broadcasting"@en ;
.
agift:broadcasting-standards
  rdf:type skos:Concept ;
  rdfs:label "Broadcasting standards"@en ;
  skos:broader agift:broadcasting ;
  skos:definition """Establishing principles and criteria for the operation of industries that transmit content simultaneously to many recipients. Monitoring industry compliance with government standards and guidelines for all broadcasting media. Includes local content quotas, children's programming, codes of practice and the protection of special events.

See also COMMUNICATIONS - Advertising standards: for the regulation of marketing material in any media.

See also JUSTICE ADMINISTRATION - Administrative law - Censorship standards: for criteria to regulate the accessibility of broadcast content.""" ;
  skos:hiddenLabel "Australian broadcast standards" ;
  skos:hiddenLabel "Broadband standards" ;
  skos:hiddenLabel "Children's television standards" ;
  skos:hiddenLabel "Film classification" ;
  skos:hiddenLabel "Local content standards" ;
  skos:hiddenLabel "Online content standards" ;
  skos:hiddenLabel "Video classification" ;
  skos:prefLabel "Broadcasting standards"@en ;
  skos:related agift:advertising-standards ;
  skos:related agift:media-ownership-regulation ;
  skos:related agift:online-transaction-standards ;
  skos:related agift:radio-broadcasting ;
  skos:related agift:television-broadcasting ;
.
agift:building-acoustics
  rdf:type skos:Concept ;
  rdfs:label "Building acoustics"@en ;
  skos:broader agift:built-environment ;
  skos:definition "Administering programs to assess the integrity of built structures. Conducting inspections to evaluate the safety of old buildings, transport infrastructure, dams and other elements of the built environment. Monitoring compliance with maintenance standards." ;
  skos:hiddenLabel "Structural integrity assessment" ;
  skos:prefLabel "Building acoustics"@en ;
.
agift:building-approval-services
  rdf:type skos:Concept ;
  rdfs:label "Building approval services"@en ;
  skos:broader agift:civic-management ;
  skos:definition """Assessing applications for the building of new structures and the alteration or demolition of existing structures. Approving applications that meet town planning and building regulations. Providing advice on applications that cannot be supported. Includes liaison across jurisdictions where joint approval is required.

See also NATURAL RESOURCES - Land use planning - Land use zoning: for assessing land development applications.""" ;
  skos:hiddenLabel "Building alterations" ;
  skos:hiddenLabel "Building applications" ;
  skos:hiddenLabel "Construction approval services" ;
  skos:hiddenLabel "Demolition approval services" ;
  skos:hiddenLabel "Housing approval services" ;
  skos:prefLabel "Building approval services"@en ;
  skos:related agift:land-use-zoning ;
  skos:related agift:town-planning ;
.
agift:building-preservation
  rdf:type skos:Concept ;
  rdfs:label "Building preservation"@en ;
  skos:broader agift:built-environment ;
  skos:definition """Administering programs to maintain and protect built structures of particular historic, scientific or social significance. Issuing orders to prevent demolition, alteration or damage. Monitoring compliance with building preservation standards. Conducting inspections to ensure building modifications do not diminish heritage value.

See also CIVIC INFRASTRUCTURE - Civic management - Architectural services: for heritage value assessments.""" ;
  skos:hiddenLabel "Building conservation" ;
  skos:hiddenLabel "Heritage building preservation" ;
  skos:prefLabel "Building preservation"@en ;
  skos:related agift:architectural-services ;
  skos:related agift:conservation-programs ;
.
agift:building-regulations-and-standards
  rdf:type skos:Concept ;
  rdfs:label "Building regulations and standards"@en ;
  skos:broader agift:civic-management ;
  skos:definition """Setting rules and guidelines for building new structures and altering or demolishing existing structures. Conducting assessments and inspections to ensure compliance with regulations and standards. Providing information and advice on building regulations and standards.

See also CIVIC INFRASTRUCTURE - Civic management - Architectural services: for professional advice on the design and construction of public buildings.

See also CIVIC INFRASTRUCTURE - Civic management - Engineering services: for professional advice on the design and construction of public works.""" ;
  skos:hiddenLabel "Building standards" ;
  skos:hiddenLabel "Building surveyors" ;
  skos:prefLabel "Building regulations and standards"@en ;
  skos:related agift:architectural-services ;
.
agift:built-environment
  rdf:type skos:Concept ;
  rdfs:label "Built environment"@en ;
  skos:broader agift:environment ;
  skos:definition """Developing policy and programs to protect structures of particular historic, scientific or social significance. Establishing standards for maintaining and preserving elements of the built environment. Providing funding for joint projects with business or the community.

See also ENVIRONMENT - Historic relic protection: for programs to conserve significant artefacts.

See also ENVIRONMENT - Natural heritage protection: for programs to conserve the biological environment.

See also INDIGENOUS AFFAIRS - Indigenous heritage conservation: for protecting areas directly associated with Aboriginal and Torres Strait Islander culture.""" ;
  skos:hiddenLabel "National Estate preservation" ;
  skos:narrower agift:building-acoustics ;
  skos:narrower agift:building-preservation ;
  skos:prefLabel "Built environment"@en ;
  skos:related agift:historic-relic-protection ;
  skos:related agift:indigenous-heritage-conservation ;
  skos:related agift:natural-heritage-protection ;
.
agift:burial-ground-management
  rdf:type skos:Concept ;
  rdfs:label "Burial ground management"@en ;
  skos:broader agift:public-land-management ;
  skos:definition """Administering areas of land set aside for depositing the bodies or ashes of the dead. Managing site layout. Ensuring facilities are kept clean and maintained. Monitoring rights of access and opening hours. Liaising with funeral directors, church and community groups. Includes war graves and overseas burial grounds managed by the Australian Government.

See also CIVIC INFRASTRUCTURE - Public land management - Memorial maintenance: for managing commemorative structures.""" ;
  skos:hiddenLabel "Cemeteries" ;
  skos:hiddenLabel "Cemetery management" ;
  skos:hiddenLabel "Crematorium management" ;
  skos:hiddenLabel "Graveyard management" ;
  skos:hiddenLabel "War graves management" ;
  skos:prefLabel "Burial ground management"@en ;
  skos:related agift:memorial-maintenance ;
.
agift:business-association
  rdf:type skos:Concept ;
  rdfs:label "Business association"@en ;
  skos:definition """Recording the details of incorporated associations. Assessing applications and issuing registration numbers. Maintaining records of registered details. Processing registration updates and renewals.

See also BUSINESS SUPPORT AND REGULATION - Business registration and licensing: for recording details of companies.

See also JUSTICE ADMINISTRATION - Associations and corporate law: for regulating the formation and governance of companies and associations.""" ;
  skos:prefLabel "Business association"@en ;
  skos:related agift:business-registration-and-licensing ;
.
agift:business-process-auditing
  rdf:type skos:Concept ;
  rdfs:label "Business process auditing"@en ;
  skos:broader agift:business-support-and-regulation ;
  skos:definition """Administering programs to examine the accounts and records of government or private sector bodies. Reviewing the performance or financial management of an organisation. Verifying statements or claims made in official reports. Providing recommendations for improvement.

See also JUSTICE ADMINISTRATION - Administrative law - Recordkeeping standards: for capturing evidence of business activities.""" ;
  skos:hiddenLabel "Auditing" ;
  skos:prefLabel "Business process auditing"@en ;
  skos:related agift:government-auditing ;
  skos:related agift:recordkeeping-standards ;
.
agift:business-registration-and-licensing
  rdf:type skos:Concept ;
  rdfs:label "Business registration and licensing"@en ;
  skos:broader agift:business-support-and-regulation ;
  skos:definition """Recording the details of companies and corporations. Assessing applications and issuing registration numbers. Maintaining records of registered details. Processing registration updates and renewals. Issuing licenses and permits, such as those required for fundraising, the sale of alcohol or signage and displays.

See also BUSINESS SUPPORT AND REGULATION - Association registration: for recording details of incorporated associations.

See also JUSTICE ADMINISTRATION - Associations and corporate law: for regulating the formation and governance of companies and associations.

See also SPORT AND RECREATION - Gaming industry regulation: for issuing poker machine licenses.""" ;
  skos:hiddenLabel "Australian Business Number" ;
  skos:hiddenLabel "Australian Business Register" ;
  skos:hiddenLabel "Australian Company Number" ;
  skos:hiddenLabel "Australian Registered Body Number" ;
  skos:hiddenLabel "Business licensing" ;
  skos:hiddenLabel "Business names" ;
  skos:hiddenLabel "Business permits and licences" ;
  skos:hiddenLabel "Business registration number" ;
  skos:hiddenLabel "Fundraising permits" ;
  skos:hiddenLabel "GST registration" ;
  skos:hiddenLabel "Liquor licensing" ;
  skos:hiddenLabel "PAYG registration" ;
  skos:prefLabel "Business registration and licensing"@en ;
  skos:related agift:association-registration ;
  skos:related agift:business-association ;
  skos:related agift:income-assessment ;
.
agift:business-sponsorship
  rdf:type skos:Concept ;
  rdfs:label "Business sponsorship"@en ;
  skos:broader agift:business-support-and-regulation ;
  skos:definition """Regulating corporate funding of organisations and events. Restricting the advertising of some types of products or services at events. Providing information about sponsorship applications and how to meet obligations in relation to marketing and merchandising.

See also BUSINESS SUPPORT AND REGULATION - Fair trading compliance - Trade practices compliance: for regulating the conduct of business transactions.

See also COMMUNICATIONS - Advertising standards: for regulating the content and presentation of marketing material.

See also SPORT AND RECREATION - Sport and fitness development - Fundraising and donation schemes: for programs to encourage investment in sporting events.

See also TRADE - Intellectual property management: for protecting the ownership of corporate designs and logos.""" ;
  skos:hiddenLabel "Business sponsors" ;
  skos:hiddenLabel "Corporate sponsors" ;
  skos:hiddenLabel "Corporate sponsorship" ;
  skos:hiddenLabel "Sponsorship" ;
  skos:hiddenLabel "Sports advertising" ;
  skos:prefLabel "Business sponsorship"@en ;
  skos:related agift:advertising-standards ;
  skos:related agift:trade-practices-compliance ;
.
agift:business-support-and-regulation
  rdf:type skos:Concept ;
  rdfs:label "BUSINESS SUPPORT AND REGULATION"@en ;
  skos:definition "Formulating policy to regulate and support the private sector, including small business and non-profit organisations. Developing strategies to assist business growth and management. Implementing advocacy programs, providing funding and administering regulatory bodies." ;
  skos:hiddenLabel "Industry" ;
  skos:narrower agift:business-process-auditing ;
  skos:narrower agift:business-registration-and-licensing ;
  skos:narrower agift:business-sponsorship ;
  skos:narrower agift:consumer-protection ;
  skos:narrower agift:fair-trading-compliance ;
  skos:narrower agift:financial-institutions-regulation ;
  skos:narrower agift:government-procurement-regulation ;
  skos:narrower agift:industry-assistance-schemes ;
  skos:narrower agift:industry-development ;
  skos:narrower agift:insurance-regulation ;
  skos:narrower agift:professional-accreditation ;
  skos:narrower agift:small-business-services ;
  skos:narrower agift:stock-market-regulation ;
  skos:prefLabel "BUSINESS SUPPORT AND REGULATION"@en ;
  skos:related agift:primary-industries ;
  skos:related agift:trade ;
.
agift:cadets
  rdf:type skos:Concept ;
  rdfs:label "Cadets"@en ;
  skos:broader agift:australian-defence-forces ;
  skos:definition """Managing the Australian Defence Force Cadets and similar programs to recruit and develop young service personnel. Developing, sponsoring and promoting Cadet activity programs and recruitment procedures. Includes Officers and Instructors of Cadets, Australian Navy Cadets, Australian Army Cadets and Australian Air Force Cadets.

See also EDUCATION AND TRAINING - Military education and training - Defence college training: for educational programs provided exclusively to defence personnel.""" ;
  skos:hiddenLabel "Cadet training" ;
  skos:hiddenLabel "Military cadets" ;
  skos:prefLabel "Cadets"@en ;
  skos:related agift:defence-college-training ;
.
agift:call-centre-administration
  rdf:type skos:Concept ;
  rdfs:label "Call centre administration"@en ;
  skos:broader agift:communications ;
  skos:definition "Managing facilities where trained staff are available to answer questions or provide advice via the telephone. Promoting the use of call centres to facilitate public access to government information." ;
  skos:hiddenLabel "Advice lines" ;
  skos:hiddenLabel "Telephone assistance services" ;
  skos:prefLabel "Call centre administration"@en ;
.
agift:capital-equipment-programs
  rdf:type skos:Concept ;
  rdfs:label "Capital equipment programs"@en ;
  skos:broader agift:defence-strategic-support ;
  skos:definition """Administering projects to purchase or build the physical resources to support Australia's defence forces and military operations. Cataloguing major equipment and scheduling refurbishment or disposal. Includes, but is not limited to, the management of weaponry, vehicles, aircraft, seagoing vessels, communications and surveillance equipment.

See also DEFENCE - Defence strategic support - Defence industry: for administering trade in military equipment.""" ;
  skos:hiddenLabel "Capital equipment acquisition" ;
  skos:hiddenLabel "Defence equipment" ;
  skos:hiddenLabel "Military equipment" ;
  skos:prefLabel "Capital equipment programs"@en ;
  skos:related agift:defence-industry ;
.
agift:caravan-and-camping-services
  rdf:type skos:Concept ;
  rdfs:label "Caravan and camping services"@en ;
  skos:broader agift:sport-and-recreation ;
  skos:definition """Regulating the provision of sites where caravans, tents and other temporary dwellings may be erected. Certifying the safety of campsite facilities and the hygiene of amenities. Providing advice to operators on administration, emergency procedures and insurance. Includes public information services, such as the production of maps and promotional literature.

See also TOURISM - Tourism industry development: for programs to support campsite businesses.""" ;
  skos:hiddenLabel "Camping grounds" ;
  skos:hiddenLabel "Campsites" ;
  skos:hiddenLabel "Caravan parks" ;
  skos:prefLabel "Caravan and camping services"@en ;
  skos:related agift:tourism-industry-development ;
.
agift:cargo-control
  rdf:type skos:Concept ;
  rdfs:label "Cargo control"@en ;
  skos:broader agift:maritime-services ;
  skos:definition """Developing policy for the transportation of goods by sea. Monitoring compliance with regulations and international standards for carriage of hazardous materials, dangerous goods and oversize containers. Includes advice on best practice cargo handling, loading and management.

See also EMPLOYMENT - Human resources development - Occupational health and safety: for working environment conditions.

See also MARITIME SERVICES - Port regulation: for managing sea-based entry and exit points.

See also TRADE - Export regulation: for trade controls.

See also TRADE - Import regulation: for trade controls.

See also TRANSPORT - Freight movement regulation: for transporting goods by air, rail or road.""" ;
  skos:hiddenLabel "Hazardous materials management" ;
  skos:hiddenLabel "Hazardous waste management" ;
  skos:hiddenLabel "Stevedores" ;
  skos:hiddenLabel "Stevedoring" ;
  skos:prefLabel "Cargo control"@en ;
  skos:related agift:export-regulation ;
  skos:related agift:freight-movement-regulation ;
  skos:related agift:import-regulation ;
  skos:related agift:occupational-health-and-safety ;
.
agift:carriage-service-providers
  rdf:type skos:Concept ;
  rdfs:label "Carriage service providers"@en ;
  skos:broader agift:telecommunications ;
  skos:definition "Monitoring the activities of suppliers of telecommunications services. Regulating the construction of facilities, installation and maintenance of equipment such as cables and optical fibre. Ensuring compliance with pricing guidelines and standards of service." ;
  skos:hiddenLabel "Telecommunications carriers" ;
  skos:prefLabel "Carriage service providers"@en ;
.
agift:carrier-licensing
  rdf:type skos:Concept ;
  rdfs:label "Carrier licensing"@en ;
  skos:broader agift:telecommunications ;
  skos:definition "Processing applications and issuing licenses to suppliers of telecommunications services. Drafting licence conditions. Monitoring compliance with legislative obligations and reporting requirements." ;
  skos:hiddenLabel "Telecommunications licensing" ;
  skos:prefLabel "Carrier licensing"@en ;
.
agift:censorship-standards
  rdf:type skos:Concept ;
  rdfs:label "Censorship standards"@en ;
  skos:broader agift:administrative-law ;
  skos:definition """Regulating the accessibility of various kinds of content for television, literature, film, radio or theatre. Establishing criteria to classify content and determine its availability to the public.

See also COMMUNICATIONS - Advertising standards: for implementing censorship standards in advertising.

See also COMMUNICATIONS - Broadcasting - Broadcasting standards: for implementing censorship standards in radio and television broadcasting.

See also COMMUNICATIONS - Publishing - Publishing standards: for implementing censorship standards in the print media.""" ;
  skos:hiddenLabel "Film classification" ;
  skos:hiddenLabel "Radio censorship" ;
  skos:hiddenLabel "Television censorship" ;
  skos:hiddenLabel "Video classification" ;
  skos:prefLabel "Censorship standards"@en ;
  skos:related agift:advertising-standards ;
  skos:related agift:publishing-standards ;
.
agift:ceremonial-events-and-representation
  rdf:type skos:Concept ;
  rdfs:label "Ceremonial events and representation"@en ;
  skos:broader agift:official-protocol ;
  skos:definition """Organising the attendance of high-level government officials at formal public occasions, either in Australia or overseas. Providing advice on conduct during ritual or traditional proceedings. Making arrangements to support official protocol such as determining guest lists, producing formal invitations, providing acceptances or apologies.

See also GOVERNANCE - Official protocol - Head of Government protocol: for the conduct of leaders in carrying out official or ceremonial duties.

See also GOVERNANCE - Official protocol - Official visits: for organising travel and itineraries for business, cultural or social visits by high-level government officials.""" ;
  skos:hiddenLabel "Official representation" ;
  skos:prefLabel "Ceremonial events and representation"@en ;
  skos:related agift:head-of-government-protocol ;
  skos:related agift:official-hospitality ;
  skos:related agift:official-visits ;
.
agift:certified-employment-conditions
  rdf:type skos:Concept ;
  rdfs:label "Certified employment conditions"@en ;
  skos:broader agift:workplace-agreement-processes ;
  skos:definition """Implementing the provisions of workplace agreements with regard to working conditions, rates of pay and performance management. Providing advice on hours of work, employment conditions, leave and other entitlements. Administering the payment of wages, allowances, overtime and penalties.

See also EMPLOYMENT - Human resources development - Occupational health and safety: for programs to prevent death, injury or disease in the workplace.

See also EMPLOYMENT - Industrial awards and conditions - Award conditions: for implementing the provisions of industrial awards.""" ;
  skos:hiddenLabel "Allowances" ;
  skos:hiddenLabel "Annual leave" ;
  skos:hiddenLabel "Bereavement leave" ;
  skos:hiddenLabel "Carer's leave" ;
  skos:hiddenLabel "Employment conditions" ;
  skos:hiddenLabel "Entitlements" ;
  skos:hiddenLabel "Junior wages" ;
  skos:hiddenLabel "Leave entitlements" ;
  skos:hiddenLabel "Long service leave" ;
  skos:hiddenLabel "Maternity leave" ;
  skos:hiddenLabel "Overtime rates" ;
  skos:hiddenLabel "Parental leave" ;
  skos:hiddenLabel "Penalty rates" ;
  skos:hiddenLabel "Performance management" ;
  skos:hiddenLabel "Personal leave" ;
  skos:hiddenLabel "Rates of pay and salary" ;
  skos:hiddenLabel "Salary regulation" ;
  skos:hiddenLabel "Shift penalties" ;
  skos:hiddenLabel "Sick leave" ;
  skos:hiddenLabel "Wages" ;
  skos:hiddenLabel "Work life balance" ;
  skos:hiddenLabel "Working conditions" ;
  skos:hiddenLabel "Youth wages and allowances" ;
  skos:prefLabel "Certified employment conditions"@en ;
  skos:related agift:occupational-health-and-safety ;
.
agift:charting-sea-lanes
  rdf:type skos:Concept ;
  rdfs:label "Charting sea lanes"@en ;
  skos:broader agift:navigation ;
  skos:definition """Administering programs to map the location of shipping channels and established routes for watercraft. Developing graphic representations to record special conditions or geographical features.

See also MARITIME SERVICES - Port regulation: for supervising the maintenance of shipping channels.

See also SCIENCE - Spatial information research: for investigating practical applications for geographical data.""" ;
  skos:hiddenLabel "Sea lane mapping" ;
  skos:hiddenLabel "Shipping channel mapping" ;
  skos:prefLabel "Charting sea lanes"@en ;
  skos:related agift:port-regulation ;
.
agift:chemical-and-pesticide-regulation
  rdf:type skos:Concept ;
  rdfs:label "Chemical and pesticide regulation"@en ;
  skos:broader agift:primary-industries ;
  skos:definition """Monitoring the use of substances to control weeds, insects and other pests that affect primary production. Maintaining a register of approved agricultural or veterinary chemicals and pesticides. Assessing product applications, specifying conditions of use and maximum residue limits. Conducting routine inspections to ensure compliance.

See also DEFENCE - Military operations - Warfare: for chemical warfare.

See also ENVIRONMENT - Conservation programs - Soil preservation programs: for counteracting the effects of chemical contamination.""" ;
  skos:hiddenLabel "Herbicide regulation" ;
  skos:hiddenLabel "Insecticide regulation" ;
  skos:hiddenLabel "Maximum residue limits" ;
  skos:hiddenLabel "Pesticide regulation" ;
  skos:hiddenLabel "Veterinary chemical regulation" ;
  skos:prefLabel "Chemical and pesticide regulation"@en ;
  skos:related agift:animal-and-veterinary-sciences ;
  skos:related agift:drugs-and-poisons-regulation ;
  skos:related agift:entomology ;
  skos:related agift:warfare ;
.
agift:child-and-youth-support
  rdf:type skos:Concept ;
  rdfs:label "Child and youth support"@en ;
  skos:broader agift:community-support ;
  skos:definition """Providing and monitoring services for young people. Assisting those who are disadvantaged or at risk of abuse or domestic violence. Running parent education programs and managing youth centres. Includes funding and support for community-based or volunteer programs providing child and youth support.

See also FINANCE MANAGEMENT - Taxation - Taxation compliance: for the provision of child support payments.""" ;
  skos:hiddenLabel "Child protection services" ;
  skos:hiddenLabel "Child welfare" ;
  skos:hiddenLabel "Children's services" ;
  skos:hiddenLabel "Parental education programs" ;
  skos:hiddenLabel "Youth support services" ;
  skos:prefLabel "Child and youth support"@en ;
  skos:related agift:adult-education-programs ;
  skos:related agift:child-care-services ;
  skos:related agift:discipline-programs ;
  skos:related agift:early-childhood-education ;
  skos:related agift:health-promotion ;
  skos:related agift:juvenile-justice ;
  skos:related agift:taxation-compliance ;
.
agift:child-care-services
  rdf:type skos:Concept ;
  rdfs:label "Child-care services"@en ;
  skos:broader agift:community-support ;
  skos:definition """Providing services for the supervision of children when their parents are not available. Monitoring private sector staff and facilities for compliance with industry standards. Includes temporary arrangements for emergency or foster care.

See also COMMUNITY SERVICES - Community support - Child and youth support: for programs to assist young people and their parents.

See also COMMUNITY SERVICES - Financial assistance: for child-care subsidies.

See also EDUCATION AND TRAINING - Early childhood education: for fostering learning and development in young children.

See also FINANCE MANAGEMENT - Taxation - Taxation compliance: for the provision of child support payments.""" ;
  skos:hiddenLabel "Babysitting services" ;
  skos:hiddenLabel "Child minding services" ;
  skos:hiddenLabel "Child-care centres" ;
  skos:hiddenLabel "Day care services" ;
  skos:hiddenLabel "Nursery schools" ;
  skos:hiddenLabel "Playgroup services" ;
  skos:prefLabel "Child-care services"@en ;
  skos:related agift:adoption-services ;
  skos:related agift:child-and-youth-support ;
.
agift:citizenship
  rdf:type skos:Concept ;
  rdfs:label "Citizenship"@en ;
  skos:broader agift:immigration ;
  skos:definition """Developing policy for Australian nationality, including the rights and obligations of citizens. Defining the legal status of Australian citizens, and the management of citizenship when people migrate. Establishing criteria for the naturalisation of immigrants. Promoting the value of Australian citizenship.

See also IMMIGRATION - Travel authorisation: for permanent entry policy.""" ;
  skos:hiddenLabel "Dual citizenship" ;
  skos:hiddenLabel "Nationality" ;
  skos:hiddenLabel "Naturalisation policy" ;
  skos:narrower agift:naturalisation-assessment ;
  skos:narrower agift:presentation-arrangements ;
  skos:prefLabel "Citizenship"@en ;
  skos:related agift:travel-authorisation ;
.
agift:civic-celebrations
  rdf:type skos:Concept ;
  rdfs:label "Civic celebrations"@en ;
  skos:broader agift:governance ;
  skos:definition """Organising community events and ceremonies to mark significant occasions. Coordinating security, publicity and entertainment. Arranging adequate public facilities, car parking and seating. Includes liaison with local businesses, volunteers and community groups.

See also CULTURAL AFFAIRS - Cultural festivals: for events that highlight artistic, literary or heritage-related activities.

See also CULTURAL AFFAIRS - Multicultural heritage promotion - Multicultural festivals: for events that highlight Australia's cultural diversity.

See also GOVERNANCE - Official protocol - Ceremonial events and representation: for attendance of high-ranking government officers at celebrations and events.

See also IMMIGRATION - Citizenship - Presentation arrangements: for citizenship ceremonies.""" ;
  skos:hiddenLabel "ANZAC Day services" ;
  skos:hiddenLabel "Australia Day celebrations" ;
  skos:hiddenLabel "Celebrations" ;
  skos:hiddenLabel "Centenary of Federation" ;
  skos:hiddenLabel "Commemorative services" ;
  skos:hiddenLabel "Federation celebrations" ;
  skos:hiddenLabel "Queen's birthday celebrations" ;
  skos:prefLabel "Civic celebrations"@en ;
  skos:related agift:cultural-festivals ;
  skos:related agift:presentation-arrangements ;
.
agift:civic-infrastructure
  rdf:type skos:Concept ;
  rdfs:label "CIVIC INFRASTRUCTURE"@en ;
  skos:definition "Developing policy to support the growth of towns and cities. Implementing programs to manage urban development and maintain essential services. Installing buildings and services to meet the administrative, social and recreational needs of local residents." ;
  skos:hiddenLabel "Bridges" ;
  skos:hiddenLabel "Buildings" ;
  skos:hiddenLabel "Dams" ;
  skos:hiddenLabel "Public works" ;
  skos:narrower agift:civic-management ;
  skos:narrower agift:energy-supply ;
  skos:narrower agift:housing-industry-policy ;
  skos:narrower agift:infrastructure-planning ;
  skos:narrower agift:integrated-services-planning ;
  skos:narrower agift:place-names ;
  skos:narrower agift:public-housing ;
  skos:narrower agift:public-land-management ;
  skos:narrower agift:regional-development ;
  skos:narrower agift:transport-network-maintenance ;
  skos:narrower agift:waste-management ;
  skos:prefLabel "CIVIC INFRASTRUCTURE"@en ;
  skos:related agift:crown-land-administration ;
  skos:related agift:mobile-telephone-services ;
  skos:related agift:spatial-information-research ;
.
agift:civic-management
  rdf:type skos:Concept ;
  rdfs:label "Civic management"@en ;
  skos:broader agift:civic-infrastructure ;
  skos:definition "Developing programs to provide integrated support for town planning and building projects. Coordinating government building projects and managing input from multiple parties. Defining responsibilities for projects that cross jurisdictional boundaries." ;
  skos:hiddenLabel "Urban development" ;
  skos:narrower agift:architectural-services ;
  skos:narrower agift:building-approval-services ;
  skos:narrower agift:building-regulations-and-standards ;
  skos:narrower agift:engineering-services ;
  skos:narrower agift:planning-approvals ;
  skos:narrower agift:town-planning ;
  skos:prefLabel "Civic management"@en ;
.
agift:civil-community-assistance
  rdf:type skos:Concept ;
  rdfs:label "Civil community assistance"@en ;
  skos:broader agift:emergency-management ;
  skos:definition """Managing the allocation of defence resources to protect the civilian population from the effects of hostilities or emergencies. Providing support to civil emergency services in times of natural disaster. Includes identifying lines of communication, chain of command, and establishing criteria for situations warranting defence forces assistance.

See also DEFENCE - Emergency management - Disaster support: for emergency defence force assistance to other countries.""" ;
  skos:hiddenLabel "Civil defence" ;
  skos:hiddenLabel "Civil disaster support" ;
  skos:hiddenLabel "Community disaster support" ;
  skos:hiddenLabel "Defence forces assistance" ;
  skos:hiddenLabel "Military assistance" ;
  skos:prefLabel "Civil community assistance"@en ;
  skos:related agift:disaster-support ;
.
agift:civil-law
  rdf:type skos:Concept ;
  rdfs:label "Civil law"@en ;
  skos:broader agift:justice-administration ;
  skos:definition "Administering the body of law that relates to social behaviour and the ordinary private matters of individuals. Establishing property rights, determining legal relationships and responsibilities." ;
  skos:narrower agift:civil-registration ;
  skos:narrower agift:conveyancing ;
  skos:narrower agift:dispute-mediation-programs ;
  skos:narrower agift:family-law-proceedings ;
  skos:narrower agift:probate-applications ;
  skos:prefLabel "Civil law"@en ;
.
agift:civil-registration
  rdf:type skos:Concept ;
  rdfs:label "Civil registration"@en ;
  skos:broader agift:civil-law ;
  skos:definition "Administering the registration of major life events, such as births, marriages and deaths. Issuing certificates and keeping records to support other civil law processes." ;
  skos:hiddenLabel "Birth certificates" ;
  skos:hiddenLabel "Death certificates" ;
  skos:hiddenLabel "Marriage certificates" ;
  skos:hiddenLabel "Registrar" ;
  skos:prefLabel "Civil registration"@en ;
.
agift:climate-information-services
  rdf:type skos:Concept ;
  rdfs:label "Climate information services"@en ;
  skos:broader agift:environment ;
  skos:definition """Providing climatic advice, information on prevailing conditions and weather forecasts. Issuing alerts for severe weather. Includes drought monitoring and updates on seasonal climate variability.

See also COMMUNITY SERVICES - Natural disasters: for emergency response to severe weather conditions.

See also SCIENCE - Earth sciences - Atmospheric sciences: for meteorology and climate research.""" ;
  skos:hiddenLabel "Weather forecasting" ;
  skos:prefLabel "Climate information services"@en ;
  skos:related agift:natural-disasters ;
.
agift:clinical-health-services
  rdf:type skos:Concept ;
  rdfs:label "Clinical health services"@en ;
  skos:broader agift:community-health-services ;
  skos:definition """Administering health programs that operate out of medical centres. Providing consultation services to allow diagnosis and treatment based on direct observation of the patient. Developing treatment care plans for medication or rehabilitation, and issuing referrals to support services.

See also COMMUNITY SERVICES - Counselling services: for the provision of group therapy or psychological advice.

See also HEALTH CARE - Special needs services: for programs to support individuals with medical conditions.

See also HEALTH CARE - Special needs services - Mental health services: for programs to treat or manage mental illness.""" ;
  skos:hiddenLabel "Family medical centres" ;
  skos:hiddenLabel "General practitioners" ;
  skos:hiddenLabel "Health clinics" ;
  skos:hiddenLabel "Medical centres" ;
  skos:hiddenLabel "Travel health clinics" ;
  skos:prefLabel "Clinical health services"@en ;
  skos:related agift:counselling-services ;
  skos:related agift:medical-quarantine-services ;
.
agift:collection-access
  rdf:type skos:Concept ;
  rdfs:label "Collection access"@en ;
  skos:broader agift:cultural-affairs ;
  skos:definition """Developing policy to assist the location and use of items held by cultural institutions. Establishing access procedures to meet legislative requirements. Providing advice about opening hours and membership or registration requirements. Includes development of online information to support remote access.

See also CULTURAL AFFAIRS - Collection access - Reference services: for personal or online assistance to clients.""" ;
  skos:narrower agift:descriptive-standards ;
  skos:narrower agift:finding-aids-development ;
  skos:narrower agift:reference-services ;
  skos:prefLabel "Collection access"@en ;
  skos:related agift:reference-services ;
.
agift:collection-accessioning
  rdf:type skos:Concept ;
  rdfs:label "Collection accessioning"@en ;
  skos:broader agift:collection-management ;
  skos:definition """Applying intellectual and physical control over items held by cultural institutions. Recording the essential details of materials as they are acquired. Includes accessioning (and de-accessioning) items for touring exhibitions and those on loan from other collections.

See also CULTURAL AFFAIRS - Collection access - Finding aids development: for creating tools to locate items in cultural collections.

See also CULTURAL AFFAIRS - Collection management - Collection acquisition: for seeking and obtaining new materials.""" ;
  skos:hiddenLabel "Accessioning" ;
  skos:hiddenLabel "Collection listing" ;
  skos:hiddenLabel "Index development" ;
  skos:prefLabel "Collection accessioning"@en ;
  skos:related agift:finding-aids-development ;
.
agift:collection-acquisition
  rdf:type skos:Concept ;
  rdfs:label "Collection acquisition"@en ;
  skos:broader agift:collection-management ;
  skos:definition """Seeking and receiving new materials for cultural institutions. Building a collection in accordance with policy and guidelines. Negotiating temporary use of items from other collections. Developing mechanisms to support a range of acquisition methods, such as purchases, donations, loans and joint investments.

See also CULTURAL AFFAIRS - Collection management - Collection accessioning for recording newly acquired materials.

See also CULTURAL AFFAIRS - Cultural gifts programs: for managing donations made under arts incentive schemes.""" ;
  skos:hiddenLabel "Acquisitions" ;
  skos:hiddenLabel "Art acquisitions" ;
  skos:hiddenLabel "Cultural materials acquisition" ;
  skos:prefLabel "Collection acquisition"@en ;
  skos:related agift:collection-management ;
.
agift:collection-management
  rdf:type skos:Concept ;
  rdfs:label "Collection management"@en ;
  skos:broader agift:cultural-affairs ;
  skos:definition "Developing policy for the acquisition, storage and preservation of cultural material and artefacts. Producing standards and guidelines for collection management procedures to ensure the safety of fragile or highly valuable items. Includes liaison with other institutions about the management of cultural materials." ;
  skos:hiddenLabel "Archival holdings management" ;
  skos:hiddenLabel "Collection development policy" ;
  skos:hiddenLabel "Holdings management" ;
  skos:hiddenLabel "Library collection management" ;
  skos:hiddenLabel "Museum collection management" ;
  skos:narrower agift:artefact-export-regulation ;
  skos:narrower agift:collection-accessioning ;
  skos:narrower agift:collection-acquisition ;
  skos:narrower agift:collection-storage ;
  skos:narrower agift:preservation-services ;
  skos:prefLabel "Collection management"@en ;
  skos:related agift:collection-acquisition ;
.
agift:collection-promotion
  rdf:type skos:Concept ;
  rdfs:label "Collection promotion"@en ;
  skos:broader agift:cultural-affairs ;
  skos:definition """Developing strategies to raise the profiles of cultural institutions and their holdings. Coordinating programs of events and publications. Establishing policy and guidelines to support exhibitions and marketing campaigns.

See also COMMUNICATIONS - Publishing: for producing information resources in print.

See also CULTURAL AFFAIRS - Arts development - Arts promotion: for strategies to encourage participation in artistic pursuits.""" ;
  skos:hiddenLabel "Cultural collection marketing" ;
  skos:narrower agift:exhibition-programs ;
  skos:narrower agift:publicity-programs ;
  skos:prefLabel "Collection promotion"@en ;
  skos:related agift:arts-promotion ;
  skos:related agift:publishing ;
.
agift:collection-storage
  rdf:type skos:Concept ;
  rdfs:label "Collection storage"@en ;
  skos:broader agift:collection-management ;
  skos:definition """Designing and managing facilities to house materials held by cultural institutions. Ensuring environmental conditions meet appropriate industry standards. Arranging facilities to support access and preservation guidelines.

See also CIVIC INFRASTRUCTURE - Public land management - Cultural centre management: for the administration of buildings that house cultural collections.""" ;
  skos:hiddenLabel "Records storage" ;
  skos:hiddenLabel "Repository management" ;
  skos:hiddenLabel "Stack management" ;
  skos:prefLabel "Collection storage"@en ;
  skos:related agift:cultural-centre-management ;
  skos:related agift:preservation-services ;
.
agift:commissions-of-inquiry
  rdf:type skos:Concept ;
  rdfs:label "Commissions of inquiry"@en ;
  skos:broader agift:justice-administration ;
  skos:definition "Establishing a body to investigate a special matter or designated subject. Conducting inquiries, hearing evidence, receiving submissions and reporting findings. Includes Royal Commissions and other bodies charged with similar duties." ;
  skos:hiddenLabel "Inquiries" ;
  skos:hiddenLabel "Royal Commissions" ;
  skos:hiddenLabel "Senate committees" ;
  skos:prefLabel "Commissions of inquiry"@en ;
.
agift:commonwealth-state-funding
  rdf:type skos:Concept ;
  rdfs:label "Commonwealth State funding"@en ;
  skos:broader agift:finance-management ;
  skos:definition "Administering the allocation of Commonwealth financial support to State governments. Conducting analysis to determine the appropriate distribution across jurisdictions. Includes general grants and specific-purpose payments as negotiated at Heads of Governments meetings." ;
  skos:hiddenLabel "Commonwealth funding" ;
  skos:hiddenLabel "Funding allocations" ;
  skos:hiddenLabel "State funding" ;
  skos:hiddenLabel "Vertical-fiscal balance" ;
  skos:prefLabel "Commonwealth State funding"@en ;
  skos:related agift:intergovernmental-relations ;
.
agift:communications
  rdf:type skos:Concept ;
  rdfs:label "COMMUNICATIONS"@en ;
  skos:definition "Supporting the growth and management of industries that facilitate the transmission of information. Regulating the provision of postal and telecommunication services to all citizens. Encouraging the development of standards for information management, information dissemination and information technology." ;
  skos:narrower agift:advertising-standards ;
  skos:narrower agift:broadcasting ;
  skos:narrower agift:call-centre-administration ;
  skos:narrower agift:electronic-commerce ;
  skos:narrower agift:government-media ;
  skos:narrower agift:information-management-standards ;
  skos:narrower agift:internet ;
  skos:narrower agift:media-ownership-regulation ;
  skos:narrower agift:postal-services ;
  skos:narrower agift:publishing ;
  skos:narrower agift:radio-communication ;
  skos:narrower agift:satellite-communication ;
  skos:narrower agift:telecommunications ;
  skos:prefLabel "COMMUNICATIONS"@en ;
  skos:related agift:navigation-systems-development ;
  skos:related agift:search-technology-development ;
.
agift:communications-infrastructure
  rdf:type skos:Concept ;
  rdfs:label "Communications infrastructure"@en ;
  skos:broader agift:telecommunications ;
  skos:definition "Developing policy and programs to support the provision and  management of physical communication infrastructure. Facilitating  communication industries including access for people with special needs and advising on the availability of new communications technology." ;
  skos:prefLabel "Communications infrastructure"@en ;
.
agift:community-based-corrections
  rdf:type skos:Concept ;
  rdfs:label "Community based corrections"@en ;
  skos:broader agift:corrective-services ;
  skos:definition "Administering programs that facilitate the reintegration of offenders into society. Aiding the development of independent living skills through a combination of sentenced probation, supervision, pre-parole reporting and pre-sentence reporting, unpaid community work and personal development opportunities." ;
  skos:hiddenLabel "Prison employment schemes" ;
  skos:hiddenLabel "Probation programs" ;
  skos:hiddenLabel "Reintegration programs" ;
  skos:hiddenLabel "Sentenced probation" ;
  skos:prefLabel "Community based corrections"@en ;
.
agift:community-education
  rdf:type skos:Concept ;
  rdfs:label "Community education"@en ;
  skos:broader agift:education-and-training ;
  skos:definition "Developing training programs designed to assist target groups of citizens. Initiating joint ventures with not-for-profit groups and local businesses. Community education is usually offered outside formal institutional structures. Includes first aid and fire safety training." ;
  skos:hiddenLabel "Fire safety training" ;
  skos:hiddenLabel "First aid training" ;
  skos:narrower agift:adult-education-programs ;
  skos:narrower agift:adult-migrant-education ;
  skos:narrower agift:road-safety-awareness ;
  skos:prefLabel "Community education"@en ;
  skos:related agift:job-placement-programs ;
.
agift:community-engagement
  rdf:type skos:Concept ;
  rdfs:label "Community engagement"@en ;
  skos:broader agift:community-services ;
  skos:definition """Inviting the community to participate in many forms of community consultations. 

See also COMMUNICATIONS - Government media: for managing media releases and dealing with journalists.
See also COMMUNICATIONS - Internet - Social media: policy and programs encouraging governments to consult widely with citizens via social media platforms.""" ;
  skos:hiddenLabel "Community consultation" ;
  skos:prefLabel "Community engagement"@en ;
  skos:related agift:government-media ;
.
agift:community-health-services
  rdf:type skos:Concept ;
  rdfs:label "Community health services"@en ;
  skos:broader agift:health-care ;
  skos:definition """Developing policy to provide for the physical and mental wellbeing of citizens in a particular district. Establishing programs that offer direct assistance to individuals or groups, and address the needs of the local community. Monitoring community health services to ensure adequate levels of care.

See also COMMUNITY SERVICES - Counselling services: for the provision of group therapy or psychological advice.

See also HEALTH CARE - Special needs services: for programs to support individuals with medical conditions.

See also HEALTH CARE - Special needs services - Mental health services: for programs to treat or manage mental illness.""" ;
  skos:hiddenLabel "Local health services" ;
  skos:hiddenLabel "Regional health services" ;
  skos:narrower agift:clinical-health-services ;
  skos:narrower agift:health-promotion ;
  skos:narrower agift:primary-health-care ;
  skos:prefLabel "Community health services"@en ;
  skos:related agift:counselling-services ;
  skos:related agift:public-health-services ;
.
agift:community-housing
  rdf:type skos:Concept ;
  rdfs:label "Community housing"@en ;
  skos:broader agift:public-housing ;
  skos:definition "Developing community housing programs delivered by community organisations and local governments to eligible individuals and families." ;
  skos:prefLabel "Community housing"@en ;
.
agift:community-policing
  rdf:type skos:Concept ;
  rdfs:label "Community policing"@en ;
  skos:broader agift:law-enforcement ;
  skos:definition "Administering programs that address local problems and crime reduction amongst target groups. Developing cooperative strategies involving police, local business and communities. Conducting safety audits of priority public sites, undertaking public safety patrols, identifying crime prone areas and advocating safe street and building design features." ;
  skos:hiddenLabel "Crime prevention" ;
  skos:hiddenLabel "Drink driving" ;
  skos:hiddenLabel "Local police" ;
  skos:hiddenLabel "Police activities" ;
  skos:hiddenLabel "Police" ;
  skos:hiddenLabel "Public safety" ;
  skos:prefLabel "Community policing"@en ;
.
agift:community-recreational-programs
  rdf:type skos:Concept ;
  rdfs:label "Community recreational programs"@en ;
  skos:broader agift:sport-and-recreation ;
  skos:definition """Administering schemes to provide organised activities to members of the public. Holding events for exercise, relaxation and enjoyment. Developing programs for specific groups, such as school children or senior citizens. Includes activities provided across public facilities such as swimming pools, libraries, community halls, sports centres, arts and cultural centres.

See also COMMUNITY SERVICES - Community support: for services and programs to develop self-reliance.""" ;
  skos:hiddenLabel "Recreation programs" ;
  skos:hiddenLabel "School holiday activities" ;
  skos:hiddenLabel "Senior citizen activities" ;
  skos:narrower agift:gambling-support-services ;
  skos:narrower agift:public-fitness-promotion ;
  skos:narrower agift:social-club-support ;
  skos:narrower agift:volunteer-support-programs ;
  skos:prefLabel "Community recreational programs"@en ;
  skos:related agift:community-support ;
.
agift:community-services
  rdf:type skos:Concept ;
  rdfs:label "COMMUNITY SERVICES"@en ;
  skos:definition "Developing policy to assist citizens in a particular district or those with common interests and needs. Providing welfare services and financial support. Administering disaster and emergency assistance programs." ;
  skos:hiddenLabel "Welfare" ;
  skos:narrower agift:accommodation-services ;
  skos:narrower agift:community-engagement ;
  skos:narrower agift:community-support ;
  skos:narrower agift:counselling-services ;
  skos:narrower agift:emergency-services ;
  skos:narrower agift:financial-assistance ;
  skos:narrower agift:natural-disasters ;
  skos:narrower agift:rural-community-development ;
  skos:narrower agift:social-justice-and-equity ;
  skos:narrower agift:social-research ;
  skos:narrower agift:transport-access-schemes ;
  skos:prefLabel "COMMUNITY SERVICES"@en ;
.
agift:community-support
  rdf:type skos:Concept ;
  rdfs:label "Community support"@en ;
  skos:broader agift:community-services ;
  skos:definition """Managing programs to assist family units. Developing targeted services and programs to foster relationships and develop community self-reliance. Includes cooperation with other jurisdictions and non-government organisations.

See also COMMUNITY SERVICES - Rural community development: for supporting country areas.

See also COMMUNITY SERVICES - Social justice and equity: for ensuring equal services to all communities.""" ;
  skos:hiddenLabel "Disability services" ;
  skos:hiddenLabel "Family support" ;
  skos:hiddenLabel "Non-profit organisations support" ;
  skos:narrower agift:adoption-services ;
  skos:narrower agift:aged-care-services ;
  skos:narrower agift:child-and-youth-support ;
  skos:narrower agift:child-care-services ;
  skos:narrower agift:defence-community-programs ;
  skos:narrower agift:family-reunion-programs ;
  skos:narrower agift:veterans-entitlements ;
  skos:prefLabel "Community support"@en ;
  skos:related agift:community-recreational-programs ;
  skos:related agift:rural-community-development ;
.
agift:conservation-programs
  rdf:type skos:Concept ;
  rdfs:label "Conservation programs"@en ;
  skos:broader agift:environment ;
  skos:definition """Maintaining land-based areas of the natural environment that are culturally or scientifically significant in their native state. Developing schemes to conserve plant or animal life in a region to protect and sustain ecosystems. Promoting community awareness of and participation in conservation activities. Promoting community awareness of and participation in sustainability activities.


See also ENVIRONMENT - Built environment - Building preservation: for conserving significant built structures.

See also ENVIRONMENT - Marine life protection programs: for maintaining sea-based environments.

See also ENVIRONMENT - Natural heritage protection: for managing areas of cultural or scientific significance.

See also NATURAL RESOURCES - Water resources - Waterway management: for strategies for salinity management and river care programs.

See also SCIENCE - Biological sciences - Biodiversity preservation: for investigating the variety of plant and animal life in a region.""" ;
  skos:hiddenLabel "Environmental conservation programs" ;
  skos:narrower agift:endangered-species-protection ;
  skos:narrower agift:landcare-programs ;
  skos:narrower agift:soil-preservation-programs ;
  skos:prefLabel "Conservation programs"@en ;
  skos:related agift:biodiversity-preservation ;
  skos:related agift:building-preservation ;
  skos:related agift:marine-life-protection-programs ;
.
agift:constitutional-conventions
  rdf:type skos:Concept ;
  rdfs:label "Constitutional conventions"@en ;
  skos:broader agift:constitutional-matters ;
  skos:definition "Organising forums for discussing and voting on change to the governance model embodied in a constitution. Selecting or appointing delegates. Providing advice on the rules of debate, order of proceedings and movement of motions and amendments. Producing, distributing and tabling of documents, notices and resolutions." ;
  skos:prefLabel "Constitutional conventions"@en ;
.
agift:constitutional-matters
  rdf:type skos:Concept ;
  rdfs:label "Constitutional matters"@en ;
  skos:broader agift:governance ;
  skos:definition "Managing the system of fundamental principles that provide the governance framework for a nation, state or municipality. Administering policy and procedures for constitutional review and amendment. Providing advice on the implications of intervention in constitutional litigation. Includes the activities of committees involved in constitutional matters." ;
  skos:hiddenLabel "Australian Constitution" ;
  skos:hiddenLabel "Governing charter" ;
  skos:hiddenLabel "Sovereignty" ;
  skos:narrower agift:constitutional-conventions ;
  skos:narrower agift:constitutional-referenda ;
  skos:prefLabel "Constitutional matters"@en ;
.
agift:constitutional-referenda
  rdf:type skos:Concept ;
  rdfs:label "Constitutional referenda"@en ;
  skos:broader agift:constitutional-matters ;
  skos:definition """Implementing the processes by which the governance model can be amended. Drafting and tabling a Bill proposing alteration to the constitution. Preparing and lodging the 'yes' and 'no' cases with the appropriate electoral commission.

See also GOVERNANCE - Electoral matters: for conducting public voting activities.""" ;
  skos:hiddenLabel "Referendums" ;
  skos:prefLabel "Constitutional referenda"@en ;
  skos:related agift:electoral-matters ;
.
agift:consular-services
  rdf:type skos:Concept ;
  rdfs:label "Consular services"@en ;
  skos:broader agift:international-relations ;
  skos:definition """Establishing and maintaining Australian government representation overseas, such as high commissions, embassies or consulates. Protecting the interests of Australian citizens travelling or living overseas. Providing country-specific trade or travel advice, and direct assistance where necessary. Includes services to Australians who are hospitalised or imprisoned in other countries, advising the families of Australians who are missing and coordinating evacuations from high-risk areas.

See also INTERNATIONAL RELATIONS - Diplomatic missions: for representation in Australia by foreign governments or international organisations.

See also INTERNATIONAL RELATIONS - International affairs: for Australian government representatives providing diplomatic advice overseas.

See also INTERNATIONAL RELATIONS - Passport services: for issuing travel documents to Australians who are overseas.""" ;
  skos:hiddenLabel "Consulates" ;
  skos:hiddenLabel "Embassies" ;
  skos:hiddenLabel "Expatriates" ;
  skos:hiddenLabel "High Commissions" ;
  skos:prefLabel "Consular services"@en ;
  skos:related agift:diplomatic-missions ;
  skos:related agift:international-affairs ;
.
agift:consumer-protection
  rdf:type skos:Concept ;
  rdfs:label "Consumer protection"@en ;
  skos:broader agift:business-support-and-regulation ;
  skos:definition "Administering programs to safeguard the purchasers of goods and services. Providing information to consumers and business about their rights and obligations. Handling complaints and managing dispute resolution procedures." ;
  skos:hiddenLabel "Consumer affairs" ;
  skos:hiddenLabel "Customer protection" ;
  skos:prefLabel "Consumer protection"@en ;
  skos:related agift:fair-trading-compliance ;
.
agift:contract-management
  rdf:type skos:Concept ;
  rdfs:label "Contract management"@en ;
  skos:broader agift:resource-management ;
  skos:definition """Developing procedures to administer agreements for the provision of goods and services, in accordance with government policy. Monitoring contracts to ensure the agreed terms are met and requirements fulfilled. 

See also BUSINESS SUPPORT AND REGULATION - Government procurement regulation: for tendering and awarding government contracts.""" ;
  skos:hiddenLabel "Government contracts" ;
  skos:prefLabel "Contract management"@en ;
  skos:related agift:government-procurement-regulation ;
.
agift:conveyancing
  rdf:type skos:Concept ;
  rdfs:label "Conveyancing"@en ;
  skos:broader agift:civil-law ;
  skos:definition "Administering the transfer of property rights between parties. Managing legal instruments that regulate the sale or purchase of domestic or commercial property." ;
  skos:hiddenLabel "Measurement standards" ;
  skos:prefLabel "Conveyancing"@en ;
.
agift:copyright-registration
  rdf:type skos:Concept ;
  rdfs:label "copyright registration"@en ;
  skos:prefLabel "copyright registration"@en ;
  skos:related agift:copyright-regulation ;
.
agift:copyright-regulation
  rdf:type skos:Concept ;
  rdfs:label "Copyright regulation"@en ;
  skos:broader agift:administrative-law ;
  skos:definition """Administering the legislation that governs the rights of ownership or control of literary, musical, dramatic or artistic works. Includes legal processes to resolve disputes over copyright ownership.

See also TRADE - Intellectual property management - Copyright registration: for licensing the intellectual property in literary, musical, dramatic or artistic works.""" ;
  skos:prefLabel "Copyright regulation"@en ;
  skos:related agift:copyright-registration ;
  skos:related agift:trademark-registration ;
.
agift:coronial-law
  rdf:type skos:Concept ;
  rdfs:label "Coronial law"@en ;
  skos:broader agift:justice-administration ;
  skos:definition "Administering the body of law that supports inquests into any death clearly not due to natural causes. Undertaking investigations on behalf of the coroner into the manner and cause of examinable deaths, or fires and explosions which damage property." ;
  skos:hiddenLabel "Coroner" ;
  skos:hiddenLabel "Coroner's court" ;
  skos:hiddenLabel "Coronial investigation" ;
  skos:prefLabel "Coronial law"@en ;
.
agift:corrective-services
  rdf:type skos:Concept ;
  rdfs:label "Corrective services"@en ;
  skos:broader agift:security ;
  skos:definition "Developing policy and programs for the punishment of individuals who have been convicted of an offence. Establishing standards and guidelines for correctional facilities and staff. Managing probation and parole activities. Includes support programs for inmates' families." ;
  skos:hiddenLabel "Correctional services" ;
  skos:hiddenLabel "Corrections" ;
  skos:hiddenLabel "Criminal punishment" ;
  skos:hiddenLabel "Parole services" ;
  skos:hiddenLabel "Penalties" ;
  skos:narrower agift:community-based-corrections ;
  skos:narrower agift:detention-centre-management ;
  skos:prefLabel "Corrective services"@en ;
.
agift:corruption-prevention
  rdf:type skos:Concept ;
  rdfs:label "Corruption prevention"@en ;
  skos:broader agift:public-administration ;
  skos:definition """Preventing, detecting and investigating serious and systemic corruption issues in government  agencies.
See also GOVERNANCE - Public administration - Government auditing:  reviewing the financial or performance management of a government organisation or entity and reporting findings to the legislative body.
See also GOVERNANCE - Public administration - Integrity compliance: encouraging ethical behaviour and compliance with official codes of conduct.
See also GOVERNANCE - Public administration - Whistleblowing: disclosing illegal, immoral or illegitimate practices under the control of their employer by government employees.
See also JUSTICE ADMINISTRATION - Criminal law: administering the body of law that governs actions punishable by the state.
See also SECURITY - Law enforcement:  formulating policy to support the maintenance of rules and regulations that govern the actions of citizens. Including activities to address 'white-collar' and corporate crime.""" ;
  skos:prefLabel "Corruption prevention"@en ;
  skos:related agift:criminal-law ;
  skos:related agift:law-enforcement ;
.
agift:counselling-services
  rdf:type skos:Concept ;
  rdfs:label "Counselling services"@en ;
  skos:broader agift:community-services ;
  skos:definition """Providing group therapy or psychological advice to individuals, families and community groups. Managing programs to treat drug addiction, emotional or behavioural problems. Includes assistance to people who have been ordered through the courts to undertake counselling.

See also HEALTH CARE - Special needs services: for programs to support individuals with medical conditions.

See also HEALTH CARE - Special needs services - Mental health services: for programs to treat or manage mental illness.

See also SPORT AND RECREATION - Community recreational programs - Gambling support services: for programs to assist compulsive gamblers in daily life.""" ;
  skos:hiddenLabel "Anger management" ;
  skos:hiddenLabel "Domestic violence programs" ;
  skos:hiddenLabel "Drug abuse counselling" ;
  skos:hiddenLabel "Grief counselling" ;
  skos:hiddenLabel "Group therapy" ;
  skos:hiddenLabel "Health counselling" ;
  skos:hiddenLabel "Marriage counselling" ;
  skos:hiddenLabel "Psychiatric counselling" ;
  skos:hiddenLabel "Psychiatry" ;
  skos:hiddenLabel "Psychological counselling" ;
  skos:hiddenLabel "Psychology" ;
  skos:hiddenLabel "Suicide prevention" ;
  skos:hiddenLabel "Therapy" ;
  skos:prefLabel "Counselling services"@en ;
  skos:related agift:clinical-health-services ;
  skos:related agift:community-health-services ;
  skos:related agift:dispute-mediation-programs ;
  skos:related agift:gambling-support-services ;
  skos:related agift:independent-living-services ;
  skos:related agift:mental-health-services ;
  skos:related agift:special-needs-services ;
.
agift:counterfeiting-control
  rdf:type skos:Concept ;
  rdfs:label "Counterfeiting control"@en ;
  skos:broader agift:currency ;
  skos:definition """Setting penalties for making or distributing forged currency. Includes procedures for reporting suspected counterfeit currency and related activities.

See also FINANCE MANAGEMENT - Currency: for security techniques to prevent counterfeiting.

See also SECURITY - Law enforcement: for apprehending counterfeiters.""" ;
  skos:prefLabel "Counterfeiting control"@en ;
  skos:related agift:currency ;
.
agift:courier-services
  rdf:type skos:Concept ;
  rdfs:label "Courier services"@en ;
  skos:broader agift:postal-services ;
  skos:definition "Administering special services to collect and deliver letters, parcels and other mail with guaranteed speed or security. Includes managing contracts with private courier companies and monitoring standards of service." ;
  skos:hiddenLabel "Certified mail services" ;
  skos:hiddenLabel "Express post services" ;
  skos:hiddenLabel "Registered mail services" ;
  skos:prefLabel "Courier services"@en ;
.
agift:court-reporting
  rdf:type skos:Concept ;
  rdfs:label "Court reporting"@en ;
  skos:broader agift:justice-administration ;
  skos:definition """Capturing and making accessible a record of what is said in a court or other judicial decision-making body. Includes recording and publishing a statement of facts, arguments and judgements of a proceeding in the form of a transcript.

See also GOVERNANCE - Parliamentary chamber support - Hansard services: for records of parliamentary proceedings.""" ;
  skos:hiddenLabel "Transcription services" ;
  skos:prefLabel "Court reporting"@en ;
  skos:related agift:hansard-services ;
.
agift:criminal-law
  rdf:type skos:Concept ;
  rdfs:label "Criminal law"@en ;
  skos:broader agift:justice-administration ;
  skos:definition """Administering the body of law that governs actions punishable by the state. Establishing rules of statute and common law to define criminal behaviour, specific penalties and the conduct of legal proceedings.

See also  GOVERNANCE - Public Administration - Corruption prevention: preventing, detecting and investigating serious and systemic corruption issues in Australian government agencies. 

See also GOVERNANCE - Public administration - Integrity compliance: encouraging ethical behaviour and compliance with official codes of conduct.""" ;
  skos:hiddenLabel "Crime prevention" ;
  skos:hiddenLabel "Crime" ;
  skos:hiddenLabel "Criminal confiscation" ;
  skos:prefLabel "Criminal law"@en ;
  skos:related agift:corruption-prevention ;
.
agift:criminology
  rdf:type skos:Concept ;
  rdfs:label "Criminology"@en ;
  skos:broader agift:law-enforcement ;
  skos:definition "Conducting research into crime and criminal justice in Australia. Analysing the causes of illegal behaviour and evaluating the operation of law enforcement agencies, the courts and correctional systems. Providing advice for the development of policy on crime control." ;
  skos:hiddenLabel "Crime research" ;
  skos:prefLabel "Criminology"@en ;
.
agift:cross-border-cooperation
  rdf:type skos:Concept ;
  rdfs:label "Cross-border cooperation"@en ;
  skos:broader agift:intergovernmental-relations ;
  skos:definition """Implementing the terms and conditions of formal agreements made between Australian government jurisdictions. Monitoring compliance with provisions and obligations. Assessing the ongoing benefits of interstate agreements.

See also GOVERNANCE - Intergovernmental relations: for negotiating agreements on matters other than trade.

See also TRADE - Interstate trade agreements: for negotiating commercial relationships between Australian government jurisdictions.""" ;
  skos:prefLabel "Cross-border cooperation"@en ;
  skos:related agift:intergovernmental-relations ;
.
agift:crown-land-administration
  rdf:type skos:Concept ;
  rdfs:label "Crown land administration"@en ;
  skos:broader agift:natural-resources ;
  skos:definition """Managing tenure of government property. Administering the sale, purchase, resumption, lease, license or transfer of Crown land. Providing property services to government agencies, such as those associated with national parks and government housing.

See also CIVIC INFRASTRUCTURE: for government buildings and construction projects on Crown land.

See also CIVIC INFRASTRUCTURE - Public land management: for maintaining areas set aside for community use.""" ;
  skos:hiddenLabel "Crown land use" ;
  skos:hiddenLabel "Crown land" ;
  skos:prefLabel "Crown land administration"@en ;
  skos:related agift:civic-infrastructure ;
  skos:related agift:public-land-management ;
.
agift:cultural-affairs
  rdf:type skos:Concept ;
  rdfs:label "CULTURAL AFFAIRS"@en ;
  skos:definition "Developing policy to support the arts and cultural organisations such as museums, libraries and galleries. Establishing programs to develop and manage cultural collections and artefacts, and to stimulate growth in cultural industries. Sponsoring activities and events to celebrate the diversity of Australian culture." ;
  skos:hiddenLabel "Archives" ;
  skos:hiddenLabel "Art galleries" ;
  skos:hiddenLabel "Cultural institutions" ;
  skos:hiddenLabel "Culture" ;
  skos:hiddenLabel "Galleries" ;
  skos:hiddenLabel "Libraries" ;
  skos:hiddenLabel "Museums" ;
  skos:hiddenLabel "Theatres" ;
  skos:narrower agift:arts-development ;
  skos:narrower agift:collection-access ;
  skos:narrower agift:collection-management ;
  skos:narrower agift:collection-promotion ;
  skos:narrower agift:cultural-awards-and-scholarships ;
  skos:narrower agift:cultural-festivals ;
  skos:narrower agift:cultural-gifts-programs ;
  skos:narrower agift:multicultural-heritage-promotion ;
  skos:prefLabel "CULTURAL AFFAIRS"@en ;
  skos:related agift:cultural-centre-management ;
  skos:related agift:immigration ;
.
agift:cultural-artefact-repatriation
  rdf:type skos:Concept ;
  rdfs:label "Cultural artefact repatriation"@en ;
  skos:broader agift:indigenous-cultural-heritage ;
  skos:definition """Developing policy to safeguard custodial rights over indigenous cultural heritage property. Implementing programs to return indigenous relics, artworks, human remains and other items of cultural significance to their traditional owners or custodians. 

See also CULTURAL AFFAIRS - Collection management - Artefact export regulation: for negotiating the international movement of cultural materials.""" ;
  skos:hiddenLabel "Return of Cultural Property programs" ;
  skos:hiddenLabel "Sacred object protection" ;
  skos:prefLabel "Cultural artefact repatriation"@en ;
  skos:related agift:artefact-export-regulation ;
.
agift:cultural-awards-and-scholarships
  rdf:type skos:Concept ;
  rdfs:label "Cultural awards and scholarships"@en ;
  skos:broader agift:cultural-affairs ;
  skos:definition """Developing schemes to confer prizes for achievement in artistic, literary or heritage-related activities. Providing grants to cultural-sector students of high merit. Includes promotional activities, assessing applications and managing payments.

See also GOVERNANCE - Honours and awards programs: for national merit lists.""" ;
  skos:hiddenLabel "Awards and scholarships" ;
  skos:hiddenLabel "Cultural scholarship programs" ;
  skos:hiddenLabel "Scholarship programs" ;
  skos:prefLabel "Cultural awards and scholarships"@en ;
  skos:related agift:honours-and-awards-programs ;
.
agift:cultural-centre-management
  rdf:type skos:Concept ;
  rdfs:label "Cultural centre management"@en ;
  skos:broader agift:public-land-management ;
  skos:definition """Administering buildings that house cultural collections or are set aside for community use. Ensuring facilities are kept clean and maintained. Monitoring rights of access and opening hours. Taking bookings and liaising with event organisers.

See also CULTURAL AFFAIRS: for functions carried out by cultural institutions.""" ;
  skos:hiddenLabel "Archive management" ;
  skos:hiddenLabel "Art gallery management" ;
  skos:hiddenLabel "Community centre management" ;
  skos:hiddenLabel "Community hall management" ;
  skos:hiddenLabel "Gallery management" ;
  skos:hiddenLabel "Library management" ;
  skos:hiddenLabel "Museum management" ;
  skos:hiddenLabel "Public library management" ;
  skos:hiddenLabel "Theatre management" ;
  skos:prefLabel "Cultural centre management"@en ;
  skos:related agift:collection-storage ;
  skos:related agift:cultural-affairs ;
.
agift:cultural-festivals
  rdf:type skos:Concept ;
  rdfs:label "Cultural festivals"@en ;
  skos:broader agift:cultural-affairs ;
  skos:definition """Promoting and funding events that highlight artistic, literary or heritage related activities. Organising festivals, performances and joint ventures with community groups where events focus on a particular genre or collection. Includes participation in international cultural festivals.

See also CULTURAL AFFAIRS - Multicultural heritage promotion - Multicultural festivals: for events that highlight Australia's cultural diversity.

See also GOVERNANCE - Civic celebrations: for marking significant community occasions.

See also INTERNATIONAL RELATIONS - Overseas promotion: for negotiating opportunities to participate in or host international tourist events.""" ;
  skos:hiddenLabel "Arts festivals" ;
  skos:hiddenLabel "Book festivals" ;
  skos:hiddenLabel "Festivals" ;
  skos:hiddenLabel "Heritage festivals" ;
  skos:prefLabel "Cultural festivals"@en ;
  skos:related agift:civic-celebrations ;
  skos:related agift:multicultural-festivals ;
  skos:related agift:overseas-promotion ;
.
agift:cultural-gifts-programs
  rdf:type skos:Concept ;
  rdfs:label "Cultural gifts programs"@en ;
  skos:broader agift:cultural-affairs ;
  skos:definition """Managing donations of cultural materials, made under arts incentive schemes. Examining materials to ensure they conform to collection development policies. Setting guidelines for the acceptance of gifts. Determining access restrictions, intellectual property rights and legal title over materials. Organising independent valuations and making submissions to the relevant taxation incentives body.

See also CULTURAL AFFAIRS - Arts development - Arts incentive schemes: for strategies to encourage investment in cultural materials.

See also CULTURAL AFFAIRS - Collection management - Collection acquisition: for managing the receipt of other donations.""" ;
  skos:hiddenLabel "Art donation schemes" ;
  skos:hiddenLabel "Public donations" ;
  skos:prefLabel "Cultural gifts programs"@en ;
  skos:related agift:arts-incentive-schemes ;
.
agift:currency
  rdf:type skos:Concept ;
  rdfs:label "Currency"@en ;
  skos:broader agift:finance-management ;
  skos:definition "Developing policy for the minting and distribution of monetary notes and coins. Designing security techniques such as watermarks to prevent counterfeiting. Includes procedures for issuing new or commemorative coins." ;
  skos:hiddenLabel "Coinage" ;
  skos:hiddenLabel "Coins" ;
  skos:hiddenLabel "Money" ;
  skos:hiddenLabel "Notes" ;
  skos:narrower agift:counterfeiting-control ;
  skos:prefLabel "Currency"@en ;
  skos:related agift:counterfeiting-control ;
.
agift:curriculum-development
  rdf:type skos:Concept ;
  rdfs:label "Curriculum development"@en ;
  skos:broader agift:education-and-training ;
  skos:definition "Researching and drafting outline study programs for any education sector. Outlining the courses and units to be completed. Includes liaison across jurisdictions to support consistency across education authorities." ;
  skos:hiddenLabel "School curriculum development" ;
  skos:hiddenLabel "Syllabus development" ;
  skos:prefLabel "Curriculum development"@en ;
.
agift:cybersafety
  rdf:type skos:Concept ;
  rdfs:label "Cybersafety"@en ;
  skos:broader agift:internet ;
  skos:definition """Developing policy and programs designed to protect consumers shopping online, vulnerable people from exposure to inappropriate material and invasion of personal privacy online. 
See also COMMUNICATIONS - Electronic commerce: for developing policy to support and regulate Australian participation in the global information economy.
See also COMMUNICATIONS - Information management standards - Information technology standards: for hardware and software regulation.""" ;
  skos:hiddenLabel "Cybersecurity" ;
  skos:prefLabel "Cybersafety"@en ;
.
agift:data-management
  rdf:type skos:Concept ;
  rdfs:label "Data management"@en ;
  skos:broader agift:information-management-standards ;
  skos:definition """Developing standards for the exchange or transfer of information between government agencies or systems. Providing guidelines for cross-matching data. Promoting the use of metadata to support resource discovery or interoperability.

See also COMMUNICATIONS - Electronic commerce - Online transaction standards: for guidelines to support electronic commerce.

See also COMMUNICATIONS - Information management standards - Information technology standards: for data transfer protocols.

See also SECURITY - Information security: for data security standards.""" ;
  skos:hiddenLabel "Data matching guidelines" ;
  skos:hiddenLabel "Metadata standards" ;
  skos:prefLabel "Data management"@en ;
  skos:related agift:online-transaction-standards ;
.
agift:declaration-of-interests
  rdf:type skos:Concept ;
  rdfs:label "Declaration of interests"@en ;
  skos:broader agift:electoral-matters ;
  skos:definition "Managing the disclosure of election campaign funding details. Facilitating the lodgement of returns by candidates and political parties. Includes notifications from broadcasters regarding electoral advertisements run during an election period." ;
  skos:hiddenLabel "Pecuniary interests" ;
  skos:hiddenLabel "Register of interests" ;
  skos:prefLabel "Declaration of interests"@en ;
.
agift:defence
  rdf:type skos:Concept ;
  rdfs:label "DEFENCE"@en ;
  skos:definition """Ensuring the safety of Australia by building, maintaining and deploying military resources. Developing policy and programs for defence of the nation, region and allies. Includes high-level administration of the Australian Defence Forces (ADF).

See also SECURITY: for protection using civilian resources.""" ;
  skos:narrower agift:australian-defence-forces ;
  skos:narrower agift:defence-estate-management ;
  skos:narrower agift:defence-force-careers ;
  skos:narrower agift:defence-strategic-development ;
  skos:narrower agift:defence-strategic-policy ;
  skos:narrower agift:defence-strategic-support ;
  skos:narrower agift:emergency-management ;
  skos:narrower agift:military-law ;
  skos:narrower agift:military-operations ;
  skos:prefLabel "DEFENCE"@en ;
  skos:related agift:security ;
.
agift:defence-attaches
  rdf:type skos:Concept ;
  rdfs:label "Defence attaches"@en ;
  skos:broader agift:defence-liaison ;
  skos:definition """Providing diplomatic representation of Australia's military interests. Liaising with governments and international bodies to build strategic alliances and defence partnerships.

See also DEFENCE - Defence strategic policy: for plans to direct the development of Australia's military capability.

See also INTERNATIONAL RELATIONS - Consular services: for other ambassadorial activities.

See also INTERNATIONAL RELATIONS - Defence liaison - Military advisors: for providing defence counsel to senior government representatives.""" ;
  skos:prefLabel "Defence attaches"@en ;
  skos:related agift:defence-strategic-policy ;
.
agift:defence-career-development
  rdf:type skos:Concept ;
  rdfs:label "Defence career development"@en ;
  skos:broader agift:defence-force-careers ;
  skos:definition """Providing career counselling, career planning, professional development and training advice to regular and reserve members of the Australian Defence Forces. Includes career transition assistance, redeployment, discharge and retirement services.

See also COMMUNITY SERVICES - Community support - Defence community programs: for other services to support service personnel and their families.

See also DEFENCE - Defence force careers - Military employment services: for workplace services and advice.

See also EDUCATION AND TRAINING - Military education and training: for courses that may improve career prospects.""" ;
  skos:prefLabel "Defence career development"@en ;
  skos:related agift:defence-community-programs ;
  skos:related agift:defence-personnel-exchanges ;
  skos:related agift:military-employment-services ;
.
agift:defence-college-training
  rdf:type skos:Concept ;
  rdfs:label "Defence college training"@en ;
  skos:broader agift:military-education-and-training ;
  skos:definition "Administering educational programs through institutions that cater specifically to military personnel, officers and cadets. Determining entry requirements. Providing scholarships and study grants." ;
  skos:hiddenLabel "Military colleges" ;
  skos:hiddenLabel "Officer college training" ;
  skos:prefLabel "Defence college training"@en ;
  skos:related agift:cadets ;
.
agift:defence-community-programs
  rdf:type skos:Concept ;
  rdfs:label "Defence community programs"@en ;
  skos:broader agift:community-support ;
  skos:definition """Providing services to support military personnel and their families. Establishing social networks and activities. Facilitating communication between family members separated by service requirements. Arranging access to support groups or counselling in times of tragedy.

See also COMMUNITY SERVICES - Accommodation services - Defence housing: for providing accommodation for military personnel.

See also COMMUNITY SERVICES - Community support - Veterans' entitlements: for social support services to returned defence service personnel and their families.

See also COMMUNITY SERVICES - Counselling services: for the provision of group therapy or psychological advice.

See also DEFENCE - Defence force careers - Defence career development: for career counselling and advice.""" ;
  skos:hiddenLabel "Defence families" ;
  skos:prefLabel "Defence community programs"@en ;
  skos:related agift:defence-career-development ;
  skos:related agift:defence-housing ;
  skos:related agift:veterans-entitlements ;
.
agift:defence-cooperation-programs
  rdf:type skos:Concept ;
  rdfs:label "Defence cooperation programs"@en ;
  skos:broader agift:defence-liaison ;
  skos:definition """Promoting international defence relations through a series of high-level dialogue, official visits and collaboration with regional and allied defence organisations. Developing a coordinated international response to a potential or imminent threat.

See also SECURITY - External security - Peacekeeping forces: for cooperative efforts to stabilise international unrest.""" ;
  skos:prefLabel "Defence cooperation programs"@en ;
  skos:related agift:peacekeeping-forces ;
.
agift:defence-efficiency-review
  rdf:type skos:Concept ;
  rdfs:label "Defence efficiency review"@en ;
  skos:broader agift:defence-strategic-development ;
  skos:definition "Investigating current defence operations to assess performance against the use of resources. Reviewing processes and consulting stakeholders. Developing strategies for efficient expenditure of funds, to maximise defence capability." ;
  skos:prefLabel "Defence efficiency review"@en ;
.
agift:defence-estate-management
  rdf:type skos:Concept ;
  rdfs:label "Defence estate management"@en ;
  skos:broader agift:defence ;
  skos:definition """Administering buildings, infrastructure, property and other corporate assets of the Defence portfolio. Developing acquisition and disposal policy. Managing repair and maintenance programs. Reviewing facilities and capital works.

See also COMMUNITY SERVICES - Accommodation services - Defence housing: for programs to provide housing for defence personnel.""" ;
  skos:prefLabel "Defence estate management"@en ;
  skos:related agift:defence-housing ;
.
agift:defence-force-careers
  rdf:type skos:Concept ;
  rdfs:label "Defence force careers"@en ;
  skos:broader agift:defence ;
  skos:definition """Developing human resources policy for defence force personnel. Conducting research into recruitment, retention and demographics. Administering recruitment programs and activities to promote defence force careers.

See also EDUCATION AND TRAINING - Military education and training: for courses that may improve career prospects.

See also EMPLOYMENT - Human resources development: for civilian personnel support.

See also INTERNATIONAL RELATIONS - Defence liaison - Defence personnel exchanges: for developing temporary reassignment programs.""" ;
  skos:hiddenLabel "Air force careers" ;
  skos:hiddenLabel "Army careers" ;
  skos:hiddenLabel "Defence personnel" ;
  skos:hiddenLabel "Enlistment" ;
  skos:hiddenLabel "Military enlistment" ;
  skos:hiddenLabel "Navy careers" ;
  skos:narrower agift:defence-career-development ;
  skos:narrower agift:military-employment-services ;
  skos:prefLabel "Defence force careers"@en ;
  skos:related agift:human-resources-development ;
  skos:related agift:military-education-and-training ;
  skos:related agift:recruitment-programs ;
.
agift:defence-force-commands
  rdf:type skos:Concept ;
  rdfs:label "Defence force commands"@en ;
  skos:broader agift:australian-defence-forces ;
  skos:definition "Managing and operating command centres of the Army, Navy or Air Force, which exercise authority over a specific geographical area, a discrete function or specialised programs." ;
  skos:hiddenLabel "Air force commands" ;
  skos:hiddenLabel "Army commands" ;
  skos:hiddenLabel "Command and control" ;
  skos:hiddenLabel "Defence commands" ;
  skos:hiddenLabel "Military commands" ;
  skos:hiddenLabel "Navy commands" ;
  skos:hiddenLabel "RAAF commands" ;
  skos:hiddenLabel "RAN commands" ;
  skos:prefLabel "Defence force commands"@en ;
.
agift:defence-housing
  rdf:type skos:Concept ;
  rdfs:label "Defence housing"@en ;
  skos:broader agift:accommodation-services ;
  skos:definition "Administering schemes to provide accommodation for defence forces personnel. Includes criteria for eligibility, subsidy entitlements, leasing arrangements, relocation and maintenance programs. Planning for housing construction and the movement of defence personnel. Liaising with local authorities and acquiring land." ;
  skos:hiddenLabel "ADF housing" ;
  skos:hiddenLabel "Defence families" ;
  skos:hiddenLabel "War service home schemes" ;
  skos:prefLabel "Defence housing"@en ;
  skos:related agift:defence-community-programs ;
  skos:related agift:defence-estate-management ;
.
agift:defence-industry
  rdf:type skos:Concept ;
  rdfs:label "Defence industry"@en ;
  skos:broader agift:defence-strategic-support ;
  skos:definition """Administering programs to build relationships with Australian industry to support defence activities. Providing funding, investment opportunities and incentives for research and development. Establishing advisory forums and other communication strategies. Operating endorsement schemes to certify products that meet Australian defence specifications. Encouraging participation in the international defence market and managing materiel cooperation activities.

See also DEFENCE - Defence strategic support - Capital equipment programs: for projects to acquire or build military equipment.""" ;
  skos:prefLabel "Defence industry"@en ;
  skos:related agift:capital-equipment-programs ;
  skos:related agift:defence-science-and-technology ;
.
agift:defence-liaison
  rdf:type skos:Concept ;
  rdfs:label "Defence liaison"@en ;
  skos:broader agift:international-relations ;
  skos:definition """Cooperating with other countries to ensure Australia's ability to resist foreign aggression or attack. Providing defence and strategic advice, negotiating agreements for the deployment of defence resources. Includes participation in joint exercises and development programs.

See also SECURITY - External security: for cooperation with other countries to protect the safety of Australian citizens and interests.""" ;
  skos:narrower agift:defence-attaches ;
  skos:narrower agift:defence-cooperation-programs ;
  skos:narrower agift:defence-personnel-exchanges ;
  skos:narrower agift:military-advisors ;
  skos:prefLabel "Defence liaison"@en ;
  skos:related agift:external-security ;
  skos:related agift:international-treaties ;
.
agift:defence-personnel-exchanges
  rdf:type skos:Concept ;
  rdfs:label "Defence personnel exchanges"@en ;
  skos:broader agift:defence-liaison ;
  skos:definition """Designing and implementing programs for temporary reassignment of defence personnel, to support professional development and promote relationships between defence forces. Providing services and training to staff on exchange, to help realise the full benefits of the program.

See also DEFENCE - Defence force careers - Defence career development: for access to exchange programs.""" ;
  skos:prefLabel "Defence personnel exchanges"@en ;
  skos:related agift:defence-career-development ;
.
agift:defence-reform-program
  rdf:type skos:Concept ;
  rdfs:label "Defence reform program"@en ;
  skos:broader agift:defence-strategic-development ;
  skos:definition "Implementing improvements in defence operations, to support long-term capability development. Evaluating the effects of reforms, to determine their impact on performance, efficiency and personnel." ;
  skos:prefLabel "Defence reform program"@en ;
.
agift:defence-science-and-technology
  rdf:type skos:Concept ;
  rdfs:label "Defence science and technology"@en ;
  skos:broader agift:defence-strategic-support ;
  skos:definition """Conducting research into the application of specialist knowledge and equipment to support military operations. Providing technical advice on the purchase of defence equipment. Includes designing, testing and overseeing the manufacture of new products.

See also DEFENCE - Defence strategic support - Defence industry: for providing incentive for commercial research and development.

See also SCIENCE: for pure research in specific disciplines.""" ;
  skos:hiddenLabel "Biological weapons" ;
  skos:prefLabel "Defence science and technology"@en ;
  skos:related agift:biotechnology-development ;
  skos:related agift:defence-industry ;
  skos:related agift:nuclear-sciences ;
.
agift:defence-strategic-development
  rdf:type skos:Concept ;
  rdfs:label "Defence strategic development"@en ;
  skos:broader agift:defence ;
  skos:definition """Identifying issues for the effective growth and advancement of defence operations. Assessing current infrastructure and facilities, and forecasting future needs. Conducting long-term planning for capability development, science and technology, acquisition, training and logistics.

See also DEFENCE - Defence strategic support: for programs to ensure military operations are fully equipped and assisted.""" ;
  skos:narrower agift:defence-efficiency-review ;
  skos:narrower agift:defence-reform-program ;
  skos:prefLabel "Defence strategic development"@en ;
  skos:related agift:defence-strategic-support ;
  skos:related agift:strategic-planning ;
.
agift:defence-strategic-policy
  rdf:type skos:Concept ;
  rdfs:label "Defence strategic policy"@en ;
  skos:broader agift:defence ;
  skos:definition """Formulating high-level policy to direct the development and deployment of Australia's defence capability. Directing the management of international defence activities and setting guidelines and priorities for military planning and decision making.

See also INTERNATIONAL RELATIONS - Defence liaison - Defence attach?s: for international diplomatic representation of Australia's military interests.""" ;
  skos:narrower agift:strategic-decisions ;
  skos:narrower agift:strategic-planning ;
  skos:prefLabel "Defence strategic policy"@en ;
  skos:related agift:defence-attaches ;
.
agift:defence-strategic-support
  rdf:type skos:Concept ;
  rdfs:label "Defence strategic support"@en ;
  skos:broader agift:defence ;
  skos:definition """Developing programs to ensure military operations are fully equipped and assisted. Building a coordinated network of infrastructure, facilities and knowledge. Formulating policy for contracting, acquisitions and defence export activities.

See also DEFENCE - Defence strategic development: for planning the growth of defence operations.""" ;
  skos:hiddenLabel "Military equipment strategy" ;
  skos:narrower agift:capital-equipment-programs ;
  skos:narrower agift:defence-industry ;
  skos:narrower agift:defence-science-and-technology ;
  skos:narrower agift:logistics ;
  skos:prefLabel "Defence strategic support"@en ;
  skos:related agift:defence-strategic-development ;
.
agift:dental-health-services
  rdf:type skos:Concept ;
  rdfs:label "Dental health services"@en ;
  skos:broader agift:special-needs-services ;
  skos:definition "Administering programs that provide treatments for oral hygiene and problems with teeth. Managing school dental services and schemes to provide access to low-income earners or disadvantaged groups. Monitoring the activities of private dental health providers." ;
  skos:hiddenLabel "Dentists" ;
  skos:hiddenLabel "Oral health services" ;
  skos:hiddenLabel "Orthodontic services" ;
  skos:hiddenLabel "Teeth" ;
  skos:prefLabel "Dental health services"@en ;
.
agift:deportation
  rdf:type skos:Concept ;
  rdfs:label "Deportation"@en ;
  skos:broader agift:immigration ;
  skos:definition """Administering the removal of foreign nationals whose presence in Australia is unlawful or poses an unacceptable level of threat to the community. Arranging the deportation of non-citizens who have committed serious crimes and those whose visas have expired. Includes the exclusion of unauthorised arrivals who are not refugees. 

See also IMMIGRATION - Detention programs: for the custody and treatment of illegal immigrants.

See also IMMIGRATION - Refugee services: for assistance to asylum seekers and victims of human rights violations.

See also JUSTICE ADMINISTRATION - Administrative law: for appeals and reviews of deportation decisions.

See also SECURITY - National security: for border protection policy.""" ;
  skos:hiddenLabel "Criminal deportation" ;
  skos:hiddenLabel "Extradition" ;
  skos:hiddenLabel "Illegal immigrants" ;
  skos:prefLabel "Deportation"@en ;
  skos:related agift:detention-programs ;
.
agift:descriptive-standards
  rdf:type skos:Concept ;
  rdfs:label "Descriptive standards"@en ;
  skos:broader agift:collection-access ;
  skos:definition """Developing and implementing agreed models to explain the content, extent and format of items in cultural collections. Includes cooperative efforts to promote common descriptive standards across a range of cultural institutions.

See also CULTURAL AFFAIRS - Collection access - Finding aids development: for creating tools to locate items in cultural collections.

See also CULTURAL AFFAIRS - Collection management - Collection accessioning: for listing newly acquired items.""" ;
  skos:hiddenLabel "Cataloguing standards" ;
  skos:hiddenLabel "Classification standards" ;
  skos:hiddenLabel "Curatorial standards" ;
  skos:hiddenLabel "Indexing standards" ;
  skos:prefLabel "Descriptive standards"@en ;
  skos:related agift:finding-aids-development ;
.
agift:design-rights-management
  rdf:type skos:Concept ;
  rdfs:label "Design rights management"@en ;
  skos:broader agift:intellectual-property-management ;
  skos:definition """Conferring legal ownership over applied intellectual property such as structures, machinery, industrial plans or complex artworks (eg those with intricate configuration or moving parts). Includes processing and approving applications for design registration, liaising with designers and licensing the use of designs.

See also TRADE - Intellectual property management - Patent rights management: for the intellectual property in inventions and industrial or scientific processes.

See also TRADE - Intellectual property management - Plant breeders' rights management: for developing policy to protect the rights of plant  breeders developing new plant varieties.

See also TRADE - Intellectual property management - Trademark registration: for the intellectual property in designs or symbols associated with a business entity or product.""" ;
  skos:prefLabel "Design rights management"@en ;
  skos:related agift:patent-rights-management ;
  skos:related agift:plant-breeders-rights-management ;
.
agift:detention-centre-management
  rdf:type skos:Concept ;
  rdfs:label "Detention centre management"@en ;
  skos:broader agift:corrective-services ;
  skos:definition """Administering humane and appropriately secure facilities where convicted offenders are incarcerated. Providing food and amenities, recreation, medical care, mail services and education. Monitoring standards where detention centre management activities are outsourced.

See also DEFENCE - Military law: for detention of defence personnel or prisoners of war.

See also IMMIGRATION - Detention programs: for the custody and treatment of illegal immigrants.""" ;
  skos:hiddenLabel "Detention centres" ;
  skos:hiddenLabel "Jail management" ;
  skos:hiddenLabel "Juvenile detention centres" ;
  skos:hiddenLabel "Police cells" ;
  skos:hiddenLabel "Prison farms" ;
  skos:hiddenLabel "Prison management" ;
  skos:hiddenLabel "Remand centres" ;
  skos:prefLabel "Detention centre management"@en ;
  skos:related agift:military-law ;
.
agift:detention-programs
  rdf:type skos:Concept ;
  rdfs:label "Detention programs"@en ;
  skos:broader agift:immigration ;
  skos:definition """Administering custodial schemes for people who have entered Australia illegally, those refused entry at international airports and seaports, and those whose visas are cancelled or expired. Managing facilities for the detention of illegal immigrants. Providing food and amenities, medical care, recreation, social support and education.

See also DEFENCE - Military law: for detention of defence personnel or prisoners of war.

See also IMMIGRATION - Deportation: for the removal of foreign nationals who are unlawfully in Australia.

See also IMMIGRATION - Refugee services: for assistance to asylum seekers and victims of human rights violations.

See also SECURITY - Corrective services - Detention centre management: for detention of Australian citizens.

See also SECURITY - National security: for border protection policy.

See also SECURITY - National security - Border protection: for coordinating operations to monitor Australian borders for unauthorised sea or air arrivals.""" ;
  skos:hiddenLabel "Migrant processing centres" ;
  skos:prefLabel "Detention programs"@en ;
  skos:related agift:deportation ;
  skos:related agift:military-law ;
.
agift:development-assistance-programs
  rdf:type skos:Concept ;
  rdfs:label "Development assistance programs"@en ;
  skos:broader agift:overseas-aid-programs ;
  skos:definition """Administering schemes to support growth and improvement in overseas communities. Providing advice and training and delivering projects in sectors such as governance, health, education, rural and infrastructure development. Includes emergency, humanitarian and reconstruction assistance in times of crisis.

See also DEFENCE - Emergency management - Disaster support: for defence forces assistance in times of crisis.

See also INTERNATIONAL RELATIONS - Overseas aid programs - Overseas student scholarship programs: for supporting access to higher education for students from developing countries.

See also SECURITY - External security - Peacekeeping forces: for defence units deployed to stabilise unrest and restore order.""" ;
  skos:prefLabel "Development assistance programs"@en ;
  skos:related agift:disaster-support ;
  skos:related agift:trade-development-programs ;
.
agift:diplomatic-missions
  rdf:type skos:Concept ;
  rdfs:label "Diplomatic missions"@en ;
  skos:broader agift:international-relations ;
  skos:definition """Providing services to representatives of foreign governments or international organisations. Assisting representatives to establish and maintain diplomatic missions, such as high commissions, embassies or consulates. Includes developing protocol guidelines and consular responsibilities for countries without diplomatic representation in Australia.

See also INTERNATIONAL RELATIONS - Consular services: for Australian government representation and services to Australian citizens overseas.

See also INTERNATIONAL RELATIONS - International affairs: for Australian government representatives providing diplomatic advice overseas.""" ;
  skos:hiddenLabel "Ambassadors" ;
  skos:hiddenLabel "Diplomatic Corps" ;
  skos:hiddenLabel "International representatives" ;
  skos:prefLabel "Diplomatic missions"@en ;
  skos:related agift:consular-services ;
.
agift:disarmament-and-arms-control
  rdf:type skos:Concept ;
  rdfs:label "Disarmament and arms control"@en ;
  skos:broader agift:international-affairs ;
  skos:definition """Implementing the terms and conditions of formal agreements to reduce or limit levels of military resources. Administering regulatory mechanisms to enable Australia to fulfil its obligations under international treaties. Includes disseminating information to stakeholders, inspecting significant facilities and declaring notable activities.

See also INTERNATIONAL RELATIONS - International affairs - Nuclear safeguards: ensuring that nuclear material and associated equipment is fully accounted for and controlled.

See also INTERNATIONAL RELATIONS - International treaties: for negotiating arms control agreements.""" ;
  skos:hiddenLabel "Arms control" ;
  skos:hiddenLabel "Chemical weapons" ;
  skos:hiddenLabel "Nuclear weapons" ;
  skos:hiddenLabel "Weapons inspections" ;
  skos:hiddenLabel "Weapons of mass destruction" ;
  skos:prefLabel "Disarmament and arms control"@en ;
  skos:related agift:nuclear-safeguards ;
  skos:related agift:treaty-administration ;
.
agift:disaster-recovery
  rdf:type skos:Concept ;
  rdfs:label "Disaster recovery"@en ;
  skos:broader agift:natural-disasters ;
  skos:definition """Coordinating programs to repair the damage caused by natural disasters - such as floods, earthquakes, cyclones, storms or major bushfires. Developing strategies for timely restoration of essential services and clearing debris. Initiating plans for demolition and rebuilding of damaged facilities.

See also COMMUNITY SERVICES - Natural Disasters - Disaster relief: for financial assistance to those affected by natural disasters.

See also DEFENCE - Emergency management - Civil community assistance: for defence forces support after natural disasters.

See also DEFENCE - Emergency management - Disaster support: for emergency defence forces support in overseas communities.

See also INTERNATIONAL RELATIONS - Overseas aid programs - Development assistance programs: for disaster recovery services in overseas communities.""" ;
  skos:prefLabel "Disaster recovery"@en ;
  skos:related agift:disaster-relief ;
  skos:related agift:disaster-support ;
.
agift:disaster-relief
  rdf:type skos:Concept ;
  rdfs:label "Disaster relief"@en ;
  skos:broader agift:natural-disasters ;
  skos:definition """Providing financial assistance to communities, individuals and businesses affected by natural disasters such as floods, earthquakes, cyclones, storms or major bushfires. Includes negotiating terms for compensation payments or low interest loans, processing claims and liaising with community services for other forms of support.

See also COMMUNITY SERVICES - Accommodation services - Emergency accommodation: for providing housing after a disaster.

See also COMMUNITY SERVICES - Emergency services - Emergency funding: for resources to support emergency services.""" ;
  skos:hiddenLabel "Drought relief" ;
  skos:hiddenLabel "Flood relief" ;
  skos:hiddenLabel "Relief funding" ;
  skos:prefLabel "Disaster relief"@en ;
  skos:related agift:disaster-recovery ;
  skos:related agift:emergency-accommodation ;
  skos:related agift:financial-assistance ;
.
agift:disaster-support
  rdf:type skos:Concept ;
  rdfs:label "Disaster support"@en ;
  skos:broader agift:emergency-management ;
  skos:definition """Managing the allocation of Australian Defence Force resources to assist overseas communities in times of crisis. Providing support to humanitarian and reconstruction efforts after natural disaster or other emergency. Includes identifying lines of communication, chain of command, and establishing criteria for situations warranting defence forces assistance.

See also COMMUNITY SERVICES - Natural disasters - Disaster recovery: for civil disaster support services.

See also DEFENCE - Emergency management - Civil community assistance: for emergency defence force assistance to Australian communities.

See also INTERNATIONAL RELATIONS - Overseas aid programs - Development assistance programs: for civil disaster support services in overseas communities.

See also SECURITY - External security - Peacekeeping forces: for units deployed to stabilise unrest and restore order.""" ;
  skos:prefLabel "Disaster support"@en ;
  skos:related agift:civil-community-assistance ;
  skos:related agift:development-assistance-programs ;
  skos:related agift:disaster-recovery ;
  skos:related agift:peacekeeping-forces ;
  skos:related agift:special-operations ;
.
agift:discipline-programs
  rdf:type skos:Concept ;
  rdfs:label "Discipline programs"@en ;
  skos:broader agift:school-education ;
  skos:definition """Developing and implementing programs to reduce or prevent behavioural problems in schools. Assisting those experiencing behavioural problems, and victims of unacceptable behaviour. Providing guidance to teachers about appropriate forms of discipline. Includes liaison with community groups, police and families to deal with behavioural problems.

See also COMMUNITY SERVICES - Community support - Child and youth support: for programs to assist young people at risk.

See also COMMUNITY SERVICES - Counselling services: for providing psychological advice or therapy.""" ;
  skos:hiddenLabel "Bullying prevention programs" ;
  skos:hiddenLabel "School detention" ;
  skos:hiddenLabel "School discipline" ;
  skos:prefLabel "Discipline programs"@en ;
  skos:related agift:child-and-youth-support ;
.
agift:dispute-mediation-programs
  rdf:type skos:Concept ;
  rdfs:label "Dispute mediation programs"@en ;
  skos:broader agift:civil-law ;
  skos:definition """Establishing procedures to settle legal debates or reconcile competing interests. Acting as an intermediary between opposing parties to bring about agreement. Includes facilitating access to these programs.

See also COMMUNITY SERVICES - Counselling services: for the provision of psychological therapy.

See also EMPLOYMENT - Human resources development - Workplace equity and justice programs: for mediating employment disputes.

See also EMPLOYMENT - Workplace agreement processes - Agreement dispute mediation: for resolving workplace agreement negotiations.

See also JUSTICE ADMINISTRATION - Administrative law - Administrative decision appeal: for applications to have a determination reconsidered.

See also JUSTICE ADMINISTRATION - Native title claims - Native title mediation programs: for reconciling Indigenous land claims.""" ;
  skos:hiddenLabel "Court counselling" ;
  skos:hiddenLabel "Dispute resolution services" ;
  skos:hiddenLabel "Legal dispute mediation" ;
  skos:hiddenLabel "Legal mediation programs" ;
  skos:hiddenLabel "Mandatory counselling" ;
  skos:hiddenLabel "Mediation programs" ;
  skos:prefLabel "Dispute mediation programs"@en ;
  skos:related agift:counselling-services ;
.
agift:doping-detection-research
  rdf:type skos:Concept ;
  rdfs:label "Doping detection research"@en ;
  skos:broader agift:sports-drugs-monitoring ;
  skos:definition "Developing tests to reveal the presence of performance-enhancing drugs or masking agents. Conducting research to identify new drugs and their effects as they come into use." ;
  skos:hiddenLabel "Sports drug testing" ;
  skos:prefLabel "Doping detection research"@en ;
.
agift:draft-bill-amendment-process
  rdf:type skos:Concept ;
  rdfs:label "Draft Bill amendment process"@en ;
  skos:broader agift:legislative-drafting ;
  skos:definition """Revising and modifying proposed legal instruments, during their passage through parliament. Incorporating changes in government policy and other developments.

See also GOVERNANCE - Legislative drafting - Legislation review: for amending existing legislation.

See also GOVERNANCE - Parliamentary chamber support - Parliamentary papers: for printing and gazetting of legislation passed through parliament

See also GOVERNANCE - Parliamentary chamber support - Tabling of official documents: for presentation of amended legislation to parliament.""" ;
  skos:prefLabel "Draft Bill amendment process"@en ;
  skos:related agift:legislation-review ;
.
agift:driving-licences-administration
  rdf:type skos:Concept ;
  rdfs:label "Driving licences administration"@en ;
  skos:broader agift:road-transport ;
  skos:definition """Managing the system to approve applications to operate various types of motor vehicles. Testing drivers, issuing or renewing permits and licenses. Includes variation, suspension and cancellation of licenses, administering demerit points and liaison to promote consistency across jurisdictions.

See also EDUCATION AND TRAINING - Community education - Road safety awareness: for driver training programs.""" ;
  skos:hiddenLabel "Driver's licenses" ;
  skos:prefLabel "Driving licences administration"@en ;
  skos:related agift:road-safety-awareness ;
  skos:related agift:road-traffic-regulation ;
  skos:related agift:vehicle-standards ;
.
agift:drugs-and-poisons-regulation
  rdf:type skos:Concept ;
  rdfs:label "Drugs and poisons regulation"@en ;
  skos:broader agift:health-protocol-administration ;
  skos:definition """Monitoring substances used for medicinal purposes, which may have toxic or lethal effects if administered incorrectly or in large doses. Maintaining a register of approved substances. Assessing product applications and manufacturing quality. Restricting the availability of drugs or poisons, and specifying conditions of use.

See also PRIMARY INDUSTRIES - Chemical and pesticide regulation: for the registration of chemicals used in agriculture.""" ;
  skos:hiddenLabel "Medicine regulation" ;
  skos:hiddenLabel "Pharmaceutical regulation" ;
  skos:hiddenLabel "Poisons regulation" ;
  skos:prefLabel "Drugs and poisons regulation"@en ;
  skos:related agift:chemical-and-pesticide-regulation ;
.
agift:early-childhood-education
  rdf:type skos:Concept ;
  rdfs:label "Early childhood education"@en ;
  skos:broader agift:education-and-training ;
  skos:definition """Administering learning programs and related services designed to foster the development of young children, usually under the age of five years. Implementing standards and guidelines to support teachers. Includes determining enrolment criteria.

See also COMMUNITY SERVICES - Community support - Child and youth support: for parental education programs.

See also COMMUNITY SERVICES - Community support - Child-care services: for supervising children when their parents are not available.""" ;
  skos:hiddenLabel "Kindergarten education" ;
  skos:hiddenLabel "Preschool education" ;
  skos:prefLabel "Early childhood education"@en ;
  skos:related agift:child-and-youth-support ;
.
agift:earth-sciences
  rdf:type skos:Concept ;
  rdfs:label "Earth sciences"@en ;
  skos:broader agift:science ;
  skos:definition "Conducting research into geological, water and atmospheric processes. Providing scientific advice on the sustainable management of land and water resources, exploitation of mineral resources, hazard and disaster assessment." ;
  skos:hiddenLabel "Geography" ;
  skos:hiddenLabel "Geological sciences" ;
  skos:hiddenLabel "Geology" ;
  skos:narrower agift:atmospheric-sciences ;
  skos:narrower agift:hydrology ;
  skos:narrower agift:mineral-exploration ;
  skos:narrower agift:oceanography ;
  skos:narrower agift:seismology ;
  skos:prefLabel "Earth sciences"@en ;
.
agift:economic-research
  rdf:type skos:Concept ;
  rdfs:label "Economic research"@en ;
  skos:broader agift:finance-management ;
  skos:definition """Developing new economic measurements and models, estimating quantitative models of economic behaviour, assessing the effects of public policies on the Australian economy, and projecting the effects of alternative policy proposals.
See also FINANCE MANAGEMENT- Financial system management: for policy to maintain stability in the financial system.
See also FINANCE MANAGEMENT- Fiscal policy: for policy for the strategic management and distribution of public money.
See also FINANCE MANAGEMENT - Monetary policy:  for policy to maintain stability of the currency.""" ;
  skos:hiddenLabel "Economic modelling" ;
  skos:prefLabel "Economic research"@en ;
  skos:related agift:financial-system-management ;
  skos:related agift:fiscal-policy ;
  skos:related agift:monetary-policy ;
.
agift:education-and-training
  rdf:type skos:Concept ;
  rdfs:label "EDUCATION AND TRAINING"@en ;
  skos:definition "Formulating policy to support programs that provide skills and knowledge to citizens. Developing strategies to make education available to the broadest possible cross-section of the community. Providing funding to schools, universities, colleges, academies or community groups that provide education and training. Establishing programs to develop and manage educational institutions." ;
  skos:hiddenLabel "Teachers" ;
  skos:hiddenLabel "Teaching" ;
  skos:narrower agift:arts-education ;
  skos:narrower agift:community-education ;
  skos:narrower agift:curriculum-development ;
  skos:narrower agift:early-childhood-education ;
  skos:narrower agift:military-education-and-training ;
  skos:narrower agift:overseas-skills-recognition ;
  skos:narrower agift:school-education ;
  skos:narrower agift:tertiary-education ;
  skos:narrower agift:vocational-education ;
  skos:prefLabel "EDUCATION AND TRAINING"@en ;
  skos:related agift:overseas-student-scholarship-programs ;
.
agift:election-campaigning
  rdf:type skos:Concept ;
  rdfs:label "Election campaigning"@en ;
  skos:broader agift:electoral-matters ;
  skos:definition """Regulating the presentation of policies and platforms by election candidates and political parties. Providing advice on the content of television and newspaper advertisements, media reporting, distribution of pamphlets, shopping centre tours and door-to-door canvassing. Establishing eligibility criteria for parliamentary and non-parliamentary parties, and the nomination and registration of political parties.

See also COMMUNICATIONS - Government media: for advertising campaigns for government programs.""" ;
  skos:hiddenLabel "Political campaigning" ;
  skos:prefLabel "Election campaigning"@en ;
  skos:related agift:government-media ;
.
agift:electoral-boundary-assessment
  rdf:type skos:Concept ;
  rdfs:label "Electoral boundary assessment"@en ;
  skos:broader agift:electoral-matters ;
  skos:definition "Assessing and reviewing the margins of electoral divisions to maintain equal representation. Assessing population projection figures, conducting quota calculations and public consultation. Publicising final boundary determinations." ;
  skos:hiddenLabel "Electorates" ;
  skos:hiddenLabel "Gerrymander prevention" ;
  skos:hiddenLabel "Redistribution Committee" ;
  skos:prefLabel "Electoral boundary assessment"@en ;
.
agift:electoral-matters
  rdf:type skos:Concept ;
  rdfs:label "Electoral matters"@en ;
  skos:broader agift:governance ;
  skos:definition """Administering voting to elect representatives for public office. Conducting referenda to amend the constitution. Maintaining electoral rolls and enrolment procedures. Providing polling booths, ballot papers and scrutiny of electoral processes. Distributing the results of elections via any medium. Includes electoral information and education programs.

See also GOVERNANCE - Constitutional matters - Constitutional referenda: for legislative processes to amend the constitution.""" ;
  skos:narrower agift:declaration-of-interests ;
  skos:narrower agift:election-campaigning ;
  skos:narrower agift:electoral-boundary-assessment ;
  skos:prefLabel "Electoral matters"@en ;
  skos:related agift:constitutional-referenda ;
.
agift:electronic-commerce
  rdf:type skos:Concept ;
  rdfs:label "Electronic commerce"@en ;
  skos:broader agift:communications ;
  skos:definition """Developing policy to support and regulate Australian participation in the global information economy. Administering programs to promote the implementation of information and communications technology for conducting business. Providing funding to foster initiatives in electronic commerce.

See also COMMUNICATIONS - Information management standards - Information technology standards: for hardware and software regulation.""" ;
  skos:hiddenLabel "Digital commerce" ;
  skos:hiddenLabel "E-Business" ;
  skos:hiddenLabel "E-Commerce" ;
  skos:hiddenLabel "Information economy" ;
  skos:hiddenLabel "Internet commerce" ;
  skos:hiddenLabel "Online commerce" ;
  skos:narrower agift:authentication ;
  skos:narrower agift:online-transaction-standards ;
  skos:prefLabel "Electronic commerce"@en ;
  skos:related agift:information-technology-standards ;
.
agift:electronic-postal-services
  rdf:type skos:Concept ;
  rdfs:label "Electronic postal services"@en ;
  skos:broader agift:postal-services ;
  skos:definition "Administering special services through the postal communications network. Providing electronic transactions such as banking, bill payments and business lodgements. Managing electronic mail processing activities, such as barcoding and postcode scanning mechanisms." ;
  skos:hiddenLabel "Internet postal services" ;
  skos:hiddenLabel "Online postal services" ;
  skos:prefLabel "Electronic postal services"@en ;
.
agift:electronic-publishing
  rdf:type skos:Concept ;
  rdfs:label "Electronic publishing"@en ;
  skos:broader agift:publishing ;
  skos:definition """Compiling, editing and disseminating government information in electronic form. Developing website content and multi-media programs.

See also COMMUNICATIONS - Government media: for managing advertising and communications activities.

See also COMMUNICATIONS - Information management standards - Information dissemination: for developing broad-ranging communication strategies.

See also COMMUNICATIONS - Publishing - Website development: for designing and maintaining online information and services.

See also TRADE - Intellectual property management - Copyright registration: for conferring legal ownership over publications.""" ;
  skos:hiddenLabel "Electronic publications" ;
  skos:hiddenLabel "Online publishing" ;
  skos:prefLabel "Electronic publishing"@en ;
  skos:related agift:government-media ;
.
agift:emergency-accommodation
  rdf:type skos:Concept ;
  rdfs:label "Emergency accommodation"@en ;
  skos:broader agift:accommodation-services ;
  skos:definition "Managing services to provide housing for the community in the event of crisis or disaster. Assisting individuals and families following a house fire, natural disaster, or other emergency. Includes accommodation placements in government and non-government housing." ;
  skos:prefLabel "Emergency accommodation"@en ;
  skos:related agift:disaster-relief ;
  skos:related agift:emergency-funding ;
  skos:related agift:emergency-management ;
  skos:related agift:emergency-services ;
  skos:related agift:natural-disasters ;
.
agift:emergency-funding
  rdf:type skos:Concept ;
  rdfs:label "Emergency funding"@en ;
  skos:broader agift:emergency-services ;
  skos:definition """Managing financial resources allocated for the provision of emergency services. Includes receiving revenue, investing funds and making payments to eligible organisations.

See also COMMUNITY SERVICES - Accommodation services - Emergency accommodation: for providing housing after a crisis.

See also COMMUNITY SERVICES - Natural disasters - Disaster relief: for financial assistance to those affected by natural disasters.

See also DEFENCE - Emergency management: for cross-jurisdictional operations to deal with large-scale crises.""" ;
  skos:hiddenLabel "Disaster funds" ;
  skos:hiddenLabel "Emergency funds" ;
  skos:prefLabel "Emergency funding"@en ;
  skos:related agift:emergency-accommodation ;
.
agift:emergency-management
  rdf:type skos:Concept ;
  rdfs:label "Emergency management"@en ;
  skos:broader agift:defence ;
  skos:definition """Managing cross-jurisdictional operations to deal with large-scale crises. Developing policy and strategies for emergency prevention, response and recovery. Coordinating services and resources to provide a comprehensive and integrated emergency management framework.

See also COMMUNITY SERVICES - Accommodation services - Emergency accommodation: for providing temporary housing in times of disaster.

See also COMMUNITY SERVICES - Emergency services: for regional programs offering urgent crisis assistance.

See also COMMUNITY SERVICES - Natural disaster: for emergencies caused by the elements such as floods, earthquakes or cyclones.

See also HEALTH CARE - Public health services - Health disaster preparedness: for strategies to handle a large-scale medical emergency.

See also MARITIME SERVICES - Search and rescue: for coordinating maritime emergency services.

See also SECURITY - Law enforcement: for police services.""" ;
  skos:hiddenLabel "Counter-terrorism activities" ;
  skos:hiddenLabel "Emergencies" ;
  skos:hiddenLabel "Martial law" ;
  skos:hiddenLabel "National emergency" ;
  skos:hiddenLabel "State of emergency" ;
  skos:hiddenLabel "Terrorism" ;
  skos:narrower agift:civil-community-assistance ;
  skos:narrower agift:disaster-support ;
  skos:prefLabel "Emergency management"@en ;
  skos:related agift:emergency-accommodation ;
  skos:related agift:external-security ;
  skos:related agift:military-law ;
.
agift:emergency-services
  rdf:type skos:Concept ;
  rdfs:label "Emergency services"@en ;
  skos:broader agift:community-services ;
  skos:definition """Managing programs to provide urgent assistance in times of crisis or unforeseen circumstances. Monitoring compliance with equipment standards and regulating the use of volunteers. Coordinating government and community-based services within a region, in times of emergency. Includes land-based search and rescue operations outside urban areas.

See also COMMUNITY SERVICES - Accommodation services - Emergency accommodation: for providing temporary housing in times of disaster.

See also COMMUNITY SERVICES - Emergency services - Firefighting services: for urban search and rescue operations.

See also COMMUNITY SERVICES - Natural disasters: for emergencies caused by the elements such as floods, earthquakes, and cyclones.

See also DEFENCE - Emergency management: for cross-jurisdictional operations to deal with large-scale emergencies.

See also HEALTH CARE - Public health services - Health disaster preparedness: for strategies to handle a large-scale medical emergency.

See also MARITIME SERVICES - Search and rescue - Rescue coordination: for coordinating maritime emergency services.

See also SECURITY - Law enforcement: for police services.""" ;
  skos:hiddenLabel "Carelink" ;
  skos:narrower agift:ambulance-services ;
  skos:narrower agift:emergency-funding ;
  skos:narrower agift:firefighting-services ;
  skos:prefLabel "Emergency services"@en ;
  skos:related agift:emergency-accommodation ;
  skos:related agift:firefighting-services ;
  skos:related agift:health-disaster-preparedness ;
  skos:related agift:rescue-coordination ;
.
agift:employment
  rdf:type skos:Concept ;
  rdfs:label "EMPLOYMENT"@en ;
  skos:definition "Formulating policy to support employment growth and regulate public or private sector working environments. Developing strategies to improve workplace relations, productivity and performance. Implementing labour market programs and providing funding. Administering regulatory bodies and arbitration services." ;
  skos:hiddenLabel "Industrial relations" ;
  skos:hiddenLabel "Public service employment" ;
  skos:hiddenLabel "Workplace management" ;
  skos:hiddenLabel "Workplace relations" ;
  skos:narrower agift:human-resources-development ;
  skos:narrower agift:industrial-awards-and-conditions ;
  skos:narrower agift:labour-market-programs ;
  skos:narrower agift:workplace-agreement-processes ;
  skos:prefLabel "EMPLOYMENT"@en ;
  skos:related agift:public-service ;
.
agift:employment-advocacy-services
  rdf:type skos:Concept ;
  rdfs:label "Employment advocacy services"@en ;
  skos:broader agift:workplace-agreement-processes ;
  skos:definition "Providing workplace relations information to employers and employees. Offering advice on rights and obligations, union membership or the implications of industrial action. Developing guidance for the negotiation and implementation of workplace agreements." ;
  skos:hiddenLabel "Advocacy services" ;
  skos:hiddenLabel "Workplace advocacy services" ;
  skos:prefLabel "Employment advocacy services"@en ;
.
agift:employment-services-marketing
  rdf:type skos:Concept ;
  rdfs:label "Employment services marketing"@en ;
  skos:broader agift:labour-market-programs ;
  skos:definition """Administering programs that encourage and assist businesses to employ more staff. Liaising with employers to evaluate their needs for support. Providing information and resources to help locate suitable staff. Managing wage assistance and subsidy schemes. Includes promotional strategies and advertising campaigns to advocate employment in particular industries.

See also EDUCATION AND TRAINING - Vocational education: for on-the-job training in particular disciplines.

See also EDUCATION AND TRAINING - Vocational education - Industry collaboration: Connecting partnerships between industry and tertiary and vocational education to train a responsive workforce based on the skillsets needed by Australian enterprises and industry sectors.""" ;
  skos:hiddenLabel "Employment marketing" ;
  skos:hiddenLabel "Job creation programs" ;
  skos:hiddenLabel "Job search" ;
  skos:hiddenLabel "JobSearch" ;
  skos:hiddenLabel "Supported wages" ;
  skos:hiddenLabel "VolunteerSearch" ;
  skos:hiddenLabel "Wage assistance" ;
  skos:prefLabel "Employment services marketing"@en ;
  skos:related agift:vocational-education ;
.
agift:endangered-species-protection
  rdf:type skos:Concept ;
  rdfs:label "Endangered species protection"@en ;
  skos:broader agift:conservation-programs ;
  skos:definition """Identifying groups of plants or animals that are under threat or at risk of extinction. Evaluating the source of the danger, whether direct harm to individual organisms or the indirect impacts of environmental change. Administering programs to protect and repopulate specific areas. Includes liaison with national parks, scientific research bodies and community groups.

See also ENVIRONMENT - Natural heritage protection - Wilderness area management: for the removal of feral animals and plants.

See also ENVIRONMENT - Natural heritage protection - Wildlife sanctuary management: for facilities to house members of endangered species.""" ;
  skos:hiddenLabel "Rare species" ;
  skos:hiddenLabel "Threatened species" ;
  skos:hiddenLabel "Vulnerable species" ;
  skos:prefLabel "Endangered species protection"@en ;
  skos:related agift:wilderness-area-management ;
  skos:related agift:wildlife-sanctuary-management ;
.
agift:energy-resources
  rdf:type skos:Concept ;
  rdfs:label "Energy resources"@en ;
  skos:broader agift:natural-resources ;
  skos:definition """Developing policy and administering legislation relating to fossil fuels, renewable and other energy industries. Providing advice on energy market reform, research and development, and environmental assessments.

See also CIVIC INFRASTRUCTURE - Energy supply: for regulating the delivery and pricing of energy resources.

See also SCIENCE: for conducting research into the use and development of energy resources.""" ;
  skos:hiddenLabel "Electricity" ;
  skos:hiddenLabel "Fuel prices" ;
  skos:hiddenLabel "Nuclear energy" ;
  skos:narrower agift:fossil-fuel-management ;
  skos:narrower agift:renewable-energy-development ;
  skos:prefLabel "Energy resources"@en ;
  skos:related agift:energy-supply ;
.
agift:energy-supply
  rdf:type skos:Concept ;
  rdfs:label "Energy supply"@en ;
  skos:broader agift:civic-infrastructure ;
  skos:definition """Regulating the provision of energy resources and other utilities. Installing infrastructure to facilitate energy supply. Monitoring providers to ensure all citizens receive an adequate level of service to meet basic requirements. Encouraging consumers to conserve energy, and to support renewable energy development.

See also BUSINESS SUPPORT AND REGULATION - Fair trading compliance - Prices surveillance: for regulating the charges for energy supply.

See also NATURAL RESOURCES - Energy resources: for developing energy-producing industries.""" ;
  skos:hiddenLabel "Electricity services" ;
  skos:hiddenLabel "Gas services" ;
  skos:hiddenLabel "Public utilities management" ;
  skos:hiddenLabel "Water services" ;
  skos:prefLabel "Energy supply"@en ;
  skos:related agift:energy-resources ;
  skos:related agift:prices-surveillance ;
  skos:related agift:water-resources ;
.
agift:engineering-and-technology-sciences
  rdf:type skos:Concept ;
  rdfs:label "Engineering and technology sciences"@en ;
  skos:broader agift:applied-sciences ;
  skos:definition """Conducting research into the practical application of scientific knowledge for systematic design, construction and management activities. Developing products and processes to support industry, communications, defence and civic infrastructure. Includes component analysis, design and manipulation of systems to solve complex problems.

See also CIVIC INFRASTRUCTURE - Civic management - Engineering services: for practical input into civic infrastructure projects.

See also DEFENCE - Defence strategic support - Defence science and technology: for applying scientific knowledge to military activities.

See also SCIENCE - Biological sciences - Genetic engineering: for the design and manipulation of biological organisms.

See also TRADE - Intellectual property management: for registering new products or processes.""" ;
  skos:hiddenLabel "Chemical engineering" ;
  skos:hiddenLabel "Electrical engineering" ;
  skos:hiddenLabel "Information technology" ;
  skos:hiddenLabel "Mechanical engineering" ;
  skos:hiddenLabel "Software engineering" ;
  skos:hiddenLabel "Systems engineering" ;
  skos:hiddenLabel "Technology research" ;
  skos:prefLabel "Engineering and technology sciences"@en ;
  skos:related agift:aircraft-standards ;
  skos:related agift:engineering-services ;
.
agift:engineering-services
  rdf:type skos:Concept ;
  rdfs:label "Engineering services"@en ;
  skos:broader agift:civic-management ;
  skos:definition """Providing professional advice and supervising the design and construction of public works, such as roads, bridges, dams or harbours. Approving plans and conducting inspections to ensure building is completed in accordance with approved plans.

See also CIVIC INFRASTRUCTURE - Civic management - Architectural services: for professional advice on the design and construction of public buildings.

See also CIVIC INFRASTRUCTURE - Civic management - Building regulations and standards: for ensuring works meet legal requirements.

See also SCIENCE - Applied sciences - Engineering and technology sciences: for engineering research and development activities.""" ;
  skos:hiddenLabel "Civil engineering" ;
  skos:prefLabel "Engineering services"@en ;
  skos:related agift:architectural-services ;
  skos:related agift:engineering-and-technology-sciences ;
  skos:related agift:transport-infrastructure-development ;
.
agift:entomology
  rdf:type skos:Concept ;
  rdfs:label "Entomology"@en ;
  skos:broader agift:biological-sciences ;
  skos:definition """Conducting research into insects and their management by understanding the role of insects and other invertebrates in the natural, urban and rural environments. Developing safe, sustainable methods of pest management.

See also PRIMARY INDUSTRIES - Chemical and pesticide regulation: for the registration and use of pesticides.""" ;
  skos:prefLabel "Entomology"@en ;
  skos:related agift:chemical-and-pesticide-regulation ;
.
agift:environment
  rdf:type skos:Concept ;
  rdfs:label "ENVIRONMENT"@en ;
  skos:definition "Developing policy to support the management of the surrounding natural and built environments. Balancing competing requirements to generate long term sustainable benefits for industry, tourism and the community. Protecting elements of the natural and built environment that are of special significance. Includes conservation of the national estate and world heritage concerns." ;
  skos:hiddenLabel "Environmental monitoring" ;
  skos:narrower agift:built-environment ;
  skos:narrower agift:climate-information-services ;
  skos:narrower agift:conservation-programs ;
  skos:narrower agift:environmental-impact-assessment ;
  skos:narrower agift:historic-relic-protection ;
  skos:narrower agift:marine-life-protection-programs ;
  skos:narrower agift:natural-heritage-protection ;
  skos:narrower agift:oceans-governance ;
  skos:narrower agift:pollutant-prevention-programs ;
  skos:narrower agift:world-heritage-listings ;
  skos:prefLabel "ENVIRONMENT"@en ;
  skos:related agift:natural-resources ;
  skos:related agift:water-conservation-plans ;
  skos:related agift:waterway-management ;
.
agift:environmental-impact-assessment
  rdf:type skos:Concept ;
  rdfs:label "Environmental impact assessment"@en ;
  skos:broader agift:environment ;
  skos:definition "Evaluating the effects of industry, tourism or community use on the natural and built environments. Conducting inspections of premises, equipment or operations. Providing advice on proposed infrastructure projects, commercial or residential developments. Includes emergency assessments following industrial accidents or natural disasters." ;
  skos:prefLabel "Environmental impact assessment"@en ;
  skos:related agift:mining-regulations ;
.
agift:epidemiology
  rdf:type skos:Concept ;
  rdfs:label "Epidemiology"@en ;
  skos:broader agift:public-health-services ;
  skos:definition """Administering programs to identify and prevent the large-scale outbreak of disease. Conducting research into the presence of communicable diseases and their distribution within the population. Developing strategies to monitor the incidence of infection and predict a possible epidemic.

See also HEALTH CARE - Medical research - Population-based research: for clinical investigation of health in particular groups.

See also HEALTH CARE - Public health services - Notifiable disease management: for collecting epidemiological data.

See also SCIENCE - Medical and health sciences: for experimental research into human health and disease.""" ;
  skos:prefLabel "Epidemiology"@en ;
  skos:related agift:notifiable-disease-management ;
  skos:related agift:population-based-research ;
.
agift:equipment-licensing
  rdf:type skos:Concept ;
  rdfs:label "Equipment licensing"@en ;
  skos:broader agift:telecommunications ;
  skos:definition "Processing applications and issuing licenses for telecommunications equipment, such as transmitters, wireless rooftop links or cable capacity. Drafting licence conditions. Establishing standards for connecting or labelling telecommunications equipment." ;
  skos:hiddenLabel "Equipment licenses" ;
  skos:prefLabel "Equipment licensing"@en ;
.
agift:ethical-compliance
  rdf:type skos:Concept ;
  rdfs:label "Ethical compliance"@en ;
  skos:broader agift:science ;
  skos:definition "Administering programs to ensure research is carried out in an acceptable manner. Assessing research methods against accepted moral principles and standards of conduct. Monitoring activities, performing inspections and handling complaints." ;
  skos:hiddenLabel "Research ethics" ;
  skos:prefLabel "Ethical compliance"@en ;
.
agift:exchange-rates
  rdf:type skos:Concept ;
  rdfs:label "Exchange rates"@en ;
  skos:broader agift:monetary-policy ;
  skos:definition "Monitoring the value of the Australian dollar currency against the value of other currencies. Forecasting the consequences and economic impact of fluctuations in exchange rates. Developing strategies to minimise those effects." ;
  skos:hiddenLabel "Currency rates" ;
  skos:hiddenLabel "Foreign exchange rates" ;
  skos:hiddenLabel "International exchange rates" ;
  skos:hiddenLabel "Money rates" ;
  skos:prefLabel "Exchange rates"@en ;
.
agift:exhibition-programs
  rdf:type skos:Concept ;
  rdfs:label "Exhibition programs"@en ;
  skos:broader agift:collection-promotion ;
  skos:definition """Planning and implementing displays of material from cultural collections. Conducting research and selecting items for inclusion in displays. Identifying relevant material in other collections. Ensuring installations meet preservation requirements.

See also CULTURAL AFFAIRS - Collection promotion - Publicity programs: for promoting and marketing exhibitions.

See also CULTURAL AFFAIRS - Collection management - Collection acquisition: for negotiating the temporary use of items from other institutions.""" ;
  skos:hiddenLabel "Displays and exhibitions" ;
  skos:prefLabel "Exhibition programs"@en ;
  skos:related agift:publicity-programs ;
.
agift:export-promotion
  rdf:type skos:Concept ;
  rdfs:label "Export promotion"@en ;
  skos:broader agift:export-regulation ;
  skos:definition """Promoting Australian businesses in the global marketplace. Developing long term sustainable exports and diversifying markets through grants schemes. Providing export advice and statistics. Includes conducting promotional programs overseas to enhance the awareness and image of Australian products.

See also INTERNATIONAL RELATIONS - Overseas promotion: for identifying opportunities to promote Australian business overseas.

See also TRADE - Trade expositions: for events to maximise marketing opportunities.""" ;
  skos:hiddenLabel "Export incentives" ;
  skos:prefLabel "Export promotion"@en ;
  skos:related agift:overseas-promotion ;
.
agift:export-regulation
  rdf:type skos:Concept ;
  rdfs:label "Export regulation"@en ;
  skos:broader agift:trade ;
  skos:definition """Controlling the international sale and movement of goods from Australia. Ensuring compliance with domestic and international protocols and guidelines. Issuing export permits and licences, directing price regulation at port terminals and exit points. Includes monitoring international trade and consulting with primary producers, industry organisations and other stakeholders.

See also MARITIME SERVICES - Cargo control: for the handling and storage of exports on marine vessels.

See also MARITIME SERVICES - Port regulation: for managing sea-based exit points.

See also TRANSPORT - Freight movement regulation: for the transportation of goods by air, road or rail.""" ;
  skos:hiddenLabel "Export monitoring" ;
  skos:narrower agift:export-promotion ;
  skos:narrower agift:prohibited-export-control ;
  skos:prefLabel "Export regulation"@en ;
  skos:related agift:cargo-control ;
.
agift:external-security
  rdf:type skos:Concept ;
  rdfs:label "External security"@en ;
  skos:broader agift:security ;
  skos:definition """Developing policy and procedures to protect Australia's international security interests Implementing strategies to maintain peace in external territories and the region. Evaluating risks to Australian citizens, territories and property overseas. Includes liaison with international security and law enforcement bodies.

See also DEFENCE - Emergency management: for cross-jurisdictional operations to deal with large-scale crises.

See also INTERNATIONAL RELATIONS - Defence liaison: for cooperating with other countries in defence matters.

See also INTERNATIONAL RELATIONS - International affairs: for representing Australia's interests overseas.""" ;
  skos:hiddenLabel "International security liaison" ;
  skos:hiddenLabel "International security" ;
  skos:narrower agift:peacekeeping-forces ;
  skos:prefLabel "External security"@en ;
  skos:related agift:defence-liaison ;
  skos:related agift:emergency-management ;
  skos:related agift:intelligence ;
  skos:related agift:national-security ;
.
agift:fair-trading-compliance
  rdf:type skos:Concept ;
  rdfs:label "Fair trading compliance"@en ;
  skos:broader agift:business-support-and-regulation ;
  skos:definition """Developing policy to ensure the ethical conduct of business, and protect consumers from excessive prices or faulty products. Promoting trading practices that support market competition.

See also BUSINESS SUPPORT AND REGULATION - Consumer protection: for educating customers on their rights and obligations.""" ;
  skos:hiddenLabel "Commerce" ;
  skos:hiddenLabel "Fair trading" ;
  skos:hiddenLabel "Industry code" ;
  skos:hiddenLabel "Market regulation" ;
  skos:hiddenLabel "Trade Practices Act" ;
  skos:narrower agift:prices-surveillance ;
  skos:narrower agift:product-safety ;
  skos:narrower agift:trade-practices-compliance ;
  skos:prefLabel "Fair trading compliance"@en ;
  skos:related agift:consumer-protection ;
.
agift:family-law-proceedings
  rdf:type skos:Concept ;
  rdfs:label "Family law proceedings"@en ;
  skos:broader agift:civil-law ;
  skos:definition """Administering the body of law relating to the rights of parents and their children, especially during break-up of the family unit. Hearing matters of divorce, custody and child support.

See also COMMUNITY SERVICES - Financial assistance - Income support schemes: for managing child support payments.""" ;
  skos:hiddenLabel "Child custody" ;
  skos:hiddenLabel "Child support" ;
  skos:hiddenLabel "Custody proceedings" ;
  skos:hiddenLabel "Divorce proceedings" ;
  skos:hiddenLabel "Divorce settlements" ;
  skos:hiddenLabel "Family courts" ;
  skos:hiddenLabel "Family support" ;
  skos:prefLabel "Family law proceedings"@en ;
  skos:related agift:income-support-schemes ;
.
agift:family-reunion-programs
  rdf:type skos:Concept ;
  rdfs:label "Family reunion programs"@en ;
  skos:broader agift:community-support ;
  skos:definition """Assisting groups and individuals to locate and contact relatives from whom they have become separated. Helping reunite birth parents and adopted children. Providing referral and research services to Indigenous and other families separated by foster programs or migration schemes.

See also IMMIGRATION - Migrant services - Migrant settlement programs: for immigration advice about bringing family members to Australia.

See also INDIGENOUS AFFAIRS - Indigenous welfare programs: for assisting Aboriginal or Torres Strait Islander communities.""" ;
  skos:hiddenLabel "Child migration schemes" ;
  skos:hiddenLabel "Family research" ;
  skos:hiddenLabel "Indigenous family reunion services" ;
  skos:hiddenLabel "Link up programs" ;
  skos:hiddenLabel "Separated families" ;
  skos:hiddenLabel "Stolen generations" ;
  skos:prefLabel "Family reunion programs"@en ;
  skos:related agift:indigenous-welfare-programs ;
  skos:related agift:migrant-settlement-programs ;
.
agift:feral-pest-control
  rdf:type skos:Concept ;
  rdfs:label "Feral pest control"@en ;
  skos:broader agift:natural-heritage-protection ;
  skos:definition "Operating programs to remove feral animals and  plants from national parks and wilderness areas." ;
  skos:prefLabel "Feral pest control"@en ;
.
agift:finance-management
  rdf:type skos:Concept ;
  rdfs:label "FINANCE MANAGEMENT"@en ;
  skos:definition "Developing policy for the administration of public funds and other resources. Determining appropriate strategies for raising revenue and regulating expenditure. Monitoring economic indicators and forecasting trends to enable financial planning." ;
  skos:hiddenLabel "Financial policy" ;
  skos:narrower agift:commonwealth-state-funding ;
  skos:narrower agift:currency ;
  skos:narrower agift:economic-research ;
  skos:narrower agift:financial-investment ;
  skos:narrower agift:financial-system-management ;
  skos:narrower agift:fiscal-policy ;
  skos:narrower agift:foreign-investment-control ;
  skos:narrower agift:international-monetary-regulation ;
  skos:narrower agift:monetary-policy ;
  skos:narrower agift:resource-management ;
  skos:narrower agift:retirement-income ;
  skos:narrower agift:taxation ;
  skos:prefLabel "FINANCE MANAGEMENT"@en ;
.
agift:financial-administration
  rdf:type skos:Concept ;
  rdfs:label "Financial administration"@en ;
  skos:broader agift:resource-management ;
  skos:definition """Developing procedures to control the income and expenditure of government organisations. Making payments to employees and suppliers. Managing revenue generated by sales of goods or services. Includes financial planning activities.

See also FINANCE MANAGEMENT - Resource management - Financial budgeting: for documenting public revenues and expenditure.""" ;
  skos:prefLabel "Financial administration"@en ;
  skos:related agift:financial-budgeting ;
.
agift:financial-assistance
  rdf:type skos:Concept ;
  rdfs:label "Financial assistance"@en ;
  skos:broader agift:community-services ;
  skos:definition """Developing policy and programs to provide monetary support to individuals. Setting eligibility criteria and determining appropriate delivery mechanisms for providing financial assistance. 
Making payments and setting policy on entitlements for those in the community in need. Includes ongoing and one-off payments following a specific event.

See also COMMUNITY SERVICES - Natural disasters - Disaster relief: for financial assistance to those affected by natural disasters.

See also COMMUNITY SERVICES - Transport access schemes: for developing eligibility criteria for travel concessions and subsidies.

See also FINANCE MANAGEMENT - Taxation - Taxation compliance: for payments made by individuals through withholding schemes.""" ;
  skos:hiddenLabel "Social security" ;
  skos:hiddenLabel "Welfare payments" ;
  skos:narrower agift:benefits ;
  skos:narrower agift:income-support-schemes ;
  skos:prefLabel "Financial assistance"@en ;
  skos:related agift:asset-assessment ;
  skos:related agift:disaster-relief ;
  skos:related agift:taxation ;
  skos:related agift:transport-access-schemes ;
.
agift:financial-budgeting
  rdf:type skos:Concept ;
  rdfs:label "Financial budgeting"@en ;
  skos:broader agift:resource-management ;
  skos:definition """Providing estimates and documentation for the annual budgeting cycle. Preparing financial statements to justify the allocation of resources. Accounting for expenditure and forecasting revenues.

See also FINANCE MANAGEMENT - Fiscal policy: for strategies to manage public spending and borrowing.""" ;
  skos:hiddenLabel "Accounting" ;
  skos:hiddenLabel "Budget" ;
  skos:hiddenLabel "Financial statements" ;
  skos:prefLabel "Financial budgeting"@en ;
  skos:related agift:financial-administration ;
  skos:related agift:fiscal-policy ;
  skos:related agift:public-expenditure ;
.
agift:financial-institutions-regulation
  rdf:type skos:Concept ;
  rdfs:label "Financial institutions regulation"@en ;
  skos:broader agift:business-support-and-regulation ;
  skos:definition """Developing policy to control banks, credit unions, building societies and friendly societies. Establishing rules for capital adequacy. Monitoring the activities of financial institutions. Investigating suspected breaches of prudential regulations and applying penalties when appropriate.

See also BUSINESS SUPPORT AND REGULATION - Insurance regulation: for monitoring the insurance industry.

See also FINANCE MANAGEMENT - Financial investment: for regulating investment schemes.

See also FINANCE MANAGEMENT - Retirement income - Superannuation regulation: for monitoring retirement funds.""" ;
  skos:hiddenLabel "ADI regulation" ;
  skos:hiddenLabel "Authorised Deposit-Taking Institutions regulation" ;
  skos:hiddenLabel "Authorised capital regulation" ;
  skos:hiddenLabel "Banking regulation" ;
  skos:hiddenLabel "Banks" ;
  skos:hiddenLabel "Building society regulation" ;
  skos:hiddenLabel "Credit union regulation" ;
  skos:hiddenLabel "Friendly society regulation" ;
  skos:hiddenLabel "Provident society regulation" ;
  skos:hiddenLabel "Prudential regulation" ;
  skos:prefLabel "Financial institutions regulation"@en ;
  skos:related agift:financial-investment ;
  skos:related agift:insurance-regulation ;
.
agift:financial-investment
  rdf:type skos:Concept ;
  rdfs:label "Financial investment"@en ;
  skos:broader agift:finance-management ;
  skos:definition """Developing policy to encourage safe and legitimate investment practices. Maintaining prudential oversight of financial instruments and participants in financial markets. Setting penalties for breaches of prudential regulations relating to investment.

See also BUSINESS SUPPORT AND REGULATION - Financial institutions regulation: for monitoring banks and credit unions.

See also BUSINESS SUPPORT AND REGULATION - Insurance regulation: for monitoring the insurance industry.

See also FINANCE MANAGEMENT - Retirement income - Superannuation regulation: for monitoring retirement funds.""" ;
  skos:hiddenLabel "Investment control" ;
  skos:hiddenLabel "Investment" ;
  skos:narrower agift:investment-scheme-regulation ;
  skos:prefLabel "Financial investment"@en ;
  skos:related agift:financial-institutions-regulation ;
.
agift:financial-system-management
  rdf:type skos:Concept ;
  rdfs:label "Financial system management"@en ;
  skos:broader agift:finance-management ;
  skos:definition """Developing policy to maintain stability in the financial system. Includes managing arrangements that allow consumers, business, other organisations, and financial institutions to transfer funds from one to another.

See also FINANCE MANAGEMENT - Economic research: for developing new economic measurements and models and assessing the effects of public policies on the Australian economy.

See also FINANCE MANAGEMENT - - Resource management - Productivity: for developing measures and programs to capture the ability of an economy to harness its physical and human resources to generate output and income.""" ;
  skos:narrower agift:financial-system-monitoring ;
  skos:narrower agift:payments-management ;
  skos:prefLabel "Financial system management"@en ;
  skos:related agift:economic-research ;
.
agift:financial-system-monitoring
  rdf:type skos:Concept ;
  rdfs:label "Financial system monitoring"@en ;
  skos:broader agift:financial-system-management ;
  skos:definition "Developing policy to maintain stability in the financial system. Developing strategies to counteract the effects of instability." ;
  skos:hiddenLabel "Financial reporting standards" ;
  skos:hiddenLabel "Financial system standards" ;
  skos:prefLabel "Financial system monitoring"@en ;
.
agift:finding-aids-development
  rdf:type skos:Concept ;
  rdfs:label "Finding aids development"@en ;
  skos:broader agift:collection-access ;
  skos:definition """Creating tools to promote and enable access to items in cultural collections. Researching and developing content for guides, information sheets or websites. Preparing entries for catalogues, indexes and databases.

See also CULTURAL AFFAIRS - Collection management - Collection accessioning: for listing newly acquired items.""" ;
  skos:hiddenLabel "Catalogue development" ;
  skos:hiddenLabel "Cataloguing" ;
  skos:hiddenLabel "Classification schemes" ;
  skos:hiddenLabel "Collection description" ;
  skos:hiddenLabel "Guide development" ;
  skos:hiddenLabel "Indexing" ;
  skos:prefLabel "Finding aids development"@en ;
  skos:related agift:collection-accessioning ;
  skos:related agift:descriptive-standards ;
  skos:related agift:reference-services ;
.
agift:firefighting-services
  rdf:type skos:Concept ;
  rdfs:label "Firefighting services"@en ;
  skos:broader agift:emergency-services ;
  skos:definition """Providing specially equipped vehicles and trained personnel to prevent, control or extinguish fires. Conducting urban search and rescue operations and managing hazardous materials incidents. Includes managing fire stations, attendance at special events and support for community-based or volunteer fire fighting services.

See also COMMUNITY SERVICES - Emergency services: for search and rescue operations outside urban areas.

See also COMMUNITY SERVICES - Natural disasters: for coordinated responses to major bushfires.

See also DEFENCE - Emergency management: for cross-jurisdictional operations to deal with large-scale crises.

See also EDUCATION AND TRAINING - Community education: for fire safety training.

See also MARITIME SERVICES - Search and rescue - Rescue coordination: for maritime search and rescue operations.""" ;
  skos:hiddenLabel "Bushfire prevention" ;
  skos:hiddenLabel "Fire brigade" ;
  skos:hiddenLabel "Fire fighting" ;
  skos:hiddenLabel "Fire prevention programs" ;
  skos:hiddenLabel "Hazardous materials management" ;
  skos:hiddenLabel "Hazardous waste management" ;
  skos:hiddenLabel "Urban search and rescue" ;
  skos:prefLabel "Firefighting services"@en ;
  skos:related agift:emergency-services ;
.
agift:fiscal-policy
  rdf:type skos:Concept ;
  rdfs:label "Fiscal policy"@en ;
  skos:broader agift:finance-management ;
  skos:definition """Developing policy for the strategic management and distribution of public money. Determining overall levels of public spending required to maintain economic stability. Regulating public borrowing and levels of public debt.

See also FINANCE MANAGEMENT - Economic research: for developing new economic measurements and models and assessing the effects of public policies on the Australian economy.

See also FINANCE MANAGEMENT - Resource management - Financial budgeting: for documenting public revenues and expenditure.

See also FINANCE MANAGEMENT - - Resource management - Productivity: for developing measures and programs to capture the ability of an economy to harness its physical and human resources to generate output and income.""" ;
  skos:narrower agift:public-borrowing ;
  skos:narrower agift:public-debt ;
  skos:narrower agift:public-expenditure ;
  skos:prefLabel "Fiscal policy"@en ;
  skos:related agift:economic-research ;
  skos:related agift:financial-budgeting ;
.
agift:fisheries-industry
  rdf:type skos:Concept ;
  rdfs:label "Fisheries industry"@en ;
  skos:broader agift:marine-and-rural-regulation ;
  skos:definition """Regulating recreational fishing practices and commercial fishing industries. Administering quotas and issuing licenses for controlled activities. Certifying products and methods of catching or harvesting. Conducting assessments and inspections to ensure compliance with standards and policy. Applying penalties for breaches of regulations.

See also ENVIRONMENT - Oceans governance: for management of ocean-based resources.

See also PRIMARY INDUSTRIES - Marine and rural support - Aquacultural industry: for programs to support and develop fishing industries.

See also PRIMARY INDUSTRIES - Marine and rural support - Pastoral industry: for programs to support and develop livestock industries.

See also SCIENCE - Animal and veterinary science: for fish and shellfish research.""" ;
  skos:hiddenLabel "Bycatch regulation" ;
  skos:hiddenLabel "Fishing industry regulation" ;
  skos:hiddenLabel "Seafood industry regulation" ;
  skos:prefLabel "Fisheries industry"@en ;
  skos:related agift:oceans-governance ;
.
agift:food-hygiene-regulation
  rdf:type skos:Concept ;
  rdfs:label "Food hygiene regulation"@en ;
  skos:broader agift:health-protocol-administration ;
  skos:definition """Administering programs to ensure food is produced and handled without risk of contamination. Evaluating performance against established standards and codes of practice. Investigating complaints and initiating disciplinary proceedings or applying penalties when appropriate. Includes product recall or closure of premises found in breach of regulations.

See also HEALTH CARE - Community health services - Health promotion: for providing basic hygiene information to consumers.

See also PRIMARY INDUSTRIES - Marine and rural regulation - Food quality assurance: for programs to support food production.

See also SCIENCE - Medical and health sciences: for research into human health and disease.""" ;
  skos:hiddenLabel "Food safety" ;
  skos:hiddenLabel "Meat inspection" ;
  skos:prefLabel "Food hygiene regulation"@en ;
  skos:related agift:food-quality-assurance ;
  skos:related agift:health-promotion ;
.
agift:food-quality-assurance
  rdf:type skos:Concept ;
  rdfs:label "Food quality assurance"@en ;
  skos:broader agift:marine-and-rural-regulation ;
  skos:definition """Regulating food and beverage production industries. Administering labelling and packaging requirements. Certifying products and methods of production or processing. Conducting assessments and inspections to ensure compliance with standards and policy. Applying penalties for breaches of regulations.

See also HEALTH CARE - Health protocol administration - Food hygiene regulation: for ensuring food is produced and handled without risk of contamination.

See also PRIMARY INDUSTRIES - Chemical and pesticide regulation: for setting maximum chemical residue limits for foodstuffs.

See also SCIENCE - Biological sciences - Biotechnology development: for research into the use of organic processes in food production.

See also SCIENCE - Biological sciences - Genetic engineering: for artificial modification of cellular material.""" ;
  skos:hiddenLabel "Australian food industry" ;
  skos:hiddenLabel "Food industry regulation" ;
  skos:hiddenLabel "Food standards code" ;
  skos:prefLabel "Food quality assurance"@en ;
  skos:related agift:food-hygiene-regulation ;
  skos:related agift:genetic-engineering ;
.
agift:foreign-investment-control
  rdf:type skos:Concept ;
  rdfs:label "Foreign investment control"@en ;
  skos:broader agift:finance-management ;
  skos:definition "Regulating the participation of overseas parties in Australian commercial or financial ventures. Restricting the ownership of Australian assets by foreigners. Includes advice to Australian governments entering into partnerships with foreign investors." ;
  skos:hiddenLabel "Foreign investment review" ;
  skos:hiddenLabel "International investment control" ;
  skos:hiddenLabel "Investment management" ;
  skos:hiddenLabel "Overseas investment control" ;
  skos:prefLabel "Foreign investment control"@en ;
.
agift:forensic-analysis
  rdf:type skos:Concept ;
  rdfs:label "Forensic analysis"@en ;
  skos:broader agift:intelligence ;
  skos:definition "Applying investigative strategies and technologies to gather intelligence or evidence that may be used in a court of law. Analysing available information to reach a conclusion and identifying data that will substantiate the results." ;
  skos:hiddenLabel "Computer forensics" ;
  skos:hiddenLabel "Criminal forensics" ;
  skos:hiddenLabel "Forensic medicine" ;
  skos:prefLabel "Forensic analysis"@en ;
.
agift:forestry-industry
  rdf:type skos:Concept ;
  rdfs:label "Forestry industry"@en ;
  skos:broader agift:marine-and-rural-regulation ;
  skos:definition """Regulating timber cultivation industries. Administering quotas and issuing licenses for controlled activities. Certifying products and methods of growing or harvesting. Conducting assessments and inspections to ensure compliance with standards and policy. Applying penalties for breaches of regulations.

See also PRIMARY INDUSTRIES - Marine and rural support - Silvicultural industry: for programs to support and develop forestry industries.

See also SCIENCE - Agricultural sciences: for conducting research into timber growing and forestry products.""" ;
  skos:hiddenLabel "Regional Forest Agreements" ;
  skos:hiddenLabel "Timber industry regulation" ;
  skos:hiddenLabel "Wood products industry" ;
  skos:prefLabel "Forestry industry"@en ;
  skos:related agift:silvicultural-industry ;
.
agift:fossil-fuel-management
  rdf:type skos:Concept ;
  rdfs:label "Fossil fuel management"@en ;
  skos:broader agift:energy-resources ;
  skos:definition """Regulating the exploitation of coal, oil and natural gas resources. Licensing infrastructure and operational activities. Conducting exploration and mapping deposits of fossil fuels. Granting acreage release for vacant onshore, offshore and coastal areas.

See also NATURAL RESOURCES - Mineral resources - Mining regulations: for granting mining titles and leases.

See also SCIENCE - Earth sciences - Mineral exploration: for conducting research into fossil fuel deposits and their environmental settings.""" ;
  skos:hiddenLabel "Coal" ;
  skos:hiddenLabel "Gas resources" ;
  skos:hiddenLabel "Natural gas resources" ;
  skos:hiddenLabel "Oil resources" ;
  skos:hiddenLabel "Petroleum resources" ;
  skos:prefLabel "Fossil fuel management"@en ;
  skos:related agift:mineral-exploration ;
  skos:related agift:mineral-resources ;
  skos:related agift:mining-regulations ;
.
agift:freedom-of-information
  rdf:type skos:Concept ;
  rdfs:label "Freedom of information"@en ;
  skos:broader agift:administrative-law ;
  skos:definition """Allowing individuals to see what information government holds about them, and to seek correction of that information if they consider it wrong or misleading. Developing  legislation and programs to enhance the transparency of policy making, administrative decision making and government service delivery. Requiring agencies to publish government information and  providing for a right of access by the public to government documents.
See also GOVERNANCE - Open government:  facilitating citizen collaboration by developing services and programs based on open government principles. 
See also JUSTICE ADMINISTRATION - Administrative law - Recordkeeping standards: regulating the creation, capture, management and disposal of government records.
See also JUSTICE ADMINISTRATION - Privacy: for ensuring the confidentiality of records containing personal information.""" ;
  skos:hiddenLabel "FOI" ;
  skos:prefLabel "Freedom of information"@en ;
  skos:related agift:open-government ;
  skos:related agift:privacy- ;
.
agift:freight-movement-regulation
  rdf:type skos:Concept ;
  rdfs:label "Freight movement regulation"@en ;
  skos:broader agift:transport ;
  skos:definition """Developing policy for the transportation of goods by air, rail or road. Monitoring compliance with regulations for carriage of hazardous materials, dangerous goods and oversize containers. Includes advice on best practice logistics and standardised freight movement across jurisdictions.

See also MARITIME SERVICES - Cargo control: for movement of sea freight.

See also TRADE - Export regulation: for trade controls.

See also TRADE - Import regulation: for trade controls.""" ;
  skos:hiddenLabel "Freight control" ;
  skos:hiddenLabel "Freight" ;
  skos:hiddenLabel "Hazardous materials management" ;
  skos:hiddenLabel "Hazardous waste management" ;
  skos:prefLabel "Freight movement regulation"@en ;
  skos:related agift:cargo-control ;
  skos:related agift:rail-transport ;
.
agift:fundraising-and-donation-schemes
  rdf:type skos:Concept ;
  rdfs:label "Fundraising and donation schemes"@en ;
  skos:broader agift:sport-and-fitness-development ;
  skos:definition """Administering programs to encourage investment in sporting events. Visiting individuals and corporations to request gifts, contributions or sponsorship. Providing advice on advertising opportunities, donation of prizes, tax incentives and bequests.

See also BUSINESS SUPPORT AND REGULATION - Association registration: for registering fundraising organisations.

See also BUSINESS SUPPORT AND REGULATION - Business registration and licensing: for issuing permits for fundraising events.

See also BUSINESS SUPPORT AND REGULATION - Business sponsorship: for regulating corporate funding of events.""" ;
  skos:hiddenLabel "Donation schemes" ;
  skos:hiddenLabel "Sports funding" ;
  skos:prefLabel "Fundraising and donation schemes"@en ;
  skos:related agift:association-registration ;
.
agift:gambling-support-services
  rdf:type skos:Concept ;
  rdfs:label "Gambling support services"@en ;
  skos:broader agift:community-recreational-programs ;
  skos:definition """Administering programs to assist people with compulsive betting problems or gambling addictions. Providing services such as group support and positive reinforcement activities. Arranging access to counselling for gamblers and their families. Includes community information services and advice to the gaming industry.

See also COMMUNITY SERVICES - Counselling services: for the provision of group therapy or psychological advice.""" ;
  skos:hiddenLabel "Gambling addiction" ;
  skos:hiddenLabel "Gambling services" ;
  skos:prefLabel "Gambling support services"@en ;
  skos:related agift:counselling-services ;
  skos:related agift:gaming-industry-regulation ;
.
agift:games-administration
  rdf:type skos:Concept ;
  rdfs:label "Games administration"@en ;
  skos:broader agift:sport-and-fitness-development ;
  skos:definition """Organising and managing major sporting events. Strategic planning and coordination of activities. Liaising with sporting bodies, sponsors, volunteers and organising committees. Arranging access to venues or facilities and overseeing tenders and infrastructure development.

See also SPORT AND RECREATION - Community recreational programs - Volunteer support programs: for organising groups to assist at major sporting events.

See also SPORT AND RECREATION - Sport and fitness development - Fundraising and donation schemes: for encouraging investment in sporting events.

See also SPORT AND RECREATION - Sport and fitness development - Games promotion: for marketing major sporting events.""" ;
  skos:hiddenLabel "Commonwealth Games administration" ;
  skos:hiddenLabel "Olympic Games administration" ;
  skos:hiddenLabel "Sporting event administration" ;
  skos:prefLabel "Games administration"@en ;
  skos:related agift:volunteer-support-programs ;
.
agift:games-promotion
  rdf:type skos:Concept ;
  rdfs:label "Games promotion"@en ;
  skos:broader agift:sport-and-fitness-development ;
  skos:definition """Developing advertising campaigns for major sporting events. Organising strategic marketing activities to reach target audiences. Liaising with sponsors, journalists and the media, locally and internationally.

See also INTERNATIONAL RELATIONS - Overseas promotion: for negotiating opportunities to host or participate in international sporting events.

See also SPORT AND RECREATION - Sport and fitness development - Fundraising and donation schemes: for encouraging sponsorship of sporting events.

See also SPORT AND RECREATION - Sport and fitness development - Games administration: for organising and managing major sporting events.""" ;
  skos:hiddenLabel "Commonwealth Games promotion" ;
  skos:hiddenLabel "Olympic Games promotion" ;
  skos:hiddenLabel "Sporting event promotion" ;
  skos:prefLabel "Games promotion"@en ;
  skos:related agift:overseas-promotion ;
.
agift:gaming-industry-regulation
  rdf:type skos:Concept ;
  rdfs:label "Gaming industry regulation"@en ;
  skos:broader agift:sport-and-recreation ;
  skos:definition """Monitoring gambling and betting activities to ensure compliance with legislation. Conducting audits of accounts, procedures and machines in organisations with gaming facilities. Issuing licences and providing training to licence holders. Promoting responsible gambling practices and allocating revenue from gaming activities to community projects.

See also SPORT AND RECREATION - Community recreational programs - Gambling support services: for programs to assist compulsive gamblers.""" ;
  skos:hiddenLabel "Casino regulation" ;
  skos:hiddenLabel "Gambling industry" ;
  skos:hiddenLabel "Greyhound racing" ;
  skos:hiddenLabel "Horse racing" ;
  skos:hiddenLabel "Poker machine licensing" ;
  skos:prefLabel "Gaming industry regulation"@en ;
  skos:related agift:gambling-support-services ;
.
agift:garden-management
  rdf:type skos:Concept ;
  rdfs:label "Garden management"@en ;
  skos:broader agift:public-land-management ;
  skos:definition """Administering public land where ornamental or useful plants are cultivated. Managing site layout, planting and landscaping. Ensuring facilities are kept clean and maintained. Monitoring rights of access and opening hours. Organising seasonal public events.

See also CIVIC INFRASTRUCTURE - Public land management - Recreational park management: for administering public leisure areas and playgrounds.

See also ENVIRONMENT - Natural heritage protection - Nature reserve management: for the maintenance of native flora and fauna reserves.""" ;
  skos:hiddenLabel "Botanic gardens" ;
  skos:hiddenLabel "Community gardens" ;
  skos:prefLabel "Garden management"@en ;
  skos:related agift:national-park-management ;
  skos:related agift:nature-reserve-management ;
  skos:related agift:park-and-reserve-services ;
  skos:related agift:recreational-park-management ;
  skos:related agift:wilderness-area-management ;
.
agift:general-insurance
  rdf:type skos:Concept ;
  rdfs:label "General insurance"@en ;
  skos:broader agift:insurance-regulation ;
  skos:definition """Monitoring the activities of general insurance providers to ensure compliance with government policy and standards. Investigating suspected breaches of prudential regulations and applying penalties when appropriate.

See also BUSINESS SUPPORT AND REGULATION - Insurance regulation - Life insurance: for regulating the activities of life insurance providers.""" ;
  skos:hiddenLabel "Accident insurance" ;
  skos:hiddenLabel "Business insurance" ;
  skos:hiddenLabel "Car insurance" ;
  skos:hiddenLabel "Contents insurance" ;
  skos:hiddenLabel "Fire insurance" ;
  skos:hiddenLabel "Home insurance" ;
  skos:hiddenLabel "Indemnity insurance" ;
  skos:hiddenLabel "Private health insurance" ;
  skos:hiddenLabel "Travel insurance" ;
  skos:prefLabel "General insurance"@en ;
  skos:related agift:health-insurance-schemes ;
  skos:related agift:life-insurance ;
.
agift:genetic-engineering
  rdf:type skos:Concept ;
  rdfs:label "Genetic engineering"@en ;
  skos:broader agift:biological-sciences ;
  skos:definition """Conducting research into the chromosome structure of reproductive cells. Copying, modifying and transferring genetic material to produce or reduce biological products, traits and characteristics in animals or plants. Includes health and environmental impact studies for genetically modified organisms (GMO).

See also PRIMARY INDUSTRIES - Marine and rural regulation - Food quality assurance: for regulating the use of genetically modified organisms in food production.

See also SCIENCE - Biological sciences - Biochemistry: for broader research into molecular biology.

See also SCIENCE - Biological sciences - Biotechnology development: for selective breeding programs.

See also TRADE - Intellectual property management: for registering new products or processes.""" ;
  skos:hiddenLabel "Gene sciences" ;
  skos:hiddenLabel "Genetic modification" ;
  skos:prefLabel "Genetic engineering"@en ;
  skos:related agift:biochemistry ;
  skos:related agift:food-quality-assurance ;
.
agift:governance
  rdf:type skos:Concept ;
  rdfs:label "GOVERNANCE"@en ;
  skos:definition "Executing legislative processes in Houses of Parliament, assemblies or councils, where officers are elected to represent citizens. Administering committees that report to legislative bodies. Managing elections of government representatives and sponsoring major community celebrations. Includes official duties carried out by the titular head of the government or municipality. Includes managing the machinery of government processes at all levels of government." ;
  skos:hiddenLabel "City council" ;
  skos:hiddenLabel "Councils" ;
  skos:hiddenLabel "Federal government" ;
  skos:hiddenLabel "Government" ;
  skos:hiddenLabel "Houses of parliament" ;
  skos:hiddenLabel "Local government" ;
  skos:hiddenLabel "Shire councils" ;
  skos:hiddenLabel "State government" ;
  skos:hiddenLabel "Territory government" ;
  skos:narrower agift:appointment-management ;
  skos:narrower agift:civic-celebrations ;
  skos:narrower agift:constitutional-matters ;
  skos:narrower agift:electoral-matters ;
  skos:narrower agift:honours-and-awards-programs ;
  skos:narrower agift:intergovernmental-relations ;
  skos:narrower agift:legislative-drafting ;
  skos:narrower agift:official-protocol ;
  skos:narrower agift:open-government ;
  skos:narrower agift:parliamentary-chamber-support ;
  skos:narrower agift:parliamentary-committee-and-member-support ;
  skos:narrower agift:public-administration ;
  skos:prefLabel "GOVERNANCE"@en ;
.
agift:government-auditing
  rdf:type skos:Concept ;
  rdfs:label "Government auditing"@en ;
  skos:broader agift:public-administration ;
  skos:definition """Reviewing the financial or performance management of a government organisation or entity and reporting findings to the legislative body.

See also BUSINESS SUPPORT AND REGULATION - Business process auditing: for general auditing.

See also  GOVERNANCE - Public  administation - Corruption  prevention: preventing, detecting and investigating serious and systemic corruption issues in government agencies. 

See also GOVERNANCE - Public administration - Integrity compliance: encouraging ethical behaviour and compliance with official codes of conduct.

See also GOVERNANCE - Public administration - Whistleblowing: disclosing illegal, immoral or illegitimate practices under the control of their employer by government employees.""" ;
  skos:prefLabel "Government auditing"@en ;
  skos:related agift:business-process-auditing ;
.
agift:government-media
  rdf:type skos:Concept ;
  rdfs:label "Government media"@en ;
  skos:broader agift:communications ;
  skos:definition """Managing government advertising and communications activities. Developing advertisements and advertising campaign material. Includes production of media releases, public notices, commercial and employment opportunities.

See also BUSINESS SUPPORT AND REGULATION - Government procurement regulation: for managing tendering processes.

See also COMMUNICATIONS - Information management standards - Information dissemination: for developing broad-ranging communication strategies.

See also COMMUNICATIONS - Internet - Social media: policy and programs encouraging governments to consult widely with citizens via social media platforms.

See also COMMUNITY SERVICES - Community engagement: Governments inviting the commmunity to participate in community consultation.

See also EMPLOYMENT - Human resources development - Recruitment programs: for managing staff selection exercises.

See also GOVERNANCE - Electoral matters - Election campaigning: for regulating the media activities of election candidates and political parties.""" ;
  skos:hiddenLabel "Government advertising" ;
  skos:hiddenLabel "Government communications" ;
  skos:hiddenLabel "Media releases" ;
  skos:hiddenLabel "Public relations" ;
  skos:prefLabel "Government media"@en ;
  skos:related agift:advertising-campaigns ;
  skos:related agift:community-engagement ;
  skos:related agift:election-campaigning ;
  skos:related agift:electronic-publishing ;
  skos:related agift:government-procurement-regulation ;
  skos:related agift:information-dissemination ;
  skos:related agift:publicity-programs ;
  skos:related agift:publishing ;
.
agift:government-procurement-regulation
  rdf:type skos:Concept ;
  rdfs:label "Government procurement regulation"@en ;
  skos:broader agift:business-support-and-regulation ;
  skos:definition """Administering the processes of tendering and awarding government contracts for the provision of goods and services. Developing policy and guidelines to direct procurement activities. Managing preferred supplier arrangements.

See also FINANCE MANAGEMENT - Resource management - Contract management: for administering agreements for the provision of goods and services.""" ;
  skos:hiddenLabel "Endorsed Supplier Arrangements" ;
  skos:hiddenLabel "Government purchasing" ;
  skos:hiddenLabel "Government tendering" ;
  skos:hiddenLabel "Preferred supplier arrangements" ;
  skos:hiddenLabel "Procurement policy" ;
  skos:hiddenLabel "Purchasing" ;
  skos:hiddenLabel "Request for Proposal" ;
  skos:hiddenLabel "Tender management" ;
  skos:prefLabel "Government procurement regulation"@en ;
  skos:related agift:contract-management ;
  skos:related agift:government-media ;
.
agift:hansard-services
  rdf:type skos:Concept ;
  rdfs:label "Hansard services"@en ;
  skos:broader agift:parliamentary-chamber-support ;
  skos:definition """Producing the official record of the proceedings of Parliament. Documenting the debates and speeches of Members, public and private hearings and parliamentary committees. Transcribing and publishing proceedings in paper and electronic format. Managing databases of Hansard reports. Includes all chambers in all levels of government.

See also JUSTICE ADMINISTRATION - Court reporting: for records of court proceedings.""" ;
  skos:hiddenLabel "Parliamentary proceedings" ;
  skos:prefLabel "Hansard services"@en ;
  skos:related agift:court-reporting ;
.
agift:harbour-management
  rdf:type skos:Concept ;
  rdfs:label "Harbour management"@en ;
  skos:broader agift:maritime-services ;
  skos:definition """Building and maintaining infrastructure to provide protection for ships from wind, waves and currents. Developing policy for commercial and recreational use of harbour facilities, and monitoring the environmental impact of activities. Includes liaison to promote coordination and consistency among harbour authorities from different jurisdictions.

See also ENVIRONMENT - Oceans governance: for management and protection of marine environments.

See also MARITIME SERVICES - Marina management: for dockage facilities for small craft.

See also MARITIME SERVICES - Port regulation: for managing sea-based entry and exit points.

See also NATURAL RESOURCES - Water resources - Waterway management: for regulating the use of rivers and catchment areas.

See also SCIENCE - Earth sciences - Oceanography: for conducting research into marine environments.""" ;
  skos:hiddenLabel "Breakwaters" ;
  skos:hiddenLabel "Sea walls" ;
  skos:prefLabel "Harbour management"@en ;
  skos:related agift:oceans-governance ;
.
agift:head-of-government-protocol
  rdf:type skos:Concept ;
  rdfs:label "Head of Government protocol"@en ;
  skos:broader agift:official-protocol ;
  skos:definition """Organising the activities of Heads of Government in carrying out their constitutional, statutory, ceremonial and public duties. Making arrangements to support official protocol such as dress code, official decoration, customs and procedures.

See also GOVERNANCE - Official protocol - Ceremonial events and representation: for official conduct during ritual or traditional proceedings.

See also GOVERNANCE - Official protocol - Official establishment management: for administering the buildings and grounds of official residences.

See also GOVERNANCE - Official protocol - Official hospitality: for planning the reception and entertainment of high-level government representatives.

See also GOVERNANCE - Official protocol - Official visits: for organising travel and itineraries for business, cultural or social visits by high-level government officials.""" ;
  skos:hiddenLabel "Governor-General's protocol" ;
  skos:hiddenLabel "Lord Mayor's protocol" ;
  skos:hiddenLabel "Mayoral protocol" ;
  skos:hiddenLabel "Premier's protocol" ;
  skos:hiddenLabel "Prime Ministerial protocol" ;
  skos:hiddenLabel "Vice regal protocol" ;
  skos:prefLabel "Head of Government protocol"@en ;
  skos:related agift:ceremonial-events-and-representation ;
.
agift:health-care
  rdf:type skos:Concept ;
  rdfs:label "HEALTH CARE"@en ;
  skos:definition "Providing and coordinating programs for the prevention, diagnosis and treatment of disease or injury. Developing policy to support the provision of health care services and medical research. Administering regulatory schemes for health care products and pharmaceuticals." ;
  skos:hiddenLabel "Health services" ;
  skos:narrower agift:community-health-services ;
  skos:narrower agift:health-insurance-schemes ;
  skos:narrower agift:health-protocol-administration ;
  skos:narrower agift:hospital-services ;
  skos:narrower agift:medical-research ;
  skos:narrower agift:public-health-services ;
  skos:narrower agift:special-needs-services ;
  skos:narrower agift:veterans-health-services ;
  skos:prefLabel "HEALTH CARE"@en ;
.
agift:health-disaster-preparedness
  rdf:type skos:Concept ;
  rdfs:label "Health disaster preparedness"@en ;
  skos:broader agift:public-health-services ;
  skos:definition """Developing strategies to handle a large-scale medical emergency. Planning a coordinated counter-disaster response to and recovery from health disasters. Ensuring adequate supplies of drugs and blood, and the availability of medical equipment and trained personnel.

See also COMMUNITY SERVICES - Emergency services: for regional programs offering urgent crisis assistance.

See also DEFENCE - Emergency management: for cross-jurisdictional operations to deal with large-scale emergencies.

See also HEALTH CARE - Public health services - Medical quarantine services: for isolating infectious individuals.

See also HEALTH CARE - Public health services - Notifiable disease management: for alerting authorities of a possible health disaster.""" ;
  skos:hiddenLabel "Health contingency" ;
  skos:hiddenLabel "Health disasters" ;
  skos:prefLabel "Health disaster preparedness"@en ;
  skos:related agift:emergency-services ;
.
agift:health-hazard-prevention
  rdf:type skos:Concept ;
  rdfs:label "Health hazard prevention"@en ;
  skos:broader agift:public-health-services ;
  skos:definition """Managing programs to reduce public exposure to health risks. Developing campaigns to raise community awareness of dangerous substances or potential sources of injury. Establishing standards and guidelines to protect individuals who come into contact with hazardous substances or environments.

See also EMPLOYMENT - Human resources development - Occupational health and safety: for implementing health hazard guidelines in the workplace.

See also HEALTH CARE - Community health services - Health promotion: for providing basic information to support good health.""" ;
  skos:hiddenLabel "Anti-smoking campaigns" ;
  skos:hiddenLabel "Biosafety" ;
  skos:hiddenLabel "Drug and alcohol awareness" ;
  skos:hiddenLabel "Early detection" ;
  skos:hiddenLabel "Health risk management" ;
  skos:hiddenLabel "Manual handling standards" ;
  skos:hiddenLabel "Needle disposal" ;
  skos:hiddenLabel "Passive smoking guidelines" ;
  skos:hiddenLabel "Repetitive strain injury" ;
  skos:prefLabel "Health hazard prevention"@en ;
  skos:related agift:occupational-health-and-safety ;
.
agift:health-insurance-schemes
  rdf:type skos:Concept ;
  rdfs:label "Health insurance schemes"@en ;
  skos:broader agift:health-care ;
  skos:definition """Administering programs that provide financial guarantees against risk of disease or injury. Developing policy to support the operation of universal health insurance schemes, allowing subsidised medical treatment within the public health system.

See also BUSINESS SUPPORT AND REGULATION - Insurance regulation - General insurance: for regulating private health insurers.

See also COMMUNITY SERVICES - Financial assistance - Benefits: for medical insurance gap cover.

See also COMMUNITY SERVICES - Financial assistance - Benefits: for private health insurance rebates.

See also EMPLOYMENT - Human resources development - Workers compensation schemes: for workplace insurance.""" ;
  skos:hiddenLabel "Medical indemnity" ;
  skos:hiddenLabel "Medical insurance" ;
  skos:hiddenLabel "Medicare" ;
  skos:hiddenLabel "Pharmaceutical benefits" ;
  skos:hiddenLabel "Public health insurance" ;
  skos:prefLabel "Health insurance schemes"@en ;
  skos:related agift:general-insurance ;
.
agift:health-promotion
  rdf:type skos:Concept ;
  rdfs:label "Health promotion"@en ;
  skos:broader agift:community-health-services ;
  skos:definition """Administering information programs to improve the physical and mental wellbeing of individuals in the community. Developing campaigns to encourage activities that result in good health. Providing advice on basic aspects of health care, and disease or injury prevention.

See also COMMUNITY SERVICES - Community support - Child and youth support: for parental education programs.

See also EDUCATION AND TRAINING - Community education - Adult education programs: for community-based health education programs.

See also EDUCATION AND TRAINING - Community education - School education: for health education of school-aged children.

See also HEALTH CARE - Public health services - Health hazard prevention: for activities to reduce public exposure to health risks.

See also SPORT AND RECREATION - Community recreational programs - Public fitness promotion: for raising awareness of the health benefits of physical activity.""" ;
  skos:hiddenLabel "Consumers health forum" ;
  skos:hiddenLabel "Food and nutrition" ;
  skos:hiddenLabel "Health information" ;
  skos:hiddenLabel "Healthy eating" ;
  skos:hiddenLabel "Nutrition advice" ;
  skos:hiddenLabel "Safe sex awareness" ;
  skos:hiddenLabel "Sanitation advice" ;
  skos:prefLabel "Health promotion"@en ;
  skos:related agift:child-and-youth-support ;
  skos:related agift:food-hygiene-regulation ;
  skos:related agift:public-fitness-promotion ;
.
agift:health-protocol-administration
  rdf:type skos:Concept ;
  rdfs:label "Health protocol administration"@en ;
  skos:broader agift:health-care ;
  skos:definition "Developing policy to regulate activities that are fundamental to the promotion of health and prevention of disease. Establishing standards and guidelines to support consistent procedures across jurisdictions." ;
  skos:hiddenLabel "Health care standards" ;
  skos:hiddenLabel "Health regulation" ;
  skos:narrower agift:drugs-and-poisons-regulation ;
  skos:narrower agift:food-hygiene-regulation ;
  skos:narrower agift:practitioner-discipline ;
  skos:narrower agift:practitioner-registration ;
  skos:prefLabel "Health protocol administration"@en ;
.
agift:historic-relic-protection
  rdf:type skos:Concept ;
  rdfs:label "Historic relic protection"@en ;
  skos:broader agift:environment ;
  skos:definition """Developing policy and programs to protect built artefacts of particular heritage, scientific or social significance. Establishing standards for maintaining and preserving historic relics. Providing funding for joint projects with business or the community.

See also ENVIRONMENT - Built environment: for programs to conserve the built environment.

See also ENVIRONMENT - Natural heritage protection: for programs to conserve the biological environment.

See also INDIGENOUS AFFAIRS - Indigenous heritage conservation: for protecting areas directly associated with Aboriginal and Torres Strait Islander culture.""" ;
  skos:hiddenLabel "Artefact protection" ;
  skos:hiddenLabel "Community relic protection" ;
  skos:hiddenLabel "Maritime heritage" ;
  skos:hiddenLabel "Relic protection" ;
  skos:hiddenLabel "Shipwreck relic protection" ;
  skos:hiddenLabel "Space debris protection" ;
  skos:prefLabel "Historic relic protection"@en ;
  skos:related agift:built-environment ;
.
agift:honours-and-awards-programs
  rdf:type skos:Concept ;
  rdfs:label "Honours and awards programs"@en ;
  skos:broader agift:governance ;
  skos:definition """Coordinating and promoting ceremonies to pay tribute to notable achievements. Establishing selection criteria and the framework of levels of honour. Designing and producing medals. Researching and evaluating nominations. Maintaining a register of awards. Preparing congratulatory messages.

See also DEFENCE - Australian Defence Forces - Badges and insignia: for military honours and awards.""" ;
  skos:hiddenLabel "Australian Service medal" ;
  skos:hiddenLabel "Australian of the Year" ;
  skos:hiddenLabel "Awards programs" ;
  skos:hiddenLabel "Commonwealth Recognition Awards" ;
  skos:prefLabel "Honours and awards programs"@en ;
  skos:related agift:badges-and-insignia ;
  skos:related agift:cultural-awards-and-scholarships ;
.
agift:horticultural-industry
  rdf:type skos:Concept ;
  rdfs:label "Horticultural industry"@en ;
  skos:broader agift:marine-and-rural-support ;
  skos:definition """Administering programs to support the commercial production of fruit, vegetables and flowers. Assisting industry growth and development. Encouraging businesses to adopt innovative practices, processes and products. Providing advice on cultivation methods and business management to improve competitiveness.

See also PRIMARY INDUSTRIES - Marine and rural regulation - Agricultural industry: for monitoring and regulating crop farming industries.

See also PRIMARY INDUSTRIES - Marine and rural support - Silvicultural industry: for programs to support and develop forestry industries.

See also PRIMARY INDUSTRIES - Marine and rural support - Viticultural industry: for programs to support and develop grape growing and wine making industries.

See also SCIENCE - Agricultural sciences: for horticultural research.""" ;
  skos:hiddenLabel "Flower industry" ;
  skos:hiddenLabel "Fruit growing industry" ;
  skos:hiddenLabel "Gardening industry" ;
  skos:hiddenLabel "Horticulture" ;
  skos:hiddenLabel "Vegetable farming industry" ;
  skos:prefLabel "Horticultural industry"@en ;
  skos:related agift:agricultural-industry ;
.
agift:hospital-administration
  rdf:type skos:Concept ;
  rdfs:label "Hospital administration"@en ;
  skos:broader agift:hospital-services ;
  skos:definition "Providing trained personnel to assist citizens who are injured or ill and require medical treatment. Managing staff and facilities at hospitals. Administering internal security, investigation and disciplinary procedures. Monitoring standards where hospital management activities are outsourced." ;
  skos:hiddenLabel "Infirmary administration" ;
  skos:prefLabel "Hospital administration"@en ;
.
agift:hospital-services
  rdf:type skos:Concept ;
  rdfs:label "Hospital services"@en ;
  skos:broader agift:health-care ;
  skos:definition "Developing policy for the provision of health care through institutions offering a wide range of treatments and services. Establishing programs to support the provision of hospital services. Includes liaison across jurisdictions to coordinate services and operations." ;
  skos:hiddenLabel "Hospitals" ;
  skos:narrower agift:hospital-administration ;
  skos:narrower agift:patient-care ;
  skos:narrower agift:pharmaceutical-and-drug-support ;
  skos:prefLabel "Hospital services"@en ;
.
agift:hospital-teaching-programs
  rdf:type skos:Concept ;
  rdfs:label "Hospital teaching programs"@en ;
  skos:broader agift:vocational-education ;
  skos:definition "Administering programs of on-the-job training for professionals within the hospital system. Managing joint ventures with tertiary institutions. Monitoring compliance with standards and guidelines. Includes nursing courses, internships and work experience for medical students." ;
  skos:hiddenLabel "Medical internship programs" ;
  skos:hiddenLabel "Nursing education programs" ;
  skos:hiddenLabel "Student doctor programs" ;
  skos:hiddenLabel "Teaching hospitals" ;
  skos:prefLabel "Hospital teaching programs"@en ;
.
agift:housing-industry-policy
  rdf:type skos:Concept ;
  rdfs:label "Housing industry policy"@en ;
  skos:broader agift:civic-infrastructure ;
  skos:definition """Developing policy and programs to ensure the adequacy of land supply and construction activity to meet demand and improve housing affordability.
See also CIVIC INFRASTRUCTURE - Civic management - Town planning: for controlled urban development.

See also NATURAL RESOURCES - Land use planning: for research into future needs for infrastructure and facilities.""" ;
  skos:hiddenLabel "Housing affordability" ;
  skos:hiddenLabel "Housing supply" ;
  skos:prefLabel "Housing industry policy"@en ;
  skos:related agift:town-planning ;
.
agift:human-resources-development
  rdf:type skos:Concept ;
  rdfs:label "Human resources development"@en ;
  skos:broader agift:employment ;
  skos:definition """Developing policy and programs for staff support and management. Providing career planning advice, professional development and training. Conducting research into recruitment, retention and organisational demographics, to support long-term planning for human resources development.

See also DEFENCE - Defence force careers: for human resources development in the defence forces.""" ;
  skos:hiddenLabel "Career development" ;
  skos:hiddenLabel "Personnel management" ;
  skos:hiddenLabel "Staff development" ;
  skos:hiddenLabel "Staffing" ;
  skos:narrower agift:occupational-health-and-safety ;
  skos:narrower agift:recruitment-programs ;
  skos:narrower agift:termination-processes ;
  skos:narrower agift:workers-compensation-schemes ;
  skos:narrower agift:workplace-discrimination-monitoring ;
  skos:narrower agift:workplace-equity-and-justice-programs ;
  skos:prefLabel "Human resources development"@en ;
  skos:related agift:defence-force-careers ;
.
agift:human-rights-obligations
  rdf:type skos:Concept ;
  rdfs:label "Human rights obligations"@en ;
  skos:broader agift:justice-administration ;
  skos:definition """Administering programs to ensure the freedoms to which all people are entitled, are upheld. Monitoring compliance with principles which may be constitutionally entrenched and guaranteed, recognised at common law, or declared by an international legal instrument. Includes investigations into breaches and promotion of human rights obligations and principles.

See also IMMIGRATION - Refugee services: for assistance to asylum seekers and victims of human rights violations.

See also JUSTICE ADMINISTRATION - Privacy guideline monitoring: for ensuring individual rights to confidentiality of personal information.""" ;
  skos:hiddenLabel "Civil liberties" ;
  skos:hiddenLabel "Civil rights" ;
  skos:prefLabel "Human rights obligations"@en ;
  skos:related agift:refugee-services ;
.
agift:hydrology
  rdf:type skos:Concept ;
  rdfs:label "Hydrology"@en ;
  skos:broader agift:earth-sciences ;
  skos:definition """Conducting research into water systems, on land and underground. Providing scientific advice on water cycles and flood warning information. Environmental and commercial assessment of projects such as dams and hydropower stations. Determining the impact of changes in land use, stream flow and climate on sediment and nutrient levels, and local ecology. Includes rivers, glaciers, catchment areas and geysers.

See also ENVIRONMENT - Oceans governance: for the management and protection of marine environments.

See also NATURAL RESOURCES - Water resources: for management and economic development of water systems.

See also SCIENCE - Earth sciences - Oceanography: for research into marine environments.""" ;
  skos:hiddenLabel "Flood research" ;
  skos:hiddenLabel "Water catchment studies" ;
  skos:hiddenLabel "Water sciences" ;
  skos:prefLabel "Hydrology"@en ;
  skos:related agift:oceans-governance ;
.
agift:immigration
  rdf:type skos:Concept ;
  rdfs:label "IMMIGRATION"@en ;
  skos:definition """Assisting people wishing to enter Australia on a permanent or temporary basis. Developing policy to establish entry or deportation requirements for migrants and visitors. Includes strategies for the management of illegal immigrants.

See also CULTURAL AFFAIRS: for activities to celebrate multiculturalism.""" ;
  skos:hiddenLabel "Ethnic affairs" ;
  skos:hiddenLabel "Migrants" ;
  skos:hiddenLabel "Migration policy" ;
  skos:narrower agift:citizenship ;
  skos:narrower agift:deportation ;
  skos:narrower agift:detention-programs ;
  skos:narrower agift:migrant-services ;
  skos:narrower agift:refugee-services ;
  skos:narrower agift:travel-authorisation ;
  skos:prefLabel "IMMIGRATION"@en ;
  skos:related agift:cultural-affairs ;
.
agift:import-regulation
  rdf:type skos:Concept ;
  rdfs:label "Import regulation"@en ;
  skos:broader agift:trade ;
  skos:definition """Controlling the international purchase and movement of goods into Australia. Ensuring compliance with domestic and international protocols and guidelines. Setting quotas, import licensing arrangements and customs regulations. Includes inspections and cargo clearance.

See also MARITIME SERVICES - Cargo control: for the handling and storage of imports on marine vessels.

See also MARITIME SERVICES - Port regulation: for managing sea-based entry points.

See also TRANSPORT - Freight movement regulation: for the transportation of goods by air, road or rail.""" ;
  skos:hiddenLabel "Customs regulation" ;
  skos:hiddenLabel "Imports" ;
  skos:hiddenLabel "Inspection services" ;
  skos:hiddenLabel "Inspections" ;
  skos:narrower agift:prohibited-import-control ;
  skos:narrower agift:tariff-regulation ;
  skos:prefLabel "Import regulation"@en ;
  skos:related agift:cargo-control ;
.
agift:income-assessment
  rdf:type skos:Concept ;
  rdfs:label "Income assessment"@en ;
  skos:broader agift:taxation ;
  skos:definition """Evaluating earnings to determine the amount of taxation payable by an individual or organisation. Developing lodgement procedures for tax returns and issuing guidelines for tax agents. Processing notices of assessment and refunds. Issuing tax file numbers to individuals. 

See also BUSINESS SUPPORT AND REGULATION - Business registration and licensing: for issuing numbers to companies and other organisations.""" ;
  skos:hiddenLabel "Company tax" ;
  skos:hiddenLabel "Income tax" ;
  skos:hiddenLabel "Medicare levy" ;
  skos:hiddenLabel "Personal tax" ;
  skos:hiddenLabel "Tax file numbers" ;
  skos:hiddenLabel "Tax returns" ;
  skos:prefLabel "Income assessment"@en ;
  skos:related agift:business-registration-and-licensing ;
  skos:related agift:taxation-compliance ;
.
agift:income-support-schemes
  rdf:type skos:Concept ;
  rdfs:label "Income support schemes"@en ;
  skos:broader agift:financial-assistance ;
  skos:definition """Administering programs to provide financial assistance to individuals with low earnings. Providing advice on entitlements. Assessing eligibility and processing payments. 

See also CIVIC INFRASTRUCTURE - Public housing: for allocating community accommodation to those in need.

See also COMMUNITY SERVICES - Community support - Veterans' entitlements: for social support to returned service personnel.

See also COMMUNITY SERVICES - Financial assistance - Benefits: for financial assistance which is not means tested.

See also FINANCE MANAGEMENT - Retirement income - Asset assessment: for evaluating the resources of retired individuals.

See also FINANCE MANAGEMENT - Taxation - Taxation compliance: for payments made by individuals through withholding schemes.

See also INDIGENOUS AFFAIRS - Indigenous welfare programs: for social support to Aboriginal and Torres Strait Islander communities.""" ;
  skos:hiddenLabel "Abstudy" ;
  skos:hiddenLabel "Age pensions" ;
  skos:hiddenLabel "Aged concession" ;
  skos:hiddenLabel "Aged pensions" ;
  skos:hiddenLabel "Allowances" ;
  skos:hiddenLabel "Austudy" ;
  skos:hiddenLabel "Carer's pensions" ;
  skos:hiddenLabel "Concession cards" ;
  skos:hiddenLabel "Defence service pensions" ;
  skos:hiddenLabel "Disability support pension" ;
  skos:hiddenLabel "Domestic assistance" ;
  skos:hiddenLabel "Entitlements" ;
  skos:hiddenLabel "Farm help" ;
  skos:hiddenLabel "Health care cards" ;
  skos:hiddenLabel "Invalid pensions" ;
  skos:hiddenLabel "Old age pensions" ;
  skos:hiddenLabel "Pension cards" ;
  skos:hiddenLabel "Pensions" ;
  skos:hiddenLabel "Rates rebate" ;
  skos:hiddenLabel "Rebates" ;
  skos:hiddenLabel "Rental assistance" ;
  skos:hiddenLabel "Service pensions" ;
  skos:hiddenLabel "Sickness benefits" ;
  skos:hiddenLabel "Single parent pensions" ;
  skos:hiddenLabel "Student benefits" ;
  skos:hiddenLabel "Unemployment benefits" ;
  skos:hiddenLabel "War pensions" ;
  skos:hiddenLabel "War widows pensions" ;
  skos:hiddenLabel "Widows' pensions" ;
  skos:prefLabel "Income support schemes"@en ;
  skos:related agift:family-law-proceedings ;
  skos:related agift:public-housing ;
.
agift:independent-living-services
  rdf:type skos:Concept ;
  rdfs:label "Independent living services"@en ;
  skos:broader agift:special-needs-services ;
  skos:definition """Managing programs to provide in-home support for aged or disabled persons, those recovering from injury, suffering disease or mental illness. Providing trained staff, carers and assistance to enable patients to remain at home. Includes 'halfway' or group houses where residents live independently under supervision.

See also COMMUNITY SERVICES - Counselling services: for the provision of group therapy or psychological advice.

See also HEALTH CARE - Special needs services - Residential services: for managing live-in facilities.""" ;
  skos:hiddenLabel "Carers" ;
  skos:hiddenLabel "Community care" ;
  skos:hiddenLabel "Disability services" ;
  skos:hiddenLabel "Halfway houses" ;
  skos:hiddenLabel "Home care" ;
  skos:hiddenLabel "Nursing aide" ;
  skos:hiddenLabel "Personal care" ;
  skos:hiddenLabel "Sheltered accommodation" ;
  skos:hiddenLabel "Supervised residences" ;
  skos:prefLabel "Independent living services"@en ;
  skos:related agift:counselling-services ;
  skos:related agift:patient-care ;
.
agift:indigenous-advocacy
  rdf:type skos:Concept ;
  rdfs:label "Indigenous advocacy"@en ;
  skos:broader agift:indigenous-affairs ;
  skos:definition """Providing access to information regarding rights, protections and entitlements for Aboriginal and Torres Strait Islander peoples. Representing and supporting individuals or groups to ensure rights are upheld.

See also COMMUNITY SERVICES - Social justice and equity: for ensuring equal access to community services.

See also INDIGENOUS AFFAIRS - Indigenous reconcilation: for administering programs and services to promote understanding and agreement between Indigenous and non-Indigenous Australians.""" ;
  skos:prefLabel "Indigenous advocacy"@en ;
  skos:related agift:indigenous-reconciliation ;
  skos:related agift:social-justice-and-equity ;
.
agift:indigenous-affairs
  rdf:type skos:Concept ;
  rdfs:label "INDIGENOUS AFFAIRS"@en ;
  skos:definition "Developing policy to support the advancement of Aboriginal and Torres Strait Islander people. Establishing programs to develop, manage and deliver services to Aboriginal and Torres Strait Islander people. Includes protecting areas directly associated with Aboriginal and Torres Strait Islander culture." ;
  skos:hiddenLabel "Aboriginal affairs" ;
  skos:hiddenLabel "Islander affairs" ;
  skos:hiddenLabel "Torres Strait Islander affairs" ;
  skos:narrower agift:indigenous-advocacy ;
  skos:narrower agift:indigenous-cultural-heritage ;
  skos:narrower agift:indigenous-enterprise-development ;
  skos:narrower agift:indigenous-health-services ;
  skos:narrower agift:indigenous-land-management ;
  skos:narrower agift:indigenous-reconciliation ;
  skos:narrower agift:indigenous-welfare-programs ;
  skos:prefLabel "INDIGENOUS AFFAIRS"@en ;
.
agift:indigenous-cultural-heritage
  rdf:type skos:Concept ;
  rdfs:label "Indigenous cultural heritage"@en ;
  skos:broader agift:indigenous-affairs ;
  skos:definition """Managing programs to protect and promote the material, intellectual and spiritual traditions of Aboriginal and Torres Strait Islander peoples. Encouraging research into Indigenous culture. Establishing and maintaining cultural resource collections. Negotiating special custodial arrangements with Indigenous peoples. Initiating projects to compile and record indigenous oral histories, genealogies and languages.

See also INDIGENOUS AFFAIRS - Indigenous heritage conservation: for protecting sacred sites and other areas of cultural significance.""" ;
  skos:hiddenLabel "Aboriginal cultural heritage" ;
  skos:hiddenLabel "Torres Strait Islander cultural heritage" ;
  skos:narrower agift:cultural-artefact-repatriation ;
  skos:prefLabel "Indigenous cultural heritage"@en ;
  skos:related agift:indigenous-enterprise-development ;
  skos:related agift:indigenous-heritage-conservation ;
  skos:related agift:multicultural-heritage-promotion ;
.
agift:indigenous-enterprise-development
  rdf:type skos:Concept ;
  rdfs:label "Indigenous enterprise development"@en ;
  skos:broader agift:indigenous-affairs ;
  skos:definition """Administering programs to support the growth of businesses owned or operated by Aboriginal and Torres Strait Islander communities or individuals. Providing advice and services to assist the establishment of new ventures.

See also INDIGENOUS AFFAIRS - Indigenous cultural heritage: for programs to protect the traditions of Aboriginal and Torres Strait Islander peoples.

See also INDIGENOUS AFFAIRS - Indigenous heritage conservation: for managing sacred sites.""" ;
  skos:hiddenLabel "Aboriginal enterprise development" ;
  skos:hiddenLabel "Torres Strait Islander enterprise development" ;
  skos:prefLabel "Indigenous enterprise development"@en ;
  skos:related agift:indigenous-cultural-heritage ;
.
agift:indigenous-health-services
  rdf:type skos:Concept ;
  rdfs:label "Indigenous health services"@en ;
  skos:broader agift:indigenous-affairs ;
  skos:definition """Developing policy and programs to support the physical and mental wellbeing of citizens in Aboriginal or Torres Strait Islander communities. Conducting planning and evaluation in consultation with local authorities. Encouraging participation to ensure community needs are adequately addressed.

See also HEALTH CARE - Community health services - Primary health care: for the provision of essential health services.""" ;
  skos:hiddenLabel "Aboriginal health services" ;
  skos:hiddenLabel "Torres Strait Islander health services" ;
  skos:prefLabel "Indigenous health services"@en ;
  skos:related agift:primary-health-care ;
.
agift:indigenous-heritage-conservation
  rdf:type skos:Concept ;
  rdfs:label "Indigenous heritage conservation"@en ;
  skos:broader agift:indigenous-land-management ;
  skos:definition """Developing policy and programs to protect areas directly associated with Aboriginal and Torres Strait Islander culture. Establishing standards for maintaining and preserving Indigenous heritage areas, such as control of public access. Providing funding for joint projects with business or the community. Developing land use agreements and site management plans.

See also ENVIRONMENT - Built environment: for programs to protect the built environment.

See also ENVIRONMENT - Historic relic protection: for programs to conserve significant artefacts.

See also ENVIRONMENT - Natural heritage protection: for programs to conserve the biological environment.

See also INDIGENOUS AFFAIRS - Indigenous cultural heritage: for protecting the material, intellectual and spiritual traditions of Indigenous Australians.""" ;
  skos:prefLabel "Indigenous heritage conservation"@en ;
  skos:related agift:built-environment ;
  skos:related agift:indigenous-cultural-heritage ;
  skos:related agift:land-councils ;
.
agift:indigenous-land-management
  rdf:type skos:Concept ;
  rdfs:label "Indigenous land management"@en ;
  skos:broader agift:indigenous-affairs ;
  skos:definition """Developing policies and programs to manage traditional lands and seas owned by Aboriginal and Torres Strait Islander peoples. Assisting in the acquisition and management of lands and seas to achieve economic, environmental, social and cultural benefits.

See also JUSTICE ADMINISTRATION - Native title claims: administering procedures to assess Indigenous interest in or rights to the use of specified areas of land or water. Identifying traditional customs and connections with a particular region. Includes processing applications, providing advice and support for litigation.""" ;
  skos:narrower agift:indigenous-heritage-conservation ;
  skos:narrower agift:land-councils ;
  skos:prefLabel "Indigenous land management"@en ;
  skos:related agift:land-councils ;
  skos:related agift:native-title-claims ;
.
agift:indigenous-reconciliation
  rdf:type skos:Concept ;
  rdfs:label "Indigenous reconciliation"@en ;
  skos:broader agift:indigenous-affairs ;
  skos:definition """Administering programs and services to promote understanding and agreement between Indigenous and non-Indigenous Australians. Ensuring government policy encompasses respect for the aspirations and rights of Aboriginal and Torres Strait Islander communities. Supporting activities to increase tolerance and cross-cultural awareness.

See also INDIGENOUS AFFAIRS - Indigenous advocacy: for providing access to information regarding rights, protections and entitlements for Aboriginal and Torres Strait Islander peoples.

See also INDIGENOUS AFFAIRS - Indigenous land management -  Indigenous cultural heritage: for programs to protect and promote Aboriginal and Torres Strait Islander traditions.""" ;
  skos:hiddenLabel "Aboriginal reconciliation" ;
  skos:hiddenLabel "Reconciliation programs" ;
  skos:hiddenLabel "Torres Strait Islander reconciliation" ;
  skos:prefLabel "Indigenous reconciliation"@en ;
  skos:related agift:indigenous-advocacy ;
.
agift:indigenous-welfare-programs
  rdf:type skos:Concept ;
  rdfs:label "Indigenous welfare programs"@en ;
  skos:broader agift:indigenous-affairs ;
  skos:definition """Providing social support services specific to Aboriginal or Torres Strait Islander communities. Includes programs to expand Indigenous access to education and employment services, improve living conditions and assist families in crisis.

See also COMMUNITY SERVICES - Community support - Family reunion programs: for assistance bringing together relatives who have become separated.

See also COMMUNITY SERVICES - Counselling services: for the provision of group therapy or psychological advice.

See also COMMUNITY SERVICES - Financial assistance: for monetary support to individuals.

See also INDIGENOUS AFFAIRS - Indigenous health services: for community health programs.""" ;
  skos:hiddenLabel "Aboriginal welfare programs" ;
  skos:hiddenLabel "Torres Strait Islander welfare programs" ;
  skos:prefLabel "Indigenous welfare programs"@en ;
  skos:related agift:family-reunion-programs ;
.
agift:industrial-awards-and-conditions
  rdf:type skos:Concept ;
  rdfs:label "Industrial awards and conditions"@en ;
  skos:broader agift:employment ;
  skos:definition """Regulating the conduct of employers and employees across a particular industry or occupation. Issuing awards with regard to rates of pay and working conditions. Developing policy to support the establishment and use of industrial awards. Hearing disputes and offering independent arbitration services.

See also DEFENCE - Defence force careers - Military employment services: for employment conditions in the defence forces.

See also EMPLOYMENT - Human resources development - Occupational health and safety: for programs to prevent death, injury or disease in the workplace.

See also EMPLOYMENT - Workplace agreement processes: for regulating the conduct of employer and employees within an organisation.""" ;
  skos:hiddenLabel "Arbitration" ;
  skos:hiddenLabel "Income awards and conditions" ;
  skos:narrower agift:award-conditions ;
  skos:narrower agift:remuneration-review ;
  skos:prefLabel "Industrial awards and conditions"@en ;
  skos:related agift:military-employment-services ;
.
agift:industry-assistance-schemes
  rdf:type skos:Concept ;
  rdfs:label "Industry assistance schemes"@en ;
  skos:broader agift:business-support-and-regulation ;
  skos:definition """Developing policy to support the growth and management of secondary and tertiary industries. Identifying markets or investment opportunities. Encouraging businesses to adopt innovative practices, processes and products. Providing advice on production methods and business management to improve competitiveness.

See also BUSINESS SUPPORT AND REGULATION - Small business services - Small business advocacy: for assistance to enterprises of limited size.

See also EDUCATION AND TRAINING - Vocational education - Industry collaboration: Connecting partnerships between industry and tertiary and vocational education to train a responsive workforce based on the skillsets needed by Australian enterprises and industry sectors.
See also PRIMARY INDUSTRIES - Marine and rural support: for assistance to primary industries.""" ;
  skos:hiddenLabel "Manufacturing industry support" ;
  skos:hiddenLabel "Secondary industry support" ;
  skos:hiddenLabel "Services industry support" ;
  skos:hiddenLabel "Tertiary industry support" ;
  skos:prefLabel "Industry assistance schemes"@en ;
  skos:related agift:marine-and-rural-regulation ;
  skos:related agift:small-business-advocacy ;
.
agift:industry-collaboration
  rdf:type skos:Concept ;
  rdfs:label "Industry collaboration"@en ;
  skos:broader agift:vocational-education ;
  skos:definition """Connecting partnerships between industry and tertiary and vocational education to train a responsive workforce based on the skillsets needed by Australian enterprises and industry sectors.
See also BUSINESS SUPPORT AND REGULATION - Industry assistance schemes: developing policy to support the growth and management of secondary and tertiary industries.
See also EMPLOYMENT - Labour market programs - Employment services marketing: for administering programs that encourage and assist businesses to employ more staff. Liaising with employers to evaluate their needs for support. Providing information and resources to help locate suitable staff. Managing wage assistance and subsidy schemes. Includes promotional strategies and advertising campaigns to advocate employment in particular industries.""" ;
  skos:prefLabel "Industry collaboration"@en ;
  skos:related agift:labour-market-programs ;
.
agift:industry-development
  rdf:type skos:Concept ;
  rdfs:label "Industry development"@en ;
  skos:broader agift:business-support-and-regulation ;
  skos:definition """Monitoring the management of secondary and tertiary industries. Developing quality assurance programs, operating standards and other regulatory mechanisms. Issuing licenses for controlled activities. Certifying products and production methods. Conducting assessments and inspections to ensure compliance with standards and policy. Applying penalties for breaches of regulations.

See also BUSINESS SUPPORT AND REGULATION - Small business services - Small business development: for monitoring enterprises of limited size.

See also PRIMARY INDUSTRIES - Marine and rural regulation: for monitoring primary industries.""" ;
  skos:hiddenLabel "Innovation" ;
  skos:hiddenLabel "Manufacturing industry regulation" ;
  skos:hiddenLabel "Secondary industry regulation" ;
  skos:hiddenLabel "Services industry regulation" ;
  skos:hiddenLabel "Tertiary industry regulation" ;
  skos:prefLabel "Industry development"@en ;
  skos:related agift:marine-and-rural-support ;
  skos:related agift:small-business-development ;
.
agift:inflation
  rdf:type skos:Concept ;
  rdfs:label "Inflation"@en ;
  skos:broader agift:monetary-policy ;
  skos:definition "Establishing inflation targets. Monitoring relative amounts of currency in circulation and the resulting price increases or decreases. Forecasting the effects of inflation and developing strategies to minimise those effects." ;
  skos:hiddenLabel "Price rises" ;
  skos:prefLabel "Inflation"@en ;
  skos:related agift:prices-surveillance ;
.
agift:information-dissemination
  rdf:type skos:Concept ;
  rdfs:label "Information dissemination"@en ;
  skos:broader agift:information-management-standards ;
  skos:definition """Developing strategies to effectively communicate government information. Promoting government-wide or cross-jurisdictional initiatives to provide access to government services and information. Planning advertising campaigns. Includes government shopfronts, remote access points and kiosks.

See also COMMUNICATIONS - Government media: for managing advertising and communications activities.

See also COMMUNICATIONS - Publishing: for producing information resources.

See also COMMUNICATIONS - Publishing - Website development: for designing and maintaining online information and services.""" ;
  skos:hiddenLabel "Government shopfronts" ;
  skos:hiddenLabel "Portals" ;
  skos:hiddenLabel "Web portals" ;
  skos:prefLabel "Information dissemination"@en ;
  skos:related agift:government-media ;
  skos:related agift:website-development ;
.
agift:information-management-standards
  rdf:type skos:Concept ;
  rdfs:label "Information management standards"@en ;
  skos:broader agift:communications ;
  skos:definition """Developing policy to support the organisation and use of government information. Providing advice on the availability of new communications technology and the implications for government business. Encouraging the implementation of best practice information management strategies. Includes guidelines for ensuring the accessibility of government information to individuals with special needs.

See also COMMUNICATIONS - Electronic commerce - Online transaction standards: for facilitating the conduct of electronic commerce.

See also JUSTICE ADMINISTRATION - Administrative law - Recordkeeping standards: for regulating the creation, capture, management and disposal of government records.

See also JUSTICE ADMINISTRATION - Privacy guideline monitoring: for ensuring the confidentiality of personal information.

See also SECURITY - Information security: for data security standards.""" ;
  skos:hiddenLabel "Accessibility standards" ;
  skos:narrower agift:data-management ;
  skos:narrower agift:information-dissemination ;
  skos:narrower agift:information-technology-standards ;
  skos:prefLabel "Information management standards"@en ;
  skos:related agift:online-transaction-standards ;
.
agift:information-security
  rdf:type skos:Concept ;
  rdfs:label "Information security"@en ;
  skos:broader agift:security ;
  skos:definition """Administering guidelines and standards for the protection of government networks and information systems. Conducting research into cryptology and the development of codes. Monitoring compliance with government security policy. Providing advice and tools to assist organisations to assess and improve their information systems.

See also COMMUNICATIONS - Electronic commerce - Authentication: for managing the infrastructure to validate online transactions.

See also COMMUNICATIONS - Information management standards - Information technology standards: for hardware and software regulation.

See also JUSTICE ADMINISTRATION - Administrative law - Recordkeeping standards: for regulating the creation, capture, management and disposal of government records.""" ;
  skos:hiddenLabel "Communication security" ;
  skos:hiddenLabel "Cryptology" ;
  skos:hiddenLabel "Cybersecurity" ;
  skos:hiddenLabel "Data security standards" ;
  skos:prefLabel "Information security"@en ;
  skos:related agift:authentication ;
.
agift:information-technology-standards
  rdf:type skos:Concept ;
  rdfs:label "Information technology standards"@en ;
  skos:broader agift:information-management-standards ;
  skos:definition """Establishing guidelines and models to regulate the implementation of government hardware and software. Promoting the application of information technology standards to support interoperability and data exchange. Providing advice on the implementation of standards and monitoring compliance.

See also COMMUNICATIONS - Electronic commerce - Online transaction standards: for guidelines to support electronic commerce.

See also COMMUNICATIONS - Information management standards - Data management: for metadata standards and data matching guidelines.

See also SECURITY - Information security: for data security standards.""" ;
  skos:hiddenLabel "Data transfer protocols" ;
  skos:hiddenLabel "Interoperability standards" ;
  skos:prefLabel "Information technology standards"@en ;
  skos:related agift:electronic-commerce ;
  skos:related agift:online-transaction-standards ;
.
agift:infrastructure-planning
  rdf:type skos:Concept ;
  rdfs:label "Infrastructure planning"@en ;
  skos:broader agift:civic-infrastructure ;
  skos:definition """Identifying strategic investment priorities, policy, and regulatory reforms in the transport, water, energy and communications sectors, and providing advice on nationally-significant economic infrastructure to governments, investors and owners.
See also CIVIC INFRASTRUCTURE - Civic management - Town planning: for controlled urban development.
See also CIVIC INFRASTRUCTURE - Integrated services planning:  for providing coordinated services across districts.
See also CIVIC INFRASTRUCTURE - Regional development: for infrastructure projects across multiple districts.
See also NATURAL RESOURCES - Land use planning: for research into future needs for infrastructure and facilities.""" ;
  skos:prefLabel "Infrastructure planning"@en ;
  skos:related agift:regional-development ;
.
agift:insurance-regulation
  rdf:type skos:Concept ;
  rdfs:label "Insurance regulation"@en ;
  skos:broader agift:business-support-and-regulation ;
  skos:definition """Developing policy to control schemes that provide financial guarantees against risk of loss or harm. Maintaining prudential oversight of insurance providers. Setting penalties for breaches of prudential regulations relating to insurance. Providing assistance and advice to citizens seeking insurance.

See also BUSINESS SUPPORT AND REGULATION - Financial institutions regulation: for monitoring banks and credit unions.

See also EMPLOYMENT - Human resources development - Workers compensation schemes: for workplace insurance.

See also FINANCE MANAGEMENT - Financial investment: for regulating investment schemes.

See also FINANCE MANAGEMENT - Retirement income - Superannuation regulation: for monitoring retirement funds.""" ;
  skos:narrower agift:general-insurance ;
  skos:narrower agift:life-insurance ;
  skos:prefLabel "Insurance regulation"@en ;
  skos:related agift:financial-institutions-regulation ;
.
agift:integrated-services-planning
  rdf:type skos:Concept ;
  rdfs:label "Integrated services planning"@en ;
  skos:broader agift:civic-infrastructure ;
  skos:definition """Developing strategies to provide essential community services in a coordinated and equitable manner. Evaluating land use data and town planning objectives. Identifying the requirements of particular districts. Bringing together related services, according to target audience.

See also CIVIC INFRASTRUCTURE - Civic management - Town planning: for controlled urban development.

See also CIVIC INFRASTRUCTURE - Infrastructure planning; providing advice on nationally-significant economic infrastructure to governments, investors and owners.

See also CIVIC INFRASTRUCTURE - Regional development: for infrastructure projects across multiple districts.

See also CIVIC INFRASTRUCTURE - Transport network maintenance: for developing interconnecting public transport services.

See also NATURAL RESOURCES - Land use planning: for research into future needs for infrastructure and facilities.

See also NATURAL RESOURCES - Land use planning - Land use zoning: for allocating areas of land with regard to their use.""" ;
  skos:hiddenLabel "Planning" ;
  skos:prefLabel "Integrated services planning"@en ;
  skos:related agift:town-planning ;
.
agift:integrity-compliance
  rdf:type skos:Concept ;
  rdfs:label "Integrity compliance"@en ;
  skos:broader agift:public-administration ;
  skos:definition """Encouraging ethical behaviour and compliance with official codes of conduct.
See also GOVERNANCE - Public administration - Corruption prevention:  preventing, detecting and investigating serious and systemic corruption issues in Australian government agencies.
See also GOVERNANCE - Public administration - Government auditing: reviewing the financial or performance management of a government organisation or entity and reporting findings to the legislative body.
See also GOVERNANCE - Public administration - Whistleblowing: disclosing illegal, immoral or illegitimate practices under the control of their employer by government employees.
See also JUSTICE ADMINISTRATION - Criminal law: administering the body of law that governs actions punishable by the state
See also SECURITY - Law enforcement:  formulating policy to support the maintenance of rules and regulations that govern the actions of citizens. Including activities to address 'white-collar' and corporate crime.""" ;
  skos:prefLabel "Integrity compliance"@en ;
.
agift:intellectual-property-management
  rdf:type skos:Concept ;
  rdfs:label "Intellectual property management"@en ;
  skos:broader agift:trade ;
  skos:definition "Developing policy to protect the rights of creative workers in literary, artistic, industrial or scientific fields. Regulating the administration of copyright, patents, trademarks and design registration. Includes proprietary knowledge such as development of new plant varieties or commercial trade secrets." ;
  skos:narrower agift:design-rights-management ;
  skos:narrower agift:patent-rights-management ;
  skos:narrower agift:plant-breeders-rights-management ;
  skos:narrower agift:trademark-registration ;
  skos:prefLabel "Intellectual property management"@en ;
.
agift:intelligence
  rdf:type skos:Concept ;
  rdfs:label "Intelligence"@en ;
  skos:broader agift:security ;
  skos:definition """Developing policy and procedures to support the collection of information by covert means, to protect Australia from threats to national security. Conducting surveillance operations and investigating the use of technology to facilitate intelligence gathering. Includes foreign intelligence gathering in relation to strategic, political, economic or scientific activities.

See also SECURITY - External security: for sharing intelligence information with other countries.

See also SECURITY - Law enforcement - Protective services: for protective surveillance.""" ;
  skos:hiddenLabel "Aerial surveillance" ;
  skos:hiddenLabel "Espionage" ;
  skos:hiddenLabel "Surveillance" ;
  skos:narrower agift:forensic-analysis ;
  skos:narrower agift:intelligence-liaison ;
  skos:narrower agift:intelligence-support ;
  skos:prefLabel "Intelligence"@en ;
  skos:related agift:external-security ;
.
agift:intelligence-liaison
  rdf:type skos:Concept ;
  rdfs:label "Intelligence liaison"@en ;
  skos:broader agift:intelligence ;
  skos:definition """Gathering information on illegal activity in support of law enforcement operations. Developing national and international networks of officers and agencies to facilitate the interchange of intelligence and reporting on criminal trends.

See also SECURITY - Intelligence - Intelligence support: for gathering military information to support special operations.""" ;
  skos:hiddenLabel "Criminal intelligence" ;
  skos:hiddenLabel "Intelligence exchange" ;
  skos:prefLabel "Intelligence liaison"@en ;
  skos:related agift:intelligence-support ;
.
agift:intelligence-support
  rdf:type skos:Concept ;
  rdfs:label "Intelligence support"@en ;
  skos:broader agift:intelligence ;
  skos:definition """Gathering military information in support of special operations. Compiling knowledge that might prove detrimental to an enemy. Conducting investigations and surveillance to support the planning and conduct of exceptional defence or security activities. 

See also DEFENCE - Military operations - Special operations: for deployment of highly trained military personnel.

See also SECURITY - Intelligence - Intelligence liaison: for gathering criminal information to support law enforcement operations.""" ;
  skos:hiddenLabel "Military intelligence" ;
  skos:hiddenLabel "Reconnaissance" ;
  skos:prefLabel "Intelligence support"@en ;
  skos:related agift:intelligence-liaison ;
  skos:related agift:protective-services ;
  skos:related agift:special-operations ;
.
agift:interest-rates
  rdf:type skos:Concept ;
  rdfs:label "Interest rates"@en ;
  skos:broader agift:monetary-policy ;
  skos:definition "Setting interest rates by buying and selling in money markets. Monitoring interest rates and forecasting the consequences and economic impact of fluctuations in interest rates. Developing strategies to minimise those effects." ;
  skos:prefLabel "Interest rates"@en ;
.
agift:intergovernment-policy-dissemination
  rdf:type skos:Concept ;
  rdfs:label "Intergovernment policy dissemination"@en ;
  skos:broader agift:intergovernmental-relations ;
  skos:definition "Managing the distribution of advice on decisions and strategies that require cooperative action across jurisdictions. Administering intergovernmental ministerial councils or committees responsible for policy reform." ;
  skos:hiddenLabel "Cross-jurisdictional policy dissemination" ;
  skos:hiddenLabel "Interstate policy dissemination" ;
  skos:prefLabel "Intergovernment policy dissemination"@en ;
.
agift:intergovernmental-relations
  rdf:type skos:Concept ;
  rdfs:label "Intergovernmental relations"@en ;
  skos:broader agift:governance ;
  skos:definition """Developing cooperative associations between Australian government jurisdictions. Hosting forums and consultation processes to assess policy proposals and their potential impacts. Administering inter-jurisdictional bodies, grants and reforms. Negotiating interstate agreements on matters other than trade.

See also FINANCE MANAGEMENT - Commonwealth State funding: for Commonwealth financial support to State governments.

See also GOVERNANCE - Intergovernmental relations - Cross-border cooperation: for implementing agreements and monitoring compliance.

See also INTERNATIONAL RELATIONS: for relations with the governments of other countries.

See also TRADE - Interstate trade agreements: for negotiating commercial relationships between Australian government jurisdictions.""" ;
  skos:hiddenLabel "Commonwealth State relations" ;
  skos:hiddenLabel "Governmental relations" ;
  skos:hiddenLabel "Interstate governmental relations" ;
  skos:narrower agift:cross-border-cooperation ;
  skos:narrower agift:intergovernment-policy-dissemination ;
  skos:prefLabel "Intergovernmental relations"@en ;
  skos:related agift:commonwealth-state-funding ;
  skos:related agift:cross-border-cooperation ;
  skos:related agift:interstate-trade-agreements ;
.
agift:international-affairs
  rdf:type skos:Concept ;
  rdfs:label "International affairs"@en ;
  skos:broader agift:international-relations ;
  skos:definition """Representing the Australian government and providing diplomatic advice overseas. Conducting consultations with foreign governments and international organisations to maintain relationships and protect national interests.

See also INTERNATIONAL RELATIONS - Consular services: for Australian government representation and services to Australian citizens overseas.

See also INTERNATIONAL RELATIONS - Defence liaison: for providing defence counsel and guidance.

See also INTERNATIONAL RELATIONS - International treaties: for negotiating conventions and agreements.""" ;
  skos:hiddenLabel "Attaches" ;
  skos:hiddenLabel "Diplomacy" ;
  skos:hiddenLabel "Diplomatic advisors" ;
  skos:hiddenLabel "Foreign affairs" ;
  skos:hiddenLabel "United Nations" ;
  skos:narrower agift:disarmament-and-arms-control ;
  skos:narrower agift:nuclear-safeguards ;
  skos:prefLabel "International affairs"@en ;
  skos:related agift:consular-services ;
.
agift:international-monetary-regulation
  rdf:type skos:Concept ;
  rdfs:label "International monetary regulation"@en ;
  skos:broader agift:finance-management ;
  skos:definition "Monitoring international currency markets and identifying trends. Forecasting market movements and developing strategies to maintain stable Australian markets" ;
  skos:hiddenLabel "Currency markets" ;
  skos:hiddenLabel "International currency markets" ;
  skos:prefLabel "International monetary regulation"@en ;
.
agift:international-relations
  rdf:type skos:Concept ;
  rdfs:label "INTERNATIONAL RELATIONS"@en ;
  skos:definition "Building and maintaining relationships with other countries and international organisations. Developing strategies to protect and advance national interests. Contributing to international security, economic development, the environment, democratic principles and human rights through aid programs, treaties and diplomatic services." ;
  skos:hiddenLabel "Australian foreign policy" ;
  skos:hiddenLabel "Foreign relations" ;
  skos:hiddenLabel "International liaison" ;
  skos:hiddenLabel "Overseas relations" ;
  skos:hiddenLabel "United Nations" ;
  skos:narrower agift:consular-services ;
  skos:narrower agift:defence-liaison ;
  skos:narrower agift:diplomatic-missions ;
  skos:narrower agift:international-affairs ;
  skos:narrower agift:international-treaties ;
  skos:narrower agift:overseas-aid-programs ;
  skos:narrower agift:overseas-promotion ;
  skos:narrower agift:passport-services ;
  skos:prefLabel "INTERNATIONAL RELATIONS"@en ;
.
agift:international-trade-agreements
  rdf:type skos:Concept ;
  rdfs:label "International trade agreements"@en ;
  skos:broader agift:trade ;
  skos:definition """Developing legislation, policy and protocols to support the supply and consumption of goods and services between countries. Negotiating treaties to reduce international trade restrictions and promote regional economic links.

See also INTERNATIONAL RELATIONS - International treaties: for negotiating international agreements on matters other than trade.

See also INTERNATIONAL RELATIONS - International treaties - Treaty administration: for implementing international trade agreements and monitoring compliance.""" ;
  skos:hiddenLabel "Regional trade agreements" ;
  skos:hiddenLabel "Trade agreements" ;
  skos:hiddenLabel "World Trade Organisation" ;
  skos:prefLabel "International trade agreements"@en ;
  skos:related agift:international-treaties ;
.
agift:international-treaties
  rdf:type skos:Concept ;
  rdfs:label "International treaties"@en ;
  skos:broader agift:international-relations ;
  skos:definition """Negotiating a formal agreement or convention between Australia and one or more other countries. Forming a bilateral partnership or a multilateral alliance which is binding under international law. Amending an existing treaty or withdrawing from a treaty. Includes consultation with stakeholders, the development of declarations that may contribute to the development or interpretation of treaties, and monitoring of treaty, convention or agreement conditions.

See also INTERNATIONAL RELATIONS - Defence liaison: for negotiating agreements for the deployment of defence forces.

See also TRADE - International trade agreements: for treaties covering the exchange of goods and services between countries.""" ;
  skos:hiddenLabel "Bilateral agreements" ;
  skos:hiddenLabel "Bilateral treaties" ;
  skos:hiddenLabel "International agreements" ;
  skos:hiddenLabel "International protocols" ;
  skos:hiddenLabel "International treaty participation" ;
  skos:hiddenLabel "Multilateral treaties" ;
  skos:hiddenLabel "Treaties" ;
  skos:hiddenLabel "Treaty negotiations" ;
  skos:narrower agift:treaty-administration ;
  skos:prefLabel "International treaties"@en ;
  skos:related agift:defence-liaison ;
  skos:related agift:international-trade-agreements ;
.
agift:internet
  rdf:type skos:Concept ;
  rdfs:label "Internet"@en ;
  skos:broader agift:communications ;
  skos:definition """Developing policy and programs to regulate and promote Australia’s role in the internet.
See also COMMUNICATIONS - Electronic commerce: for developing policy to support and regulate Australian participation in the global information economy.""" ;
  skos:narrower agift:cybersafety ;
  skos:narrower agift:social-media ;
  skos:prefLabel "Internet"@en ;
.
agift:interpreter-services
  rdf:type skos:Concept ;
  rdfs:label "Interpreter services"@en ;
  skos:broader agift:migrant-services ;
  skos:definition """Administering programs that offer oral and written translations between English and other languages. Providing face-to-face interpreter services, telephone interpretation and document translations. Includes services to community organisations that may assist migrants and refugees.

See also EDUCATION AND TRAINING - Community education - Adult migrant education: for English language training.""" ;
  skos:hiddenLabel "Interpreters" ;
  skos:hiddenLabel "Language services" ;
  skos:hiddenLabel "Language" ;
  skos:hiddenLabel "Translation services" ;
  skos:prefLabel "Interpreter services"@en ;
  skos:related agift:adult-migrant-education ;
.
agift:interstate-trade-agreements
  rdf:type skos:Concept ;
  rdfs:label "Interstate trade agreements"@en ;
  skos:broader agift:trade ;
  skos:definition """Developing legislation, policy and protocols to support the supply and consumption of goods and services across Australia. Negotiating agreements that promote commerce between states and encourage competition. Includes agreements on quarantine zones, transport and infrastructure arrangements in support of trade.

See also GOVERNANCE - Intergovernmental relations: for negotiating interstate agreements on matters other than trade.

See also GOVERNANCE - Intergovernmental relations - Cross-border cooperation: for implementing interstate trade agreements and monitoring compliance.

See also PRIMARY INDUSTRIES - Quarantine: for inspections and implementing protective measures in support of trade agreements.""" ;
  skos:hiddenLabel "Trade agreements" ;
  skos:prefLabel "Interstate trade agreements"@en ;
  skos:related agift:intergovernmental-relations ;
.
agift:investment-scheme-regulation
  rdf:type skos:Concept ;
  rdfs:label "Investment scheme regulation"@en ;
  skos:broader agift:financial-investment ;
  skos:definition "Monitoring financial investment practices to ensure compliance with government policy and standards. Investigating suspected breaches of prudential regulations and applying penalties when appropriate." ;
  skos:hiddenLabel "Investment management" ;
  skos:hiddenLabel "Prudential regulation" ;
  skos:prefLabel "Investment scheme regulation"@en ;
  skos:related agift:superannuation-regulation ;
.
agift:job-placement-programs
  rdf:type skos:Concept ;
  rdfs:label "Job placement programs"@en ;
  skos:broader agift:labour-market-programs ;
  skos:definition """Administering programs that encourage and assist individuals to enter the workforce. Liaising with jobseekers to evaluate their needs for support. Providing information and resources to help locate suitable employment. Assessing jobseeker eligibility for subsidy schemes. Includes promotional strategies and advertising campaigns to advocate the employment of individuals from target groups.

See also EDUCATION AND TRAINING - Community education: for training programs to assist job seekers to find work.

See also EDUCATION AND TRAINING - Vocational education: for on-the-job training in particular disciplines.

See also EMPLOYMENT - Labour market programs: for licensing job placement providers.""" ;
  skos:hiddenLabel "Aboriginal employment services" ;
  skos:hiddenLabel "Community work" ;
  skos:hiddenLabel "Disability employment services" ;
  skos:hiddenLabel "Employment National" ;
  skos:hiddenLabel "Job Network" ;
  skos:hiddenLabel "Job centres" ;
  skos:hiddenLabel "Job seekers" ;
  skos:hiddenLabel "Recruitment services" ;
  skos:hiddenLabel "Torres Strait Islander employment services" ;
  skos:hiddenLabel "Transition to work" ;
  skos:hiddenLabel "Work for the Dole" ;
  skos:prefLabel "Job placement programs"@en ;
  skos:related agift:community-education ;
.
agift:job-vacancy-data-management
  rdf:type skos:Concept ;
  rdfs:label "Job vacancy data management"@en ;
  skos:broader agift:labour-market-programs ;
  skos:definition "Administering information about employment opportunities. Evaluating and monitoring unemployment levels. Collecting statistics on skill shortages and vacancy trends. Managing resources and facilities for the advertisement of job vacancies." ;
  skos:hiddenLabel "Unemployment figures" ;
  skos:prefLabel "Job vacancy data management"@en ;
.
agift:justice-administration
  rdf:type skos:Concept ;
  rdfs:label "JUSTICE ADMINISTRATION"@en ;
  skos:definition """Developing, interpreting and applying legislation, regulations or by-laws. Regulating the conduct of individuals, business and government, to conform to agreed rules and principles. Establishing programs and services to support the operation of the justice system.

See also SECURITY: for law enforcement.""" ;
  skos:hiddenLabel "Courts" ;
  skos:hiddenLabel "Judiciary" ;
  skos:hiddenLabel "Law" ;
  skos:narrower agift:administrative-law ;
  skos:narrower agift:associations-and-corporate-law ;
  skos:narrower agift:civil-law ;
  skos:narrower agift:commissions-of-inquiry ;
  skos:narrower agift:coronial-law ;
  skos:narrower agift:court-reporting ;
  skos:narrower agift:criminal-law ;
  skos:narrower agift:human-rights-obligations ;
  skos:narrower agift:juvenile-justice ;
  skos:narrower agift:legal-aid-services ;
  skos:narrower agift:local-laws-and-ordinances ;
  skos:narrower agift:native-title-claims ;
  skos:narrower agift:privacy- ;
  skos:narrower agift:prosecution-services ;
  skos:prefLabel "JUSTICE ADMINISTRATION"@en ;
  skos:related agift:security ;
.
agift:juvenile-justice
  rdf:type skos:Concept ;
  rdfs:label "Juvenile justice"@en ;
  skos:broader agift:justice-administration ;
  skos:definition """Administering special courts for the trial of children and young persons under a statutory age. Developing diversionary programs as an alternative to sentencing, opportunities for restorative justice and reintegration into the community.

See also COMMUNITY SERVICES - Community support - Child and youth support: for programs to assist disadvantaged juveniles.""" ;
  skos:hiddenLabel "Children's court" ;
  skos:hiddenLabel "Children's crime" ;
  skos:hiddenLabel "Juvenile crime" ;
  skos:hiddenLabel "Youth crime" ;
  skos:prefLabel "Juvenile justice"@en ;
  skos:related agift:child-and-youth-support ;
.
agift:labour-market-programs
  rdf:type skos:Concept ;
  rdfs:label "Labour market programs"@en ;
  skos:broader agift:employment ;
  skos:definition """Developing policy and programs to support the growth and stability of labour markets. Includes programs to increase employment among individuals in target groups or across specific industries. Establishing mechanisms for managing and disseminating job vacancy data. Issuing licenses to organisations or individuals who provide employment services.

See also EDUCATION AND TRAINING - Vocational education - Industry collaboration: Connecting partnerships between industry and tertiary and vocational education to train a responsive workforce based on the skillsets needed by Australian enterprises and industry sectors.""" ;
  skos:hiddenLabel "Employment marketing" ;
  skos:hiddenLabel "Employment services" ;
  skos:hiddenLabel "Job creation" ;
  skos:hiddenLabel "Unemployment policy" ;
  skos:narrower agift:employment-services-marketing ;
  skos:narrower agift:job-placement-programs ;
  skos:narrower agift:job-vacancy-data-management ;
  skos:prefLabel "Labour market programs"@en ;
  skos:related agift:industry-collaboration ;
.
agift:land-councils
  rdf:type skos:Concept ;
  rdfs:label "Land councils"@en ;
  skos:broader agift:indigenous-land-management ;
  skos:definition """Consulting with stakeholders and providing assistance for the development of land rights for Aboriginal and Torres Strait Islander peoples. Supports land and sea acquisition, establishment of commercial enterprises and community benefit schemes.

See also INDIGENOUS AFFAIRS - Indigenous land management -  Indigenous heritage conservation: for programs to protect significant cultural sites.
See also JUSTICE ADMINISTRATION - Native title claims: administering procedures to assess Indigenous interest in or rights to the use of specified areas of land or water. Identifying traditional customs and connections with a particular region. Includes processing applications, providing advice and support for litigation.""" ;
  skos:prefLabel "Land councils"@en ;
  skos:related agift:indigenous-heritage-conservation ;
  skos:related agift:indigenous-land-management ;
.
agift:land-rehabilitation-programs
  rdf:type skos:Concept ;
  rdfs:label "Land rehabilitation programs"@en ;
  skos:broader agift:mineral-resources ;
  skos:definition """Administering environmental support schemes to restore areas damaged by mineral excavation and extraction. Includes reviewing proposed projects and providing advice on rehabilitation strategies.

See also ENVIRONMENT - Conservation programs - Landcare programs: for programs to regenerate the environment.""" ;
  skos:hiddenLabel "Land regeneration" ;
  skos:hiddenLabel "Natural regeneration" ;
  skos:hiddenLabel "Restoration programs" ;
  skos:prefLabel "Land rehabilitation programs"@en ;
  skos:related agift:landcare-programs ;
  skos:related agift:soil-preservation-programs ;
.
agift:land-use-planning
  rdf:type skos:Concept ;
  rdfs:label "Land use planning"@en ;
  skos:broader agift:natural-resources ;
  skos:definition """Developing policy for the effective management and allocation of land resources. Promoting strategies for integrated land use and balancing competing interests. Providing advice on rural and urban developments. Conducting surveys and demographic analysis, forecasting needs for infrastructure and facilities, and identifying heritage and significant areas.


See also CIVIC INFRASTRUCTURE - Civic management - Town planning: for controlled urban development.

See also CIVIC INFRASTRUCTURE - Housing industry policy: for policy and programs to ensure the adequacy of land supply and construction activity.

See also CIVIC INFRASTRUCTURE - Infrastructure planning; providing advice on nationally-significant economic infrastructure to governments, investors and owners.

See also INDIGENOUS AFFAIRS - Indigenous heritage conservation: for land use agreements with traditional owners.""" ;
  skos:hiddenLabel "Commercial land use" ;
  skos:hiddenLabel "Land planning" ;
  skos:narrower agift:land-use-zoning ;
  skos:prefLabel "Land use planning"@en ;
  skos:related agift:town-planning ;
.
agift:land-use-zoning
  rdf:type skos:Concept ;
  rdfs:label "Land use zoning"@en ;
  skos:broader agift:land-use-planning ;
  skos:definition """Marking out areas of land with regard to their use. Implementing strategic land use plans for the allocation of land resources. Administering land zones and assessing development applications.


See also CIVIC INFRASTRUCTURE - Civic management - Building approval services: for construction permission.

See also CIVIC INFRASTRUCTURE - Civic management - Town planning: for controlled urban development.""" ;
  skos:hiddenLabel "Commercial land use" ;
  skos:hiddenLabel "Commercial zoning" ;
  skos:hiddenLabel "Development approval services" ;
  skos:hiddenLabel "Land zoning" ;
  skos:hiddenLabel "Public land zoning" ;
  skos:hiddenLabel "Residential zoning" ;
  skos:hiddenLabel "Zoning" ;
  skos:prefLabel "Land use zoning"@en ;
  skos:related agift:building-approval-services ;
.
agift:land-valuation
  rdf:type skos:Concept ;
  rdfs:label "Land valuation"@en ;
  skos:broader agift:natural-resources ;
  skos:definition "Assessing land resources to estimate their material worth for rating and taxation purposes. Providing advice on the unimproved value of land or in acquisition compensation disputes. Includes valuations for heritage listed land and rating concessions where land is held under nominated lease or tenure from the Crown." ;
  skos:hiddenLabel "Land value" ;
  skos:hiddenLabel "Valuation services" ;
  skos:prefLabel "Land valuation"@en ;
.
agift:landcare-programs
  rdf:type skos:Concept ;
  rdfs:label "Landcare programs"@en ;
  skos:broader agift:conservation-programs ;
  skos:definition """Managing programs to prevent or repair damage to the natural environment. Restoring specific areas to their native state or preventing further degradation. Conducting activities such as planting or feral weed control. Includes funding for joint projects with local business or community groups.

See also NATURAL RESOURCES - Mineral resources - Land rehabilitation programs: for restoring areas damaged by mineral excavation and extraction.""" ;
  skos:hiddenLabel "Community land care" ;
  skos:hiddenLabel "Land conservation programs" ;
  skos:hiddenLabel "Sustainable agriculture" ;
  skos:prefLabel "Landcare programs"@en ;
  skos:related agift:land-rehabilitation-programs ;
.
agift:law-enforcement
  rdf:type skos:Concept ;
  rdfs:label "Law enforcement"@en ;
  skos:broader agift:security ;
  skos:definition """Formulating policy to support the maintenance of rules and regulations that govern the actions of citizens. Coordinating the services of law enforcement agencies across jurisdictions. Developing programs to reduce violence and the use of illicit substances, improve public safety and reduce repeat offences. Includes activities to address 'white-collar' and corporate crime.

See also  GOVERNANCE - Public Administration - Corruption prevention: preventing, detecting and investigating serious and systemic corruption issues in Australian government agencies. 

See also GOVERNANCE - Public administration - Integrity compliance: encouraging ethical behaviour and compliance with official codes of conduct.""" ;
  skos:hiddenLabel "Detector dog programs" ;
  skos:hiddenLabel "Enforcement" ;
  skos:hiddenLabel "Federal police" ;
  skos:hiddenLabel "National police" ;
  skos:hiddenLabel "Police" ;
  skos:narrower agift:community-policing ;
  skos:narrower agift:criminology ;
  skos:narrower agift:police-administration ;
  skos:narrower agift:protective-services ;
  skos:prefLabel "Law enforcement"@en ;
  skos:related agift:corruption-prevention ;
  skos:related agift:road-safety-awareness ;
.
agift:legal-aid-services
  rdf:type skos:Concept ;
  rdfs:label "Legal aid services"@en ;
  skos:broader agift:justice-administration ;
  skos:definition "Providing financial assistance for the purpose of legal proceedings in courts. Facilitating access to legal advice and services according to an income-based scale." ;
  skos:hiddenLabel "Aboriginal legal services" ;
  skos:hiddenLabel "Community legal centres" ;
  skos:hiddenLabel "Public defenders" ;
  skos:prefLabel "Legal aid services"@en ;
  skos:related agift:prosecution-services ;
.
agift:legislation-review
  rdf:type skos:Concept ;
  rdfs:label "Legislation review"@en ;
  skos:broader agift:legislative-drafting ;
  skos:definition """Revising or amending legal instruments that already exist on statute books. Incorporating changes in government policy and other developments to ensure laws are relevant and equitable. Managing legislative review programs. Administering inter-departmental committees. Conducting enquiries, consultation and research. Providing advice on law reform.

See also GOVERNANCE - Legislative drafting - Draft Bill amendment process: for revising proposed legislation.""" ;
  skos:hiddenLabel "Law reform" ;
  skos:hiddenLabel "Legislative amendment" ;
  skos:prefLabel "Legislation review"@en ;
  skos:related agift:draft-bill-amendment-process ;
.
agift:legislative-drafting
  rdf:type skos:Concept ;
  rdfs:label "Legislative drafting"@en ;
  skos:broader agift:governance ;
  skos:definition """Preparing legal instruments for the parliament of any jurisdiction. Analysing government policy and the constitutional environment. Interpreting the legal effect of existing legislation. Providing advice on legislative proposals.

See also GOVERNANCE - Parliamentary chamber support - Parliamentary papers: for printing and gazetting of legislation passed through parliament.

See also GOVERNANCE - Parliamentary chamber support - Tabling of official documents: for presentation of draft legislation to parliament.""" ;
  skos:hiddenLabel "Acts of Parliament" ;
  skos:hiddenLabel "Law-making" ;
  skos:hiddenLabel "Legislation development" ;
  skos:narrower agift:draft-bill-amendment-process ;
  skos:narrower agift:legislation-review ;
  skos:narrower agift:preparation-of-legislative-regulations ;
  skos:prefLabel "Legislative drafting"@en ;
  skos:related agift:parliamentary-papers ;
.
agift:life-insurance
  rdf:type skos:Concept ;
  rdfs:label "Life insurance"@en ;
  skos:broader agift:insurance-regulation ;
  skos:definition """Monitoring the activities of life insurance providers to ensure compliance with government policy and standards. Investigating suspected breaches of prudential regulations and applying penalties when appropriate.

See also BUSINESS SUPPORT AND REGULATION - Insurance regulation - General insurance: for regulating the activities of general insurance providers.""" ;
  skos:hiddenLabel "Death insurance" ;
  skos:hiddenLabel "Disablement insurance" ;
  skos:hiddenLabel "Total and permanent disablement insurance" ;
  skos:prefLabel "Life insurance"@en ;
  skos:related agift:general-insurance ;
.
agift:light-station-maintenance
  rdf:type skos:Concept ;
  rdfs:label "Light station maintenance"@en ;
  skos:broader agift:navigation ;
  skos:definition """Administering programs to plan and manage navigational aids and markers for maritime transport. Supervising upgrades and regular maintenance to ensure the safe movement of vessels through shipping channels and approaches to ports. Includes decommissioning of light stations.

See also ENVIRONMENT - Natural heritage protection: for heritage-listed lighthouses in national parks.

See also MARITIME SERVICES - Navigation - Navigation systems development: for maritime navigation.""" ;
  skos:hiddenLabel "Beacon maintenance" ;
  skos:hiddenLabel "Lighthouse maintenance" ;
  skos:hiddenLabel "Lighthouses" ;
  skos:hiddenLabel "Navigation aid maintenance" ;
  skos:prefLabel "Light station maintenance"@en ;
  skos:related agift:natural-heritage-protection ;
.
agift:local-laws-and-ordinances
  rdf:type skos:Concept ;
  rdfs:label "Local laws and ordinances"@en ;
  skos:broader agift:justice-administration ;
  skos:definition "Administering legal processes at town or district level. Establishing public regulations and courts with limited civil or criminal jurisdiction. Includes management of permits, rates and registration of domestic or native animals." ;
  skos:hiddenLabel "Animal welfare" ;
  skos:hiddenLabel "Councils" ;
  skos:hiddenLabel "Dog registration" ;
  skos:hiddenLabel "Domestic animal registration" ;
  skos:hiddenLabel "Domestic animal services" ;
  skos:hiddenLabel "Fines" ;
  skos:hiddenLabel "Native animal registration" ;
  skos:hiddenLabel "Ordinances" ;
  skos:hiddenLabel "Permits and licence applications" ;
  skos:hiddenLabel "Rates" ;
  skos:hiddenLabel "Sex industry regulation" ;
  skos:prefLabel "Local laws and ordinances"@en ;
.
agift:logistics
  rdf:type skos:Concept ;
  rdfs:label "Logistics"@en ;
  skos:broader agift:defence-strategic-support ;
  skos:definition "Administering programs to manage military transportation and supply. Developing procedural frameworks and systems to move bodies of troops or deliver services and equipment." ;
  skos:hiddenLabel "Army logistics" ;
  skos:hiddenLabel "Defence logistics" ;
  skos:hiddenLabel "Defence supply systems" ;
  skos:prefLabel "Logistics"@en ;
.
agift:marina-management
  rdf:type skos:Concept ;
  rdfs:label "Marina management"@en ;
  skos:broader agift:maritime-services ;
  skos:definition """Building and maintaining facilities offering dockage and other services for watercraft. Licensing operators of private marinas. Regulating boating activities, to protect waterways and marine industries from environmental impact. Includes inspections and assessment of procedures for managing sewage, spills and other discharge.

See also ENVIRONMENT - Oceans governance: for management and protection of marine environments.

See also MARITIME SERVICES - Harbour management: for regulating coastal areas that provide protection for ships.

See also MARITIME SERVICES - Port regulation: for managing sea-based entry and exit points.

See also NATURAL RESOURCES - Water resources - Waterway management: for regulating the use of rivers and catchment areas.""" ;
  skos:hiddenLabel "Marina" ;
  skos:hiddenLabel "Marinas" ;
  skos:prefLabel "Marina management"@en ;
  skos:related agift:oceans-governance ;
.
agift:marine-and-rural-regulation
  rdf:type skos:Concept ;
  rdfs:label "Marine and rural regulation"@en ;
  skos:broader agift:primary-industries ;
  skos:definition """Monitoring the management of sea-based and farming industries. Encouraging efficient and sustainable cultivation practices. Developing quality assurance programs, operating standards and other regulatory mechanisms.

See also BUSINESS SUPPORT AND REGULATION - Industry assistance schemes: for monitoring the secondary or tertiary industries.

See also ENVIRONMENT - Environmental impact assessment: for regulating the wider effects of primary industries on local ecosystems.""" ;
  skos:hiddenLabel "Marine industries regulation" ;
  skos:hiddenLabel "Rural industries regulation" ;
  skos:narrower agift:agricultural-industry ;
  skos:narrower agift:fisheries-industry ;
  skos:narrower agift:food-quality-assurance ;
  skos:narrower agift:forestry-industry ;
  skos:prefLabel "Marine and rural regulation"@en ;
  skos:related agift:industry-assistance-schemes ;
.
agift:marine-and-rural-support
  rdf:type skos:Concept ;
  rdfs:label "Marine and rural support"@en ;
  skos:broader agift:primary-industries ;
  skos:definition """Developing policy to assist the growth and management of sea-based or farming industries. 
Identifying markets and facilitating trade or investment opportunities. Providing grants, financial incentives or subsidies for initiatives. 

See also BUSINESS SUPPORT AND REGULATION - Industry development: for supporting secondary or tertiary industries.

See also COMMUNITY SERVICES - Financial assistance: for monetary assistance provided to individuals.

See also COMMUNITY SERVICES - Natural disasters - Disaster relief: for financial assistance to those affected by natural disasters.""" ;
  skos:narrower agift:aquaculture-industry ;
  skos:narrower agift:horticultural-industry ;
  skos:narrower agift:pastoral-industry ;
  skos:narrower agift:silvicultural-industry ;
  skos:narrower agift:viticultural-industry ;
  skos:prefLabel "Marine and rural support"@en ;
  skos:related agift:industry-development ;
.
agift:marine-life-protection-programs
  rdf:type skos:Concept ;
  rdfs:label "Marine life protection programs"@en ;
  skos:broader agift:environment ;
  skos:definition """Maintaining sea-based areas of the natural environment that are culturally or scientifically significant in their native state. Developing schemes to conserve plant or animal life in a region, to protect and sustain ecosystems. Promoting community awareness and participation in conservation activities.

See also ENVIRONMENT - Conservation programs: for maintaining land-based environments.

See also ENVIRONMENT - Oceans governance: for the management and protection of marine resources.

See also SCIENCE - Biological sciences: for research into the existence and functioning of marine life.

See also SCIENCE - Earth sciences - Oceanography: for research into marine environments and the physical geography of the seas.""" ;
  skos:hiddenLabel "Aquarium programs" ;
  skos:hiddenLabel "Marine protection programs" ;
  skos:hiddenLabel "Ocean conservation programs" ;
  skos:hiddenLabel "Sea conservation programs" ;
  skos:prefLabel "Marine life protection programs"@en ;
  skos:related agift:conservation-programs ;
  skos:related agift:oceans-governance ;
.
agift:maritime-services
  rdf:type skos:Concept ;
  rdfs:label "MARITIME SERVICES"@en ;
  skos:definition """Developing policy to regulate use of the sea as a means of transport. Negotiating passage for sea transport and maritime jurisdiction. Planning and managing maritime infrastructure. Monitoring the safety of seagoing vessels, pilots and personnel. Administering programs for marine search and rescue. Providing resources for the development of navigational aids.

See also DEFENCE - Australian Defence Forces - Navy: for the sea capability of Australia's defence forces.

See also TRANSPORT: for regulating road, rail and air transportation.""" ;
  skos:hiddenLabel "Marine authorities" ;
  skos:hiddenLabel "Merchant shipping" ;
  skos:hiddenLabel "Shipping" ;
  skos:narrower agift:cargo-control ;
  skos:narrower agift:harbour-management ;
  skos:narrower agift:marina-management ;
  skos:narrower agift:navigation ;
  skos:narrower agift:pilotage-management ;
  skos:narrower agift:port-regulation ;
  skos:narrower agift:sea-passengers ;
  skos:narrower agift:search-and-rescue ;
  skos:narrower agift:ship-personnel ;
  skos:narrower agift:ship-safety ;
  skos:prefLabel "MARITIME SERVICES"@en ;
  skos:related agift:navy ;
  skos:related agift:transport ;
.
agift:mathematical-sciences
  rdf:type skos:Concept ;
  rdfs:label "Mathematical sciences"@en ;
  skos:broader agift:science ;
  skos:definition """Conducting research into quantities, magnitudes and forms by the use of numbers. Providing data analysis, simulation or mathematical modelling to illustrate trends and predict outcomes. Performing optimisation tests to determine the best operating conditions for a process. Includes training and consultancy in mathematical analysis.

See also FINANCE MANAGEMENT - Statistical analysis: for the collection of social and economic trends of relevance to government activities.

See also SCIENCE - Applied sciences: for the use of mathematics in an operational or industry setting.

See also SCIENCE - Applied sciences - Engineering and technology sciences: for the application of mathematical knowledge to systematic design, construction and management activities.""" ;
  skos:hiddenLabel "Statistical research" ;
  skos:prefLabel "Mathematical sciences"@en ;
  skos:related agift:statistical-analysis ;
.
agift:media-ownership-regulation
  rdf:type skos:Concept ;
  rdfs:label "Media ownership regulation"@en ;
  skos:broader agift:communications ;
  skos:definition """Developing policy and legislation to support Australian control of domestic communication channels. Setting limits on who can own and control Australian media outlets. Encouraging diversity among the more influential broadcasting services.

See also COMMUNICATIONS - Broadcasting - Broadcasting standards: for regulating the broadcast coverage of major events.""" ;
  skos:hiddenLabel "Mass media services" ;
  skos:hiddenLabel "Media ownership" ;
  skos:prefLabel "Media ownership regulation"@en ;
  skos:related agift:broadcasting-standards ;
.
agift:medical-aids-regulation
  rdf:type skos:Concept ;
  rdfs:label "Medical aids regulation"@en ;
  skos:broader agift:medical-research ;
  skos:definition "Monitoring the availability and manufacturing quality of appliances that assist people suffering from disease or disability. Assessing products to determine eligibility for subsidies, special tax treatment or limited distribution, in accordance with government policy." ;
  skos:hiddenLabel "Disability aids" ;
  skos:hiddenLabel "Disabled equipment" ;
  skos:hiddenLabel "Hearing aids" ;
  skos:hiddenLabel "Medical alert devices" ;
  skos:hiddenLabel "Prosthetics" ;
  skos:hiddenLabel "Respirators" ;
  skos:hiddenLabel "Vehicle modifications" ;
  skos:hiddenLabel "Walking aids" ;
  skos:hiddenLabel "Wheelchairs" ;
  skos:prefLabel "Medical aids regulation"@en ;
.
agift:medical-and-health-sciences
  rdf:type skos:Concept ;
  rdfs:label "Medical and health sciences"@en ;
  skos:broader agift:science ;
  skos:definition """Conducting experimental research into the causes, effects and symptoms of illness. Applying knowledge from a range of scientific disciplines to advance the diagnosis, treatment and prevention of disease. Developing products and processes to improve community health. Providing advice on diet, nutrition and the use of pharmaceuticals. Includes safety assessments for therapeutic goods, and the development of new surgical techniques.

See also HEALTH CARE - Medical research: for funding and regulation of medical and health science activities.

See also HEALTH CARE - Medical research - Population-based research: for clinical investigation into the health of particular groups.

See also SCIENCE - Biological sciences: for other research that may contribute to medical and health sciences.

See also SPORT AND RECREATION - Sports drugs monitoring - Doping detection research: for developing tests to reveal performance-enhancing drugs.""" ;
  skos:hiddenLabel "Health sciences" ;
  skos:hiddenLabel "Medicine" ;
  skos:prefLabel "Medical and health sciences"@en ;
  skos:related agift:apparatus-licensing ;
  skos:related agift:biological-sciences ;
  skos:related agift:medical-research ;
  skos:related agift:national-referral-laboratory-services ;
  skos:related agift:physiology ;
.
agift:medical-quarantine-services
  rdf:type skos:Concept ;
  rdfs:label "Medical quarantine services"@en ;
  skos:broader agift:public-health-services ;
  skos:definition """Protecting the health of human populations from risks associated with exotic or infectious disease. Providing surveillance and isolation of persons who have potentially been exposed to a particular disease. Managing facilities at Antarctic stations, airports and seaports.

See also HEALTH CARE - Community health services - Clinical health services: for advice on travel-related illness.

See also HEALTH CARE - Public health services - Notifiable disease management: for strategies to monitor the incidence of communicable disease.

See also PRIMARY INDUSTRIES - Quarantine: for protecting plants and animals from exotic pests and disease.""" ;
  skos:prefLabel "Medical quarantine services"@en ;
  skos:related agift:clinical-health-services ;
  skos:related agift:quarantine ;
.
agift:medical-radiation-services
  rdf:type skos:Concept ;
  rdfs:label "Medical radiation services"@en ;
  skos:broader agift:public-health-services ;
  skos:definition """Developing programs and policies to support the effective use of ionising radiation in medicine. Delivering auditing and quality assurance services, measured against national standards, aimed at providing an integrated national approach to promoting safety and quality in radiotherapy.
See also HEALTH CARE - Public health services - Radiation protection: regulating the safe use of radioactive substances.""" ;
  skos:prefLabel "Medical radiation services"@en ;
.
agift:medical-research
  rdf:type skos:Concept ;
  rdfs:label "Medical research"@en ;
  skos:broader agift:health-care ;
  skos:definition """Regulating the scientific investigation of human health and disease. Endorsing standards for ethical conduct. Developing policy to support the availability of medical equipment or research services. Establishing criteria for the allocation of funding to medical research.

See also SCIENCE - Medical and health sciences: for experimental research into human health and disease.""" ;
  skos:hiddenLabel "Health research regulation" ;
  skos:hiddenLabel "Medical technologies" ;
  skos:narrower agift:medical-aids-regulation ;
  skos:narrower agift:medical-research-funding ;
  skos:narrower agift:national-referral-laboratory-services ;
  skos:narrower agift:population-based-research ;
  skos:prefLabel "Medical research"@en ;
  skos:related agift:medical-and-health-sciences ;
.
agift:medical-research-funding
  rdf:type skos:Concept ;
  rdfs:label "Medical research funding"@en ;
  skos:broader agift:medical-research ;
  skos:definition "Providing financial support for the scientific investigation of human health and disease. Assessing proposals and applications against established criteria. Allocating funds to successful projects and providing advice to unsuccessful applicants." ;
  skos:hiddenLabel "Health research funding" ;
  skos:prefLabel "Medical research funding"@en ;
.
agift:memorial-maintenance
  rdf:type skos:Concept ;
  rdfs:label "Memorial maintenance"@en ;
  skos:broader agift:public-land-management ;
  skos:definition """Administering areas of land set aside to commemorate a person or event. Managing site layout. Ensuring facilities are kept clean and maintained. Monitoring rights of access and opening hours.

See also CIVIC INFRASTRUCTURE - Public land management - Burial ground management: for administering cemeteries.""" ;
  skos:hiddenLabel "Commemorative monument maintenance" ;
  skos:hiddenLabel "Memorials" ;
  skos:hiddenLabel "Monument maintenance" ;
  skos:hiddenLabel "War memorial maintenance" ;
  skos:prefLabel "Memorial maintenance"@en ;
  skos:related agift:burial-ground-management ;
.
agift:mental-health-services
  rdf:type skos:Concept ;
  rdfs:label "Mental health services"@en ;
  skos:broader agift:special-needs-services ;
  skos:definition """Administering programs to treat or manage disorders and diseases of the mind. Monitoring the activities of private mental health providers. Includes assessment, therapeutic intervention, referral to support services and mental health advocacy.

See also COMMUNITY SERVICES - Counselling services: for the provision of group therapy or psychological advice.

See also HEALTH CARE - Special needs services - Independent living services: for in-home assistance or sheltered accommodation.

See also HEALTH CARE - Special needs services - Residential services: for managing live-in facilities.""" ;
  skos:hiddenLabel "Psychiatric health services" ;
  skos:hiddenLabel "Psychological health services" ;
  skos:hiddenLabel "Suicide prevention" ;
  skos:prefLabel "Mental health services"@en ;
  skos:related agift:counselling-services ;
.
agift:merger-regulation
  rdf:type skos:Concept ;
  rdfs:label "Merger regulation"@en ;
  skos:broader agift:associations-and-corporate-law ;
  skos:definition "Regulating the statutory combination of two or more corporations by transfer of assets and property to a single enterprise. Assessing possible economic consequences of mergers, such as inflated prices, reduced quality or anti-competitive behaviour." ;
  skos:hiddenLabel "Business mergers" ;
  skos:hiddenLabel "Company takeovers" ;
  skos:hiddenLabel "Corporate takeover" ;
  skos:hiddenLabel "Mergers" ;
  skos:hiddenLabel "Takeovers" ;
  skos:prefLabel "Merger regulation"@en ;
.
agift:migrant-accommodation-services
  rdf:type skos:Concept ;
  rdfs:label "Migrant accommodation services"@en ;
  skos:broader agift:migrant-services ;
  skos:definition """Administering programs to assist new immigrants or refugees to find housing. 
Assessing eligibility and allocating accommodation to approved applicants. Providing advice to tenants about their rights and obligations. Includes interim housing in camps or hostels.

See also CIVIC INFRASTRUCTURE - Public housing: for the design, construction and maintenance of public housing.

See also COMMUNITY SERVICES - Accommodation services: for providing public housing to those in need.

See also IMMIGRATION - Detention programs: for the custody and treatment of illegal immigrants.""" ;
  skos:hiddenLabel "Immigrant accommodation" ;
  skos:hiddenLabel "Migrant camps" ;
  skos:hiddenLabel "Migrant hostels" ;
  skos:hiddenLabel "Migrant housing" ;
  skos:prefLabel "Migrant accommodation services"@en ;
  skos:related agift:public-housing ;
.
agift:migrant-services
  rdf:type skos:Concept ;
  rdfs:label "Migrant services"@en ;
  skos:broader agift:immigration ;
  skos:definition """Developing programs to provide information and support to foreign nationals who intend to settle in Australia. Evaluating the needs of migrants and providing advice before embarkation and upon arrival. Includes liaison with community groups and across jurisdictions to ensure appropriate support.

See also EDUCATION AND TRAINING - Community education - Adult migrant education: for training people from various ethnic backgrounds.

See also IMMIGRATION - Refugee services: for assistance to asylum seekers and victims of human rights violations.""" ;
  skos:hiddenLabel "Assisted migration" ;
  skos:hiddenLabel "Immigration services" ;
  skos:narrower agift:interpreter-services ;
  skos:narrower agift:migrant-accommodation-services ;
  skos:narrower agift:migrant-settlement-programs ;
  skos:prefLabel "Migrant services"@en ;
  skos:related agift:adult-migrant-education ;
  skos:related agift:multicultural-services ;
  skos:related agift:permanent-entry-arrangements ;
  skos:related agift:refugee-services ;
.
agift:migrant-settlement-programs
  rdf:type skos:Concept ;
  rdfs:label "Migrant settlement programs"@en ;
  skos:broader agift:migrant-services ;
  skos:definition """Administering schemes to assist new immigrants or refugees to become established in Australia. Managing migrant resource centres. Providing orientation information and support services. Includes advice about bringing family members to Australia and liaison with immigration officials on behalf of migrants.

See also COMMUNITY SERVICES - Community support - Family reunion programs: for assistance locating and contacting relatives.

See also EDUCATION AND TRAINING - Community education - Adult migrant education: for training people from various ethnic backgrounds.

See also IMMIGRATION - Refugee services: for assistance to asylum seekers and victims of human rights violations.""" ;
  skos:hiddenLabel "Migrant resource centres" ;
  skos:prefLabel "Migrant settlement programs"@en ;
  skos:related agift:family-reunion-programs ;
.
agift:military-advisors
  rdf:type skos:Concept ;
  rdfs:label "Military advisors"@en ;
  skos:broader agift:defence-liaison ;
  skos:definition """Providing defence counsel to senior government representatives. Developing guidance on defence capability and the conduct of military operations. Making recommendations to support command and control of the Australian Defence Force and strategic preparation of its service elements.

See also DEFENCE - Defence strategic policy - Strategic decisions: for reaching conclusions on the conduct of military operations.

See also INTERNATIONAL RELATIONS - Defence liaison - Defence attaches: for diplomatic representation of Australia's military interests.""" ;
  skos:hiddenLabel "Defence advisors" ;
  skos:hiddenLabel "Military advice" ;
  skos:prefLabel "Military advisors"@en ;
  skos:related agift:strategic-decisions ;
.
agift:military-bands
  rdf:type skos:Concept ;
  rdfs:label "Military bands"@en ;
  skos:broader agift:australian-defence-forces ;
  skos:definition "Raising, developing and maintaining companies of musicians to provide musical support for defence force ceremonies, community events and other activities. Administering bookings, arranging concerts and tours." ;
  skos:hiddenLabel "Bands" ;
  skos:hiddenLabel "Military tattoo" ;
  skos:prefLabel "Military bands"@en ;
.
agift:military-education-and-training
  rdf:type skos:Concept ;
  rdfs:label "Military education and training"@en ;
  skos:broader agift:education-and-training ;
  skos:definition """Developing programs designed to instruct and exercise defence recruits. Managing specialised institutions or facilities to provide suitable training for active personnel. Initiating joint ventures to provide tertiary level education or residential schools for service personnel.

See also DEFENCE - Australian Defence Forces: for the basic training provided to service personnel on recruitment.

See also DEFENCE - Australian Defence Forces - Cadets: for programs to recruit and develop young service personnel.

See also DEFENCE - Defence force careers - Defence career development: for advice on training to improve career prospects.

See also DEFENCE - Military operations - Military exercises: for executing manoeuvres in preparation for war.""" ;
  skos:hiddenLabel "Air training units" ;
  skos:hiddenLabel "Army training units" ;
  skos:hiddenLabel "Navy training units" ;
  skos:narrower agift:army-reserve-training ;
  skos:narrower agift:defence-college-training ;
  skos:prefLabel "Military education and training"@en ;
  skos:related agift:australian-defence-forces ;
  skos:related agift:defence-force-careers ;
  skos:related agift:vocational-education ;
  skos:related agift:workplace-training ;
.
agift:military-employment-services
  rdf:type skos:Concept ;
  rdfs:label "Military employment services"@en ;
  skos:broader agift:defence-force-careers ;
  skos:definition """Administering personnel support services for regular and reserve members of the Australian Defence Forces. Providing advice on wages and employment conditions, leave and other entitlements. Managing complaints, health and safety or harassment issues. Initiating disciplinary proceedings. Includes work experience placements and spouse employment services.

See also DEFENCE - Defence force careers - Defence career development: for career planning and advisory services.

See also DEFENCE - Military law: for conducting disciplinary proceedings against defence personnel.""" ;
  skos:hiddenLabel "Defence employment services" ;
  skos:hiddenLabel "Discharge processes" ;
  skos:hiddenLabel "Military discharge" ;
  skos:prefLabel "Military employment services"@en ;
  skos:related agift:defence-career-development ;
  skos:related agift:industrial-awards-and-conditions ;
  skos:related agift:termination-processes ;
  skos:related agift:workplace-agreement-processes ;
.
agift:military-exercises
  rdf:type skos:Concept ;
  rdfs:label "Military exercises"@en ;
  skos:broader agift:military-operations ;
  skos:definition """Executing air, sea and land training manoeuvres in preparation for warfare. Managing war games and other practical exercises in real or simulated environments. Testing communications and information systems that support operations. Evaluating exercises and conducting research to develop strategies for future operations. Includes activities to meet environmental obligations and safety standards during exercises.

See also DEFENCE - Australian Defence Forces: for basic training of new recruits.

See also EDUCATION AND TRAINING - Military education and training: for courses that may improve career prospects.""" ;
  skos:hiddenLabel "Defence exercises" ;
  skos:hiddenLabel "Military training exercises" ;
  skos:hiddenLabel "War games" ;
  skos:prefLabel "Military exercises"@en ;
  skos:related agift:australian-defence-forces ;
.
agift:military-law
  rdf:type skos:Concept ;
  rdfs:label "Military law"@en ;
  skos:broader agift:defence ;
  skos:definition """Administering the body of law that relates to the discipline, trial and punishment of defence personnel. Establishing military courts and conducting hearings to determine whether a command is lawful, or if service personnel have met their obligations. Regulating the treatment of prisoners of war and captured civilians in times of war.

See also DEFENCE - Emergency management: for states of emergency where martial law may be declared.

See also IMMIGRATION - Detention programs: for the custody and treatment of illegal immigrants.

See also INTERNATIONAL RELATIONS - International Treaties - Treaty administration: for monitoring compliance with international agreements.

See also JUSTICE ADMINISTRATION - Human rights obligations: for regulating the treatment of political prisoners.

See also SECURITY - Corrective services - Detention centre management: for the custody and treatment of civilians.""" ;
  skos:hiddenLabel "Courts martial" ;
  skos:hiddenLabel "Military courts" ;
  skos:hiddenLabel "Military detention" ;
  skos:hiddenLabel "Prisoners of war" ;
  skos:prefLabel "Military law"@en ;
  skos:related agift:detention-centre-management ;
  skos:related agift:detention-programs ;
  skos:related agift:emergency-management ;
.
agift:military-operations
  rdf:type skos:Concept ;
  rdfs:label "Military operations"@en ;
  skos:broader agift:defence ;
  skos:definition """Implementing strategic decisions for the deployment of Australia's defence capability. Directing the conduct of campaigns and other activities for the defence of Australia and its interests. Evaluating joint operations and exercises to prepare for future action.

See also DEFENCE - Defence strategic policy - Strategic decisions: for determinations that influence the conduct of military operations.

See also INTERNATIONAL RELATIONS - Defence liaison - Military advisors: for guidance on capability and the conduct of military operations.

See also SECURITY - External security - Peacekeeping forces: for units deployed to stabilise unrest and restore order.""" ;
  skos:hiddenLabel "Defence operations" ;
  skos:narrower agift:australian-theatre-of-war ;
  skos:narrower agift:military-exercises ;
  skos:narrower agift:special-operations ;
  skos:narrower agift:warfare ;
  skos:prefLabel "Military operations"@en ;
  skos:related agift:strategic-decisions ;
.
agift:mineral-exploration
  rdf:type skos:Concept ;
  rdfs:label "Mineral exploration"@en ;
  skos:broader agift:earth-sciences ;
  skos:definition """Conducting research into ore deposits and their environmental settings. Applying geological and geochemical methods to advance the understanding of mineral origin and distribution. Developing tools and models to support deposit location, excavation and extraction processes. Promoting collaborative programs across government, university and industry sectors. Includes training programs for geologists, industry researchers and students.

See also NATURAL RESOURCES - Energy resources - Fossil fuel management: for mapping deposits of oil, coal or natural gas.

See also NATURAL RESOURCES - Mineral resources: for management and economic development of ore deposits.

See also NATURAL RESOURCES - Mineral resources - Mining regulation: for mapping ore and other mineral deposits.

See also SCIENCE - Earth Sciences - Seismology: for monitoring of quarry blasts and related mining activities.""" ;
  skos:hiddenLabel "Mine exploration" ;
  skos:hiddenLabel "Mining activities" ;
  skos:hiddenLabel "Mining exploration" ;
  skos:hiddenLabel "Mining" ;
  skos:prefLabel "Mineral exploration"@en ;
  skos:related agift:fossil-fuel-management ;
.
agift:mineral-resources
  rdf:type skos:Concept ;
  rdfs:label "Mineral resources"@en ;
  skos:broader agift:natural-resources ;
  skos:definition """Administering legislation relating to mining and mineral processing. Developing policy to support the management of mineral resources and the economic development of related industries. Negotiating partnership programs with the traditional owners of mineral-rich lands.

See also NATURAL RESOURCES - Energy resources - Fossil fuel management: for regulating the fossil fuel industries.

See also SCIENCE - Earth sciences - Mineral exploration: for conducting research into ore deposits and their environmental settings.""" ;
  skos:hiddenLabel "Mining" ;
  skos:narrower agift:land-rehabilitation-programs ;
  skos:narrower agift:mining-regulations ;
  skos:prefLabel "Mineral resources"@en ;
  skos:related agift:fossil-fuel-management ;
.
agift:mining-regulations
  rdf:type skos:Concept ;
  rdfs:label "Mining regulations"@en ;
  skos:broader agift:mineral-resources ;
  skos:definition """Managing the exploitation of ores and mineral resources. Licensing infrastructure and operational activities. Conducting exploration and mapping mineral deposits. Granting mining titles and leases for excavation and extraction. Monitoring compliance with standards, regulations and risk management procedures.

See also ENVIRONMENT - Environmental impact assessment: for estimating the effects of mining activities.

See also SCIENCE - Earth sciences - Mineral exploration: for conducting research into ore deposits and their environmental settings.""" ;
  skos:hiddenLabel "Mining activities" ;
  skos:hiddenLabel "Mining exploration" ;
  skos:prefLabel "Mining regulations"@en ;
  skos:related agift:environmental-impact-assessment ;
  skos:related agift:fossil-fuel-management ;
.
agift:mobile-telephone-services
  rdf:type skos:Concept ;
  rdfs:label "Mobile telephone services"@en ;
  skos:broader agift:telecommunications ;
  skos:definition """Monitoring the activities of suppliers of wireless telecommunications services. Ensuring compliance with pricing guidelines, standards of service and maintenance requirements. Encouraging the development of the mobile telephone industry.

See also CIVIC INFRASTRUCTURE: for planning of facilities to support mobile telecommunications.

See also COMMUNICATIONS - Radio communication - Apparatus licensing: for radio communications equipment.""" ;
  skos:hiddenLabel "Cellular telephone services" ;
  skos:hiddenLabel "Mobile phones" ;
  skos:hiddenLabel "Wireless telecommunications services" ;
  skos:prefLabel "Mobile telephone services"@en ;
  skos:related agift:civic-infrastructure ;
  skos:related agift:telephone-services ;
.
agift:monetary-policy
  rdf:type skos:Concept ;
  rdfs:label "Monetary policy"@en ;
  skos:broader agift:finance-management ;
  skos:definition """Developing policy to maintain stability of the currency, improve economic performance and employment levels. Setting interest rates by buying and selling in money markets. Includes activities to control inflation within predefined limits.

See also FINANCE MANAGEMENT - Economic research: for developing new economic measurements and models and assessing the effects of public policies on the Australian economy.

See also FINANCE MANAGEMENT - - Resource management - Productivity: for developing measures and programs to capture the ability of an economy to harness its physical and human resources to generate output and income.""" ;
  skos:hiddenLabel "Economic policy" ;
  skos:hiddenLabel "Interest rate policy" ;
  skos:hiddenLabel "Macroeconomic policy" ;
  skos:narrower agift:exchange-rates ;
  skos:narrower agift:inflation ;
  skos:narrower agift:interest-rates ;
  skos:prefLabel "Monetary policy"@en ;
  skos:related agift:economic-research ;
.
agift:multicultural-festivals
  rdf:type skos:Concept ;
  rdfs:label "Multicultural festivals"@en ;
  skos:broader agift:multicultural-heritage-promotion ;
  skos:definition """Promoting and funding events that reflect Australia's cultural diversity and multi-ethnic population. Organising festivals, performances and joint ventures with community groups where events highlight the origin of particular cultural activities. Includes participation in international cultural festivals.

See also CULTURAL AFFAIRS - Cultural festivals: for events that highlight artistic, literary or heritage related activities.

See also GOVERNANCE - Civic celebrations: for marking significant community occasions.

See also INTERNATIONAL RELATIONS - Overseas promotion: for negotiating opportunities to participate in or host international tourist events.""" ;
  skos:hiddenLabel "Ethnic festivals" ;
  skos:hiddenLabel "Food fairs" ;
  skos:hiddenLabel "International cultural displays" ;
  skos:hiddenLabel "International food fairs" ;
  skos:prefLabel "Multicultural festivals"@en ;
  skos:related agift:cultural-festivals ;
.
agift:multicultural-heritage-promotion
  rdf:type skos:Concept ;
  rdfs:label "Multicultural heritage promotion"@en ;
  skos:broader agift:cultural-affairs ;
  skos:definition """Managing programs to protect and promote Australia's cultural diversity. Sponsoring community events and activities. Recognising internationally significant dates and events. Encouraging research into multicultural experiences. Initiating projects to compile and document ethnic oral histories and folklore.

See also INDIGENOUS AFFAIRS - Indigenous cultural heritage: for protecting the heritage of Aboriginal and Torres Strait Islander peoples.""" ;
  skos:narrower agift:multicultural-festivals ;
  skos:narrower agift:multicultural-services ;
  skos:prefLabel "Multicultural heritage promotion"@en ;
  skos:related agift:indigenous-cultural-heritage ;
.
agift:multicultural-services
  rdf:type skos:Concept ;
  rdfs:label "Multicultural services"@en ;
  skos:broader agift:multicultural-heritage-promotion ;
  skos:definition """Encouraging migrant communities to retain their cultural identity. Establishing and maintaining ethnic cultural resource collections. Providing assistance in the conduct of religious ceremonies or social events. Includes liaison across jurisdictions to support and promote multiculturalism.

See also IMMIGRATION - Migrant services: for assistance to recent immigrants.

See also SPORT AND RECREATION - Community recreational programs - Social club support: for assistance to community groups.""" ;
  skos:hiddenLabel "Cultural diversity programs" ;
  skos:hiddenLabel "Ethnic services" ;
  skos:prefLabel "Multicultural services"@en ;
  skos:related agift:migrant-services ;
.
agift:national-park-management
  rdf:type skos:Concept ;
  rdfs:label "National park management"@en ;
  skos:broader agift:natural-heritage-protection ;
  skos:definition """Administering designated national park areas. Monitoring access restrictions and maintaining public amenities. Issuing permits for commercial or recreational activities. Assessing applications for development within national parks. Implementing plans for regeneration following erosion or natural disasters.

See also CIVIC INFRASTRUCTURE - Public land management - Garden management: for administering public land where ornamental or useful plants are cultivated.

See also CIVIC INFRASTRUCTURE - Public land management - Recreational park management: for administering public leisure areas and playgrounds.

See also ENVIRONMENT - Natural heritage protection - Nature reserve management: for the maintenance of native flora and fauna reserves.

See also ENVIRONMENT - Natural heritage protection - Wilderness area management: for the maintenance of areas where the ecology is undisturbed.

See also ENVIRONMENT - Natural heritage protection - Wildlife sanctuary management: for sheltered facilities for wild animals.

See also INDIGENOUS AFFAIRS - Indigenous heritage conservation: for land use agreements with traditional owners.""" ;
  skos:hiddenLabel "Forest management" ;
  skos:hiddenLabel "Marine parks" ;
  skos:hiddenLabel "National park access and permits" ;
  skos:hiddenLabel "National parks" ;
  skos:hiddenLabel "Parks" ;
  skos:prefLabel "National park management"@en ;
  skos:related agift:garden-management ;
.
agift:national-referral-laboratory-services
  rdf:type skos:Concept ;
  rdfs:label "National referral laboratory services"@en ;
  skos:broader agift:medical-research ;
  skos:definition """Managing programs that administer scientific testing on behalf of health and medical practitioners. Packaging and transporting specimens for analysis. Conducting screening and assessment of patients. Examining specimens and providing results.

See also SCIENCE - Medical and health sciences: for experimental research into human health and disease.""" ;
  skos:hiddenLabel "Analytical testing" ;
  skos:hiddenLabel "Health testing services" ;
  skos:hiddenLabel "Laboratory services" ;
  skos:hiddenLabel "Medical testing services" ;
  skos:hiddenLabel "Pathology" ;
  skos:hiddenLabel "Specimen collection services" ;
  skos:prefLabel "National referral laboratory services"@en ;
  skos:related agift:medical-and-health-sciences ;
.
agift:national-security
  rdf:type skos:Concept ;
  rdfs:label "National security"@en ;
  skos:broader agift:security ;
  skos:definition """Developing policy and procedures to protect the Australian continent. Implementing strategies to identify and apprehend individuals who may pose a threat to national security. Reviewing the powers of the security and intelligence services.

See also SECURITY - External security: for maintaining Australia's security interests overseas.""" ;
  skos:hiddenLabel "Community protection" ;
  skos:hiddenLabel "Counter terrorism" ;
  skos:hiddenLabel "Homeland security" ;
  skos:hiddenLabel "Internal security" ;
  skos:narrower agift:border-protection ;
  skos:prefLabel "National security"@en ;
  skos:related agift:external-security ;
.
agift:native-title-claims
  rdf:type skos:Concept ;
  rdfs:label "Native title claims"@en ;
  skos:broader agift:justice-administration ;
  skos:definition """Administering procedures to assess Indigenous interest in or rights to the use of specified areas of land or water. Identifying traditional customs and connections with a particular region. Includes processing applications, providing advice and support for litigation.

See also INDIGENOUS AFFAIRS- Indigneous land management: developing policies and programs to manage traditional lands and seas owned by Aboriginal and Torres Strait Islander peoples.

See also INDIGENOUS AFFAIRS - Indigenous land management - Land councils: consulting with stakeholders and providing assistance for the development of land rights for Aboriginal and Torres Strait Islander peoples.

See also INDIGENOUS AFFAIRS - Indigenous land management -  Indigenous heritage conservation: for programs to protect significant cultural sites.""" ;
  skos:hiddenLabel "Aboriginal land rights" ;
  skos:hiddenLabel "Application for Native Title" ;
  skos:hiddenLabel "Indigenous land rights" ;
  skos:hiddenLabel "Land claims" ;
  skos:hiddenLabel "Land rights" ;
  skos:hiddenLabel "Litigation processes" ;
  skos:narrower agift:native-title-mediation-programs ;
  skos:narrower agift:native-title-settlement-negotiations ;
  skos:prefLabel "Native title claims"@en ;
  skos:related agift:indigenous-land-management ;
.
agift:native-title-mediation-programs
  rdf:type skos:Concept ;
  rdfs:label "Native title mediation programs"@en ;
  skos:broader agift:native-title-claims ;
  skos:definition """Providing arbitration services to parties involved in claims for Indigenous land rights. Acting as an intermediary in an effort to reconcile competing interests and bring about agreement. Includes facilitating access to these programs.

See also JUSTICE ADMINISTRATION - Native title claims - Native title settlement negotiations: for discussion of land use arrangements and compensation payments, once agreement is reached.""" ;
  skos:hiddenLabel "Land claim mediation" ;
  skos:hiddenLabel "Mediation programs" ;
  skos:hiddenLabel "Native title mediation" ;
  skos:prefLabel "Native title mediation programs"@en ;
  skos:related agift:native-title-settlement-negotiations ;
.
agift:native-title-settlement-negotiations
  rdf:type skos:Concept ;
  rdfs:label "Native title settlement negotiations"@en ;
  skos:broader agift:native-title-claims ;
  skos:definition """Establishing procedures for mutual discussions to resolve claims for Indigenous land rights. Attempting to reach a compromise in disputes, and agree on arrangements for shared land use. Includes management of compensation payments, where rights have been infringed.

See also JUSTICE ADMINISTRATION - Native title claims - Native title mediation programs: for intermediary services to parties involved in Indigenous land claims.""" ;
  skos:prefLabel "Native title settlement negotiations"@en ;
  skos:related agift:native-title-mediation-programs ;
.
agift:natural-disasters
  rdf:type skos:Concept ;
  rdfs:label "Natural disasters"@en ;
  skos:broader agift:community-services ;
  skos:definition """Managing programs to provide urgent assistance during emergencies caused by the elements - such as floods, earthquakes, cyclones, storms or major bushfires. Monitoring conditions to anticipate the likelihood and effects of natural disasters. Coordinating government and community-based services, and regulating the use of volunteers. Includes liaison with defence forces, where civil community assistance is provided.

See also COMMUNITY SERVICES - Accommodation services - Emergency accommodation: for providing housing after a crisis.

See also COMMUNITY SERVICES - Emergency services - Firefighting services: for managing localised fire emergencies.

See also DEFENCE - Emergency management: for cross-jurisdictional operations dealing with large-scale crises.

See also DEFENCE - Emergency management - Civil community assistance: for defence forces support during natural disasters.

See also ENVIRONMENT - Climate information services: for providing weather forecasts.

See also MARITIME SERVICES - Search and rescue: for coordinating maritime emergency services.

See also SCIENCE - Earth sciences - Atmospheric sciences: for conducting research into severe weather.""" ;
  skos:hiddenLabel "Acts of God" ;
  skos:hiddenLabel "Disasters" ;
  skos:narrower agift:disaster-recovery ;
  skos:narrower agift:disaster-relief ;
  skos:prefLabel "Natural disasters"@en ;
  skos:related agift:ambulance-services ;
  skos:related agift:atmospheric-sciences ;
  skos:related agift:climate-information-services ;
  skos:related agift:emergency-accommodation ;
  skos:related agift:search-and-rescue ;
.
agift:natural-heritage-protection
  rdf:type skos:Concept ;
  rdfs:label "Natural heritage protection"@en ;
  skos:broader agift:environment ;
  skos:definition """Developing policy and programs to manage and conserve elements of the biological environment that have particular historic, scientific or social significance. Establishing standards for maintaining and preserving natural heritage areas, such as access and development restrictions, or regeneration requirements.

See also ENVIRONMENT - Built environment: for programs to protect the built environment.

See also ENVIRONMENT - Conservation programs: for developing schemes to protect plant or animal life in a region.

See also ENVIRONMENT - Historic relic protection: for programs to conserve significant artefacts.

See also INDIGENOUS AFFAIRS - Indigenous heritage conservation: for protecting areas directly associated with Aboriginal and Torres Strait Islander culture.""" ;
  skos:hiddenLabel "Maritime heritage" ;
  skos:hiddenLabel "National Estate preservation" ;
  skos:narrower agift:feral-pest-control ;
  skos:narrower agift:national-park-management ;
  skos:narrower agift:nature-reserve-management ;
  skos:narrower agift:wilderness-area-management ;
  skos:narrower agift:wildlife-sanctuary-management ;
  skos:prefLabel "Natural heritage protection"@en ;
  skos:related agift:built-environment ;
  skos:related agift:light-station-maintenance ;
.
agift:natural-resources
  rdf:type skos:Concept ;
  rdfs:label "NATURAL RESOURCES"@en ;
  skos:definition """Developing policy for the sustainable use and management of energy, mineral, land and water supplies. Administering programs to evaluate resource consumption and exploitation practices. Regulating and supporting industries that realise the economic potential of resources.

See also ENVIRONMENT: for the impacts of resource extraction.

See also SCIENCE: for conducting research into the exploitation of resources.""" ;
  skos:hiddenLabel "Natural resource management" ;
  skos:narrower agift:crown-land-administration ;
  skos:narrower agift:energy-resources ;
  skos:narrower agift:land-use-planning ;
  skos:narrower agift:land-valuation ;
  skos:narrower agift:mineral-resources ;
  skos:narrower agift:pollution-emission-control ;
  skos:narrower agift:water-resources ;
  skos:prefLabel "NATURAL RESOURCES"@en ;
  skos:related agift:environment ;
.
agift:naturalisation-assessment
  rdf:type skos:Concept ;
  rdfs:label "Naturalisation assessment"@en ;
  skos:broader agift:citizenship ;
  skos:definition "Administering programs to evaluate applications for Australian citizenship. Managing procedures for lodging submissions. Conducting interviews and assessing applicants against standard criteria. Notifying applicants of the outcome of assessment." ;
  skos:hiddenLabel "Citizenship applications" ;
  skos:hiddenLabel "Naturalisation" ;
  skos:prefLabel "Naturalisation assessment"@en ;
.
agift:nature-reserve-management
  rdf:type skos:Concept ;
  rdfs:label "Nature reserve management"@en ;
  skos:broader agift:natural-heritage-protection ;
  skos:definition """Administering designated native flora and fauna reserves, including nature parks, bush reserves and wetlands. Monitoring access restrictions and maintaining public amenities. Issuing permits for commercial or recreational activities. Assessing applications for development within nature reserves. Implementing regeneration or breeding programs for indigenous plants and animals.

See also CIVIC INFRASTRUCTURE - Public land management - Garden management: for administering public land where ornamental or useful plants are cultivated.

See also CIVIC INFRASTRUCTURE - Public land management - Recreational park management: for administering public leisure areas and playgrounds.

See also ENVIRONMENT - Natural heritage protection - National park management: for administering designated national park areas.

See also ENVIRONMENT - Natural heritage protection - Wilderness area management: for the maintenance of areas where the ecology is undisturbed.

See also ENVIRONMENT - Natural heritage protection - Wildlife sanctuary management: for sheltered facilities for wild animals.

See also INDIGENOUS AFFAIRS - Indigenous heritage conservation: for land use agreements with traditional owners.

See also SPORT AND RECREATION - Park and reserve services: for managing sporting grounds.""" ;
  skos:hiddenLabel "Bush reserves" ;
  skos:hiddenLabel "Marine reserves" ;
  skos:hiddenLabel "Nature parks" ;
  skos:hiddenLabel "Reserve management" ;
  skos:hiddenLabel "Wetlands management" ;
  skos:prefLabel "Nature reserve management"@en ;
  skos:related agift:garden-management ;
.
agift:navigation
  rdf:type skos:Concept ;
  rdfs:label "Navigation"@en ;
  skos:broader agift:maritime-services ;
  skos:definition """Developing policy to regulate the movement of ships and other commercial or private vessels. Managing shipping channels and monitoring the movement of ships at sea. Administering standards for safe and efficient navigation. Installing infrastructure to support maritime navigation.

See also MARITIME SERVICES - Port regulation: for supervising the maintenance of shipping channels.""" ;
  skos:hiddenLabel "Sea lane management" ;
  skos:hiddenLabel "Sea lanes" ;
  skos:hiddenLabel "Shipping channel management" ;
  skos:narrower agift:charting-sea-lanes ;
  skos:narrower agift:light-station-maintenance ;
  skos:narrower agift:navigation-systems-development ;
  skos:prefLabel "Navigation"@en ;
  skos:related agift:port-regulation ;
.
agift:navigation-systems-development
  rdf:type skos:Concept ;
  rdfs:label "Navigation systems development"@en ;
  skos:broader agift:navigation ;
  skos:definition """Conducting research into the application of specialist knowledge and equipment to support the plotting of courses at sea. Providing technical advice on the purchase of maritime navigational equipment and the development of global positioning networks. Includes designing, testing and overseeing the manufacture of new products.

See also COMMUNICATIONS: for industry regulations and standards.

See also MARITIME SERVICES - Navigation - Lightstation maintenance: for managing navigational aids and markers.

See also MARITIME SERVICES - Search and rescue - Search technology development: for investigating the use of systems to assist marine rescue operations.

See also SCIENCE - Spatial information research: for investigating practical applications for geographical data.""" ;
  skos:prefLabel "Navigation systems development"@en ;
  skos:related agift:communications ;
  skos:related agift:satellite-communication ;
.
agift:navy
  rdf:type skos:Concept ;
  rdfs:label "Navy"@en ;
  skos:broader agift:australian-defence-forces ;
  skos:definition """Raising, equipping and maintaining the seagoing capability of Australia's defence forces. Administering Navy activities, implementing defence policy and coordinating joint defence forces operations. Includes on-the-job and basic training of new Navy recruits.

See also DEFENCE - Australian Defence Forces - Reserves: for activities involving Naval Reserves.

See also MARITIME SERVICES: for regulating seagoing transport and commerce.""" ;
  skos:hiddenLabel "Naval forces" ;
  skos:hiddenLabel "RAN" ;
  skos:hiddenLabel "Royal Australian Navy" ;
  skos:hiddenLabel "Sailors" ;
  skos:prefLabel "Navy"@en ;
  skos:related agift:maritime-services ;
  skos:related agift:personnel-safety-standards ;
  skos:related agift:reserves ;
  skos:related agift:ship-commissioning ;
  skos:related agift:ship-personnel ;
.
agift:notifiable-disease-management
  rdf:type skos:Concept ;
  rdfs:label "Notifiable disease management"@en ;
  skos:broader agift:public-health-services ;
  skos:definition """Monitoring the incidence of communicable diseases and preventing large-scale outbreaks or epidemics. Compiling and managing data on the location and circumstances of infection. Developing reporting mechanisms to support the collection of data. Alerting authorities to significant occurrences or levels of contamination.

See also HEALTH CARE - Public health services - Epidemiology: for studying the incidence of communicable diseases.

See also HEALTH CARE - Public health services - Health disaster preparedness: for strategies to handle a large-scale medical emergency.

See also HEALTH CARE - Public health services - Medical quarantine services: for isolating infectious individuals.""" ;
  skos:hiddenLabel "Communicable diseases prevention" ;
  skos:hiddenLabel "Contagious disease management" ;
  skos:hiddenLabel "Disease reporting" ;
  skos:hiddenLabel "Infectious disease management" ;
  skos:prefLabel "Notifiable disease management"@en ;
  skos:related agift:epidemiology ;
.
agift:nuclear-safeguards
  rdf:type skos:Concept ;
  rdfs:label "Nuclear safeguards"@en ;
  skos:broader agift:international-affairs ;
  skos:definition """Ensuring that nuclear material and associated equipment is fully accounted for and controlled. Developing and implementing security measures and precautions for the physical protection of nuclear items. Includes the operation of bilateral safeguards agreements.

See also HEALTH CARE- Public health services - Radiation protection: regulating the safe use of radioactive substances. 

See also INTERNATIONAL RELATIONS - International affairs - Disarmament and arms control: for administering nuclear non-proliferation treaty obligations.""" ;
  skos:hiddenLabel "Nuclear safety" ;
  skos:prefLabel "Nuclear safeguards"@en ;
  skos:related agift:disarmament-and-arms-control ;
  skos:related agift:radiation-protection ;
.
agift:nuclear-sciences
  rdf:type skos:Concept ;
  rdfs:label "Nuclear sciences"@en ;
  skos:broader agift:physical-sciences ;
  skos:definition """Conducting research into the structure and nature of subatomic particles and related energy. Analysing changes in the behaviour and state of a nucleus in various conditions. Observing nuclear reactions to identify or develop products or processes for use in medical, industrial or defence applications, or to support other fields of scientific research. Determining the effects of nuclear weapons, radiation and fallout. Includes the management of reactors and other specialist equipment, and training programs for students and industry researchers.

See also DEFENCE - Defence strategic support - Defence science and technology: for applying scientific knowledge to military activities.

See also HEALTH CARE- Public health services - Medical radiation services: developing programs and policies to support the effective use of ionising radiation in medicine. 

See also SCIENCE - Physical sciences - Atomic and molecular sciences: for research into the fundamental particles of chemical elements.""" ;
  skos:hiddenLabel "Atomic energy" ;
  skos:hiddenLabel "Nuclear power" ;
  skos:prefLabel "Nuclear sciences"@en ;
  skos:related agift:defence-science-and-technology ;
.
agift:occupational-health-and-safety
  rdf:type skos:Concept ;
  rdfs:label "Occupational health and safety"@en ;
  skos:broader agift:human-resources-development ;
  skos:definition """Administering programs to prevent death, injury or disease in the workplace. Implementing standards for occupational health and safety. Conducting research and collecting statistics. Monitoring workplace conditions and safety training programs.

See also EMPLOYMENT - Human resources development - Workers compensation schemes: for workplace insurance schemes.

See also HEALTH CARE - Public health services - Health hazard prevention: for developing guidelines to support safe work practices.""" ;
  skos:hiddenLabel "Employment conditions" ;
  skos:hiddenLabel "OH&S" ;
  skos:hiddenLabel "Safety" ;
  skos:hiddenLabel "Working conditions" ;
  skos:hiddenLabel "Workplace health and safety" ;
  skos:hiddenLabel "Workplace safety" ;
  skos:prefLabel "Occupational health and safety"@en ;
  skos:related agift:award-conditions ;
  skos:related agift:cargo-control ;
  skos:related agift:certified-employment-conditions ;
  skos:related agift:health-hazard-prevention ;
  skos:related agift:workers-compensation-schemes ;
.
agift:oceanography
  rdf:type skos:Concept ;
  rdfs:label "Oceanography"@en ;
  skos:broader agift:earth-sciences ;
  skos:definition """Conducting research into marine environments and the physical geography of seas. Studying interactions between oceans, continents, atmosphere and biosphere. Providing scientific advice on the sustainable use of coastal and ocean resources, and the impact of climate change. Analysing waves, currents, tides, ocean temperatures, salinity and acoustic properties. Includes oceanographic data collection, such as drilling and mapping of sea floor geology, and consultancy services in support of maritime activities.

See also ENVIRONMENT - Oceans governance: for the management and protection of marine environments.

See also SCIENCE - Biological sciences: for marine biology.""" ;
  skos:hiddenLabel "El Nino effect" ;
  skos:hiddenLabel "Marine science" ;
  skos:prefLabel "Oceanography"@en ;
  skos:related agift:oceans-governance ;
.
agift:oceans-governance
  rdf:type skos:Concept ;
  rdfs:label "Oceans governance"@en ;
  skos:broader agift:environment ;
  skos:definition """Developing policy for the management and protection of marine environments. Planning for the sustainable development of ocean resources. Conducting negotiations across jurisdictions to ascertain authority over particular ocean regions. 

See also ENVIRONMENT - Marine life protection programs: for ocean conservation programs.

See also NATURAL RESOURCES - Water resources - Waterway management: for strategies for river care programs.

See also PRIMARY INDUSTRIES - Marine and rural regulation - Fisheries industry: for regulating commercial and recreational fishing.

See also SCIENCE - Earth sciences - Oceanography: for research into marine environments and the physical geography of the seas.""" ;
  skos:hiddenLabel "Coastal engineering programs" ;
  skos:hiddenLabel "Harbour protection programs" ;
  skos:prefLabel "Oceans governance"@en ;
  skos:related agift:aquaculture-industry ;
  skos:related agift:fisheries-industry ;
  skos:related agift:harbour-management ;
  skos:related agift:hydrology ;
  skos:related agift:marina-management ;
  skos:related agift:marine-life-protection-programs ;
  skos:related agift:oceanography ;
  skos:related agift:port-regulation ;
.
agift:official-establishment-management
  rdf:type skos:Concept ;
  rdfs:label "Official establishment management"@en ;
  skos:broader agift:official-protocol ;
  skos:definition """Administering the buildings and grounds of official residences of high-level government representatives. Overseeing maintenance and tenancy arrangements. Managing public visits to official residences. Includes liaison with occupants and official establishment committees, in accordance with official protocol.

See also GOVERNANCE - Official protocol - Official hospitality: for planning the reception and entertainment of high-level government representatives.""" ;
  skos:hiddenLabel "Government residences" ;
  skos:hiddenLabel "Official residences" ;
  skos:prefLabel "Official establishment management"@en ;
  skos:related agift:official-hospitality ;
.
agift:official-hospitality
  rdf:type skos:Concept ;
  rdfs:label "Official hospitality"@en ;
  skos:broader agift:official-protocol ;
  skos:definition """Planning the reception and entertainment of high-level government representatives. Making arrangements to support official protocol, such as arranging gifts, researching customs and procedures. Organising accommodation, catering and decorations.

See also GOVERNANCE - Official protocol - Ceremonial events and representation: for official conduct during ritual or traditional proceedings.

See also GOVERNANCE - Official protocol - Head of Government protocol: for the conduct of leaders in carrying out official or ceremonial duties.

See also GOVERNANCE - Official protocol - Official establishment management: for administering the buildings and grounds of official residences, including public visits.

See also GOVERNANCE - Official protocol - Official visits: for organising travel and itineraries for business, cultural or social visits by high-level government officials.""" ;
  skos:hiddenLabel "Government hospitality" ;
  skos:prefLabel "Official hospitality"@en ;
  skos:related agift:ceremonial-events-and-representation ;
  skos:related agift:official-establishment-management ;
.
agift:official-protocol
  rdf:type skos:Concept ;
  rdfs:label "Official protocol"@en ;
  skos:broader agift:governance ;
  skos:definition "Developing policy and guidelines to support the activities of high-level government representatives in carrying out their official duties. Determining appropriate conventions, customs and arrangements required during formal procedures and functions, either in Australia or overseas. Includes research, advice and support services for occasions where official protocol is to be followed." ;
  skos:hiddenLabel "Ceremonial protocol" ;
  skos:hiddenLabel "Government protocol" ;
  skos:hiddenLabel "International protocol" ;
  skos:narrower agift:ceremonial-events-and-representation ;
  skos:narrower agift:head-of-government-protocol ;
  skos:narrower agift:official-establishment-management ;
  skos:narrower agift:official-hospitality ;
  skos:narrower agift:official-visits ;
  skos:prefLabel "Official protocol"@en ;
.
agift:official-visits
  rdf:type skos:Concept ;
  rdfs:label "Official visits"@en ;
  skos:broader agift:official-protocol ;
  skos:definition """Planning visits for domestic government representatives, and making arrangements for visits by representatives of other governments. Developing programs and itineraries. Managing publicity. Organising accommodation, travel and security. Includes visits for business, cultural or social reasons.

See also GOVERNANCE - Official protocol - Ceremonial events and representation: for official conduct during ritual or traditional proceedings.

See also GOVERNANCE - Official protocol - Head of Government protocol: for the conduct of leaders in carrying out official or ceremonial duties.

See also GOVERNANCE - Official protocol - Official establishment management: for administering the buildings and grounds of official residences, including public visits.

See also GOVERNANCE - Official protocol - Official hospitality: for planning the reception and entertainment of high-level government representatives.""" ;
  skos:hiddenLabel "Government visits" ;
  skos:hiddenLabel "Royal visits" ;
  skos:prefLabel "Official visits"@en ;
  skos:related agift:ceremonial-events-and-representation ;
.
agift:online-transaction-standards
  rdf:type skos:Concept ;
  rdfs:label "Online transaction standards"@en ;
  skos:broader agift:electronic-commerce ;
  skos:definition """Establishing guidelines and models to facilitate the conduct of electronic commerce. Supporting the application of existing commercial legislation in an online environment. Providing advice on the implementation of standards and monitoring compliance.

See also COMMUNICATIONS - Broadcasting - Broadcasting standards: for online content regulation.

See also COMMUNICATIONS - Electronic commerce - Authentication: for managing the infrastructure to validate online transactions.

See also COMMUNICATIONS - Information management standards - Information technology standards: for hardware and software regulation.

See also COMMUNICATIONS - Publishing - Electronic publishing: for online content regulation.

See also SECURITY - Information security: for data security standards.""" ;
  skos:hiddenLabel "Digital transactions standards" ;
  skos:hiddenLabel "Electronic transactions standards" ;
  skos:prefLabel "Online transaction standards"@en ;
  skos:related agift:authentication ;
  skos:related agift:broadcasting-standards ;
  skos:related agift:data-management ;
  skos:related agift:information-management-standards ;
  skos:related agift:information-technology-standards ;
.
agift:open-government
  rdf:type skos:Concept ;
  rdfs:label "Open government"@en ;
  skos:broader agift:governance ;
  skos:definition """Facilitating citizen collaboration by developing services and programs based on open government principles. Encouraging public engagement in policy and service design and delivery. 

See also JUSTICE ADMINISTRATION - Administrative law - Freedom of information: providing a right of access to  government  documents.

See also JUSTICE ADMINISTRATION - Administrative law - Recordkeeping standards: regulating the creation, capture, management and disposal of government records.""" ;
  skos:prefLabel "Open government"@en ;
  skos:related agift:freedom-of-information ;
.
agift:overseas-aid-programs
  rdf:type skos:Concept ;
  rdfs:label "Overseas aid programs"@en ;
  skos:broader agift:international-relations ;
  skos:definition "Developing policy and schemes to assist developing countries to reduce poverty, promote sustainable economic growth and recover from conflict or disasters. Working in partnership with other governments, businesses, non-government organisations and international agencies. Fostering links between the Australian community and the people of developing countries. Includes contributions to multilateral development banks and direct assistance packages." ;
  skos:hiddenLabel "Aid development" ;
  skos:hiddenLabel "Aid programs" ;
  skos:hiddenLabel "International aid" ;
  skos:narrower agift:development-assistance-programs ;
  skos:narrower agift:overseas-student-scholarship-programs ;
  skos:prefLabel "Overseas aid programs"@en ;
.
agift:overseas-promotion
  rdf:type skos:Concept ;
  rdfs:label "Overseas promotion"@en ;
  skos:broader agift:international-relations ;
  skos:definition """Undertaking liaison activities to raise Australia's international profile. Developing cultural exchange programs and advocating the benefits of international business. Establishing corporate networks and reciprocal visitor programs. Includes identifying and negotiating opportunities to promote Australia overseas, such as participating in international expositions, hosting major sporting events or cultural festivals.

See also CULTURAL AFFAIRS - Cultural festivals: for participation in international cultural events.

See also SPORT AND RECREATION - Sport and fitness development - Games promotion: for marketing international sporting events.

See also TOURISM - Tourist event promotion: for marketing international activities for travellers.

See also TRADE - Export regulation - Export promotion: for advocating Australian business in overseas markets.

See also TRADE - Trade expositions: for participation in international trade fairs.""" ;
  skos:hiddenLabel "Expos" ;
  skos:hiddenLabel "Expositions" ;
  skos:hiddenLabel "International cultural exchanges" ;
  skos:hiddenLabel "International expositions" ;
  skos:prefLabel "Overseas promotion"@en ;
  skos:related agift:cultural-festivals ;
  skos:related agift:export-promotion ;
  skos:related agift:games-promotion ;
  skos:related agift:tourist-event-promotion ;
  skos:related agift:trade-expositions ;
.
agift:overseas-skills-recognition
  rdf:type skos:Concept ;
  rdfs:label "Overseas skills recognition"@en ;
  skos:broader agift:education-and-training ;
  skos:definition "Endorsing or accrediting educational qualifications obtained outside Australia. Recognising Australians who have studied overseas or migrants wishing to apply their qualifications in Australia. Includes processing applications, managing examinations and setting conditions on the right to apply qualifications in certain fields." ;
  skos:hiddenLabel "Accreditation criteria" ;
  skos:hiddenLabel "International qualifications" ;
  skos:hiddenLabel "International skills recognition" ;
  skos:hiddenLabel "Overseas qualifications" ;
  skos:prefLabel "Overseas skills recognition"@en ;
  skos:related agift:practitioner-registration ;
  skos:related agift:professional-accreditation ;
.
agift:overseas-student-scholarship-programs
  rdf:type skos:Concept ;
  rdfs:label "Overseas student scholarship programs"@en ;
  skos:broader agift:overseas-aid-programs ;
  skos:definition """Supporting access to higher education for students from developing countries and the Pacific region. Providing assistance to study at regional education institutions, or opportunities to attend Australian education institutions. Includes services and training to help scholarship students realise the full benefits of the program.

See also EDUCATION AND TRAINING: for domestic student scholarships.""" ;
  skos:hiddenLabel "International scholarship programs" ;
  skos:hiddenLabel "Regional scholarship programs" ;
  skos:hiddenLabel "Scholarship programs" ;
  skos:prefLabel "Overseas student scholarship programs"@en ;
  skos:related agift:education-and-training ;
.
agift:park-and-reserve-services
  rdf:type skos:Concept ;
  rdfs:label "Park and reserve services"@en ;
  skos:broader agift:sport-and-recreation ;
  skos:definition """Administering areas of public land set aside for sport and recreational activities. Managing bookings, programs and payments. Controlling access and issuing permits for the use of parks and reserves. Supervising the allocation of sponsorships and corporate memberships. Ensuring the availability of staff such as referees or umpires.

See also CIVIC INFRASTRUCTURE - Public land management - Garden management: for administering public land where ornamental or useful plants are cultivated.

See also CIVIC INFRASTRUCTURE - Public land management - Recreational park management: for administering public leisure areas and playgrounds.

See also CIVIC INFRASTRUCTURE - Public land management - Sporting facilities management: for maintaining sporting grounds and amenities.

See also ENVIRONMENT - Natural heritage protection - National park management: for administering designated national park areas.

See also ENVIRONMENT - Natural heritage protection - Nature reserve management: for the maintenance of native flora and fauna reserves.

See also INDIGENOUS AFFAIRS - Indigenous heritage conservation: for land use agreements with traditional owners.

See also SPORT AND RECREATION - Sport and fitness development - Sporting grants administration: for funding to build and develop sporting facilities.""" ;
  skos:hiddenLabel "Cricket grounds" ;
  skos:hiddenLabel "Football stadiums" ;
  skos:hiddenLabel "Park access and permits" ;
  skos:hiddenLabel "Reserve management" ;
  skos:hiddenLabel "Sporting field management" ;
  skos:prefLabel "Park and reserve services"@en ;
  skos:related agift:garden-management ;
.
agift:parliamentary-chamber-support
  rdf:type skos:Concept ;
  rdfs:label "Parliamentary chamber support"@en ;
  skos:broader agift:governance ;
  skos:definition """Providing corporate assistance and security services to Houses of Parliament, assemblies or governing councils. Making arrangements for accommodation, equipment and catering. Overseeing building and maintenance requirements. Supervising broadcasts of parliamentary proceedings.

See also GOVERNANCE - Parliamentary committee and member support: for assistance to elected members.""" ;
  skos:hiddenLabel "Council chambers support" ;
  skos:hiddenLabel "House of Representatives support" ;
  skos:hiddenLabel "Joint Standing Committee support" ;
  skos:hiddenLabel "Legislative Assembly support" ;
  skos:hiddenLabel "Municipal council support" ;
  skos:hiddenLabel "Parliamentary support services" ;
  skos:narrower agift:hansard-services ;
  skos:narrower agift:parliamentary-papers ;
  skos:narrower agift:tabling-of-official-documents ;
  skos:prefLabel "Parliamentary chamber support"@en ;
  skos:related agift:parliamentary-committee-and-member-support ;
.
agift:parliamentary-committee-and-member-support
  rdf:type skos:Concept ;
  rdfs:label "Parliamentary committee and member support"@en ;
  skos:broader agift:governance ;
  skos:definition """Supplying administrative assistance to elected members, in all tiers of Australian government, to help them fulfil their duties. Managing secretariat support and secretarial staff. Providing access to reference and research services. Offering advice on procedures and the interpretation of standing orders.

See also GOVERNANCE - Parliamentary chamber support: for assistance to Houses of Parliament, assemblies or governing councils.""" ;
  skos:hiddenLabel "Lord Mayor" ;
  skos:hiddenLabel "Mayor" ;
  skos:prefLabel "Parliamentary committee and member support"@en ;
  skos:related agift:parliamentary-chamber-support ;
.
agift:parliamentary-papers
  rdf:type skos:Concept ;
  rdfs:label "Parliamentary papers"@en ;
  skos:broader agift:parliamentary-chamber-support ;
  skos:definition """Managing reports and other documents that have been officially tabled before parliament or an assembly. Organising the printing of presented papers, to support public scrutiny of government policy and parliamentary processes. Includes printing and gazetting of legislation passed through parliament.

See also GOVERNANCE - Parliamentary chamber support - Tabling of official documents: for submitting documents to parliament.""" ;
  skos:prefLabel "Parliamentary papers"@en ;
  skos:related agift:legislative-drafting ;
  skos:related agift:tabling-of-official-documents ;
.
agift:passenger-services
  rdf:type skos:Concept ;
  rdfs:label "Passenger services"@en ;
  skos:broader agift:transport ;
  skos:definition """Developing policy for the transportation of people by air, rail or road. Monitoring compliance with pricing regulations or the provision of appropriate facilities for passenger convenience. Includes services such as timetables, route maps or ticketing.

See also CIVIC INFRASTRUCTURE - Transport network maintenance: for managing public transport at local level.

See also COMMUNITY SERVICES - Transport access schemes: for programs to make services available to targeted community groups.

See also EDUCATION AND TRAINING - School education - School transport regulation: for helping children travel to and from school.

See also MARITIME SERVICES - Sea passengers: for transportation of people by sea.

See also TRANSPORT - Public transport: developing and maintaining a system of vehicles such as buses and trains that operates at regular times on fixed routes and are used by the public.""" ;
  skos:prefLabel "Passenger services"@en ;
  skos:related agift:sea-passengers ;
  skos:related agift:transport-network-maintenance ;
.
agift:passport-services
  rdf:type skos:Concept ;
  rdfs:label "Passport services"@en ;
  skos:broader agift:international-relations ;
  skos:definition """Issuing passports and travel documents to Australian citizens in Australia and overseas. Managing applications and renewals, providing advice and liaising with outlets that provide lodgement services.

See also IMMIGRATION - Travel authorisation: for issuing Australian visas to citizens of other countries.

See also INTERNATIONAL RELATIONS - Consular services: for other government services to Australians overseas.""" ;
  skos:hiddenLabel "Passports" ;
  skos:prefLabel "Passport services"@en ;
  skos:related agift:travel-authorisation ;
.
agift:pastoral-industry
  rdf:type skos:Concept ;
  rdfs:label "Pastoral industry"@en ;
  skos:broader agift:marine-and-rural-support ;
  skos:definition """Administering programs to support commercial game and livestock farming. Assisting industry growth and development. Encouraging businesses to adopt innovative practices, processes and products. Providing advice on production methods and business management to improve competitiveness.

See also PRIMARY INDUSTRIES - Marine and rural regulation - Agricultural industry: for monitoring and regulating livestock farming industries.

See also PRIMARY INDUSTRIES - Marine and rural support - Horticultural industry: for programs to support and develop crop farming industries.

See also SCIENCE - Animal and veterinary sciences: for research into livestock health and management practices.""" ;
  skos:hiddenLabel "Dairy industry support" ;
  skos:hiddenLabel "Game animal industry" ;
  skos:hiddenLabel "Livestock industry support" ;
  skos:hiddenLabel "Wool industry support" ;
  skos:prefLabel "Pastoral industry"@en ;
  skos:related agift:agricultural-industry ;
.
agift:patent-rights-management
  rdf:type skos:Concept ;
  rdfs:label "Patent rights management"@en ;
  skos:broader agift:intellectual-property-management ;
  skos:definition """Conferring exclusive legal rights to the production or sale of an invention or an industrial or scientific process. Registering and granting patent rigths and making patent specifications  available to the public.


See also TRADE - Intellectual property management - Design rights management: for the intellectual property in structures, machinery, industrial plans or complex artworks.

See also TRADE - Intellectual property management - Plant breeders' rights management: for developing policy to protect the rights of plant  breeders developing new plant varieties.

See also TRADE - Intellectual property management - Trademark registration: for the intellectual property in designs or symbols associated with a business entity or product.""" ;
  skos:prefLabel "Patent rights management"@en ;
  skos:related agift:design-rights-management ;
.
agift:patient-care
  rdf:type skos:Concept ;
  rdfs:label "Patient care"@en ;
  skos:broader agift:hospital-services ;
  skos:definition """Providing direct supervision and nursing for individuals under medical or surgical treatment. Implementing hospital policy and standards of best practice to ensure patients recover as fully and quickly as possible. Supplying food, amenities and recreation. Includes follow-up services after a patient has been released.

See also HEALTH CARE - Special needs services - Independent living services: for patient care offered outside hospitals.

See also HEALTH CARE - Special needs services - Residential services: for patient care offered outside hospitals.""" ;
  skos:hiddenLabel "Nursing" ;
  skos:hiddenLabel "Outpatient services" ;
  skos:prefLabel "Patient care"@en ;
  skos:related agift:independent-living-services ;
.
agift:payments-management
  rdf:type skos:Concept ;
  rdfs:label "Payments management"@en ;
  skos:broader agift:financial-system-management ;
  skos:definition "Managing the transfer of funds between consumers, businesses and financial institutions. Monitoring the payment instruments (cash, cheque and electronic funds transfer) used by consumers and businesses to transact business, and the transfer of funds from accounts in one financial institution to another." ;
  skos:hiddenLabel "Automatic teller machine (ATM)" ;
  skos:hiddenLabel "Cheques" ;
  skos:hiddenLabel "Credit cards" ;
  skos:hiddenLabel "Debit cards" ;
  skos:hiddenLabel "EFT/POS" ;
  skos:hiddenLabel "Electronic Funds Transfer (EFT)" ;
  skos:hiddenLabel "Real-time gross settlement (RTGS)" ;
  skos:prefLabel "Payments management"@en ;
.
agift:peacekeeping-forces
  rdf:type skos:Concept ;
  rdfs:label "Peacekeeping forces"@en ;
  skos:broader agift:external-security ;
  skos:definition """Deploying defence units to stabilise unrest and restore order in a designated international arena. Participating in cooperative efforts to alleviate international conflict, establish and maintain peace.

See also COMMUNITY SERVICES - Natural disasters - Disaster support: for the Australian Defence Forces assistance overseas during an emergency.

See also DEFENCE - Military operations - Special operations: for training provided to foreign local forces.

See also INTERNATIONAL RELATIONS - Defence liaison - Defence cooperation programs: for developing a coordinated international response to a potential or imminent threat.

See also INTERNATIONAL RELATIONS - Overseas aid programs - Development assistance programs: for supporting growth and improvement in other countries.""" ;
  skos:prefLabel "Peacekeeping forces"@en ;
  skos:related agift:defence-cooperation-programs ;
  skos:related agift:disaster-support ;
.
agift:permanent-entry-arrangements
  rdf:type skos:Concept ;
  rdfs:label "Permanent entry arrangements"@en ;
  skos:broader agift:travel-authorisation ;
  skos:definition """Administering programs to ensure lawful entrance of foreign nationals or refugees intending to settle in Australia. Processing applications for visas or migration and providing advice to applicants. Includes family reunion and special eligibility streams.

See also IMMIGRATION - Migrant services: for advice and support to foreign nationals intending to settle in Australia.""" ;
  skos:hiddenLabel "Migration applications" ;
  skos:hiddenLabel "Permanent residence visas" ;
  skos:hiddenLabel "Resident return visas" ;
  skos:hiddenLabel "Skilled migrant program" ;
  skos:hiddenLabel "Visa applications" ;
  skos:prefLabel "Permanent entry arrangements"@en ;
  skos:related agift:migrant-services ;
.
agift:personnel-safety-standards
  rdf:type skos:Concept ;
  rdfs:label "Personnel safety standards"@en ;
  skos:broader agift:ship-personnel ;
  skos:definition """Monitoring compliance with standards and guidelines for the operation of private or commercial marine vessels. Conducting safety training, competency checks and inspections to assess operational practices.

See also DEFENCE - Australian Defence Forces - Navy: for ship personnel in the Australian Defence Forces.

See also EMPLOYMENT - Human resources development - Occupational health and safety: for working environment conditions.

See also MARITIME SERVICES - Sea passengers: for services to travellers on ships.

See also MARITIME SERVICES - Ship personnel - Pilot licensing: for certifying personnel engaged in operating marine vessels.

See also MARITIME SERVICES - Ship safety - Ship inspection: for monitoring compliance with construction and maintenance standards.""" ;
  skos:hiddenLabel "Crew safety standards" ;
  skos:hiddenLabel "Ship operation standards" ;
  skos:prefLabel "Personnel safety standards"@en ;
  skos:related agift:navy ;
.
agift:pharmaceutical-and-drug-support
  rdf:type skos:Concept ;
  rdfs:label "Pharmaceutical and drug support"@en ;
  skos:broader agift:hospital-services ;
  skos:definition "Providing information about medical substances to hospitals and other health services. Administering drug management systems and offering advice on drug interactions for prescribers. Maintaining patient histories, including drug sensitivities and allergies." ;
  skos:hiddenLabel "Drug support services" ;
  skos:hiddenLabel "Pharmaceutical information" ;
  skos:prefLabel "Pharmaceutical and drug support"@en ;
.
agift:physical-sciences
  rdf:type skos:Concept ;
  rdfs:label "Physical sciences"@en ;
  skos:broader agift:science ;
  skos:definition """Conducting research into the properties of inanimate matter, substances and energy. Analysing and manipulating such material to identify the principles and processes that govern its behaviour. Includes the development of new methods to exploit physical substances or energy.

See also SCIENCE - Applied sciences: for the direct use of physical science research in an operational or industrial setting.

See also SCIENCE - Biological sciences - Biochemistry: for the chemical analysis of biological organisms.""" ;
  skos:hiddenLabel "Chemical analysis" ;
  skos:hiddenLabel "Chemistry" ;
  skos:hiddenLabel "Physics" ;
  skos:narrower agift:astronomical-sciences ;
  skos:narrower agift:atomic-and-molecular-sciences ;
  skos:narrower agift:nuclear-sciences ;
  skos:prefLabel "Physical sciences"@en ;
  skos:related agift:applied-sciences ;
.
agift:physiology
  rdf:type skos:Concept ;
  rdfs:label "Physiology"@en ;
  skos:broader agift:biological-sciences ;
  skos:definition """Conducting research into biological functions and systems. Analysing the structure and anatomy of organisms. Investigating the internal processes of plants and animals at tissue- and organ-level. Determining how particular physiological attributes contribute to an organism's fitness and performance. Includes pharmacological and immunological studies to develop new drugs or vaccines.

See also SCIENCE - Medical and health sciences: for research into human health and disease.""" ;
  skos:hiddenLabel "Anatomy" ;
  skos:hiddenLabel "Neurology" ;
  skos:prefLabel "Physiology"@en ;
  skos:related agift:medical-and-health-sciences ;
.
agift:pilot-licensing
  rdf:type skos:Concept ;
  rdfs:label "pilot licensing"@en ;
  skos:prefLabel "pilot licensing"@en ;
  skos:related agift:pilotage-management ;
.
agift:pilotage-management
  rdf:type skos:Concept ;
  rdfs:label "Pilotage management"@en ;
  skos:broader agift:maritime-services ;
  skos:definition """Providing qualified operators to steer vessels into and out of ports. Monitoring pilotage procedures and clarifying the responsibilities of pilots and pilotage providers. Developing and administering standards for pilotage operations that support international requirements.

See also MARITIME SERVICES - Ship personnel - Pilot licensing: for certifying vessel pilots.""" ;
  skos:hiddenLabel "Coastal pilotage" ;
  skos:hiddenLabel "Marine pilotage" ;
  skos:hiddenLabel "Vessel piloting" ;
  skos:prefLabel "Pilotage management"@en ;
  skos:related agift:pilot-licensing ;
.
agift:place-names
  rdf:type skos:Concept ;
  rdfs:label "Place names"@en ;
  skos:broader agift:civic-infrastructure ;
  skos:definition "Approving and registering the formal names of rivers, mountains, plains, towns, suburbs, reefs, shoals and undersea features." ;
  skos:hiddenLabel "Geographic names" ;
  skos:prefLabel "Place names"@en ;
.
agift:planning-approvals
  rdf:type skos:Concept ;
  rdfs:label "Planning approvals"@en ;
  skos:broader agift:civic-management ;
  skos:prefLabel "Planning approvals"@en ;
.
agift:plant-breeders-rights-management
  rdf:type skos:Concept ;
  rdfs:label "Plant breeders' rights management"@en ;
  skos:broader agift:intellectual-property-management ;
  skos:definition """Developing policy to protect the rights of plant  breeders developing new plant varieties.

See also TRADE - Intellectual property management - Design rights management: for the intellectual property in structures, machinery, industrial plans or complex artworks.

See also TRADE - Intellectual property management - Patent rights management: for the intellectual property in inventions and industrial or scientific processes.

See also TRADE - Intellectual property management - Trademark registration: for the intellectual property in designs or symbols associated with a business entity or product.""" ;
  skos:prefLabel "Plant breeders' rights management"@en ;
  skos:related agift:design-rights-management ;
.
agift:police-administration
  rdf:type skos:Concept ;
  rdfs:label "Police administration"@en ;
  skos:broader agift:law-enforcement ;
  skos:definition "Providing trained personnel to assist citizens who have been victims of crime, or in matters of law enforcement. Managing staff and facilities at police stations. Administering internal command, investigation and disciplinary procedures." ;
  skos:hiddenLabel "Police stations" ;
  skos:prefLabel "Police administration"@en ;
.
agift:pollutant-prevention-programs
  rdf:type skos:Concept ;
  rdfs:label "Pollutant prevention programs"@en ;
  skos:broader agift:environment ;
  skos:definition """Establishing standards and developing initiatives to reduce contamination of the air, water and land by emissions and waste. Developing strategies to counteract the effects of pollutants if accidents occur. Raising awareness and supporting community activities to change common practice. Promoting environmentally friendly alternatives.

See also CIVIC INFRASTRUCTURE - Waste management: for services to collect and dispose of garbage.

See also NATURAL RESOURCES - Pollution emission control: for monitoring compliance with environmental standards.

See also NATURAL RESOURCES - Water resources - Waterway management: for strategies for salinity management and river care programs.

See also SCIENCE - Earth sciences - Atmospheric sciences: for conducting research into the environmental impact of pollution.""" ;
  skos:hiddenLabel "Noise pollution" ;
  skos:hiddenLabel "Oil spill prevention programs" ;
  skos:hiddenLabel "Smog prevention programs" ;
  skos:hiddenLabel "Waste control programs" ;
  skos:prefLabel "Pollutant prevention programs"@en ;
  skos:related agift:pollution-emission-control ;
  skos:related agift:waste-management ;
.
agift:pollution-emission-control
  rdf:type skos:Concept ;
  rdfs:label "Pollution emission control"@en ;
  skos:broader agift:natural-resources ;
  skos:definition """Monitoring compliance with standards for the discharge of industrial contaminants and waste. Regulating industry practices through waste minimisation strategies and pollutant inventories. Includes assessment, inspections and providing emissions information to the community.

See also ENVIRONMENT - Pollutant prevention programs: for setting standards and developing initiatives to reduce pollution.

See also SCIENCE - Earth sciences - Atmospheric sciences: for conducting research into the environmental impact of pollution.""" ;
  skos:hiddenLabel "Effluent control" ;
  skos:hiddenLabel "Emissions control" ;
  skos:hiddenLabel "Pollution" ;
  skos:prefLabel "Pollution emission control"@en ;
  skos:related agift:pollutant-prevention-programs ;
  skos:related agift:water-quality-monitoring ;
.
agift:population-based-research
  rdf:type skos:Concept ;
  rdfs:label "Population-based research"@en ;
  skos:broader agift:medical-research ;
  skos:definition """Conducting clinical investigations of the health of particular groups of individuals. Evaluating the incidence of particular diseases within a geographical area or demographic category. Making recommendations to support public health policy development.

See also STATISTICAL SERVICES- Statistical collection: for collecting statistics and analysing this collected data to identify trends.

See also SCIENCE - Medical and health sciences: for experimental research into human health and disease.""" ;
  skos:hiddenLabel "Drug support services" ;
  skos:prefLabel "Population-based research"@en ;
  skos:related agift:epidemiology ;
  skos:related agift:statistical-collection ;
.
agift:port-regulation
  rdf:type skos:Concept ;
  rdfs:label "Port regulation"@en ;
  skos:broader agift:maritime-services ;
  skos:definition """Managing sea-based entry and exit points. Building and maintaining infrastructure to allow ships to load or unload passengers and cargo. Monitoring private terminal operators and regulating port activities to protect against environmental impacts. Assessing the integration of road, rail and air transport infrastructure with maritime services. Includes liaison to promote coordination and consistency among port authorities from different jurisdictions.

See also ENVIRONMENT - Oceans governance: for ecologically sustainable development of marine resources.

See also MARITIME SERVICES - Cargo control: for handling and storage of goods on marine vessels.

See also MARITIME SERVICES - Harbour management: for managing infrastructure that provides protection for ships.

See also MARITIME SERVICES - Harbour management: for shipping movements.

See also MARITIME SERVICES - Marina management: for dockage facilities for small craft.

See also NATURAL RESOURCES - Water resources - Waterway management: for regulating the use of rivers and catchment areas.

See also TRADE - Export regulation: for controlling the international movement of goods.

See also TRADE - Import regulation: for controlling the international movement of goods.

See also TRADE - Import regulation - Tariff regulation: for levies and taxes charged at ports.""" ;
  skos:hiddenLabel "Ports" ;
  skos:hiddenLabel "Seaport regulation" ;
  skos:hiddenLabel "Shipping channel management" ;
  skos:hiddenLabel "Wharf management" ;
  skos:prefLabel "Port regulation"@en ;
  skos:related agift:charting-sea-lanes ;
  skos:related agift:navigation ;
  skos:related agift:oceans-governance ;
.
agift:postal-services
  rdf:type skos:Concept ;
  rdfs:label "Postal services"@en ;
  skos:broader agift:communications ;
  skos:definition "Developing policy and guidelines to support the collection and delivery of letters, parcels and other mail. Establishing standards for pricing and processing, such as ensuring dangerous goods are intercepted. Designing and issuing postage stamps." ;
  skos:hiddenLabel "Australia Post" ;
  skos:hiddenLabel "Mail services" ;
  skos:hiddenLabel "Postage stamps" ;
  skos:narrower agift:courier-services ;
  skos:narrower agift:electronic-postal-services ;
  skos:narrower agift:retail-postal-services ;
  skos:prefLabel "Postal services"@en ;
.
agift:practitioner-discipline
  rdf:type skos:Concept ;
  rdfs:label "Practitioner discipline"@en ;
  skos:broader agift:health-protocol-administration ;
  skos:definition "Administering guidelines to assess the professional conduct of health care providers. Evaluating performance against established standards and codes of practice. Investigating complaints and initiating disciplinary proceedings or applying penalties when appropriate. Includes suspending or deregistering practitioners found in breach of regulations." ;
  skos:hiddenLabel "Malpractice" ;
  skos:hiddenLabel "Medical negligence" ;
  skos:prefLabel "Practitioner discipline"@en ;
.
agift:practitioner-registration
  rdf:type skos:Concept ;
  rdfs:label "Practitioner registration"@en ;
  skos:broader agift:health-protocol-administration ;
  skos:definition """Evaluating the qualifications of health care providers to determine their fitness for medical practice. Assessing applications and providing advice to unsuccessful applicants. Maintaining a register of approved applicants who may legally practice.

See also EDUCATION AND TRAINING - Overseas skills recognition: for endorsing qualifications obtained outside Australia.

See also HEALTH CARE - Health protocol administration - Practitioner discipline: for suspending or deregistering health care providers.""" ;
  skos:hiddenLabel "Doctor registration" ;
  skos:hiddenLabel "General practitioner registration" ;
  skos:hiddenLabel "Health accreditation" ;
  skos:hiddenLabel "Health practitioner registration" ;
  skos:prefLabel "Practitioner registration"@en ;
  skos:related agift:overseas-skills-recognition ;
.
agift:preparation-of-legislative-regulations
  rdf:type skos:Concept ;
  rdfs:label "Preparation of legislative regulations"@en ;
  skos:broader agift:legislative-drafting ;
  skos:definition "Drafting statutory rules to support the implementation of laws and parliamentary acts. Analysing government policy and existing legislation. Managing submission and approval processes, printing and gazetting." ;
  skos:hiddenLabel "Regulation development" ;
  skos:hiddenLabel "Statutory rules" ;
  skos:prefLabel "Preparation of legislative regulations"@en ;
.
agift:presentation-arrangements
  rdf:type skos:Concept ;
  rdfs:label "Presentation arrangements"@en ;
  skos:broader agift:citizenship ;
  skos:definition """Organising and conducting ceremonies to confer Australian citizenship. Preparing participants to take their citizenship pledge and arranging the presentation of certificates. Coordinating security, publicity and facilities. Includes affirmation ceremonies for existing Australian citizens.

See also GOVERNANCE - Civic celebrations: for other community events and ceremonies to mark significant occasions.""" ;
  skos:hiddenLabel "Citizenship ceremonies" ;
  skos:hiddenLabel "Naturalisation ceremonies" ;
  skos:prefLabel "Presentation arrangements"@en ;
  skos:related agift:civic-celebrations ;
.
agift:preservation-services
  rdf:type skos:Concept ;
  rdfs:label "Preservation services"@en ;
  skos:broader agift:collection-management ;
  skos:definition """Developing strategies to protect and conserve material in cultural collections. Applying treatments to prevent decomposition over time or through excessive handling. Includes repair of badly damaged items or transfer to stable media. 

See also CULTURAL AFFAIRS - Collection management - Collection storage: for environmental controls that protect cultural materials.""" ;
  skos:hiddenLabel "Collection preservation" ;
  skos:hiddenLabel "Conservation services" ;
  skos:hiddenLabel "Restoration services" ;
  skos:prefLabel "Preservation services"@en ;
  skos:related agift:collection-storage ;
.
agift:prices-surveillance
  rdf:type skos:Concept ;
  rdfs:label "Prices surveillance"@en ;
  skos:broader agift:fair-trading-compliance ;
  skos:definition """Monitoring and regulating the charges for goods or services offered for sale. Evaluating proposed price increases, where an industry or organisation is under surveillance. Making recommendations on pricing practices.

See also FINANCE MANAGEMENT - Monetary policy - Inflation: for monitoring amounts of currency in circulation and the effect on prices.""" ;
  skos:hiddenLabel "Price control" ;
  skos:hiddenLabel "Price fixing" ;
  skos:hiddenLabel "Price surveillance" ;
  skos:prefLabel "Prices surveillance"@en ;
  skos:related agift:energy-supply ;
  skos:related agift:inflation ;
.
agift:primary-health-care
  rdf:type skos:Concept ;
  rdfs:label "Primary health care"@en ;
  skos:broader agift:community-health-services ;
  skos:definition """Administering programs that deliver essential health care services at the most local level. Ensuring all members of the community have access to basic methods of prevention and treatment for disease or injury. Monitoring the provision of primary health care services in remote or isolated areas.

See also EDUCATION AND TRAINING - Community education - Adult education programs: for community-based health education programs.

See also EDUCATION AND TRAINING - School education: for health education of school-aged children.

See also HEALTH CARE - Community health services - Clinical health services: for programs operating out of medical centres.

See also HEALTH CARE - Community health services - Health promotion: for basic advice and information to support good health.

See also INDIGENOUS AFFAIRS - Indigenous health services: for developing programs for Aboriginal and Torres Strait Islander communities.""" ;
  skos:hiddenLabel "Community health centres" ;
  skos:hiddenLabel "Community midwifery" ;
  skos:hiddenLabel "Family planning" ;
  skos:hiddenLabel "Immunisation programs" ;
  skos:hiddenLabel "Maternal health services" ;
  skos:hiddenLabel "Remote community health care" ;
  skos:hiddenLabel "Vaccination programs" ;
  skos:prefLabel "Primary health care"@en ;
  skos:related agift:adult-education-programs ;
  skos:related agift:indigenous-health-services ;
.
agift:primary-industries
  rdf:type skos:Concept ;
  rdfs:label "PRIMARY INDUSTRIES"@en ;
  skos:definition """Developing policy to support and regulate rural and marine industries. Promoting strategies for efficient and sustainable operations. Administering programs to monitor current practices, to meet national and international standards. Includes liaison with industry bodies and across jurisdictions in relation to the needs of primary industries.

See also BUSINESS SUPPORT AND REGULATION: for supporting and regulating other industries.

See also NATURAL RESOURCES: for supporting and regulating mining industries.

See also SCIENCE: for research to assist primary industries.""" ;
  skos:hiddenLabel "Agriculture" ;
  skos:hiddenLabel "Industry" ;
  skos:hiddenLabel "Marine industry" ;
  skos:hiddenLabel "Rural industry" ;
  skos:narrower agift:chemical-and-pesticide-regulation ;
  skos:narrower agift:marine-and-rural-regulation ;
  skos:narrower agift:marine-and-rural-support ;
  skos:narrower agift:quarantine ;
  skos:narrower agift:rural-field-day-promotion ;
  skos:narrower agift:rural-partnership-programs ;
  skos:prefLabel "PRIMARY INDUSTRIES"@en ;
  skos:related agift:business-support-and-regulation ;
.
agift:privacy-
  rdf:type skos:Concept ;
  rdfs:label "Privacy "@en ;
  skos:broader agift:justice-administration ;
  skos:definition """Establishing privacy principles to ensure an individual's rights to the confidentiality of their personal information. Monitoring compliance with legislation and guidelines. Includes investigating breaches of privacy and evaluating new technology for potential risks to individual privacy.

See also JUSTICE ADMINISTRATION - Administrative law - Freedom of information: providing a right of access to  government  documents.

See also JUSTICE ADMINISTRATION - Administrative law - Recordkeeping standards: for regulating the management of government information in accordance with legislative requirements.

See also SECURITY - Information security: for policy and technology to control data access.""" ;
  skos:hiddenLabel "Privacy Act" ;
  skos:hiddenLabel "Privacy guideline monitoring" ;
  skos:hiddenLabel "Privacy protection" ;
  skos:prefLabel "Privacy "@en ;
  skos:related agift:freedom-of-information ;
.
agift:probate-applications
  rdf:type skos:Concept ;
  rdfs:label "Probate applications"@en ;
  skos:broader agift:civil-law ;
  skos:definition "Managing the registration and validation of wills. Authorising a named executor to administer the estate of a deceased person. Includes procedures to handle contested probate requests." ;
  skos:hiddenLabel "Deceased estates" ;
  skos:hiddenLabel "Will registration" ;
  skos:prefLabel "Probate applications"@en ;
.
agift:product-safety
  rdf:type skos:Concept ;
  rdfs:label "Product safety"@en ;
  skos:broader agift:fair-trading-compliance ;
  skos:definition "Administering programs to ensure the quality of products offered for sale. Assessing statements made about the goods - such as origin, conditions of sale, warranties and guarantees. Evaluating product safety, banning goods or issuing product recalls. Imposing penalties as appropriate." ;
  skos:prefLabel "Product safety"@en ;
.
agift:productivity
  rdf:type skos:Concept ;
  rdfs:label "Productivity"@en ;
  skos:broader agift:resource-management ;
  skos:definition """Developing measures and programs to capture the ability of an economy to harness its physical and human resources to generate output and income.
See also FINANCE MANAGEMENT- Financial system management: for policy to maintain stability in the financial system.
See also FINANCE MANAGEMENT- Fiscal policy: for policy for the strategic management and distribution of public money.
See also FINANCE MANAGEMENT - Monetary policy:  for policy to maintain stability of the currency.""" ;
  skos:prefLabel "Productivity"@en ;
.
agift:professional-accreditation
  rdf:type skos:Concept ;
  rdfs:label "Professional accreditation"@en ;
  skos:broader agift:business-support-and-regulation ;
  skos:definition """Administering programs to certify individuals as meeting official requirements to perform a skilled occupation. Includes processing applications, managing examinations and setting conditions on the right to apply qualifications in certain fields.

See also EDUCATION AND TRAINING - Overseas skills recognition: for endorsing qualifications obtained outside Australia.""" ;
  skos:hiddenLabel "Accreditation criteria" ;
  skos:hiddenLabel "Competency standards" ;
  skos:hiddenLabel "Professional codes of practice" ;
  skos:hiddenLabel "Qualified professionals" ;
  skos:prefLabel "Professional accreditation"@en ;
  skos:related agift:overseas-skills-recognition ;
.
agift:prohibited-export-control
  rdf:type skos:Concept ;
  rdfs:label "Prohibited export control"@en ;
  skos:broader agift:export-regulation ;
  skos:definition """Regulating the international sale and movement out of Australia of restricted goods such as wildlife, heritage artefacts, weaponry, military equipment, nuclear material, chemicals and toxins, electronics, software and technology, currency, illicit drugs. Includes policy development, procedures for inspection and seizure, and liaison with other jurisdictions.

See also CULTURAL AFFAIRS - Collection management - Artefact export regulation: for negotiating the international movement of cultural material.""" ;
  skos:prefLabel "Prohibited export control"@en ;
  skos:related agift:artefact-export-regulation ;
.
agift:prohibited-import-control
  rdf:type skos:Concept ;
  rdfs:label "Prohibited import control"@en ;
  skos:broader agift:import-regulation ;
  skos:definition """Regulating the international purchase and movement into Australia of restricted goods such as medicines and illicit drugs, animals and animal-derived products, plants and plant-derived products, weaponry, military equipment, nuclear material, chemicals and toxins, heritage artefacts, motor vehicles, currency. Includes policy development, procedures for inspection and seizure, and liaison with other jurisdictions.

See also CULTURAL AFFAIRS - Collection management - Artefact export regulation: for negotiating the international movement of cultural material.

See also PRIMARY INDUSTRIES - Quarantine: for activities to protect Australia from exotic plants, animals and diseases.

See also SECURITY - National security - Border protection: for coordinating operations to monitor Australian borders for unauthorised sea or air arrivals. 

See also TRADE - Import regulation - Tariff regulation: for the imposition of duties or taxes on imports.""" ;
  skos:prefLabel "Prohibited import control"@en ;
  skos:related agift:artefact-export-regulation ;
.
agift:prosecution-services
  rdf:type skos:Concept ;
  rdfs:label "Prosecution services"@en ;
  skos:broader agift:justice-administration ;
  skos:definition """Bringing individuals or organisations to trial for criminal offences. Carrying on of legal proceedings against a party, in the interests of the public.

See also JUSTICE ADMINISTRATION - Legal aid services: for subsidised defence representation.

See also SECURITY - Corrective services: for punishment and rehabilitation programs.

See also SECURITY - Law enforcement: for crime prevention programs.""" ;
  skos:hiddenLabel "Public prosecutions" ;
  skos:prefLabel "Prosecution services"@en ;
  skos:related agift:legal-aid-services ;
.
agift:protective-services
  rdf:type skos:Concept ;
  rdfs:label "Protective services"@en ;
  skos:broader agift:law-enforcement ;
  skos:definition """Providing specialist security products and services to shield an individual from threat of attack. Managing physical security programs, designated persons protection, X-ray screening, bomb threat management and protective surveillance. Includes administration of security personnel through staff vetting and clearance procedures.

See also SECURITY - Intelligence - Intelligence support: for investigative surveillance activities.""" ;
  skos:hiddenLabel "Bodyguards" ;
  skos:hiddenLabel "Diplomatic protection" ;
  skos:hiddenLabel "Security guards" ;
  skos:prefLabel "Protective services"@en ;
  skos:related agift:intelligence-support ;
.
agift:public-administration
  rdf:type skos:Concept ;
  rdfs:label "Public administration"@en ;
  skos:broader agift:governance ;
  skos:definition """Administering programs to implement the policies and programs of the executive and elected representatives. Review the performance of such programs. Developing policy and guidelines to improve public administration.

See also JUSTICE ADMINISTRATION - Administrative law: for the administration of laws relating to the functions of public agencies.""" ;
  skos:narrower agift:corruption-prevention ;
  skos:narrower agift:government-auditing ;
  skos:narrower agift:integrity-compliance ;
  skos:narrower agift:public-service ;
  skos:narrower agift:territories-administration ;
  skos:narrower agift:whistleblowing ;
  skos:prefLabel "Public administration"@en ;
  skos:related agift:administrative-law ;
.
agift:public-borrowing
  rdf:type skos:Concept ;
  rdfs:label "Public borrowing"@en ;
  skos:broader agift:fiscal-policy ;
  skos:definition """Administering programs to raise funds to finance government expenditure, in accordance with fiscal policy. Includes the issue and sale of government bonds.

See also FINANCE MANAGEMENT - Fiscal policy - Public debt: for redeeming government bonds.""" ;
  skos:hiddenLabel "Bonds" ;
  skos:hiddenLabel "Government bonds" ;
  skos:hiddenLabel "Government borrowing" ;
  skos:hiddenLabel "Treasury bonds" ;
  skos:prefLabel "Public borrowing"@en ;
  skos:related agift:public-debt ;
.
agift:public-debt
  rdf:type skos:Concept ;
  rdfs:label "Public debt"@en ;
  skos:broader agift:fiscal-policy ;
  skos:definition """Managing the repayment of public borrowings, including the redemption of government bonds. Minimising associated costs such as interest payments by coordinating payments with tax revenue inflows.

See also FINANCE MANAGEMENT - Fiscal policy - Public borrowing: for the issue and sale of government bonds.""" ;
  skos:hiddenLabel "Government debt management" ;
  skos:prefLabel "Public debt"@en ;
  skos:related agift:public-borrowing ;
.
agift:public-expenditure
  rdf:type skos:Concept ;
  rdfs:label "Public expenditure"@en ;
  skos:broader agift:fiscal-policy ;
  skos:definition """Managing the disbursement of public money in accordance with fiscal policy. Monitoring revenue forecasts and projecting the costs of proposed programs or services. Determining the economic impact of government spending.

See also FINANCE MANAGEMENT - Resource management - Financial budgeting: for documenting public revenues and expenditure.""" ;
  skos:hiddenLabel "Government spending" ;
  skos:prefLabel "Public expenditure"@en ;
  skos:related agift:financial-budgeting ;
.
agift:public-fitness-promotion
  rdf:type skos:Concept ;
  rdfs:label "Public fitness promotion"@en ;
  skos:broader agift:community-recreational-programs ;
  skos:definition """Administering schemes to encourage physical activity across the community. Developing programs to raise awareness of the health benefits of fitness. Providing activities for target groups and supporting clubs and community groups that promote physical fitness.

See also HEALTH CARE - Community health services - Health promotion: for raising public awareness of other health issues.

See also SPORT AND RECREATION - Sport and fitness development: for funding for sport and fitness programs.""" ;
  skos:hiddenLabel "Fitness promotion" ;
  skos:hiddenLabel "National fitness campaigns" ;
  skos:prefLabel "Public fitness promotion"@en ;
  skos:related agift:health-promotion ;
.
agift:public-health-services
  rdf:type skos:Concept ;
  rdfs:label "Public health services"@en ;
  skos:broader agift:health-care ;
  skos:definition """Developing policy to protect the physical and mental wellbeing of all people at a broad level. Establishing programs to understand and control the determinants of disease, and reduce public exposure to risks encountered as part of lifestyle or the environment.

See also HEALTH CARE - Community health services: for programs that offer direct assistance to individuals or groups.""" ;
  skos:hiddenLabel "Public health" ;
  skos:narrower agift:blood-and-organ-donation-management ;
  skos:narrower agift:epidemiology ;
  skos:narrower agift:health-disaster-preparedness ;
  skos:narrower agift:health-hazard-prevention ;
  skos:narrower agift:medical-quarantine-services ;
  skos:narrower agift:medical-radiation-services ;
  skos:narrower agift:notifiable-disease-management ;
  skos:narrower agift:radiation-protection ;
  skos:prefLabel "Public health services"@en ;
  skos:related agift:community-health-services ;
.
agift:public-housing
  rdf:type skos:Concept ;
  rdfs:label "Public housing"@en ;
  skos:broader agift:civic-infrastructure ;
  skos:definition """Administering programs to supply low cost government-owned accommodation. Providing guidelines to direct the design of public housing. Evaluating the need for public housing and setting construction targets. Allocating appropriate funds to enable ongoing maintenance.

See also COMMUNITY SERVICES - Accommodation services: for making public housing available to those in need.

See also NATURAL RESOURCES - Crown land administration: for managing the tenure of government property.""" ;
  skos:hiddenLabel "Commission housing" ;
  skos:hiddenLabel "Government housing" ;
  skos:hiddenLabel "Housing" ;
  skos:hiddenLabel "Indigenous housing" ;
  skos:hiddenLabel "Social housing" ;
  skos:narrower agift:community-housing ;
  skos:narrower agift:public-housing-construction ;
  skos:narrower agift:public-housing-design ;
  skos:narrower agift:public-housing-maintenance ;
  skos:prefLabel "Public housing"@en ;
  skos:related agift:accommodation-services ;
  skos:related agift:income-support-schemes ;
  skos:related agift:migrant-accommodation-services ;
  skos:related agift:public-housing-entitlements ;
.
agift:public-housing-construction
  rdf:type skos:Concept ;
  rdfs:label "Public housing construction"@en ;
  skos:broader agift:public-housing ;
  skos:definition """Building low cost government-owned accommodation. Managing tenders and overseeing construction projects. Negotiating value for money on materials and services to support affordability. Ensuring that public housing construction meets government targets.

See also CIVIC INFRASTRUCTURE - Civic management - Architectural services: for professional advice on the design and construction of public buildings.

See also CIVIC INFRASTRUCTURE - Civic management - Building regulations and standards: for ensuring housing meets legal requirements.""" ;
  skos:prefLabel "Public housing construction"@en ;
  skos:related agift:architectural-services ;
.
agift:public-housing-design
  rdf:type skos:Concept ;
  rdfs:label "Public housing design"@en ;
  skos:broader agift:public-housing ;
  skos:definition """Planning and drafting low cost government-owned accommodation. Implementing best practice design strategies to incorporate facilities for tenants with special needs. Ensuring that public housing design meets government guidelines.

See also CIVIC INFRASTRUCTURE - Civic management - Architectural services: for professional advice on the design and construction of public buildings.""" ;
  skos:prefLabel "Public housing design"@en ;
  skos:related agift:architectural-services ;
.
agift:public-housing-entitlements
  rdf:type skos:Concept ;
  rdfs:label "Public housing entitlements"@en ;
  skos:broader agift:accommodation-services ;
  skos:definition """Assessing eligibility for community accommodation, against established criteria. Allocating public housing to approved applicants. Providing advice to tenants about their rights and obligations, and options to purchase public housing. Includes entitlement review and complaint processes.

See also CIVIC INFRASTRUCTURE - Public housing: for the design, construction and maintenance of public housing.

See also COMMUNITY SERVICES - Financial assistance - Income support schemes: for rental assistance.""" ;
  skos:prefLabel "Public housing entitlements"@en ;
  skos:related agift:public-housing ;
.
agift:public-housing-maintenance
  rdf:type skos:Concept ;
  rdfs:label "Public housing maintenance"@en ;
  skos:broader agift:public-housing ;
  skos:definition "Preserving and repairing low cost government-owned accommodation. Implementing programs of regular maintenance. Reporting on the condition of public housing and recommending upgrades or major renovation when necessary." ;
  skos:hiddenLabel "Maintenance" ;
  skos:prefLabel "Public housing maintenance"@en ;
.
agift:public-land-management
  rdf:type skos:Concept ;
  rdfs:label "Public land management"@en ;
  skos:broader agift:civic-infrastructure ;
  skos:definition """Controlling and maintaining buildings or areas of land set aside for community use. Providing guidelines to direct the use of public land. Allocating appropriate funds to enable ongoing maintenance. Evaluating the need for public land and providing advice for planning purposes.

See also NATURAL RESOURCES - Crown land administration: for managing the tenure of government property.

See also NATURAL RESOURCES - Land use planning: for research into future needs for infrastructure and facilities.""" ;
  skos:hiddenLabel "Property" ;
  skos:hiddenLabel "Street light maintenance" ;
  skos:hiddenLabel "Street tree management" ;
  skos:hiddenLabel "Urban land management" ;
  skos:hiddenLabel "Urban tree management" ;
  skos:narrower agift:burial-ground-management ;
  skos:narrower agift:cultural-centre-management ;
  skos:narrower agift:garden-management ;
  skos:narrower agift:memorial-maintenance ;
  skos:narrower agift:recreational-park-management ;
  skos:narrower agift:sporting-facilities-management ;
  skos:prefLabel "Public land management"@en ;
  skos:related agift:crown-land-administration ;
.
agift:public-service
  rdf:type skos:Concept ;
  rdfs:label "Public service"@en ;
  skos:broader agift:public-administration ;
  skos:definition """Implementing the policies of the executive and elected representatives. Providing services to the community in accordance with agreed performance standards.

See also EMPLOYMENT: for conditions of employment.""" ;
  skos:prefLabel "Public service"@en ;
  skos:related agift:employment ;
.
agift:public-transport
  rdf:type skos:Concept ;
  rdfs:label "Public transport"@en ;
  skos:broader agift:transport ;
  skos:definition """Developing and maintaining a system of vehicles such as buses and trains that operates at regular times on fixed routes and are used by the public.

See also CIVIC INFRASTRUCTURE - Transport network maintenance: for managing public transport at local level.

See also COMMUNITY SERVICES - Transport access schemes: for programs to make services available to targeted community groups.

See also TRANSPORT - Passenger services: developing policy for the transportation of people by air, rail or road.""" ;
  skos:narrower agift:transport-accessibility ;
  skos:prefLabel "Public transport"@en ;
  skos:related agift:transport-network-maintenance ;
.
agift:publicity-programs
  rdf:type skos:Concept ;
  rdfs:label "Publicity programs"@en ;
  skos:broader agift:collection-promotion ;
  skos:definition """Planning and implementing campaigns to promote cultural institutions and their collections. Developing media releases, advertising material and catalogues for exhibitions. Organising tours, visits and speaking engagements.

See also COMMUNICATIONS - Government media: for managing media releases and dealing with journalists.

See also COMMUNICATIONS - Publishing: for producing information resources in print.

See also CULTURAL AFFAIRS - Collection promotion - Exhibition programs: for displays of material from cultural collections.""" ;
  skos:hiddenLabel "Marketing campaigns" ;
  skos:prefLabel "Publicity programs"@en ;
  skos:related agift:exhibition-programs ;
  skos:related agift:government-media ;
.
agift:publishing
  rdf:type skos:Concept ;
  rdfs:label "Publishing"@en ;
  skos:broader agift:communications ;
  skos:definition """Developing policy to support the compilation and distribution of government information via print or electronic media. Managing applications to use material under government copyright. Includes editing and publishing material in printed formats.

See also COMMUNICATIONS - Government media: for managing advertising and communications activities.

See also COMMUNICATIONS - Information management standards - Information dissemination: for developing broad-ranging communication strategies.

See also CULTURAL AFFAIRS - Arts development: for assistance to literary endeavours.

See also TRADE - Intellectual property management - Copyright registration: for conferring legal ownership over publications.""" ;
  skos:hiddenLabel "Publications" ;
  skos:narrower agift:electronic-publishing ;
  skos:narrower agift:publishing-standards ;
  skos:narrower agift:website-development ;
  skos:prefLabel "Publishing"@en ;
  skos:related agift:collection-promotion ;
  skos:related agift:government-media ;
.
agift:publishing-standards
  rdf:type skos:Concept ;
  rdfs:label "Publishing standards"@en ;
  skos:broader agift:publishing ;
  skos:definition """Establishing principles and criteria for the compilation and distribution of government information via print or electronic media. Monitoring compliance with government standards and guidelines. Includes advice on layout, style, use of logos, formats for electronic delivery or legal deposit arrangements.

See also JUSTICE ADMINISTRATION - Administrative law - Censorship standards: for regulating the accessibility of content in publications.""" ;
  skos:prefLabel "Publishing standards"@en ;
  skos:related agift:censorship-standards ;
.
agift:quarantine
  rdf:type skos:Concept ;
  rdfs:label "Quarantine"@en ;
  skos:broader agift:primary-industries ;
  skos:definition """Developing strategies to protect the health of Australia's plant and animal populations from risks associated with exotic pests and disease. Conducting inspections at borders, ports, airports and other entry or exit points. Managing isolation and disinfection facilities. Applying penalties for breaches of regulations.

See also HEALTH CARE - Public health services - Medical quarantine services: for isolating people who have been exposed to disease.

See also TRADE - Export regulation - Prohibited export control: for regulating the international trade of restricted goods.

See also TRADE - Import regulation - Prohibited import control: for regulating the international trade of restricted goods.""" ;
  skos:hiddenLabel "Animal quarantine" ;
  skos:hiddenLabel "Isolation facilities" ;
  skos:prefLabel "Quarantine"@en ;
  skos:related agift:medical-quarantine-services ;
.
agift:radiation-protection
  rdf:type skos:Concept ;
  rdfs:label "Radiation protection"@en ;
  skos:broader agift:public-health-services ;
  skos:definition """Regulating the safe use of radioactive substances. Developing legislation and standards for keeping and using radioactive substances. Includes the sale, transfer, storage, possession, transport, installation, maintenance and remediation of regulated material.

See also INTERNATIONAL RELATIONS - International affairs - Nuclear safeguards: ensuring that nuclear material and associated equipment is fully accounted for and controlled.""" ;
  skos:prefLabel "Radiation protection"@en ;
  skos:related agift:nuclear-safeguards ;
.
agift:radio-broadcasting
  rdf:type skos:Concept ;
  rdfs:label "Radio broadcasting"@en ;
  skos:broader agift:broadcasting ;
  skos:definition """Supporting industries that transmit content as electromagnetic waves sent through the air to a receiver. Managing publicly owned radio stations and issuing commercial broadcasting licenses. Developing strategies to promote Australian radio programming. Providing radio broadcasting services locally, nationally and internationally. Negotiating retransmission arrangements.

See also COMMUNICATIONS - Broadcasting - Broadcasting standards: for regulating the accessibility of radio content.

See also COMMUNICATIONS - Radio communication: for licensing of radio transmitters.""" ;
  skos:hiddenLabel "Broadcasting licenses" ;
  skos:hiddenLabel "Commercial radio" ;
  skos:hiddenLabel "Wireless broadcasting" ;
  skos:prefLabel "Radio broadcasting"@en ;
  skos:related agift:broadcasting-standards ;
  skos:related agift:radio-communication ;
.
agift:radio-communication
  rdf:type skos:Concept ;
  rdfs:label "Radio communication"@en ;
  skos:broader agift:communications ;
  skos:definition """Developing policy to support and regulate the operation of wireless communications infrastructure. Maintaining a regulatory framework for the radio communications industry. Supporting market entry, enabling firms to acquire spectrum to introduce new technologies. Includes liaison across jurisdictions on radio communications issues.

See also COMMUNICATIONS - Broadcasting - Radio broadcasting: for regulating the transmission of content via radio.

See also COMMUNICATIONS - Telecommunications - Mobile telephone services: for wireless telecommunications.""" ;
  skos:hiddenLabel "Radio communications" ;
  skos:narrower agift:apparatus-licensing ;
  skos:narrower agift:spectrum-management ;
  skos:prefLabel "Radio communication"@en ;
  skos:related agift:radio-broadcasting ;
.
agift:rail-harmonisation-standards
  rdf:type skos:Concept ;
  rdfs:label "Rail harmonisation standards"@en ;
  skos:broader agift:rail-transport ;
  skos:definition "Developing a consistent approach to technical and operational railway practices across jurisdictions. Includes standards relating to locomotives, track gauge, signalling, control systems and emissions." ;
  skos:hiddenLabel "Locomotive standards" ;
  skos:hiddenLabel "Railway gauge standards" ;
  skos:prefLabel "Rail harmonisation standards"@en ;
.
agift:rail-land-acquisition-regulation
  rdf:type skos:Concept ;
  rdfs:label "Rail land acquisition regulation"@en ;
  skos:broader agift:rail-transport ;
  skos:definition "Developing policy and procedures for the purchase or possession of property to accommodate railway infrastructure. Regulating proposals and payments for compensation in relation to acquired land." ;
  skos:prefLabel "Rail land acquisition regulation"@en ;
.
agift:rail-transport
  rdf:type skos:Concept ;
  rdfs:label "Rail transport"@en ;
  skos:broader agift:transport ;
  skos:definition """Regulating the railway industry and developing policy relating to all aspects of the rail network system. Administering rail transport standards, security and services and licensing of rail transport operators. Includes liaison to promote coordination and consistency among rail authorities from different jurisdictions.

See also TRANSPORT - Freight movement regulation: for managing the transportation of goods by rail.

See also TRANSPORT - Passenger services: for managing the transportation of people by rail.""" ;
  skos:hiddenLabel "Railways" ;
  skos:hiddenLabel "Train travel" ;
  skos:narrower agift:rail-harmonisation-standards ;
  skos:narrower agift:rail-land-acquisition-regulation ;
  skos:narrower agift:rail-transport-safety ;
  skos:narrower agift:railway-maintenance ;
  skos:narrower agift:rolling-stock-regulation ;
  skos:prefLabel "Rail transport"@en ;
  skos:related agift:freight-movement-regulation ;
.
agift:rail-transport-safety
  rdf:type skos:Concept ;
  rdfs:label "Rail transport safety"@en ;
  skos:broader agift:rail-transport ;
  skos:definition """Regulating all railway activities to improve security, reducing the risk of accidents or emergencies and investigating accidents and incidents. Monitoring compliance with rail safety standards, signalling procedures and other regulations. Includes training and advice, consultation and inspection services and cooperation on railway safety issues across jurisdictions.

See also TRANSPORT - Rail transport - Railway maintenance: for preservation of train tracks and related infrastructure.

See also TRANSPORT - Rail transport - Rolling stock regulation: for train design, maintenance and operation standards.""" ;
  skos:hiddenLabel "Accident investigation" ;
  skos:hiddenLabel "Safety investigation" ;
  skos:prefLabel "Rail transport safety"@en ;
  skos:related agift:railway-maintenance ;
.
agift:railway-maintenance
  rdf:type skos:Concept ;
  rdfs:label "Railway maintenance"@en ;
  skos:broader agift:rail-transport ;
  skos:definition """Managing and preserving railway tracks and associated infrastructure. Ensuring that railway stations, crossings, signals, bridges and tunnels meet operating standards. Includes inspections, assessments and ongoing repair work.

See also CIVIC INFRASTRUCTURE - Transport infrastructure development: for designing and installing transport systems.

See also TRANSPORT - Rail transport - Rolling stock regulation: for maintenance of vehicles such as locomotives, trams and train carriages.""" ;
  skos:hiddenLabel "Railway crossings" ;
  skos:hiddenLabel "Railway lines" ;
  skos:hiddenLabel "Railway stations" ;
  skos:hiddenLabel "Railway tracks" ;
  skos:hiddenLabel "Train tracks" ;
  skos:hiddenLabel "Tram lines" ;
  skos:prefLabel "Railway maintenance"@en ;
  skos:related agift:rail-transport-safety ;
  skos:related agift:transport-infrastructure-development ;
.
agift:recordkeeping-standards
  rdf:type skos:Concept ;
  rdfs:label "Recordkeeping standards"@en ;
  skos:broader agift:administrative-law ;
  skos:definition """Regulating the creation, capture, management and disposal of government records. Monitoring compliance to ensure appropriate availability of authentic evidence of government or business activities.

See also BUSINESS SUPPORT AND REGULATION - Business process auditing: for examining the records or accounts of an organisation.

See also GOVERNANCE - Open government: facilitating citizen engagement in policy and service design and delivery. 

See also JUSTICE ADMINISTRATION - Administrative law - Freedom of information: providing a right of access to  government  documents.

See also JUSTICE ADMINISTRATION - Privacy: for ensuring the confidentiality of records containing personal information.""" ;
  skos:hiddenLabel "Archives" ;
  skos:hiddenLabel "Records management" ;
  skos:prefLabel "Recordkeeping standards"@en ;
  skos:related agift:business-process-auditing ;
.
agift:recreational-park-management
  rdf:type skos:Concept ;
  rdfs:label "Recreational park management"@en ;
  skos:broader agift:public-land-management ;
  skos:definition """Administering public leisure areas and playgrounds. Managing site layout and landscaping. Ensuring facilities are kept clean and maintained. Monitoring rights of access and opening hours.

See also CIVIC INFRASTRUCTURE - Public land management - Garden management: for administering public land where ornamental or useful plants are cultivated.

See also ENVIRONMENT - Natural heritage protection - National park management: for administering designated national park areas.

See also ENVIRONMENT - Natural heritage protection - Nature reserve management: for the maintenance of native flora and fauna reserves.

See also SPORT AND RECREATION - Park and reserve services: for administration of sporting grounds.""" ;
  skos:hiddenLabel "Park management" ;
  skos:hiddenLabel "Playground management" ;
  skos:hiddenLabel "Public leisure areas" ;
  skos:prefLabel "Recreational park management"@en ;
  skos:related agift:garden-management ;
  skos:related agift:sporting-facilities-management ;
.
agift:recruitment-programs
  rdf:type skos:Concept ;
  rdfs:label "Recruitment programs"@en ;
  skos:broader agift:human-resources-development ;
  skos:definition """Managing activities to engage staff and promote employment with the organisation. Developing selection documentation, conducting interviews and appointing new employees. Establishing procedures for advertising public sector vacancies or managing recruitment exercises in accordance with government policy.

See also DEFENCE - Defence force careers: for military recruitment programs.

See also EDUCATION AND TRAINING - Vocational education: for on-the-job training programs and traineeships.""" ;
  skos:prefLabel "Recruitment programs"@en ;
  skos:related agift:defence-force-careers ;
.
agift:reference-services
  rdf:type skos:Concept ;
  rdfs:label "Reference services"@en ;
  skos:broader agift:collection-access ;
  skos:definition """Providing personal or online assistance to help clients locate and use items held in cultural collections. Explaining access provisions and restrictions, and the procedures to view material. Includes research and referral services, mobile or special services for target community groups.

See also CULTURAL AFFAIRS - Collection access - Finding aids development: for creating tools to locate items in cultural collections.""" ;
  skos:hiddenLabel "Access services" ;
  skos:hiddenLabel "Client services" ;
  skos:hiddenLabel "Information services" ;
  skos:hiddenLabel "Reader services" ;
  skos:prefLabel "Reference services"@en ;
  skos:related agift:collection-access ;
  skos:related agift:finding-aids-development ;
.
agift:refuge-support
  rdf:type skos:Concept ;
  rdfs:label "Refuge support"@en ;
  skos:broader agift:accommodation-services ;
  skos:definition """Managing sheltered accommodation to provide assistance to members of the community at risk. Includes funding and services to support private facilities or refuges operated by non-government organisations.

See also HEALTH CARE - Special needs services - Residential services: for managing live-in nursing facilities.""" ;
  skos:prefLabel "Refuge support"@en ;
  skos:related agift:residential-services ;
.
agift:refugee-services
  rdf:type skos:Concept ;
  rdfs:label "Refugee services"@en ;
  skos:broader agift:immigration ;
  skos:definition """Providing assistance to asylum seekers and victims of human rights violations. Assessing applications for refugee status. Arranging health checks, counselling, community support and special services as required. Includes liaison with community groups and across jurisdictions to ensure appropriate support.

See also IMMIGRATION - Migrant services: for orientation and settlement programs.""" ;
  skos:hiddenLabel "Asylum seekers" ;
  skos:hiddenLabel "Exiles" ;
  skos:prefLabel "Refugee services"@en ;
  skos:related agift:human-rights-obligations ;
  skos:related agift:migrant-services ;
.
agift:regional-development
  rdf:type skos:Concept ;
  rdfs:label "Regional development"@en ;
  skos:broader agift:civic-infrastructure ;
  skos:definition """Managing infrastructure projects to support multiple districts, such as building schools or hospitals. Extending facilities beyond urban boundaries to supply services to remote or rural areas. Installing equipment to enable communications. 

See also CIVIC INFRASTRUCTURE - Infrastructure planning; providing advice on nationally-significant economic infrastructure to governments, investors and owners.

See also CIVIC INFRASTRUCTURE - Integrated services planning: for providing coordinated services across districts.

See also TRANSPORT - Transport infrastructure development: for designing and building transport systems.""" ;
  skos:hiddenLabel "Territories" ;
  skos:prefLabel "Regional development"@en ;
  skos:related agift:infrastructure-planning ;
  skos:related agift:rural-community-development ;
.
agift:remuneration-review
  rdf:type skos:Concept ;
  rdfs:label "Remuneration review"@en ;
  skos:broader agift:industrial-awards-and-conditions ;
  skos:definition "Monitoring the salary levels and employment conditions of specified public sector and statutory appointees. Evaluating remuneration against market rates for equivalent positions. Making recommendations for the review of salary, allowances, leave or entitlements." ;
  skos:hiddenLabel "Statutory appointees" ;
  skos:prefLabel "Remuneration review"@en ;
.
agift:renewable-energy-development
  rdf:type skos:Concept ;
  rdfs:label "Renewable energy development"@en ;
  skos:broader agift:energy-resources ;
  skos:definition """Promoting the development and use of renewable energy resources. Licensing infrastructure and operational activities. Supporting industry partnerships and collaboration between research institutions. Providing assistance to commercialise research and development in renewable energy technologies.

See also NATURAL RESOURCES - Water resources - Water usage management: for policy and approvals relating to water-related energy facilities.

See also SCIENCE: for conducting research into the use and development of energy resources.""" ;
  skos:hiddenLabel "Alternative energy" ;
  skos:hiddenLabel "Clean energy" ;
  skos:hiddenLabel "Geothermal energy" ;
  skos:hiddenLabel "Hydroelectric power" ;
  skos:hiddenLabel "Hydroelectricity" ;
  skos:hiddenLabel "Solar energy" ;
  skos:hiddenLabel "Tidal energy" ;
  skos:hiddenLabel "Wind farms" ;
  skos:prefLabel "Renewable energy development"@en ;
  skos:related agift:water-usage-management ;
.
agift:rescue-coordination
  rdf:type skos:Concept ;
  rdfs:label "Rescue coordination"@en ;
  skos:broader agift:search-and-rescue ;
  skos:definition """Directing and controlling operations to locate individuals, vessels or aircraft lost at sea and return them to safety. Providing specially equipped vehicles and trained personnel. Includes liaison with community-based services, or across jurisdictions. 

See also COMMUNITY SERVICES - Emergency services: for land-based search and rescue operations outside urban areas.

See also COMMUNITY SERVICES - Emergency services - Firefighting services: for urban search and rescue operations.""" ;
  skos:prefLabel "Rescue coordination"@en ;
  skos:related agift:emergency-services ;
.
agift:reserves
  rdf:type skos:Concept ;
  rdfs:label "Reserves"@en ;
  skos:broader agift:australian-defence-forces ;
  skos:definition """Managing Australia's part-time defence units. Developing policy and programs for recruitment, training and deployment of Army, Navy or Air Force Reserves. Coordinating activities to provide support to permanent forces during peacetime and conflict.

See also EDUCATION AND TRAINING - Military education and training - Army reserve training: for educational programs for Army Reservists.""" ;
  skos:prefLabel "Reserves"@en ;
  skos:related agift:air-force ;
  skos:related agift:army ;
  skos:related agift:army-reserve-training ;
  skos:related agift:navy ;
.
agift:residential-services
  rdf:type skos:Concept ;
  rdfs:label "Residential services"@en ;
  skos:broader agift:special-needs-services ;
  skos:definition """Administering programs that provide care and accommodation for aged or disabled persons, or those suffering from disease or mental illness. Providing trained personnel to attend residents. Managing staff and facilities. Monitoring the activities of private residential care providers.

See also COMMUNITY SERVICES - Accommodation services - Refuge support: for sheltered emergency accommodation.

See also COMMUNITY SERVICES - Counselling services: for the provision of group therapy or psychological advice.

See also HEALTH CARE - Special needs services - Independent living services: for providing in-home assistance or supervising 'half-way' houses.""" ;
  skos:hiddenLabel "Aged care facilities" ;
  skos:hiddenLabel "Asylums" ;
  skos:hiddenLabel "Disability care facilities" ;
  skos:hiddenLabel "Homes" ;
  skos:hiddenLabel "Hospices" ;
  skos:hiddenLabel "Hostels" ;
  skos:hiddenLabel "Nursing homes" ;
  skos:hiddenLabel "Old people's homes" ;
  skos:hiddenLabel "Retirement villages" ;
  skos:prefLabel "Residential services"@en ;
  skos:related agift:refuge-support ;
.
agift:resource-management
  rdf:type skos:Concept ;
  rdfs:label "Resource management"@en ;
  skos:broader agift:finance-management ;
  skos:definition "Developing policy for the management of financial and other government assets. Providing advice on legislative responsibilities and reporting requirements. Supporting accountable use and management of government resources." ;
  skos:narrower agift:contract-management ;
  skos:narrower agift:financial-administration ;
  skos:narrower agift:financial-budgeting ;
  skos:narrower agift:productivity ;
  skos:prefLabel "Resource management"@en ;
.
agift:retail-postal-services
  rdf:type skos:Concept ;
  rdfs:label "Retail postal services"@en ;
  skos:broader agift:postal-services ;
  skos:definition "Administering general services to collect and deliver letters, parcels and other mail. Coordinating routes and schedules for postal delivery. Managing post offices and other retail outlets providing mail products and services." ;
  skos:hiddenLabel "General post offices" ;
  skos:hiddenLabel "Post offices" ;
  skos:prefLabel "Retail postal services"@en ;
.
agift:retirement-income
  rdf:type skos:Concept ;
  rdfs:label "Retirement income"@en ;
  skos:broader agift:finance-management ;
  skos:definition "Formulating policy to safeguard the savings of individuals who have left the workforce. Setting criteria to evaluate a retiree's assets, for tax or benefit purposes. Developing standards for the operation of superannuation funds. Implementing mechanisms to support retirement saving by individuals." ;
  skos:hiddenLabel "Part-pension retirees" ;
  skos:hiddenLabel "Retirees" ;
  skos:hiddenLabel "Self-funded retirees" ;
  skos:narrower agift:asset-assessment ;
  skos:narrower agift:retirement-saving ;
  skos:narrower agift:superannuation-regulation ;
  skos:prefLabel "Retirement income"@en ;
.
agift:retirement-saving
  rdf:type skos:Concept ;
  rdfs:label "Retirement saving"@en ;
  skos:broader agift:retirement-income ;
  skos:definition """Encouraging individuals to set aside funds to support themselves after they leave the work force. Administering programs to support and regulate retirement saving. Developing incentives for the ongoing management of retirement savings. Includes advice to employers, employees and self-employed individuals.

See also FINANCE MANAGEMENT - Retirement income - Superannuation regulation: for monitoring the activities of superannuation funds.""" ;
  skos:hiddenLabel "Savings bonus" ;
  skos:hiddenLabel "Superannuation guarantee" ;
  skos:prefLabel "Retirement saving"@en ;
  skos:related agift:superannuation-regulation ;
.
agift:revenue-raising
  rdf:type skos:Concept ;
  rdfs:label "Revenue raising"@en ;
  skos:broader agift:taxation ;
  skos:definition """Developing mechanisms to support the collection of taxes from individuals and organisations. Includes deductions at point of sale, services for making payments or having sums withheld from earnings.

See also FINANCE MANAGEMENT - Taxation - Taxation compliance: for managing payments made by individuals through withholding schemes.

See also JUSTICE ADMINISTRATION - Local laws and ordinances: for setting rates.""" ;
  skos:hiddenLabel "BAS" ;
  skos:hiddenLabel "Business Activity Statements" ;
  skos:hiddenLabel "Departure tax" ;
  skos:hiddenLabel "Excise" ;
  skos:hiddenLabel "Fines" ;
  skos:hiddenLabel "Government charges" ;
  skos:hiddenLabel "PAYG instalments" ;
  skos:hiddenLabel "PAYG withholding" ;
  skos:hiddenLabel "Pay As You Go taxation" ;
  skos:hiddenLabel "Payments to government" ;
  skos:hiddenLabel "Stamp Duty" ;
  skos:hiddenLabel "Tolls" ;
  skos:hiddenLabel "Withholding schemes" ;
  skos:prefLabel "Revenue raising"@en ;
  skos:related agift:taxation-compliance ;
.
agift:road-safety-awareness
  rdf:type skos:Concept ;
  rdfs:label "Road safety awareness"@en ;
  skos:broader agift:community-education ;
  skos:definition """Administering training designed to educate the community about the importance of road safety. Includes traffic training centres, driving instruction, school visits and campaigns to illustrate the consequences of dangerous behaviour.

See also SECURITY - Law enforcement: for policing road safety regulations.""" ;
  skos:hiddenLabel "Driver training" ;
  skos:hiddenLabel "Traffic training school" ;
  skos:prefLabel "Road safety awareness"@en ;
  skos:related agift:driving-licences-administration ;
  skos:related agift:law-enforcement ;
  skos:related agift:road-transport-safety ;
.
agift:road-surface-maintenance
  rdf:type skos:Concept ;
  rdfs:label "Road surface maintenance"@en ;
  skos:broader agift:road-transport ;
  skos:definition """Managing and preserving road surfaces and associated infrastructure. Ensuring traffic lights, road markings and signage meet legislative requirements. Includes inspections, assessments and ongoing repair work.

See also CIVIC INFRASTRUCTURE - Transport infrastructure development: for designing and installing transport systems.""" ;
  skos:hiddenLabel "Roads" ;
  skos:prefLabel "Road surface maintenance"@en ;
  skos:related agift:transport-infrastructure-development ;
.
agift:road-traffic-regulation
  rdf:type skos:Concept ;
  rdfs:label "Road traffic regulation"@en ;
  skos:broader agift:road-transport ;
  skos:definition """Developing and implementing regulations for all road users - such as motor vehicle drivers, cyclists and pedestrians. Determining appropriate speed limits, signage and road markings, identifying the need for traffic lights, facilities for parking, pedestrians and cyclists. Includes developing and maintaining the traffic code for interaction and behaviour of all road users.

See also TRANSPORT - Road transport - Driving licenses administration: for certification of motor vehicle operators.

See also TRANSPORT - Road transport - Road surface maintenance: for repair and preservation of traffic lights, road markings and other traffic regulation indicators.

See also TRANSPORT - Road transport - Road transport safety: for regulations to reduce the risk of accidents.

See also TRANSPORT - Road transport - Vehicle registration: for identification of motor vehicles and their legal owners.

See also TRANSPORT - Road transport - Vehicle standards: for certificates of roadworthiness.""" ;
  skos:prefLabel "Road traffic regulation"@en ;
  skos:related agift:driving-licences-administration ;
.
agift:road-transport
  rdf:type skos:Concept ;
  rdfs:label "Road transport"@en ;
  skos:broader agift:transport ;
  skos:definition "Developing policy relating to all aspects of private or commercial road usage. Administering road transport standards, security and services. Includes liaison across jurisdictions to provide uniform road regulations and enforcement practices." ;
  skos:narrower agift:driving-licences-administration ;
  skos:narrower agift:road-surface-maintenance ;
  skos:narrower agift:road-traffic-regulation ;
  skos:narrower agift:road-transport-safety ;
  skos:narrower agift:vehicle-registration ;
  skos:narrower agift:vehicle-standards ;
  skos:prefLabel "Road transport"@en ;
.
agift:road-transport-safety
  rdf:type skos:Concept ;
  rdfs:label "Road transport safety"@en ;
  skos:broader agift:road-transport ;
  skos:definition """Regulating all road-use activities to improve security and reduce the risk of accidents or emergencies. Investigating accidents and incidents. Monitoring compliance with safety standards in the road transport industry. Developing standards for driver fitness, such as limits for alcohol consumption or driving hours. Encouraging the use of helmets or pedestrian crossings. Promoting road safety through programs targeting driver health and on-road behaviour. Includes training and advice, consultation and inspection services and cooperation across jurisdictions on road safety issues.

See also EDUCATION AND TRAINING - Community education - Road safety awareness: for community programs to educate road users.

See also SECURITY - Law enforcement: for policing road safety regulations.

See also TRANSPORT - Freight movement regulation: for managing the safe transportation of goods by road.

See also TRANSPORT - Passenger services: for managing the safe transportation of people by road.

See also TRANSPORT - Road transport - Driving licenses administration: for certifying driver ability and issuing penalties for road safety infringements.

See also TRANSPORT - Road transport - Vehicle standards: for maintaining the safety of motor vehicles.""" ;
  skos:hiddenLabel "Accident investigation" ;
  skos:hiddenLabel "Road safety" ;
  skos:hiddenLabel "Safety investigation" ;
  skos:prefLabel "Road transport safety"@en ;
  skos:related agift:road-safety-awareness ;
.
agift:rolling-stock-regulation
  rdf:type skos:Concept ;
  rdfs:label "Rolling stock regulation"@en ;
  skos:broader agift:rail-transport ;
  skos:definition "Developing policy to support the design, construction, maintenance and operation of any vehicle operating on a railway track - such as locomotives, carriages, rail cars, rail motors, light rail vehicles, trains, trams or wagons. Ensuring rolling stock conform to operational standards. Conducting inspections, testing and licensing. Includes certification of engine drivers, railway engineers and other personnel engaged in the use or maintenance of rolling stock." ;
  skos:hiddenLabel "Coupling standards" ;
  skos:hiddenLabel "Engine drivers" ;
  skos:hiddenLabel "Locomotives" ;
  skos:hiddenLabel "Rail motors" ;
  skos:hiddenLabel "Train drivers" ;
  skos:hiddenLabel "Trains" ;
  skos:hiddenLabel "Trams" ;
  skos:prefLabel "Rolling stock regulation"@en ;
.
agift:rural-community-development
  rdf:type skos:Concept ;
  rdfs:label "Rural community development"@en ;
  skos:broader agift:community-services ;
  skos:definition """Supporting outback and country communities through targeted services and programs to develop self-reliance. Establishing social networks and activities. Providing funding and support for community-based or volunteer organisations. Includes activities to improve rural access to government services and liaising with local business to support community projects.

See also CIVIC INFRASTRUCTURE - Regional development: for infrastructure projects in rural areas.

See also INDIGENOUS AFFAIRS - Indigenous welfare programs: for social support to Aboriginal and Torres Strait Islander communities.

See also PRIMARY INDUSTRIES - Rural partnership programs: for business and industry support services.""" ;
  skos:hiddenLabel "Community development" ;
  skos:prefLabel "Rural community development"@en ;
  skos:related agift:community-support ;
  skos:related agift:regional-development ;
  skos:related agift:rural-partnership-programs ;
.
agift:rural-field-day-promotion
  rdf:type skos:Concept ;
  rdfs:label "Rural field day promotion"@en ;
  skos:broader agift:primary-industries ;
  skos:definition "Developing programs to support shows, exhibitions and conferences to encourage agricultural innovation. Includes financial assistance and advice on planning and marketing strategies." ;
  skos:hiddenLabel "Agricultural shows" ;
  skos:prefLabel "Rural field day promotion"@en ;
.
agift:rural-partnership-programs
  rdf:type skos:Concept ;
  rdfs:label "Rural partnership programs"@en ;
  skos:broader agift:primary-industries ;
  skos:definition """Initiating cooperative projects to support change in the operation of primary industries and agricultural business ventures. Developing strategies to help rural enterprises and communities adjust to changing commercial conditions, to improve profitability and competitiveness. Providing advice, training and project funding assistance.

See also COMMUNITY SERVICES - Rural community development: for social support services to country districts.

See also PRIMARY INDUSTRIES - Marine and rural support: for programs to grow and develop specific industries.""" ;
  skos:hiddenLabel "Agricultural Development Partnership Program" ;
  skos:prefLabel "Rural partnership programs"@en ;
  skos:related agift:rural-community-development ;
.
agift:satellite-communication
  rdf:type skos:Concept ;
  rdfs:label "Satellite communication"@en ;
  skos:broader agift:communications ;
  skos:definition """Developing policy to support and regulate industries that relay radio and television signals via equipment located in space. Managing government-owned satellite equipment. Providing advice on the introduction of new technology and the effects of government policy on the satellite communication industry. Includes liaison with international bodies on shared access to satellite equipment.

See also MARITIME SERVICES - Navigation - Navigation systems development: for the use of satellites in plotting courses at sea.

See also MARITIME SERVICES - Search and rescue - Search technology development: for the use of satellites in locating individuals, vessels or aircraft that become lost at sea.

See also SCIENCE - Physical sciences - Astronomical sciences: for the use of satellites in space research.

See also SCIENCE - Spatial information research: for the use of satellites in global positioning research.""" ;
  skos:hiddenLabel "Satellites" ;
  skos:prefLabel "Satellite communication"@en ;
  skos:related agift:astronomical-sciences ;
  skos:related agift:navigation-systems-development ;
.
agift:scheme2014
  rdf:type skos:ConceptScheme ;
  dc:rights """This work is copyright. It may be adapted or reproduced for personal, in-house or non-commercial use without formal permission subject to appropriate citation. The work may not be used for other purposes – apart from any use as permitted under the Copyright Act 1968 – without prior written permission from the National Archives of Australia. Requests and inquiries concerning reproduction and rights should be sent to the Agency Service Centre.

This publication should be cited as: National Archives of Australia, Australian Governments’ Interactive Functions Thesaurus, 3rd Edition, November 2014."""^^xsd:string ;
  rdfs:comment """The Australian Governments’ Interactive Functions Thesaurus (AGIFT) is a three-level hierarchical thesaurus that describes the business functions carried out across Commonwealth, state and local governments in Australia.

It contains 25 high-level functions, each with second and third level terms, as well as non-preferred terms and related terms. Its main purpose is to describe web-based resources to aid online discovery of government information and services.

Terms can be searched by function, alphabetically and via full-text searching.

In the thesaurus you will find:

Function – the broadest unit of business performed by Australian Governments' Interactive Functions Thesaurus
Level 2 – major tasks or areas of service undertaken within each function
Level 3 – topics being addressed within function/activities
For each term, the thesaurus shows:
Scope Notes – notes that provide guidance on the use of a term
Broader Terms – terms at a higher level
Narrower Terms – terms at a lower level
Related Terms – terms at the same level
Use – approved terms used to identify and save documents
Non-preferred Term – other terms, not to be used to identify and save documents"""^^xsd:string ;
  rdfs:label "Australian Governments' Interactive Functions Thesaurus (AGIFT)"^^xsd:string ;
  skos:hasTopConcept agift:business-support-and-regulation ;
  skos:hasTopConcept agift:civic-infrastructure ;
  skos:hasTopConcept agift:communications ;
  skos:hasTopConcept agift:community-services ;
  skos:hasTopConcept agift:cultural-affairs ;
  skos:hasTopConcept agift:defence ;
  skos:hasTopConcept agift:education-and-training ;
  skos:hasTopConcept agift:employment ;
  skos:hasTopConcept agift:environment ;
  skos:hasTopConcept agift:finance-management ;
  skos:hasTopConcept agift:governance ;
  skos:hasTopConcept agift:health-care ;
  skos:hasTopConcept agift:immigration ;
  skos:hasTopConcept agift:indigenous-affairs ;
  skos:hasTopConcept agift:international-relations ;
  skos:hasTopConcept agift:justice-administration ;
  skos:hasTopConcept agift:maritime-services ;
  skos:hasTopConcept agift:natural-resources ;
  skos:hasTopConcept agift:primary-industries ;
  skos:hasTopConcept agift:science ;
  skos:hasTopConcept agift:security ;
  skos:hasTopConcept agift:sport-and-recreation ;
  skos:hasTopConcept agift:statistical-services ;
  skos:hasTopConcept agift:tourism ;
  skos:hasTopConcept agift:trade ;
  skos:hasTopConcept agift:transport ;
  skos:prefLabel "Australian Governments' Interactive Functions Thesaurus (AGIFT)"@en ;
.
agift:school-education
  rdf:type skos:Concept ;
  rdfs:label "School education"@en ;
  skos:broader agift:education-and-training ;
  skos:definition """Administering programs that offer instruction to children, to impart knowledge and develop skills. Providing public school education for children in Years 1 to 12. Monitoring and regulating non-government schools. Managing school facilities. Implementing standards and guidelines to support teachers. Includes the provision of scholarships and study grants.

See also EDUCATION AND TRAINING - Arts education: for programs to further artistic talent at individual or community level.

See also EDUCATION AND TRAINING - Curriculum development: for researching and drafting outline study programs.

See also EDUCATION AND TRAINING - Early childhood education: for teaching children under the age of five years.

See also INTERNATIONAL RELATIONS - Overseas aid programs - Overseas student scholarship programs: for access to higher education for students from developing countries or the Pacific region.""" ;
  skos:hiddenLabel "Health education" ;
  skos:hiddenLabel "Primary schools" ;
  skos:hiddenLabel "Private school regulation" ;
  skos:hiddenLabel "Secondary schools" ;
  skos:hiddenLabel "Sex education" ;
  skos:hiddenLabel "State schools" ;
  skos:narrower agift:discipline-programs ;
  skos:narrower agift:school-transport-regulation ;
  skos:narrower agift:special-needs-programs ;
  skos:prefLabel "School education"@en ;
  skos:related agift:arts-education ;
.
agift:school-transport-regulation
  rdf:type skos:Concept ;
  rdfs:label "School transport regulation"@en ;
  skos:broader agift:school-education ;
  skos:definition """Designing services to help children travel to and from school. Developing standards and guidelines to assist bus drivers or children with special needs. Identifying requirements for bus stops, cycle routes, footpaths, crossings and low speed limits. Liaising with government and non-government organisations to implement and regulate school transport services.

See also CIVIC INFRASTRUCTURE - Transport network maintenance: for managing school transport services.

See also COMMUNITY SERVICES - Transport access schemes: for programs to make services available to targeted community groups.

See also EDUCATION AND TRAINING - Community education - Road safety awareness: for setting low speed limits in school zones.

See also TRANSPORT - Passenger services: for timetables, route maps and ticketing.""" ;
  skos:hiddenLabel "School bus services" ;
  skos:prefLabel "School transport regulation"@en ;
  skos:related agift:transport-network-maintenance ;
.
agift:science
  rdf:type skos:Concept ;
  rdfs:label "SCIENCE"@en ;
  skos:definition "Developing policy and standards to support research and systematic studies. Administering scientific bodies and monitoring industry research and development programs. Providing funding and implementing promotional strategies. Includes research into living things and their environments, natural laws and the application of knowledge to practical problems." ;
  skos:hiddenLabel "Research" ;
  skos:narrower agift:agricultural-sciences ;
  skos:narrower agift:animal-and-veterinary-sciences ;
  skos:narrower agift:applied-sciences ;
  skos:narrower agift:biological-sciences ;
  skos:narrower agift:earth-sciences ;
  skos:narrower agift:ethical-compliance ;
  skos:narrower agift:mathematical-sciences ;
  skos:narrower agift:medical-and-health-sciences ;
  skos:narrower agift:physical-sciences ;
  skos:narrower agift:spatial-information-research ;
  skos:prefLabel "SCIENCE"@en ;
.
agift:sea-passengers
  rdf:type skos:Concept ;
  rdfs:label "Sea passengers"@en ;
  skos:broader agift:maritime-services ;
  skos:definition """Developing policy for the transportation of people by sea. Monitoring compliance with pricing regulations or the provision of appropriate facilities for passenger convenience. Includes services such as timetables, route maps or ticketing.

See also TRANSPORT - Passenger services: for transportation of people by road, rail or air.""" ;
  skos:prefLabel "Sea passengers"@en ;
  skos:related agift:passenger-services ;
.
agift:search-and-rescue
  rdf:type skos:Concept ;
  rdfs:label "Search and rescue"@en ;
  skos:broader agift:maritime-services ;
  skos:definition """Developing policy and providing resources to ensure the safety of individuals, vessels or aircraft that become lost at sea. Managing reporting systems. Monitoring compliance with equipment standards and response requirements. Includes support for community-based services and regulating the use of volunteers and coordinating maritime emergency services.

See also COMMUNITY SERVICES - Natural disasters: for emergencies caused by the elements such as floods, earthquakes, and cyclones.

See also DEFENCE - Emergency management: for cross-jurisdictional operations to deal with large-scale emergencies.

See also DEFENCE - Emergency management - Civil community assistance: for defence forces support in search and rescue operations.""" ;
  skos:hiddenLabel "Coastguard" ;
  skos:narrower agift:rescue-coordination ;
  skos:narrower agift:search-technology-development ;
  skos:prefLabel "Search and rescue"@en ;
  skos:related agift:natural-disasters ;
.
agift:search-technology-development
  rdf:type skos:Concept ;
  rdfs:label "Search technology development"@en ;
  skos:broader agift:search-and-rescue ;
  skos:definition """Conducting research into the application of specialist knowledge and equipment to assist marine rescue operations. Developing communications systems to help locate individuals, vessels or aircraft lost at sea. Providing technical advice on the purchase of search equipment. Includes designing, testing and overseeing the manufacture of new products.

See also COMMUNICATIONS: for industry regulations and standards.

See also MARITIME SERVICES - Navigation - Navigation systems development: for investigating the use of technology to plot courses at sea.

See also SCIENCE - Spatial information research: for investigating practical applications for geographical data.""" ;
  skos:prefLabel "Search technology development"@en ;
  skos:related agift:communications ;
.
agift:seaworthiness
  rdf:type skos:Concept ;
  rdfs:label "Seaworthiness"@en ;
  skos:broader agift:ship-safety ;
  skos:definition """Certifying private or commercial marine vessels as fit for use at sea. Assessing applications to ensure compliance with standards and inspection requirements. Providing training and advice on safety requirements.

See also MARITIME SERVICES - Ship safety - Ship inspection: for assessing the seaworthiness of vessels.""" ;
  skos:hiddenLabel "Unseaworthiness" ;
  skos:prefLabel "Seaworthiness"@en ;
  skos:related agift:ship-inspection ;
.
agift:security
  rdf:type skos:Concept ;
  rdfs:label "SECURITY"@en ;
  skos:definition """Maintaining the safety of Australia at all levels of society. Developing policy and programs to guard against internal or external threats to peace and stability. Providing funding for law enforcement, community protection and corrective services. Coordinating intelligence gathering and international security activities.

See also DEFENCE: for protection using military resources.""" ;
  skos:narrower agift:corrective-services ;
  skos:narrower agift:external-security ;
  skos:narrower agift:information-security ;
  skos:narrower agift:intelligence ;
  skos:narrower agift:law-enforcement ;
  skos:narrower agift:national-security ;
  skos:prefLabel "SECURITY"@en ;
  skos:related agift:defence ;
  skos:related agift:justice-administration ;
.
agift:seismology
  rdf:type skos:Concept ;
  rdfs:label "Seismology"@en ;
  skos:broader agift:earth-sciences ;
  skos:definition "Conducting research into earthquakes. Monitoring and recording seismic surface waves, quarry blasts and mining activities, and data mapping of tectonic plate structures. Providing scientific advice on hazard management. Includes asset vulnerability assessment and emergency simulation and training, to deal with seismic events and their effects." ;
  skos:hiddenLabel "Earthquake studies" ;
  skos:hiddenLabel "Seismography" ;
  skos:prefLabel "Seismology"@en ;
.
agift:ship-commissioning
  rdf:type skos:Concept ;
  rdfs:label "Ship commissioning"@en ;
  skos:broader agift:ship-safety ;
  skos:definition """Transferring commercial and private marine vessels into or out of active service. Includes ship building activities and supply of captain and crew.

See also DEFENCE - Australian Defence Forces - Navy: for commissioning vessels in the Australian Defence Forces.

See also MARITIME SERVICES - Ship safety - Seaworthiness: for certifying ship safety and construction.""" ;
  skos:hiddenLabel "Decommissioning" ;
  skos:hiddenLabel "Shipbuilding" ;
  skos:prefLabel "Ship commissioning"@en ;
  skos:related agift:navy ;
.
agift:ship-inspection
  rdf:type skos:Concept ;
  rdfs:label "Ship inspection"@en ;
  skos:broader agift:ship-safety ;
  skos:definition """Monitoring compliance with standards and guidelines for the design, construction and maintenance of private or commercial marine vessels. Conducting inspections of structural integrity, safety equipment or emissions. Examining foreign flagships in Australian ports to monitor compliance with international regulations.

See also MARITIME SERVICES - Ship safety - Seaworthiness: for certifying ship safety and construction.""" ;
  skos:prefLabel "Ship inspection"@en ;
  skos:related agift:seaworthiness ;
.
agift:ship-personnel
  rdf:type skos:Concept ;
  rdfs:label "Ship personnel"@en ;
  skos:broader agift:maritime-services ;
  skos:definition """Regulating the operation of private or commercial marine vessels to improve security and reduce the risk of accidents or emergencies. Developing standards and guidelines for operational practices and crew competencies. Includes cooperation on maritime personnel safety across jurisdictions.

See also DEFENCE - Australian Defence Forces - Navy: for ship personnel in the Australian Defence Forces.

See also MARITIME SERVICES - Sea passengers: for services to travellers on ships.

See also MARITIME SERVICES - Ship safety: for investigating incidents or accidents.""" ;
  skos:hiddenLabel "Crew" ;
  skos:hiddenLabel "Maritime personnel" ;
  skos:hiddenLabel "Ship captains" ;
  skos:narrower agift:personnel-safety-standards ;
  skos:prefLabel "Ship personnel"@en ;
  skos:related agift:navy ;
  skos:related agift:ship-safety ;
.
agift:ship-safety
  rdf:type skos:Concept ;
  rdfs:label "Ship safety"@en ;
  skos:broader agift:maritime-services ;
  skos:definition """Regulating the design, construction and maintenance of private or commercial marine vessels. Developing standards and guidelines for safety equipment, seaworthiness, noise or emissions. Investigating the circumstances and causes of marine accidents. Promoting safety awareness across the maritime industry.

See also MARITIME SERVICES - Ship personnel: for regulating the operation of marine vessels.""" ;
  skos:hiddenLabel "Accident investigation" ;
  skos:hiddenLabel "Boat safety" ;
  skos:hiddenLabel "Marine safety" ;
  skos:hiddenLabel "Safety investigation" ;
  skos:hiddenLabel "Sea safety" ;
  skos:hiddenLabel "Shipbuilding standards" ;
  skos:narrower agift:seaworthiness ;
  skos:narrower agift:ship-commissioning ;
  skos:narrower agift:ship-inspection ;
  skos:prefLabel "Ship safety"@en ;
  skos:related agift:ship-personnel ;
.
agift:silvicultural-industry
  rdf:type skos:Concept ;
  rdfs:label "Silvicultural industry"@en ;
  skos:broader agift:marine-and-rural-support ;
  skos:definition """Administering programs to support commercial cultivation of forests. Assisting industry growth and development. Encouraging businesses to adopt innovative practices, processes and products. Providing advice on growing or harvesting methods and business management to improve competitiveness.

See also PRIMARY INDUSTRIES - Marine and rural regulation - Forestry industry: for monitoring and regulating timber industries.

See also SCIENCE - Agricultural science: for conducting research into timber growing and forestry products.""" ;
  skos:hiddenLabel "Forest support" ;
  skos:hiddenLabel "National Forestry Inventory" ;
  skos:hiddenLabel "Plantation management support" ;
  skos:prefLabel "Silvicultural industry"@en ;
  skos:related agift:botany ;
  skos:related agift:forestry-industry ;
.
agift:small-business-advocacy
  rdf:type skos:Concept ;
  rdfs:label "Small business advocacy"@en ;
  skos:broader agift:small-business-services ;
  skos:definition "Administering programs to support the interests of commercial enterprises of limited size or capital. Promoting the establishment of small businesses. Providing advice on the impact of government policy on small business. Includes liaison with industry groups and small business representatives." ;
  skos:prefLabel "Small business advocacy"@en ;
  skos:related agift:industry-assistance-schemes ;
.
agift:small-business-development
  rdf:type skos:Concept ;
  rdfs:label "Small business development"@en ;
  skos:broader agift:small-business-services ;
  skos:definition "Administering programs to encourage the growth of commercial enterprises of limited size or capital. Identifying markets or investment opportunities for small business. Developing quality assurance systems and reporting requirements appropriate to the scale of operations. Allocating grants or incentives for new initiatives." ;
  skos:prefLabel "Small business development"@en ;
  skos:related agift:industry-development ;
.
agift:small-business-services
  rdf:type skos:Concept ;
  rdfs:label "Small business services"@en ;
  skos:broader agift:business-support-and-regulation ;
  skos:definition "Developing policy and programs to assist commercial enterprises of limited size or capital. Providing advisory services to support the start-up and ongoing operation of small businesses. Encouraging the adoption of innovative practices, processes and products. Includes the establishment of communication networks or resource centres." ;
  skos:narrower agift:small-business-advocacy ;
  skos:narrower agift:small-business-development ;
  skos:prefLabel "Small business services"@en ;
.
agift:social-club-support
  rdf:type skos:Concept ;
  rdfs:label "Social club support"@en ;
  skos:broader agift:community-recreational-programs ;
  skos:definition "Providing financial assistance and services for community-based and non-profit organisations that promote friendship and recreation. Raising awareness of local groups though sponsorship, advertising and facilitating links between organisations." ;
  skos:hiddenLabel "Non-profit organisations support" ;
  skos:prefLabel "Social club support"@en ;
.
agift:social-justice-and-equity
  rdf:type skos:Concept ;
  rdfs:label "Social justice and equity"@en ;
  skos:broader agift:community-services ;
  skos:definition """Developing policy to support the fair treatment of all people, regardless of gender, race, colour, ethnicity, age, marital or parental status, sexual preference, disability or religious belief. Ensuring that government services are implemented with fairness and sensitivity to community needs. Reviewing services and making recommendations to improve access. Promoting equal opportunity and anti-discrimination principles. Includes liaison with target groups to evaluate the effectiveness of equity programs.

See also EMPLOYMENT - Human resources development - Workplace equity and justice programs: for ensuring equal employment opportunities.""" ;
  skos:hiddenLabel "Affirmative action" ;
  skos:hiddenLabel "Age discrimination" ;
  skos:hiddenLabel "Anti-discrimination programs" ;
  skos:hiddenLabel "Anti-discrimination" ;
  skos:hiddenLabel "Community access programs" ;
  skos:hiddenLabel "Cultural diversity programs" ;
  skos:hiddenLabel "Disability rights" ;
  skos:hiddenLabel "Discrimination" ;
  skos:hiddenLabel "Equal opportunity programs" ;
  skos:hiddenLabel "Equity programs" ;
  skos:hiddenLabel "Gender discrimination" ;
  skos:hiddenLabel "Inclusion" ;
  skos:hiddenLabel "Racial discrimination" ;
  skos:hiddenLabel "Religious discrimination" ;
  skos:hiddenLabel "Sex discrimination" ;
  skos:hiddenLabel "Status of women" ;
  skos:hiddenLabel "Welfare complaint services" ;
  skos:prefLabel "Social justice and equity"@en ;
  skos:related agift:indigenous-advocacy ;
  skos:related agift:workplace-discrimination-monitoring ;
  skos:related agift:workplace-equity-and-justice-programs ;
.
agift:social-media
  rdf:type skos:Concept ;
  rdfs:label "Social media"@en ;
  skos:broader agift:internet ;
  skos:definition """Developing policy and programs to enable governments to  consult widely with citizens via social media platforms. 
See also COMMUNICATIONS - Government media: for managing media releases and dealing with journalists.
See also COMMUNITY SERVICES - Community engagement: Governments inviting the commmunity to participate in community consultations.""" ;
  skos:prefLabel "Social media"@en ;
.
agift:social-research
  rdf:type skos:Concept ;
  rdfs:label "Social research"@en ;
  skos:broader agift:community-services ;
  skos:definition "Developing research programs to examine Australians'  attitudes, beliefs, trends, stratifications and rules." ;
  skos:hiddenLabel "Family research" ;
  skos:prefLabel "Social research"@en ;
.
agift:soil-preservation-programs
  rdf:type skos:Concept ;
  rdfs:label "Soil preservation programs"@en ;
  skos:broader agift:conservation-programs ;
  skos:definition """Managing programs to prevent or repair damage to the ground or earth. Restoring specific areas to their native state or preventing further degradation. Conducting activities to counteract soil erosion or chemical contamination. Includes funding for joint projects with local business or community groups.

See also NATURAL RESOURCES - Mineral resources - Land rehabilitation programs: for restoring areas damaged by mineral excavation and extraction.

See also NATURAL RESOURCES - Water resources - Waterway management: for strategies for salinity management and river care programs.""" ;
  skos:hiddenLabel "Beach stabilisation programs" ;
  skos:hiddenLabel "Erosion prevention programs" ;
  skos:hiddenLabel "Sustainable agriculture" ;
  skos:prefLabel "Soil preservation programs"@en ;
  skos:related agift:agricultural-sciences ;
  skos:related agift:land-rehabilitation-programs ;
.
agift:spatial-information-research
  rdf:type skos:Concept ;
  rdfs:label "Spatial information research"@en ;
  skos:broader agift:science ;
  skos:definition """Investigating practical applications for geographical data. Providing advice on the development of standards, protocols and specifications for spatial information systems. Includes developing integrated access to information via the Internet, mobile information systems and global positioning systems (GPS).

See also CIVIC INFRASTRUCTURE: for planning of facilities to support GPS.

See also COMMUNICATIONS: for broadcasting and data transfer standards.

See also DEFENCE - Defence strategic support - Defence science and technology: for applying scientific knowledge to military activities.

See also MARITIME SERVICES - Navigation - Navigation systems development: for applying scientific knowledge to the plotting of courses at sea.

See also MARITIME SERVICES - Search and rescue - Search technology development: for applying scientific knowledge to marine rescue operations.""" ;
  skos:hiddenLabel "Geographical Information Systems" ;
  skos:hiddenLabel "Global positioning systems" ;
  skos:prefLabel "Spatial information research"@en ;
  skos:related agift:civic-infrastructure ;
.
agift:special-needs-programs
  rdf:type skos:Concept ;
  rdfs:label "Special needs programs"@en ;
  skos:broader agift:school-education ;
  skos:definition "Administering learning and community support programs for primary and secondary students in target groups. Providing remedial education to assist those in difficulty, and extension programs for the gifted. Includes children with physical or intellectual disabilities, those with English as a second language, migrant or Indigenous children." ;
  skos:hiddenLabel "Extension education programs" ;
  skos:hiddenLabel "Remedial education programs" ;
  skos:hiddenLabel "Tutoring" ;
  skos:prefLabel "Special needs programs"@en ;
  skos:related agift:adult-migrant-education ;
.
agift:special-needs-services
  rdf:type skos:Concept ;
  rdfs:label "Special needs services"@en ;
  skos:broader agift:health-care ;
  skos:definition """Developing policy to support the physical and mental wellbeing of people with particular requirements. Establishing health care programs to assist target groups. Includes advisory and support services for individuals with a particular medical condition.

See also COMMUNITY SERVICES - Community support - Aged care services: for social support for elderly people.

See also COMMUNITY SERVICES - Counselling services: for the provision of group therapy or psychological advice.

See also HEALTH CARE - Veterans' health services: for programs to assist returned services personnel.

See also INDIGENOUS AFFAIRS - Indigenous health services: for programs to assist Aboriginal or Torres Strait Islander communities.""" ;
  skos:hiddenLabel "Adolescent health services" ;
  skos:hiddenLabel "Brain injury support services" ;
  skos:hiddenLabel "Cancer support services" ;
  skos:hiddenLabel "Child and adolescent health services" ;
  skos:hiddenLabel "Disability services" ;
  skos:hiddenLabel "Hearing services" ;
  skos:hiddenLabel "Infant health services" ;
  skos:hiddenLabel "Migrant health services" ;
  skos:hiddenLabel "Occupational therapy" ;
  skos:hiddenLabel "Physiotherapy" ;
  skos:hiddenLabel "Rehabilitation services" ;
  skos:hiddenLabel "Sexual assault victims support" ;
  skos:hiddenLabel "Speech pathology" ;
  skos:hiddenLabel "Support groups" ;
  skos:hiddenLabel "Women's health services" ;
  skos:hiddenLabel "Youth health services" ;
  skos:narrower agift:dental-health-services ;
  skos:narrower agift:independent-living-services ;
  skos:narrower agift:mental-health-services ;
  skos:narrower agift:residential-services ;
  skos:prefLabel "Special needs services"@en ;
  skos:related agift:aged-care-services ;
  skos:related agift:counselling-services ;
.
agift:special-operations
  rdf:type skos:Concept ;
  rdfs:label "Special operations"@en ;
  skos:broader agift:military-operations ;
  skos:definition """Developing unique approaches to achieve specific military objectives. Deploying small units of highly trained combat personnel, in response to extraordinary circumstances or where specialist skills and equipment are required. Includes training provided to foreign local forces, when military aid is given to other countries.

See also DEFENCE - Emergency management - Disaster support: for emergency defence force assistance to other countries.

See also DEFENCE - Military law: for determining the legality of unconventional warfare.

See also SECURITY - Intelligence - Intelligence support: for gathering military intelligence in support of special operations.

See also SECURITY - External security - Peacekeeping forces: for units deployed to stabilise unrest and restore order.""" ;
  skos:hiddenLabel "Unconventional warfare" ;
  skos:prefLabel "Special operations"@en ;
  skos:related agift:australian-theatre-of-war ;
  skos:related agift:disaster-support ;
  skos:related agift:intelligence-support ;
.
agift:spectrum-management
  rdf:type skos:Concept ;
  rdfs:label "Spectrum management"@en ;
  skos:broader agift:radio-communication ;
  skos:definition "Administering the allocation and use of radio spectrum or 'space'. Assessing compliance with government regulations. Processing licence applications for bandwidth and radiofrequency. Monitoring signals allocation to reduce interference and developing long-term spectrum plans with defence, scientific, aircraft and maritime industries." ;
  skos:hiddenLabel "Bandwidth licensing" ;
  skos:hiddenLabel "Radio bandwidth licensing" ;
  skos:prefLabel "Spectrum management"@en ;
.
agift:sport-and-fitness-development
  rdf:type skos:Concept ;
  rdfs:label "Sport and fitness development"@en ;
  skos:broader agift:sport-and-recreation ;
  skos:definition """Developing policy and programs to support the growth of competitive sports and associated industries. Encouraging increased participation and funding for sports and fitness programs. Providing training institutions and facilities for elite athletes.

See also BUSINESS SUPPORT AND REGULATION - Association registration: for processes to incorporate a sporting body.

See also SPORT AND RECREATION - Community recreational programs - Public fitness promotion: for schemes to encourage physical activity.""" ;
  skos:narrower agift:athlete-scholarship-programs ;
  skos:narrower agift:fundraising-and-donation-schemes ;
  skos:narrower agift:games-administration ;
  skos:narrower agift:games-promotion ;
  skos:narrower agift:sporting-grants-administration ;
  skos:prefLabel "Sport and fitness development"@en ;
  skos:related agift:association-registration ;
.
agift:sport-and-recreation
  rdf:type skos:Concept ;
  rdfs:label "SPORT AND RECREATION"@en ;
  skos:definition "Developing policy and programs to encourage community participation in organised games or leisure activities. Implementing promotional strategies, providing funding and administering regulatory bodies." ;
  skos:narrower agift:caravan-and-camping-services ;
  skos:narrower agift:community-recreational-programs ;
  skos:narrower agift:gaming-industry-regulation ;
  skos:narrower agift:park-and-reserve-services ;
  skos:narrower agift:sport-and-fitness-development ;
  skos:narrower agift:sports-drugs-monitoring ;
  skos:prefLabel "SPORT AND RECREATION"@en ;
.
agift:sporting-facilities-management
  rdf:type skos:Concept ;
  rdfs:label "Sporting facilities management"@en ;
  skos:broader agift:public-land-management ;
  skos:definition """Overseeing the care and preparation of land set aside for sporting grounds and amenities. Ensuring facilities are kept clean and maintained. Includes field or court markings, turf or pitch quality, spectator seating, and swimming pools.

See also CIVIC INFRASTRUCTURE - Public land management - Recreational park management: for administration of public leisure areas and playgrounds.

See also SPORT AND RECREATION - Park and reserve services: for administration of sporting grounds.

See also SPORT AND RECREATION - Sport and fitness development - Sporting grants administration: for funding to build and develop sporting facilities.""" ;
  skos:hiddenLabel "Oval maintenance" ;
  skos:hiddenLabel "Playing fields" ;
  skos:hiddenLabel "Public swimming pool maintenance" ;
  skos:hiddenLabel "Skate parks" ;
  skos:hiddenLabel "Swimming pools" ;
  skos:prefLabel "Sporting facilities management"@en ;
  skos:related agift:recreational-park-management ;
  skos:related agift:sporting-grants-administration ;
.
agift:sporting-grants-administration
  rdf:type skos:Concept ;
  rdfs:label "Sporting grants administration"@en ;
  skos:broader agift:sport-and-fitness-development ;
  skos:definition """Providing financial assistance to help build and develop sporting facilities. Identifying groups that may have less access to opportunities in sport. Allocating funds to support the training and development of athletes, coaches, officials and sports administrators.

See also CIVIC INFRASTRUCTURE - Public land management - Sporting facilities management: for administration of sporting facilities.

See also SPORT AND RECREATION - Sport and fitness development - Athlete scholarship programs: for financial assistance to highly skilled athletes.

See also SPORT AND RECREATION - Sport and fitness development - Fundraising and donation schemes: for encouraging investment in sporting events.""" ;
  skos:hiddenLabel "Measurement standards" ;
  skos:prefLabel "Sporting grants administration"@en ;
  skos:related agift:athlete-scholarship-programs ;
  skos:related agift:sporting-facilities-management ;
.
agift:sports-drugs-monitoring
  rdf:type skos:Concept ;
  rdfs:label "Sports drugs monitoring"@en ;
  skos:broader agift:sport-and-recreation ;
  skos:definition "Developing policy to reduce the supply and use of banned or performance-enhancing substances. Preparing criteria to determine whether a substance is illegal and applying penalties for athletes found in breach of policy. Establishing measures to improve accountability in the prescription of sports drugs. Providing funding for research into doping detection tests. Collaborating with scientists and sporting bodies to share information and research." ;
  skos:hiddenLabel "Drugs" ;
  skos:hiddenLabel "Performance-enhancing drugs" ;
  skos:narrower agift:doping-detection-research ;
  skos:prefLabel "Sports drugs monitoring"@en ;
.
agift:statistical-analysis
  rdf:type skos:Concept ;
  rdfs:label "statistical analysis"@en ;
  skos:prefLabel "statistical analysis"@en ;
  skos:related agift:mathematical-sciences ;
.
agift:statistical-collection
  rdf:type skos:Concept ;
  rdfs:label "Statistical collection"@en ;
  skos:broader agift:statistical-services ;
  skos:definition """Collecting statistics from official providers in Australia and as well as using administrative data to generate statistics. Analysing this collected data to identify trends and other significant information about social or economic activities.

See also STATISTICAL SERVICES - Statistical design:  designing statistical outputs, concepts, methodologies, metadata, and collection instruments.

See also STATISTICAL SERVICES - Statistical standards: providing standards for numerical facts issued to the Australian community to ensure the information is coherent, comprehensible and consistent.

See also STATISTICAL SERVICES - Statistics dissemination: disseminating statistical information for use by a broad cross-section of the community.""" ;
  skos:hiddenLabel "Demographic surveys" ;
  skos:hiddenLabel "Household census" ;
  skos:hiddenLabel "Population census" ;
  skos:hiddenLabel "Statistical analysis" ;
  skos:prefLabel "Statistical collection"@en ;
  skos:related agift:population-based-research ;
  skos:related agift:statistical-design ;
  skos:related agift:statistical-standards ;
  skos:related agift:statistics-dissemination ;
.
agift:statistical-design
  rdf:type skos:Concept ;
  rdfs:label "Statistical design"@en ;
  skos:broader agift:statistical-services ;
  skos:definition """Designing statistical outputs, concepts, methodologies, metadata, and collection instruments .

See also STATISTICAL SERVICES - Statistical collection:  for collecting statistics and analysing this collected data to identify trends.

See also STATISTICAL SERVICES - Statistical standards: providing standards for numerical facts issued to the Australian community to ensure the information is coherent, comprehensible and consistent. 

See also STATISTICAL SERVICES - Statistics dissemination: disseminating statistical information for use by a broad cross-section of the community.""" ;
  skos:prefLabel "Statistical design"@en ;
  skos:related agift:statistical-collection ;
.
agift:statistical-services
  rdf:type skos:Concept ;
  rdfs:label "STATISTICAL SERVICES"@en ;
  skos:definition "Providing a high quality, objective and responsive statistical service to assist and encourage informed decision making, research and discussion within governments and the community." ;
  skos:narrower agift:statistical-collection ;
  skos:narrower agift:statistical-design ;
  skos:narrower agift:statistical-standards ;
  skos:narrower agift:statistics-dissemination ;
  skos:prefLabel "STATISTICAL SERVICES"@en ;
.
agift:statistical-standards
  rdf:type skos:Concept ;
  rdfs:label "Statistical standards"@en ;
  skos:broader agift:statistical-services ;
  skos:definition """Supporting and providing standards for numerical facts issued to the Australian community to ensure the information is coherent, comprehensible and consistent. Representing Australia on international standards bodies (such as the System of National Accounts and the International Monetary Fund's Balance of Payments Manual), advising official bodies within Australia about existing statistical standards and consulting on the development of new standards.

See also STATISTICAL SERVICES - Statistical collection:  for collecting statistics and analysing this collected data to identify trends.
 
See also STATISTICAL SERVICES - Statistical design:  designing statistical outputs, concepts, methodologies, metadata, and collection instruments.

See also STATISTICAL SERVICES - Statistics dissemination: disseminating statistical information for use by a broad cross-section of the community.""" ;
  skos:prefLabel "Statistical standards"@en ;
  skos:related agift:statistical-collection ;
.
agift:statistics-dissemination
  rdf:type skos:Concept ;
  rdfs:label "Statistics dissemination"@en ;
  skos:broader agift:statistical-services ;
  skos:definition """Disseminating statistical information for use by a broad cross-section of the community, businesses, the research sector, the media, government departments and agencies, other governments and international agencies. Statistical categories may focus on environmental matters,  government activities,  population, economic or social matters.

See also STATISTICAL SERVICES - Statistical collection:  for collecting statistics and analysing this collected data to identify trends.

See also STATISTICAL SERVICES - Statistical design:  designing statistical outputs, concepts, methodologies, metadata, and collection instruments.

See also STATISTICAL SERVICES - Statistical standards: providing standards for numerical facts issued to the Australian community to ensure the information is coherent, comprehensible and consistent.""" ;
  skos:prefLabel "Statistics dissemination"@en ;
  skos:related agift:statistical-collection ;
.
agift:stock-market-regulation
  rdf:type skos:Concept ;
  rdfs:label "Stock market regulation"@en ;
  skos:broader agift:business-support-and-regulation ;
  skos:definition "Developing policy to control the buying, selling and trading of shares and securities. Monitoring the activities of stock exchanges and stockbrokers. Issuing licenses, investigating suspected breaches of regulations and applying penalties when appropriate." ;
  skos:hiddenLabel "Capital stock regulation" ;
  skos:hiddenLabel "Company shares" ;
  skos:hiddenLabel "Securities exchange" ;
  skos:hiddenLabel "Shares regulation" ;
  skos:hiddenLabel "Stock exchange" ;
  skos:prefLabel "Stock market regulation"@en ;
.
agift:strategic-decisions
  rdf:type skos:Concept ;
  rdfs:label "Strategic decisions"@en ;
  skos:broader agift:defence-strategic-policy ;
  skos:definition """Determining a course of action in relation to the deployment of Australia's defence capability. Reaching a conclusion to direct the conduct of military operations. Resolving a dilemma or choosing from a range of options, to realise defence strategic policy.

See also DEFENCE - Defence strategic policy - Strategic planning: for evaluating defence policy and military advice.

See also DEFENCE - Military operations: for implementing strategic decisions in the conduct of campaigns.

See also INTERNATIONAL RELATIONS - Defence liaison - Military advisors: for guidance to support strategic decisions.""" ;
  skos:prefLabel "Strategic decisions"@en ;
  skos:related agift:military-advisors ;
  skos:related agift:military-operations ;
  skos:related agift:strategic-planning ;
.
agift:strategic-planning
  rdf:type skos:Concept ;
  rdfs:label "Strategic planning"@en ;
  skos:broader agift:defence-strategic-policy ;
  skos:definition """Assessing military and diplomatic advice. Evaluating circumstances and the relative merits of various recommendations regarding deployment of defence resources or the conduct of military operations. Preparing materials to support decision making to realise defence strategic policy.

See also DEFENCE - Defence strategic development: for planning the growth of defence operations.

See also DEFENCE - Defence strategic policy - Strategic decisions: for determining a course of action in matters of defence.

See also INTERNATIONAL RELATIONS - Defence liaison - Military advisors: for guidance to support strategic planning.""" ;
  skos:prefLabel "Strategic planning"@en ;
  skos:related agift:defence-strategic-development ;
  skos:related agift:strategic-decisions ;
.
agift:superannuation-regulation
  rdf:type skos:Concept ;
  rdfs:label "Superannuation regulation"@en ;
  skos:broader agift:retirement-income ;
  skos:definition """Certifying trust funds as superannuation funds, allowing them to accept superannuation contributions and receive concessional tax treatment. Assessing applications against set criteria. Monitoring activities to ensure compliance with superannuation regulations.

See also FINANCE MANAGEMENT - Financial investment - Investment scheme regulation: for prudential supervision of superannuation funds.

See also FINANCE MANAGEMENT - Retirement income - Retirement saving: for encouraging individuals to invest in superannuation.""" ;
  skos:hiddenLabel "Superannuation industry supervision" ;
  skos:prefLabel "Superannuation regulation"@en ;
  skos:related agift:investment-scheme-regulation ;
  skos:related agift:retirement-saving ;
.
agift:tabling-of-official-documents
  rdf:type skos:Concept ;
  rdfs:label "Tabling of official documents"@en ;
  skos:broader agift:parliamentary-chamber-support ;
  skos:definition "Submitting reports and other official documents to parliament or an assembly for discussion. Tabled documents allow review and scrutiny of government policy and through tabling become public documents. Includes programming documents and other procedures associated with their official tabling." ;
  skos:prefLabel "Tabling of official documents"@en ;
  skos:related agift:parliamentary-papers ;
.
agift:tariff-regulation
  rdf:type skos:Concept ;
  rdfs:label "Tariff regulation"@en ;
  skos:broader agift:import-regulation ;
  skos:definition """Setting and collecting taxes or duties on imported goods and resources. Developing policy to control the imposition of charges, and procedures to process tariff payments.

See also FINANCE MANAGEMENT - Taxation: for collecting other levies and taxes.

See also TRADE - Import regulation - Prohibited import control: for inspections and procedures to handle goods that are subject to tariffs.""" ;
  skos:hiddenLabel "Duties" ;
  skos:hiddenLabel "Industry protection" ;
  skos:hiddenLabel "Tariffs" ;
  skos:prefLabel "Tariff regulation"@en ;
  skos:related agift:taxation ;
.
agift:taxation
  rdf:type skos:Concept ;
  rdfs:label "Taxation"@en ;
  skos:broader agift:finance-management ;
  skos:definition """Developing policy to support the collection of taxes and levies from business and the community. Assessing and reviewing the operation of the tax system. Providing taxation advice to individuals and organisations.

See also COMMUNITY SERVICES - Financial assistance: for rebates processed through the tax system.

See also JUSTICE ADMINISTRATION - Local laws and ordinances: for setting rates.

See also TRADE - Import regulation - Tariff regulation: for the collection of import duties and taxes.""" ;
  skos:hiddenLabel "GST" ;
  skos:hiddenLabel "Goods and Services Tax" ;
  skos:hiddenLabel "Levies" ;
  skos:hiddenLabel "Payroll tax" ;
  skos:hiddenLabel "Tax exemptions" ;
  skos:narrower agift:income-assessment ;
  skos:narrower agift:revenue-raising ;
  skos:narrower agift:taxation-compliance ;
  skos:prefLabel "Taxation"@en ;
  skos:related agift:financial-assistance ;
  skos:related agift:tariff-regulation ;
.
agift:taxation-compliance
  rdf:type skos:Concept ;
  rdfs:label "Taxation compliance"@en ;
  skos:broader agift:taxation ;
  skos:definition """Monitoring the documentation submitted by individuals and organisations to ensure it is completed according to taxation laws. Investigating suspected tax avoidance and applying penalties where appropriate. Determining amounts of outstanding tax and implementing recovery procedures. Includes managing payments made by individuals through withholding schemes.

See also FINANCE MANAGEMENT - Taxation - Income assessment: for procedures to submit taxation documentation.

See also FINANCE MANAGEMENT - Taxation - Revenue raising: for mechanisms to collect taxes from individuals or organisations.""" ;
  skos:hiddenLabel "Child support payments" ;
  skos:hiddenLabel "HECS payments" ;
  skos:hiddenLabel "Higher Education Contribution Scheme payments" ;
  skos:hiddenLabel "Tax avoidance" ;
  skos:prefLabel "Taxation compliance"@en ;
  skos:related agift:child-and-youth-support ;
  skos:related agift:income-assessment ;
  skos:related agift:revenue-raising ;
.
agift:telecommunications
  rdf:type skos:Concept ;
  rdfs:label "Telecommunications"@en ;
  skos:broader agift:communications ;
  skos:definition "Developing policy to support and regulate industries that transmit signals along a wire or cable to a receiver. Providing advice on the introduction of new technology and the effects of government policy on the telecommunications industry. Includes consultation with peak industry bodies." ;
  skos:hiddenLabel "Broadband networks" ;
  skos:hiddenLabel "Telephones" ;
  skos:narrower agift:carriage-service-providers ;
  skos:narrower agift:carrier-licensing ;
  skos:narrower agift:communications-infrastructure ;
  skos:narrower agift:equipment-licensing ;
  skos:narrower agift:mobile-telephone-services ;
  skos:narrower agift:telephone-services ;
  skos:prefLabel "Telecommunications"@en ;
.
agift:telephone-services
  rdf:type skos:Concept ;
  rdfs:label "Telephone services"@en ;
  skos:broader agift:telecommunications ;
  skos:definition """Monitoring the activities of suppliers of fixed-line telecommunications services. Ensuring compliance with pricing guidelines, standards of service and maintenance requirements. Managing and maintaining government-owned telecommunications equipment. Setting minimum standards for community access to telephone services.

See also COMMUNICATIONS - Telecommunications - Mobile telephone services: for developing the mobile telephone industry.""" ;
  skos:hiddenLabel "Phone services" ;
  skos:prefLabel "Telephone services"@en ;
  skos:related agift:mobile-telephone-services ;
.
agift:television-broadcasting
  rdf:type skos:Concept ;
  rdfs:label "Television broadcasting"@en ;
  skos:broader agift:broadcasting ;
  skos:definition """Supporting industries that transmit content as transient images accompanied by a sound signal. Managing publicly owned television stations and issuing commercial broadcasting licenses. Developing strategies to promote Australian television programming. Providing television broadcasting services locally, nationally and internationally. Negotiating retransmission arrangements.

See also COMMUNICATIONS - Broadcasting - Broadcasting standards: for regulating the accessibility of television content.""" ;
  skos:hiddenLabel "Broadcasting licenses" ;
  skos:hiddenLabel "Commercial television" ;
  skos:prefLabel "Television broadcasting"@en ;
  skos:related agift:broadcasting-standards ;
.
agift:temporary-entry-arrangements
  rdf:type skos:Concept ;
  rdfs:label "Temporary entry arrangements"@en ;
  skos:broader agift:travel-authorisation ;
  skos:definition "Administering programs to ensure lawful entrance of foreign nationals intending to visit Australia for a limited time. Processing applications for visas and providing advice to applicants. Includes visitors entering the country for business or cultural purposes." ;
  skos:hiddenLabel "Business visas" ;
  skos:hiddenLabel "Cultural stay visas" ;
  skos:hiddenLabel "Holiday visas" ;
  skos:hiddenLabel "Short stay visas" ;
  skos:hiddenLabel "Student entry visas" ;
  skos:hiddenLabel "Temporary residence visas" ;
  skos:hiddenLabel "Transit visas" ;
  skos:hiddenLabel "Visa applications" ;
  skos:hiddenLabel "Visitor visas" ;
  skos:hiddenLabel "Work permits" ;
  skos:hiddenLabel "Work visas" ;
  skos:prefLabel "Temporary entry arrangements"@en ;
.
agift:termination-processes
  rdf:type skos:Concept ;
  rdfs:label "Termination processes"@en ;
  skos:broader agift:human-resources-development ;
  skos:definition """Managing activities associated with staff separation from the organisation. Issuing warnings and initiating disciplinary proceedings for unacceptable conduct. Arranging exit interviews. Providing access to counselling and advice for retirement or redundancy. Establishing procedures for public sector separations or transfers in accordance with government policy.

See also DEFENCE - Defence force careers - Military employment services: for termination processes in the defence forces.""" ;
  skos:hiddenLabel "Disciplinary proceedings" ;
  skos:hiddenLabel "Personnel termination processes" ;
  skos:hiddenLabel "Redundancy" ;
  skos:hiddenLabel "Retirement" ;
  skos:hiddenLabel "Retrenchment" ;
  skos:hiddenLabel "Severance" ;
  skos:hiddenLabel "Staff separations" ;
  skos:hiddenLabel "Staff transfers" ;
  skos:prefLabel "Termination processes"@en ;
  skos:related agift:military-employment-services ;
.
agift:territories-administration
  rdf:type skos:Concept ;
  rdfs:label "Territories administration"@en ;
  skos:broader agift:public-administration ;
  skos:definition "Developing policy and administering programs for Australia's self governing and non self-governing territories. Includes providing services in non self-governing territories. Includes policy advice and administration of Commonwealth functions in the national capital." ;
  skos:prefLabel "Territories administration"@en ;
.
agift:tertiary-education
  rdf:type skos:Concept ;
  rdfs:label "Tertiary education"@en ;
  skos:broader agift:education-and-training ;
  skos:definition """Administering programs that offer instruction beyond secondary school education, to impart knowledge and develop skills. Developing and implementing entry requirements. Managing tertiary education institutions and facilities. Implementing standards and guidelines to support lecturers. Includes the provision of scholarships and study grants.

See also EDUCATION AND TRAINING - Arts education: for programs to further artistic talent at individual or community level.

See also EDUCATION AND TRAINING - Curriculum development: for researching and drafting outline study programs.

See also FINANCE MANAGEMENT - Taxation - Taxation compliance: for higher education payments made through the tax system.

See also INTERNATIONAL RELATIONS - Overseas aid programs - Overseas student scholarship programs: for access to higher education for students from developing countries or the Pacific region.""" ;
  skos:hiddenLabel "Colleges of advanced education" ;
  skos:hiddenLabel "Higher education" ;
  skos:hiddenLabel "Institutes of technology" ;
  skos:hiddenLabel "Teachers colleges" ;
  skos:hiddenLabel "Tertiary institutions" ;
  skos:hiddenLabel "Universities" ;
  skos:prefLabel "Tertiary education"@en ;
  skos:related agift:arts-education ;
.
agift:tourism
  rdf:type skos:Concept ;
  rdfs:label "TOURISM"@en ;
  skos:definition "Developing policy and programs to encourage recreational visitors to a region. Supporting and regulating the tourism industry. Implementing long-term strategies for tourism development and coordinating across jurisdictions on large-scale projects. Providing funding for promotional campaigns." ;
  skos:narrower agift:tourism-industry-development ;
  skos:narrower agift:tourist-event-promotion ;
  skos:narrower agift:travel-missions ;
  skos:prefLabel "TOURISM"@en ;
.
agift:tourism-industry-development
  rdf:type skos:Concept ;
  rdfs:label "Tourism industry development"@en ;
  skos:broader agift:tourism ;
  skos:definition """Supporting the growth of businesses that provide travel products and other services to visitors. Identifying the potential of new and emerging markets. Providing grants and sponsorship. Encouraging partnerships and coordinating initiatives to optimise tourism employment and create a favourable environment for investment. Includes recognising excellence in the Australian tourism industry through the presentation of awards.

See also TRADE - Trade expositions: for organising and participating in exhibitions and trade fairs.""" ;
  skos:hiddenLabel "Tourism awards" ;
  skos:prefLabel "Tourism industry development"@en ;
  skos:related agift:caravan-and-camping-services ;
  skos:related agift:trade-expositions ;
.
agift:tourist-event-promotion
  rdf:type skos:Concept ;
  rdfs:label "Tourist event promotion"@en ;
  skos:broader agift:tourism ;
  skos:definition """Developing special activities to draw visitors to a region. Marketing and promoting events and attractions as catalysts for tourism growth. Managing publicity to increase awareness of tourism initiatives, exhibitions and trade fairs. Includes the promotion of overseas tourist events.

See also INTERNATIONAL RELATIONS - Overseas promotion: for negotiating opportunities to participate in or host international tourist events.

See also SPORT AND RECREATION - Sport and fitness development - Games promotion: for publicising major sporting events.

See also TOURISM - Tourism industry development: for sponsorship of selected events.

See also TRADE - Trade expositions: for organising and participating in exhibitions and trade fairs.""" ;
  skos:hiddenLabel "Exhibition marketing" ;
  skos:hiddenLabel "Exhibition promotion" ;
  skos:hiddenLabel "Trade fair promotion" ;
  skos:narrower agift:advertising-campaigns ;
  skos:prefLabel "Tourist event promotion"@en ;
  skos:related agift:overseas-promotion ;
.
agift:town-planning
  rdf:type skos:Concept ;
  rdfs:label "Town planning"@en ;
  skos:broader agift:civic-management ;
  skos:definition """Establishing a framework of objectives and strategies for controlled urban development. Initiating projects to meet current and future needs for infrastructure and facilities. Providing guidelines to assist applicants for building approval.

See also CIVIC INFRASTRUCTURE - Civic management - Building approval services: for assessing applications to build or alter structures.

See also CIVIC INFRASTRUCTURE - Housing industry policy: for policy and programs to ensure the adequacy of land supply and construction activity.

See also CIVIC INFRASTRUCTURE - Infrastructure planning; providing advice on nationally-significant economic infrastructure to governments, investors and owners.
See also CIVIC INFRASTRUCTURE - Integrated services planning: for coordinated provision of essential community services.

See also NATURAL RESOURCES - Land use planning: for research into future needs for infrastructure and facilities.

See also NATURAL RESOURCES - Land use planning - Land use zoning: for allocating areas of land with regard to their use.""" ;
  skos:prefLabel "Town planning"@en ;
  skos:related agift:building-approval-services ;
  skos:related agift:housing-industry-policy ;
  skos:related agift:integrated-services-planning ;
  skos:related agift:land-use-planning ;
.
agift:trade
  rdf:type skos:Concept ;
  rdfs:label "TRADE"@en ;
  skos:definition """Developing policy to regulate the purchase, sale or exchange of commodities. Monitoring the balance of trade, industry protection and subsidy schemes. Includes foreign and domestic activities, and liaison across jurisdictions to support trade agreement negotiations.

See also BUSINESS SUPPORT AND REGULATION: for compliance with fair-trading practices.""" ;
  skos:hiddenLabel "Balance of payments" ;
  skos:narrower agift:export-regulation ;
  skos:narrower agift:import-regulation ;
  skos:narrower agift:intellectual-property-management ;
  skos:narrower agift:international-trade-agreements ;
  skos:narrower agift:interstate-trade-agreements ;
  skos:narrower agift:trade-development-programs ;
  skos:narrower agift:trade-expositions ;
  skos:narrower agift:trade-measurement-compliance ;
  skos:prefLabel "TRADE"@en ;
  skos:related agift:business-support-and-regulation ;
.
agift:trade-development-programs
  rdf:type skos:Concept ;
  rdfs:label "Trade development programs"@en ;
  skos:broader agift:trade ;
  skos:definition """Implementing schemes to assist local businesses to compete in regional or international markets and win overseas or interstate contracts. Includes programs to attract investment to Australia, liaison with other governments and industry partners, providing practical assistance such as identifying foreign investment partners and administering grants.

See also INTERNATIONAL RELATIONS - Overseas aid programs - Development assistance program: for schemes to foster economic growth in other countries.""" ;
  skos:prefLabel "Trade development programs"@en ;
  skos:related agift:development-assistance-programs ;
.
agift:trade-expositions
  rdf:type skos:Concept ;
  rdfs:label "Trade expositions"@en ;
  skos:broader agift:trade ;
  skos:definition """Organising national and international events to promote trade and maximise marketing opportunities. Participating in trade fairs and developing exhibits. Includes activities to raise business profiles in a specific industry, or across a range of sectors.

See also INTERNATIONAL RELATIONS - Overseas promotion: for negotiating opportunities to host or participate in international trade fairs.

See also TOURISM - Tourist event promotion: for managing the publicity of trade expositions.""" ;
  skos:hiddenLabel "Expositions" ;
  skos:hiddenLabel "Trade fairs" ;
  skos:prefLabel "Trade expositions"@en ;
  skos:related agift:overseas-promotion ;
  skos:related agift:tourism-industry-development ;
.
agift:trade-measurement-compliance
  rdf:type skos:Concept ;
  rdfs:label "Trade measurement compliance"@en ;
  skos:broader agift:trade ;
  skos:definition """Administering national trade measurement compliance and enforcement with trade measurement legislation.
See also SCIENCE - Applied sciences  - Weights and measures standards: conducting research into methods of ascertaining dimensions, extent, size or amounts. Setting and maintaining standards consistent with international conventions for units, values and industrial measurements.""" ;
  skos:prefLabel "Trade measurement compliance"@en ;
  skos:related agift:weights-and-measures-standards ;
.
agift:trade-practices-compliance
  rdf:type skos:Concept ;
  rdfs:label "Trade practices compliance"@en ;
  skos:broader agift:fair-trading-compliance ;
  skos:definition "Administering programs to ensure that individuals and businesses comply with competition, fair-trading and consumer protection laws. Investigating misleading or deceptive action in commercial transactions. Imposing penalties when appropriate." ;
  skos:hiddenLabel "Trade practices" ;
  skos:prefLabel "Trade practices compliance"@en ;
  skos:related agift:business-sponsorship ;
.
agift:trademark-registration
  rdf:type skos:Concept ;
  rdfs:label "Trademark registration"@en ;
  skos:broader agift:intellectual-property-management ;
  skos:definition """Conferring legal ownership over signs or symbols used to distinguish the goods and services associated with a business entity or product. Including processing and approving trademark applications, liaising with trademark owners, granting registrations for trademarks and issuing decisions on disputes over the registration or refusal of  trademark rights.

See also JUSTICE ADMINISTRATION - Administrative law - Copyright regulation: for legal processes and disputes over copyright ownership.


See also TRADE - Intellectual property management - Design rights management: for the intellectual property in structures, machinery, industrial plans or complex artworks.

See also TRADE - Intellectual property management - Patent rights management: for the intellectual property in inventions and industrial or scientific processes.

See also TRADE - Intellectual property management - Plant breeders' rights management: for developing policy to protect the rights of plant  breeders developing new plant varieties.""" ;
  skos:hiddenLabel "Brand names" ;
  skos:hiddenLabel "Logo registration" ;
  skos:prefLabel "Trademark registration"@en ;
  skos:related agift:copyright-regulation ;
.
agift:trainee-programs
  rdf:type skos:Concept ;
  rdfs:label "Trainee programs"@en ;
  skos:broader agift:vocational-education ;
  skos:definition """Administering industry-based training schemes where students learn on-the-job - such as general office traineeships, graduate or cadet programs and service industry training in tourism or hospitality. Monitoring compliance with standards and guidelines.

See also EDUCATION AND TRAINING - Vocational education - Apprenticeship programs: for industry-based training in trades and technical vocations.

See also EMPLOYMENT: for the employment conditions of trainees.""" ;
  skos:hiddenLabel "Graduate programs" ;
  skos:hiddenLabel "Hospitality training" ;
  skos:hiddenLabel "Office traineeships" ;
  skos:hiddenLabel "Service industry training" ;
  skos:hiddenLabel "Tourism training" ;
  skos:hiddenLabel "Traineeships" ;
  skos:prefLabel "Trainee programs"@en ;
  skos:related agift:apprenticeship-programs ;
.
agift:transport
  rdf:type skos:Concept ;
  rdfs:label "TRANSPORT"@en ;
  skos:definition """Developing policy to regulate road, rail and air transportation systems. Planning and managing schemes for the movement of people or freight. Monitoring the safety of vehicles and their operators. Providing resources for the development of transport infrastructure.

See also MARITIME SERVICES: for regulating sea transport.""" ;
  skos:narrower agift:air-transport ;
  skos:narrower agift:freight-movement-regulation ;
  skos:narrower agift:passenger-services ;
  skos:narrower agift:public-transport ;
  skos:narrower agift:rail-transport ;
  skos:narrower agift:road-transport ;
  skos:narrower agift:transport-infrastructure-development ;
  skos:prefLabel "TRANSPORT"@en ;
  skos:related agift:maritime-services ;
.
agift:transport-access-schemes
  rdf:type skos:Concept ;
  rdfs:label "Transport access schemes"@en ;
  skos:broader agift:community-services ;
  skos:definition """Managing programs to ensure public transport facilities are readily available to all sectors of the community. Formulating policy to support the provision of transport services to those in need. Developing strategies to assist specific community groups and establishing eligibility criteria for concessions. Includes liaison with areas responsible for public transport construction, to determine short-term and long-term community transport needs.

See also COMMUNITY SERVICES - Financial assistance: for providing concessions and subsidies.

See also EDUCATION AND TRAINING - School education - School transport regulation: for developing services to help children travel to and from school.

See also TRANSPORT - Public transport - Transport accessibility: developing standards and policies to make public transport accessible to people with disabilities.""" ;
  skos:hiddenLabel "Community transport" ;
  skos:hiddenLabel "Transport concessions" ;
  skos:hiddenLabel "Travel concession schemes" ;
  skos:prefLabel "Transport access schemes"@en ;
  skos:related agift:financial-assistance ;
  skos:related agift:transport-network-maintenance ;
.
agift:transport-accessibility
  rdf:type skos:Concept ;
  rdfs:label "Transport accessibility"@en ;
  skos:broader agift:public-transport ;
  skos:definition """Developing standards and policies to make public transport accessible to people with disabilities.
See also COMMUNITY SERVICES - Transport access schemes: for programs such as taxi subsidies to make services available to targeted community groups.""" ;
  skos:hiddenLabel "Disabled transport" ;
  skos:prefLabel "Transport accessibility"@en ;
.
agift:transport-infrastructure-development
  rdf:type skos:Concept ;
  rdfs:label "Transport infrastructure development"@en ;
  skos:broader agift:transport ;
  skos:definition """Designing systems for the movement of people or goods. Installing facilities to support a network of air, rail and road transport services. Assessing existing infrastructure and planning for future requirements. Includes developing transport corridors, links to airport and rail terminals, and collaborating across jurisdictions on infrastructure development.

See also CIVIC INFRASTRUCTURE - Civic management - Engineering services: for professional advice and supervision of construction projects.

See also CIVIC INFRASTRUCTURE - Transport network maintenance: for managing public transport at a local level.

See also MARITIME SERVICES - Port regulation: for developing sea transport infrastructure.

See also TRANSPORT - Air transport - Airport services: for repair and preservation of transport infrastructure.

See also TRANSPORT - Rail transport - Railway maintenance: for repair and preservation of transport infrastructure.

See also TRANSPORT - Road transport - Road surface maintenance: for repair and preservation of road transport infrastructure.""" ;
  skos:hiddenLabel "Road building" ;
  skos:hiddenLabel "Road construction" ;
  skos:prefLabel "Transport infrastructure development"@en ;
  skos:related agift:engineering-services ;
  skos:related agift:railway-maintenance ;
  skos:related agift:road-surface-maintenance ;
.
agift:transport-network-maintenance
  rdf:type skos:Concept ;
  rdfs:label "Transport network maintenance"@en ;
  skos:broader agift:civic-infrastructure ;
  skos:definition """Managing public transport networks at a local level. Developing interconnecting services for road, rail and air transport. Maintaining public car parks, bus shelters, train stations, footpaths and cycle ways.

See also COMMUNITY SERVICES - Transport access schemes: for programs to make services available to targeted community groups.

See also EDUCATION AND TRAINING - School education - School transport regulation: for guidance in developing services for children travelling to and from school.

See also TRANSPORT - Air transport - Airport services: for preserving transport infrastructure.

See also TRANSPORT - Passenger services: for timetables and route maps.

See also TRANSPORT - Rail transport - Railway maintenance: for preserving transport infrastructure.

See also TRANSPORT - Road transport - Road surface maintenance: for preserving transport infrastructure.

See also TRANSPORT - Transport infrastructure development: for designing and building transport systems.""" ;
  skos:hiddenLabel "Bus services" ;
  skos:hiddenLabel "Cycle path maintenance" ;
  skos:hiddenLabel "Footpath maintenance" ;
  skos:hiddenLabel "Train services" ;
  skos:hiddenLabel "Tram services" ;
  skos:prefLabel "Transport network maintenance"@en ;
  skos:related agift:passenger-services ;
  skos:related agift:public-transport ;
  skos:related agift:school-transport-regulation ;
  skos:related agift:transport-access-schemes ;
.
agift:travel-authorisation
  rdf:type skos:Concept ;
  rdfs:label "Travel authorisation"@en ;
  skos:broader agift:immigration ;
  skos:definition """Developing policy to regulate the entry and presence of non-citizens or foreign nationals in Australia. Establishing eligibility criteria, visa classes and entry conditions. Providing on-arrival immigration clearance through the passenger entry control system.

See also INTERNATIONAL RELATIONS - Passport services: for issuing travel documents to Australian citizens.

See also SECURITY - National security - Border protection: for monitoring unauthorised sea or air arrivals.""" ;
  skos:hiddenLabel "Arrivals" ;
  skos:hiddenLabel "Passenger entry control" ;
  skos:hiddenLabel "Passport control" ;
  skos:narrower agift:permanent-entry-arrangements ;
  skos:narrower agift:temporary-entry-arrangements ;
  skos:prefLabel "Travel authorisation"@en ;
  skos:related agift:citizenship ;
  skos:related agift:passport-services ;
.
agift:travel-missions
  rdf:type skos:Concept ;
  rdfs:label "Travel missions"@en ;
  skos:broader agift:tourism ;
  skos:definition "Marketing activities carried out overseas for the promotion of Australia or specific regions as a travel and tourism destination. Organising meetings between members of the Australian tourism industry, travel agents and overseas tour operators. Includes familiarisation tours in Australia for international travel agents, tour operators and members of the travel press." ;
  skos:prefLabel "Travel missions"@en ;
.
agift:treaty-administration
  rdf:type skos:Concept ;
  rdfs:label "Treaty administration"@en ;
  skos:broader agift:international-treaties ;
  skos:definition """Implementing the terms and conditions of formal agreements made between Australia and one or more other countries. Monitoring compliance with provisions and obligations. Assessing the ongoing benefits of treaty participation.

See also INTERNATIONAL RELATIONS - International affairs - Disarmament and arms control: for administering treaties to reduce or limit levels of military resources.

See also JUSTICE ADMINISTRATION - Human rights obligations: for upholding personal freedoms that may be set down in treaties.""" ;
  skos:hiddenLabel "Treaty participation" ;
  skos:prefLabel "Treaty administration"@en ;
  skos:related agift:disarmament-and-arms-control ;
.
agift:vehicle-registration
  rdf:type skos:Concept ;
  rdfs:label "Vehicle registration"@en ;
  skos:broader agift:road-transport ;
  skos:definition """Administering arrangements to uniquely identify motor vehicles. Issuing certificates of ownership and maintaining records to allocate responsibility for individual motor vehicles. Includes processing applications, renewals, transfer, suspension and cancellation of vehicle registrations.

See also TRANSPORT - Road transport - Vehicle standards: for certificates of roadworthiness.""" ;
  skos:hiddenLabel "Car registration" ;
  skos:hiddenLabel "Licence plates" ;
  skos:hiddenLabel "Motor vehicle national certification" ;
  skos:hiddenLabel "Registration" ;
  skos:prefLabel "Vehicle registration"@en ;
  skos:related agift:vehicle-standards ;
.
agift:vehicle-standards
  rdf:type skos:Concept ;
  rdfs:label "Vehicle standards"@en ;
  skos:broader agift:road-transport ;
  skos:definition """Regulating the design, construction, maintenance and operation of any machine intended for use on public roads. Setting standards for vehicle safety, configuration, noise and emissions. Monitoring conformance through inspections and testing. Issuing or declining certificates of roadworthiness, to support the process of vehicle registration.

See also TRANSPORT - Road transport - Driving licences administration: for certifying operators of motor vehicles.""" ;
  skos:hiddenLabel "Roadworthy certificates" ;
  skos:hiddenLabel "Vehicle regulation" ;
  skos:prefLabel "Vehicle standards"@en ;
  skos:related agift:driving-licences-administration ;
  skos:related agift:vehicle-registration ;
.
agift:veterans-entitlements
  rdf:type skos:Concept ;
  rdfs:label "Veterans' entitlements"@en ;
  skos:broader agift:community-support ;
  skos:definition """\"Managing social support services to returned defence service personnel and their families. Providing advice on rights to financial or other assistance, such as residential care or medical services. Includes funding and support for community-based or volunteer programs providing veterans' services.


See also COMMUNITY SERVICES - Community support - Defence community programs: for services to current defence force personnel and their families.

See also COMMUNITY SERVICES - Financial assistance: for monetary support to individuals.\"
"""^^xsd:string ;
  skos:definition """Managing social support services to returned defence service personnel and their families. Providing advice on rights to financial or other assistance, such as residential care or medical services. Includes funding and support for community-based or volunteer programs providing veterans' services.


See also COMMUNITY SERVICES - Community support - Defence community programs: for services to current defence force personnel and their families.

See also COMMUNITY SERVICES - Financial assistance: for monetary support to individuals.""" ;
  skos:hiddenLabel "Veteran" ;
  skos:hiddenLabel "War pensions" ;
  skos:prefLabel "Veterans' entitlements"@en ;
  skos:related agift:aged-care-services ;
  skos:related agift:benefits ;
  skos:related agift:defence-community-programs ;
  skos:related agift:veterans-health-services ;
.
agift:veterans-health-services
  rdf:type skos:Concept ;
  rdfs:label "Veterans' health services"@en ;
  skos:broader agift:health-care ;
  skos:definition """Developing policy to support the physical and mental wellbeing of returned defence service personnel and their families. Managing health care programs that address the specific needs of veterans. Establishing eligibility criteria for access to health services.

See also COMMUNITY SERVICES - Community support - Veterans' entitlements: for social support to returned service personnel.""" ;
  skos:hiddenLabel "Returned services health programs" ;
  skos:prefLabel "Veterans' health services"@en ;
  skos:related agift:veterans-entitlements ;
.
agift:viticultural-industry
  rdf:type skos:Concept ;
  rdfs:label "Viticultural industry"@en ;
  skos:broader agift:marine-and-rural-support ;
  skos:definition """Administering programs to support commercial grape growing and wine production. Assisting industry growth and development. Encouraging businesses to adopt innovative practices, processes and products. Providing advice on cultivation methods and business management to improve competitiveness.

See also PRIMARY INDUSTRIES - Marine and rural regulation - Agricultural industry: for monitoring and regulating viticultural industries.

See also SCIENCE - Agricultural sciences: for conducting research into grape growing and wine production.""" ;
  skos:hiddenLabel "Grape growing industry" ;
  skos:hiddenLabel "Viticulture" ;
  skos:hiddenLabel "Wine industry support" ;
  skos:hiddenLabel "Wine making industry" ;
  skos:prefLabel "Viticultural industry"@en ;
  skos:related agift:agricultural-industry ;
.
agift:vocational-education
  rdf:type skos:Concept ;
  rdfs:label "Vocational education"@en ;
  skos:broader agift:education-and-training ;
  skos:definition """Developing and promoting programs that offer training and further education for work-related disciplines. Setting standards and guidelines to support the operation of vocational education programs. Initiating joint ventures with industry, schools and tertiary institutions to make use of facilities. Includes the provision of scholarships and study grants.

See also EDUCATION AND TRAINING - Military education and training: for vocational training offered to defence force personnel.

See also EMPLOYMENT: for employment conditions.""" ;
  skos:hiddenLabel "Business schools" ;
  skos:hiddenLabel "Competency standards" ;
  skos:hiddenLabel "Professional education" ;
  skos:hiddenLabel "Technical and further education" ;
  skos:narrower agift:apprenticeship-programs ;
  skos:narrower agift:hospital-teaching-programs ;
  skos:narrower agift:industry-collaboration ;
  skos:narrower agift:trainee-programs ;
  skos:narrower agift:workplace-training ;
  skos:prefLabel "Vocational education"@en ;
  skos:related agift:employment-services-marketing ;
  skos:related agift:military-education-and-training ;
.
agift:volunteer-support-programs
  rdf:type skos:Concept ;
  rdfs:label "Volunteer support programs"@en ;
  skos:broader agift:community-recreational-programs ;
  skos:definition "Providing financial assistance and services for groups and individuals who offer their time and labour to the community free of charge. Raising awareness of volunteer programs groups though sponsorship, advertising and facilitating links between organisations. Includes organising large volunteer groups for major sporting events." ;
  skos:prefLabel "Volunteer support programs"@en ;
  skos:related agift:games-administration ;
.
agift:warfare
  rdf:type skos:Concept ;
  rdfs:label "Warfare"@en ;
  skos:broader agift:military-operations ;
  skos:definition """Entering into armed combat with opposing defence forces. Conducting military, naval or air attacks against designated targets. Performing offensive or defensive operations on the battlefield to win campaigns.

See also DEFENCE - Military operations - Australian theatre of war: for coordinating campaigns across all locations involved in warfare.

See also DEFENCE - Military operations - Special operations: for unconventional warfare or the deployment of highly trained military personnel.

See also SECURITY - External security - Peacekeeping forces: for units deployed to stabilise unrest and restore order.""" ;
  skos:hiddenLabel "Armed combat" ;
  skos:hiddenLabel "Battlefront operations" ;
  skos:hiddenLabel "Conflicts" ;
  skos:hiddenLabel "Military action" ;
  skos:hiddenLabel "Military engagement" ;
  skos:hiddenLabel "War" ;
  skos:prefLabel "Warfare"@en ;
  skos:related agift:australian-theatre-of-war ;
  skos:related agift:chemical-and-pesticide-regulation ;
.
agift:waste-management
  rdf:type skos:Concept ;
  rdfs:label "Waste management"@en ;
  skos:broader agift:civic-infrastructure ;
  skos:definition """Providing services to collect and dispose of garbage. Operating waste management centres, landfill sites, recycling depots and sewerage facilities. Developing and promoting strategies for consumer waste minimisation. Providing services for graffiti removal and street cleaning.

See also ENVIRONMENT - Pollutant prevention programs: for standards and guidelines to reduce waste.

See also NATURAL RESOURCES - Pollution emission control: for monitoring industrial waste management.""" ;
  skos:hiddenLabel "Garbage collection" ;
  skos:hiddenLabel "Graffiti removal" ;
  skos:hiddenLabel "Hazardous materials management" ;
  skos:hiddenLabel "Hazardous waste management" ;
  skos:hiddenLabel "Landfill sites" ;
  skos:hiddenLabel "Needle disposal" ;
  skos:hiddenLabel "Public toilets" ;
  skos:hiddenLabel "Recycling" ;
  skos:hiddenLabel "Refuse management" ;
  skos:hiddenLabel "Rubbish collection" ;
  skos:hiddenLabel "Sewerage" ;
  skos:hiddenLabel "Waste disposal" ;
  skos:hiddenLabel "Wheelie bins" ;
  skos:prefLabel "Waste management"@en ;
  skos:related agift:pollutant-prevention-programs ;
.
agift:water-conservation-plans
  rdf:type skos:Concept ;
  rdfs:label "Water conservation plans"@en ;
  skos:broader agift:water-resources ;
  skos:definition """Developing strategies to prevent the loss or waste of water resources. Monitoring dam and reservoir levels, rainfall and projected water usage figures. Recommending water restrictions and other measures to ensure water supplies continue to meet user needs over time. Conducting consultation exercises and education programs to raise community awareness of water conservation issues.

See also ENVIRONMENT: for programs to conserve or protect wetlands and waterway ecosystems.""" ;
  skos:prefLabel "Water conservation plans"@en ;
  skos:related agift:environment ;
.
agift:water-quality-monitoring
  rdf:type skos:Concept ;
  rdfs:label "Water quality monitoring"@en ;
  skos:broader agift:water-resources ;
  skos:definition """Administering programs to assess the characteristics of water resources, to determine their fitness for purpose. Analysing water samples for the presence of contaminants or minerals to ensure it is potable. Includes testing for salinity, bacteria, pesticides and other pollutants.

See also NATURAL RESOURCES - Pollution emission control: for monitoring the discharge of industrial contaminants and waste.""" ;
  skos:prefLabel "Water quality monitoring"@en ;
  skos:related agift:pollution-emission-control ;
.
agift:water-resources
  rdf:type skos:Concept ;
  rdfs:label "Water resources"@en ;
  skos:broader agift:natural-resources ;
  skos:definition """Developing policy and administering legislation relating to waterways and water resources. Supporting industry partnerships and cooperative approaches to the management and use of water. Regulating the exploitation of water resources to ensure sustainable quality and availability for household, industrial and agricultural use.

See also CIVIC INFRASTRUCTURE - Energy supply: for regulating the delivery and pricing of water resources.

See also ENVIRONMENT - Oceans governance: for planning sustainable development of ocean resources.

See also SCIENCE - Earth sciences - Hydrology: for conducting research into water systems.""" ;
  skos:hiddenLabel "Water supplies" ;
  skos:hiddenLabel "Water supply" ;
  skos:narrower agift:water-conservation-plans ;
  skos:narrower agift:water-quality-monitoring ;
  skos:narrower agift:water-usage-management ;
  skos:narrower agift:waterway-management ;
  skos:prefLabel "Water resources"@en ;
  skos:related agift:energy-supply ;
.
agift:water-usage-management
  rdf:type skos:Concept ;
  rdfs:label "Water usage management"@en ;
  skos:broader agift:water-resources ;
  skos:definition """Monitoring water consumption and implementing schemes to regulate water usage. Implementing water conservation recommendations, such as water restrictions. Administering water rights and evaluating compliance with the terms of waterway agreements. Assessing agricultural and industrial water usage practices. Issuing permits for the use of bore water.

See also NATURAL RESOURCES - Energy resources - Renewable energy development: for supporting hydroelectric initiatives.""" ;
  skos:hiddenLabel "Water services" ;
  skos:hiddenLabel "Water supply" ;
  skos:prefLabel "Water usage management"@en ;
  skos:related agift:renewable-energy-development ;
.
agift:waterway-management
  rdf:type skos:Concept ;
  rdfs:label "Waterway management"@en ;
  skos:broader agift:water-resources ;
  skos:definition """Monitoring river flows and catchment areas. Implementing strategies for salinity management and river care programs. Evaluating the effects of land use and climate on waterways. Developing agreements for the equitable use of water resources from river systems that may cross jurisdictional boundaries.

See also ENVIRONMENT: for programs to conserve or protect wetlands and waterway ecosystems.

See also ENVIRONMENT - Oceans governance: for planning sustainable development of ocean resources.

See also MARITIME SERVICES - Harbour management: for administering coastal areas that provide protection for ships.

See also MARITIME SERVICES - Marina management: for regulating boating activities to protect waterways.

See also PRIMARY INDUSTRIES: for regulating or supporting water-based industries.""" ;
  skos:hiddenLabel "Floodplain management" ;
  skos:prefLabel "Waterway management"@en ;
  skos:related agift:environment ;
.
agift:website-development
  rdf:type skos:Concept ;
  rdfs:label "Website development"@en ;
  skos:broader agift:publishing ;
  skos:definition """Designing and maintaining online information and services. Managing the supporting software to make electronic publications and transactions available via internal or external networks. Planning the layout of web pages and marking up content.

See also COMMUNICATIONS - Information management standards - Information dissemination: for developing strategic or overall web frameworks.

See also COMMUNICATIONS - Publishing - Electronic publishing: for developing website content.""" ;
  skos:prefLabel "Website development"@en ;
  skos:related agift:information-dissemination ;
.
agift:weights-and-measures-standards
  rdf:type skos:Concept ;
  rdfs:label "Weights and measures standards"@en ;
  skos:broader agift:applied-sciences ;
  skos:definition """Conducting research into methods of ascertaining dimensions, extent, size or amounts. Setting and maintaining standards consistent with international conventions for units, values and industrial measurements. Includes testing and calibration of measuring equipment, training and consultancy in measurement science.

See also TRADE - Trade measurement compliance: administering national trade measurement compliance and enforcement with trade measurement legislation.""" ;
  skos:hiddenLabel "Industrial measurement" ;
  skos:hiddenLabel "Measurement standards" ;
  skos:prefLabel "Weights and measures standards"@en ;
  skos:related agift:trade-measurement-compliance ;
.
agift:whistleblowing
  rdf:type skos:Concept ;
  rdfs:label "Whistleblowing"@en ;
  skos:broader agift:public-administration ;
  skos:definition """Disclosure  of illegal, immoral or illegitimate practices under the control of their employer by government employees (former or current ) to persons or organisations that may be able to effect action such as  watchdog  bodies,  the media or the public.
See also GOVERNANCE - Public administration - Corruption prevention:  preventing, detecting and investigating serious and systemic corruption issues in Australian government agencies.
See also GOVERNANCE - Public administration - Integrity compliance: encouraging ethical behaviour and compliance with official codes of conduct.
See also JUSTICE ADMINISTRATION - administrative law: administering the body of law that relates to the executive functions of government.""" ;
  skos:hiddenLabel "Protected disclosure" ;
  skos:hiddenLabel "Public interest disclosure" ;
  skos:prefLabel "Whistleblowing"@en ;
.
agift:wilderness-area-management
  rdf:type skos:Concept ;
  rdfs:label "Wilderness area management"@en ;
  skos:broader agift:natural-heritage-protection ;
  skos:definition """Administering designated wilderness areas, where the ecology is undisturbed. Monitoring access restrictions. Issuing permits for commercial or recreational activities. Providing advice on developments that might encroach on wilderness areas. 

See also CIVIC INFRASTRUCTURE - Public land administration - Garden management: for administering public land where ornamental or useful plants are cultivated.

See also ENVIRONMENT - Conservation programs - Endangered species protection: for programs to protect or repopulate flora and fauna at risk.

See also ENVIRONMENT - Natural heritage protection - National park management: for administering designated national park areas.

See also ENVIRONMENT - Natural heritage protection - Nature reserve management: for the maintenance of native flora and fauna reserves.

See also ENVIRONMENT - Natural heritage protection - Wildlife sanctuary management: for sheltered facilities for wild animals.

See also INDIGENOUS AFFAIRS - Indigenous heritage conservation: for land use agreements with traditional owners.""" ;
  skos:hiddenLabel "Bushland management" ;
  skos:prefLabel "Wilderness area management"@en ;
  skos:related agift:endangered-species-protection ;
  skos:related agift:garden-management ;
.
agift:wildlife-sanctuary-management
  rdf:type skos:Concept ;
  rdfs:label "Wildlife sanctuary management"@en ;
  skos:broader agift:natural-heritage-protection ;
  skos:definition """Administering sheltered facilities where animals live in conditions that resemble their natural habitat. Building special amenities, or allocating space from wilderness areas or nature reserves. Supporting protection programs for endangered species and services to rehabilitate injured wildlife. Monitoring the activities of privately run sanctuaries and zoos.

See also ENVIRONMENT - Conservation programs - Endangered species protection: for programs to protect or repopulate flora and fauna at risk.

See also ENVIRONMENT - Natural heritage protection - National park management: for administering designated national park areas.

See also ENVIRONMENT - Natural heritage protection - Nature reserve management: for the maintenance of native flora and fauna reserves.

See also ENVIRONMENT - Natural heritage protection - Wilderness area management: for the maintenance of areas where the ecology is undisturbed.""" ;
  skos:hiddenLabel "Wildlife park management" ;
  skos:hiddenLabel "Zoo management" ;
  skos:prefLabel "Wildlife sanctuary management"@en ;
  skos:related agift:endangered-species-protection ;
.
agift:workers-compensation-schemes
  rdf:type skos:Concept ;
  rdfs:label "Workers compensation schemes"@en ;
  skos:broader agift:human-resources-development ;
  skos:definition """Administering workplace insurance programs. Granting financial compensation for death, injury or disease incurred in the course of employment activities. Providing access to rehabilitation services. Monitoring compliance with government policy on workers compensation schemes. Includes liaison across jurisdictions to promote a consistent benefits structure.

See also EMPLOYMENT - Human resources development - Occupational health and safety: for programs to prevent death, injury or disease in the workplace.""" ;
  skos:hiddenLabel "Asbestos related compensation claims" ;
  skos:hiddenLabel "Compensation schemes" ;
  skos:hiddenLabel "Employment insurance schemes" ;
  skos:hiddenLabel "Work cover" ;
  skos:prefLabel "Workers compensation schemes"@en ;
  skos:related agift:occupational-health-and-safety ;
.
agift:workplace-agreement-processes
  rdf:type skos:Concept ;
  rdfs:label "Workplace agreement processes"@en ;
  skos:broader agift:employment ;
  skos:definition """Regulating the conduct of employer and employees across a particular organisation, or between an employer and an individual employee. Certifying agreements with regard to rates of pay and working conditions. Developing policy to support the establishment and use of workplace agreements. Includes enterprise codes of practice.

See also DEFENCE - Defence force careers - Military employment services: for employment conditions in the defence forces.

See also EMPLOYMENT - Human resources development - Occupational health and safety: for programs to prevent death, injury or disease in the workplace.

See also EMPLOYMENT - Industrial awards and conditions: for regulating the conduct of employers and employees across a particular industry or occupation.""" ;
  skos:hiddenLabel "Arbitration" ;
  skos:hiddenLabel "Australian Workplace Agreements" ;
  skos:hiddenLabel "Certified agreements" ;
  skos:hiddenLabel "Enterprise codes of practice" ;
  skos:hiddenLabel "Enterprise employment conditions" ;
  skos:hiddenLabel "Working conditions" ;
  skos:narrower agift:agreement-bargaining-processes ;
  skos:narrower agift:agreement-dispute-mediation ;
  skos:narrower agift:certified-employment-conditions ;
  skos:narrower agift:employment-advocacy-services ;
  skos:prefLabel "Workplace agreement processes"@en ;
  skos:related agift:military-employment-services ;
.
agift:workplace-discrimination-monitoring
  rdf:type skos:Concept ;
  rdfs:label "Workplace discrimination monitoring"@en ;
  skos:broader agift:human-resources-development ;
  skos:definition """Evaluating the effectiveness of workplace equity programs. Monitoring human resource practices to ensure compliance with government policy. Collecting statistics to assess workplace diversity by gender, race, colour, ethnicity, age, marital or parental status, sexual preference, disability or religious belief.

See also COMMUNITY SERVICES - Social justice and equity: for ensuring equal access to community services.

See also DEFENCE - Defence force careers - Military employment services: for monitoring discrimination in the defence forces.

See also EMPLOYMENT - Human resources development - Workplace equity and justice programs: for promoting fairness and diversity in the workplace.""" ;
  skos:hiddenLabel "Defence families" ;
  skos:prefLabel "Workplace discrimination monitoring"@en ;
  skos:related agift:social-justice-and-equity ;
.
agift:workplace-equity-and-justice-programs
  rdf:type skos:Concept ;
  rdfs:label "Workplace equity and justice programs"@en ;
  skos:broader agift:human-resources-development ;
  skos:definition """Administering programs that support workplace diversity in accordance with human resources policy. Ensuring all people have equal access to employment opportunities and conditions, regardless of gender, race, colour, ethnicity, age, marital or parental status, sexual preference, disability or religious belief. Mediating disputes and managing resolution processes. Discouraging offensive behaviour, intimidation or harassment through training and information programs.

See also COMMUNITY SERVICES - Social justice and equity: for ensuring equal access to community services.

See also DEFENCE - Defence force careers - Military employment services: for workplace programs in the defence forces.

See also EMPLOYMENT - Human resources development - Workplace discrimination monitoring: for evaluating the effectiveness of equity and justice programs.

See also EMPLOYMENT - Workplace agreement processes - Agreement dispute mediation: for resolving queries about the application of workplace agreements.""" ;
  skos:hiddenLabel "Dispute resolution services" ;
  skos:hiddenLabel "Diversity programs" ;
  skos:hiddenLabel "Equal employment opportunity" ;
  skos:hiddenLabel "Harassment" ;
  skos:hiddenLabel "Workplace dispute mediation" ;
  skos:hiddenLabel "Workplace diversity" ;
  skos:hiddenLabel "Workplace harassment" ;
  skos:hiddenLabel "Workplace justice services" ;
  skos:prefLabel "Workplace equity and justice programs"@en ;
  skos:related agift:agreement-dispute-mediation ;
  skos:related agift:social-justice-and-equity ;
.
agift:workplace-training
  rdf:type skos:Concept ;
  rdfs:label "Workplace training"@en ;
  skos:broader agift:vocational-education ;
  skos:definition """Administering programs of training that provide learning and development opportunities for personnel already employed in an organisation. Includes courses to improve computer literacy, learn job-specific skills, personal or career development programs and training to maintain or upgrade professional qualifications.

See also EDUCATION AND TRAINING - Military education and training: for workplace training offered to defence personnel.

See also EMPLOYMENT - Human resources development: for career development advice.""" ;
  skos:hiddenLabel "Career development training" ;
  skos:hiddenLabel "Personal development training" ;
  skos:hiddenLabel "Professional development training" ;
  skos:hiddenLabel "Trade union training" ;
  skos:prefLabel "Workplace training"@en ;
  skos:related agift:military-education-and-training ;
.
agift:world-heritage-listings
  rdf:type skos:Concept ;
  rdfs:label "World heritage listings"@en ;
  skos:broader agift:environment ;
  skos:definition "Developing policy to support the maintenance of items or areas registered by UNESCO in accordance with the World Heritage Convention for protection and conservation. Assessing natural, Indigenous and historic sites in Australia for possible inclusion on international heritage lists. Includes liaison with international bodies and community groups to manage the listing process." ;
  skos:hiddenLabel "Heritage listings" ;
  skos:hiddenLabel "UNESCO World Heritage listings" ;
  skos:prefLabel "World heritage listings"@en ;
.
<http://data.gov.au/def/agift2014>
  rdf:type owl:Ontology ;
  dc:contributor "Megan Williams, CSIRO"^^xsd:string ;
  dc:contributor "Simon Cox, CSIRO"^^xsd:string ;
  dc:creator <http://www.synercon.com.au/> ;
  dc:description "Ontology document containing a SKOS representation of the Australian Governments' Interactive Functions Thesaurus (AGIFT) - 2014 revision"@en ;
  dc:publisher <http://naa.gov.au/> ;
  dc:rights """This work is copyright. It may be adapted or reproduced for personal, in-house or non-commercial use without formal permission subject to appropriate citation. The work may not be used for other purposes – apart from any use as permitted under the Copyright Act 1968 – without prior written permission from the National Archives of Australia. Requests and inquiries concerning reproduction and rights should be sent to the Agency Service Centre.

This publication should be cited as: National Archives of Australia, Australian Governments’ Interactive Functions Thesaurus, 3rd Edition, November 2014."""^^xsd:string ;
  dc:title "Australian Governments' Interactive Functions Thesaurus (AGIFT)"^^xsd:string ;
  dcterms:created "2014-11-27"^^xsd:string ;
  dcterms:license <http://opendatacommons.org/licenses/by/1.0> ;
  vann:preferredNamespacePrefix "agift"^^xsd:string ;
  vann:preferredNamespaceUri <http://data.gov.au/def/agift#> ;
  rdfs:comment "SKOS representation prepared by Megan Williams and Simon Cox"^^xsd:string ;
  rdfs:comment """The Australian Governments’ Interactive Functions Thesaurus (AGIFT) is a three-level hierarchical thesaurus that describes the business functions carried out across Commonwealth, state and local governments in Australia.

It contains 25 high-level functions, each with second and third level terms, as well as non-preferred terms and related terms. Its main purpose is to describe web-based resources to aid online discovery of government information and services.

Terms can be searched by function, alphabetically and via full-text searching.

In the thesaurus you will find:

Function – the broadest unit of business performed by Australian Governments' Interactive Functions Thesaurus
Level 2 – major tasks or areas of service undertaken within each function
Level 3 – topics being addressed within function/activities
For each term, the thesaurus shows:
Scope Notes – notes that provide guidance on the use of a term
Broader Terms – terms at a higher level
Narrower Terms – terms at a lower level
Related Terms – terms at the same level
Use – approved terms used to identify and save documents
Non-preferred Term – other terms, not to be used to identify and save documents"""^^xsd:string ;
  rdfs:label "Australian Governments' Interactive Functions Thesaurus (AGIFT)"@en ;
  rdfs:seeAlso <http://agift.naa.gov.au/index.htm> ;
  owl:imports dc: ;
  owl:imports <http://www.w3.org/2004/02/skos/core> ;
.
